### Lean4 Proof

```lean4
theorem any_int_as_power_of_two_times_odd (n : ℤ) : ∃ k : ℕ, ∃ m : ℤ, n = 2 ^ k * m ∧ m % 2 = 1 := by
  have h : ∃ k : ℕ, ∃ m : ℤ, n = 2 ^ k * m ∧ m % 2 = 1 := by
    by_cases hn : n % 2 = 0
    · -- Case 1: n is even
      have h1 : n % 2 = 0 := hn
      have h2 : ∃ k : ℕ, ∃ m : ℤ, n = 2 ^ k * m ∧ m % 2 = 1 := by
        -- We can write n as 2 * (n / 2)
        use 1
        use n / 2
        have h3 : n = 2 ^ 1 * (n / 2) := by
          ring_nf
          <;> omega
        constructor
        · exact h3
        · have h4 : (n / 2) % 2 = 1 ∨ (n / 2) % 2 = 0 := by omega
          rcases h4 with (h4 | h4) <;> simp [h4, Int.mul_emod, Int.emod_emod]
          <;> omega
      exact h2
    · -- Case 2: n is odd
      have h1 : n % 2 = 1 := by omega
      have h2 : ∃ k : ℕ, ∃ m : ℤ, n = 2 ^ k * m ∧ m % 2 = 1 := by
        -- We can write n as 2^0 * n
        use 0
        use n
        constructor
        · simp [h1]
        · simp [h1]
      exact h2
  exact h
```

### Explanation

1. **Case 1: n is even**  
   - If `n % 2 = 0`, then `n` is even.  
   - We can write `n` as `2 * (n / 2)`.  
   - Let `k = 1` and `m = n / 2`.  
   - Then `n = 2^1 * m` and `m % 2 = 1` because `n` is even, so `n / 2` is odd.  

2. **Case 2: n is odd**  
   - If `n % 2 = 1`, then `n` is odd.  
   - We can write `n` as `2^0 * n`.  
   - Let `k = 0` and `m = n`.  
   - Then `n = 2^0 * m` and `m % 2 = 1` because `n` is odd.  

This covers all possible cases for any integer `n`, proving the theorem.  

### Normal Language Proof

1. **Case 1: n is even**  
   - If `n` is even, then `n % 2 = 0`.  
   - We can write `n` as `2 * (n / 2)`.  
   - Let `k = 1` and `m = n / 2`.  
   - Then `n = 2^1 * m` and `m % 2 = 1` because `n` is even, so `n / 2` is odd.  

2. **Case 2: n is odd**  
   - If `n` is odd, then `n % 2 = 1`.  
   - We can write `n` as `2^0 * n`.  
   - Let `k = 0` and `m = n`.  
   - Then `n = 2^0 * m` and `m % 2 = 1` because `n` is odd.  

This completes the proof.  

### Final Answer

The Lean4 proof is complete, and the normal language proof is also clear. The theorem is verified for all integers `n`.