### Part (a)

**Lean4 Proof Sketch:**

```lean4
theorem part_a (p : ℕ) (a n : ℕ) (hp : Nat.Prime p) (h : p ∣ a^n) : p^n ∣ a^n := by
  have h₁ : p ∣ a := by
    apply Nat.Prime.dvd_of_dvd_pow hp
    exact h
  have h₂ : p^n ∣ a^n := by
    exact pow_dvd_pow_of_dvd h₁ n
  exact h₂
```

**Explanation:**
1. Since \( p \) is prime and \( p \mid a^n \), by the property of primes, \( p \mid a \). This is because if a prime divides a power of an integer, it must divide the integer itself.
2. Once \( p \mid a \), we can use the fact that if \( p \mid a \), then \( p^n \mid a^n \) for any \( n \geq 1 \). This is because \( a^n = (a)^n \), and if \( p \mid a \), then \( p^n \mid a^n \).
3. The result follows directly from the above reasoning.

### Part (b)

**Lean4 Proof Sketch:**

```lean4
theorem part_b (p : ℕ) (a b : ℕ) (hp : Nat.Prime p) (h : Nat.gcd a b = p) :
    Nat.gcd (a^2) (b^2) = p^2 ∧ Nat.gcd (a^2) b = p^2 ∧ Nat.gcd (a^3) (b^2) = p^2 := by
  have h₁ : p ∣ a := by
    have h₂ : p ∣ Nat.gcd a b := by simp [h]
    exact Nat.dvd_trans h₂ (Nat.gcd_dvd_left a b)
  have h₂ : p ∣ b := by
    have h₃ : p ∣ Nat.gcd a b := by simp [h]
    exact Nat.dvd_trans h₃ (Nat.gcd_dvd_right a b)
  have h₃ : Nat.gcd (a^2) (b^2) = p^2 := by
    have h₄ : p^2 ∣ a^2 := by
      have h₅ : p^2 ∣ a^2 := by
        exact pow_dvd_pow_of_dvd h₁ 2
      exact h₅
    have h₅ : p^2 ∣ b^2 := by
      have h₆ : p^2 ∣ b^2 := by
        exact pow_dvd_pow_of_dvd h₂ 2
      exact h₆
    have h₆ : Nat.gcd (a^2) (b^2) = p^2 := by
      have h₇ : Nat.gcd (a^2) (b^2) = p^2 := by
        rw [Nat.gcd_eq_right] <;> simp_all [Nat.pow_dvd_pow_iff]
        <;> omega
      exact h₇
    exact h₆
  have h₄ : Nat.gcd (a^2) b = p^2 := by
    have h₅ : p^2 ∣ a^2 := by
      have h₆ : p^2 ∣ a^2 := by
        exact pow_dvd_pow_of_dvd h₁ 2
      exact h₆
    have h₆ : p^2 ∣ b := by
      have h₇ : p^2 ∣ b := by
        exact pow_dvd_pow_of_dvd h₂ 2
      exact h₇
    have h₇ : Nat.gcd (a^2) b = p^2 := by
      have h₈ : Nat.gcd (a^2) b = p^2 := by
        rw [Nat.gcd_eq_right] <;> simp_all [Nat.pow_dvd_pow_iff]
        <;> omega
      exact h₈
    exact h₇
  have h₅ : Nat.gcd (a^3) (b^2) = p^2 := by
    have h₆ : p^2 ∣ a^3 := by
      have h₇ : p^2 ∣ a^3 := by
        have h₈ : p ∣ a := h₁
        have h₉ : p^2 ∣ a^3 := by
          calc
            p^2 ∣ a^2 := pow_dvd_pow_of_dvd h₁ 2
            _ ∣ a^3 := pow_dvd_pow a (by norm_num)
        exact h₉
      exact h₇
    have h₇ : p^2 ∣ b^2 := by
      have h₈ : p^2 ∣ b^2 := by
        have h₉ : p ∣ b := h₂
        have h₁₀ : p^2 ∣ b^2 := by
          calc
            p^2 ∣ b^2 := pow_dvd_pow_of_dvd h₂ 2
            _ ∣ b^2 := by rfl
        exact h₁₀
      exact h₈
    have h₈ : Nat.gcd (a^3) (b^2) = p^2 := by
      have h₉ : Nat.gcd (a^3) (b^2) = p^2 := by
        rw [Nat.gcd_eq_right] <;> simp_all [Nat.pow_dvd_pow_iff]
        <;> omega
      exact h₉
    exact h₈
  exact ⟨h₃, h₄, h₅⟩
```

**Explanation:**
1. Since \( \gcd(a, b) = p \), we know that \( p \mid a \) and \( p \mid b \). This is because \( p \) divides the gcd of \( a \) and \( b \).
2. For \( \gcd(a^2, b^2) \):
   - \( p^2 \) divides \( a^2 \) because \( p \mid a \) implies \( p^2 \mid a^2 \).
   - Similarly, \( p^2 \) divides \( b^2 \).
   - Thus, \( \gcd(a^2, b^2) = p^2 \).
3. For \( \gcd(a^2, b) \):
   - \( p^2 \) divides \( a^2 \) because \( p \mid a \) implies \( p^2 \mid a^2 \).
   - \( p^2 \) divides \( b \) because \( p \mid b \) implies \( p^2 \mid b^2 \), and \( p^2 \mid b^2 \) implies \( p^2 \mid b \) (since \( p \) is prime).
   - Thus, \( \gcd(a^2, b) = p^2 \).
4. For \( \gcd(a^3, b^2) \):
   - \( p^2 \) divides \( a^3 \) because \( p \mid a \) implies \( p^2 \mid a^2 \), and \( p^2 \mid a^2 \) implies \( p^2 \mid a^3 \).
   - \( p^2 \) divides \( b^2 \) because \( p \mid b \) implies \( p^2 \mid b^2 \).
   - Thus, \( \gcd(a^3, b^2) = p^2 \).

### Normal Language Explanation

1. **Part (a):**
   - Since \( p \) is prime and \( p \mid a^n \), it follows that \( p \mid a \).
   - Because \( p \mid a \), we have \( p^n \mid a^n \) for any \( n \geq 1 \).

2. **Part (b):**
   - Given \( \gcd(a, b) = p \), we know \( p \mid a \) and \( p \mid b \).
   - For \( \gcd(a^2, b^2) \):
     - \( p^2 \) divides \( a^2 \) and \( b^2 \), so \( \gcd(a^2, b^2) = p^2 \).
   - For \( \gcd(a^2, b) \):
     - \( p^2 \) divides \( a^2 \) and \( p^2 \) divides \( b \), so \( \gcd(a^2, b) = p^2 \).
   - For \( \gcd(a^3, b^2) \):
     - \( p^2 \) divides \( a^3 \) and \( p^2 \) divides \( b^2 \), so \( \gcd(a^3, b^2) = p^