### Lean4 Proof

```lean4
theorem consecutive_composites (n : ℕ) (hn : n > 2) : 
  ∀ k : ℕ, k ≤ n → ¬ Nat.Prime ((n + 1)! - k) := by
  intro k hk
  have h₁ : (n + 1)! - k ≤ (n + 1)! - 1 := by
    apply Nat.sub_le_sub_left
    omega
  have h₂ : (n + 1)! - k > 1 := by
    have h₃ : (n + 1)! ≥ (n + 1) * n ! := by
      simp [Nat.factorial_succ, Nat.mul_comm]
      <;> nlinarith [Nat.factorial_pos n]
    have h₄ : (n + 1)! - k ≥ (n + 1) * n ! - k := by
      omega
    have h₅ : (n + 1) * n ! - k > 1 := by
      have h₆ : n ! ≥ 2 := by
        have h₇ : n ≥ 3 := by omega
        have h₈ : n ! ≥ 3! := Nat.factorial_le (by omega)
        have h₉ : 3! = 6 := by decide
        omega
      have h₇ : (n + 1) * n ! ≥ (n + 1) * 2 := by
        nlinarith
      have h₈ : (n + 1) * 2 - k > 1 := by
        have h₉ : k ≤ n := by omega
        have h₁₀ : n ≥ 3 := by omega
        have h₁₁ : (n + 1) * 2 - k ≥ 5 - k := by
          nlinarith
        have h₁₂ : 5 - k > 1 := by
          omega
        omega
      omega
    omega
  have h₃ : ¬ Nat.Prime ((n + 1)! - k) := by
    intro h
    have h₄ := Nat.Prime.eq_one_or_self_of_dvd h 2
    have h₅ : 2 ∣ (n + 1)! - k := by
      have h₆ : (n + 1)! - k ≥ 2 := by omega
      have h₇ : 2 ∣ (n + 1)! := by
        apply Nat.dvd_factorial
        omega
        omega
      have h₈ : 2 ∣ (n + 1)! - k := by
        omega
      exact h₈
    have h₆ : (n + 1)! - k = 2 := by
      omega
    have h₇ : (n + 1)! ≥ (n + 1) * n ! := by
      simp [Nat.factorial_succ, Nat.mul_comm]
      <;> nlinarith [Nat.factorial_pos n]
    have h₈ : (n + 1)! - k ≥ (n + 1) * n ! - k := by
      omega
    have h₉ : (n + 1) * n ! - k ≥ (n + 1) * 2 - k := by
      have h₁₀ : n ! ≥ 2 := by
        have h₁₁ : n ≥ 3 := by omega
        have h₁₂ : n ! ≥ 3! := Nat.factorial_le (by omega)
        have h₁₃ : 3! = 6 := by decide
        omega
      nlinarith
    have h₁₀ : (n + 1) * 2 - k ≥ 5 - k := by
      nlinarith
    have h₁₁ : 5 - k ≥ 2 := by
      omega
    omega
  exact h₃
```

### Explanation

1. **Bounds on the Terms**:
   - We first establish that each term in the sequence is bounded below by `(n + 1)! - (n + 1)` and above by `(n + 1)! - 1`.
   - This is straightforward since `k` ranges from `1` to `n`, and `k` is decreasing.

2. **Lower Bound on Terms**:
   - We show that each term `(n + 1)! - k` is greater than `1` because `(n + 1)!` is a product of numbers starting from `(n + 1)`, and subtracting `k` (where `k ≤ n`) ensures the result is at least `(n + 1) * n! - k`, which is greater than `1` for `n > 2`.

3. **Composite Nature**:
   - We prove that each term is composite by showing it is divisible by `2`. This is because `(n + 1)!` is divisible by `2` (since `n + 1 ≥ 3` for `n > 2`), and thus `(n + 1)! - k` is also divisible by `2` for the same reason.
   - Since `(n + 1)! - k > 1` and divisible by `2`, it cannot be prime.

### Normal Language Explanation

1. **Sequence Definition**:
   - The sequence is `(n + 1)! - k` for `k` ranging from `1` to `n`.

2. **Bounds**:
   - The terms are bounded below by `(n + 1)! - n` and above by `(n + 1)! - 1`.

3. **Lower Bound**:
   - Each term is greater than `1` because `(n + 1)!` is a product of numbers starting from `(n + 1)`, and subtracting `k` (where `k ≤ n`) ensures the result is at least `(n + 1) * n! - k`, which is greater than `1` for `n > 2`.

4. **Composite Nature**:
   - Each term is divisible by `2` because `(n + 1)!` is divisible by `2` (since `n + 1 ≥ 3` for `n > 2`), and thus `(n + 1)! - k` is also divisible by `2` for the same reason.
   - Since the term is greater than `1` and divisible by `2`, it cannot be prime.

### Conclusion

The sequence `(n + 1)! - k` for `k` from `1` to `n` produces `n` consecutive composite integers for `n > 2`. This is because each term is greater than `1` and divisible by `2`, ensuring it is composite.