### Part (a): Proving that every pth term in the arithmetic progression is divisible by p.

**Lean4 Proof Sketch:**

```lean4
theorem p_divides_every_pth_term (p : ℕ) (hp : Nat.Prime p) (a b : ℤ) (hb : p ∣ b) : ∀ n : ℕ, p ∣ (a + n * b) := by
  intro n
  have h : p ∣ b := hb
  have h1 : p ∣ (a + n * b) := by
    -- Use the fact that p divides b to show that p divides a + n * b
    have h2 : p ∣ n * b := by
      apply dvd_mul_of_dvd_right
      exact h
    have h3 : p ∣ a + n * b := by
      -- Since p divides n * b, and p divides a + n * b, we can use the fact that p divides the sum
      exact dvd_add (by assumption) h2
    exact h3
  exact h1
```

**Explanation:**
1. We start by assuming `p` is a prime, `p` divides `b`, and `a`, `b` are integers.
2. For any natural number `n`, we need to show that `p` divides `a + n * b`.
3. Since `p` divides `b`, we can write `b = k * p` for some integer `k`.
4. Then, `a + n * b = a + n * (k * p) = a + (n * k) * p = a + (n * k) * p`, which is clearly divisible by `p` because it is a multiple of `p`.
5. This completes the proof.

### Part (b): Concluding that every other term in the progression is even if `b` is odd.

**Lean4 Proof Sketch:**

```lean4
theorem every_other_term_even_if_b_odd (b : ℤ) (hb : Odd b) : ∀ n : ℕ, Even (a + n * b) ↔ n % 2 = 0 := by
  intro n
  have h : b % 2 = 1 := by
    cases' hb with k hk
    omega
  have h1 : ∀ n : ℕ, (a + n * b) % 2 = (a % 2 + n * (b % 2)) % 2 := by
    intro n
    simp [Int.add_emod, Int.mul_emod]
  have h2 : a % 2 = 0 ∨ a % 2 = 1 := by omega
  have h3 : n % 2 = 0 ∨ n % 2 = 1 := by omega
  rcases h2 with (h2 | h2) <;> rcases h3 with (h3 | h3) <;> simp [h1, h, h2, h3, Nat.even_iff, Nat.odd_iff, Int.even_iff, Int.odd_iff]
  <;> omega
```

**Explanation:**
1. We start by assuming `b` is odd, so `b % 2 = 1`.
2. We then consider the parity of `a` and `n` to determine the parity of `a + n * b`.
3. We use modular arithmetic to simplify the expression `a + n * b` modulo 2.
4. We consider all combinations of the parities of `a` and `n` to show that `a + n * b` is even if and only if `n` is even.
5. This completes the proof.