Establish the formulas below by mathematical induction:
   $1 + 2 + 3 + \ldots  + n = \frac{n(n+1)}{2}$ for all n $\geq{1}$.

### Lean4 Proof
Establish the formulas below by mathematical induction:
   $1 + 2 + 3 + \ldots  + n = \frac{n(n+1)}{2}$ for all n $\geq{1}$.

```lean4
theorem sum_formula (n : ℕ) : ∑ i in Finset.range n, (i + 1) = n * (n + 1) / 2 := by
  induction n with
  | zero => simp
  | succ n ih =>
    cases n with
    | zero => simp
    | succ n =>
      simp_all [Finset.sum_range_succ, Nat.succ_eq_add_one, Nat.div_eq_of_lt, Nat.mul_add, Nat.add_mul]
      ring_nf at *
      <;> omega
```
