Establish the formulas below by mathematical induction:
   $1^3 + 2^3 + 3^3 + \ldots + n^3 = [\frac{n(n+1)}{2}]^2$ for all n $\geq{1}$.

### Lean4 Proof

```lean4
theorem sum_of_cubes (n : ℕ) : ∑ i in Finset.range n, (i + 1)^3 = (n * (n + 1) / 2)^2 := by
  induction n with
  | zero =>
    -- Base case: when n = 0, the sum is 0, and the formula simplifies to 0.
    simp
  | succ n ih =>
    -- Inductive step: assume the formula holds for n, prove it for n + 1.
    cases n with
    | zero =>
      -- Base case: when n = 1, the sum is 1^3 = 1, and the formula simplifies to (1 * 2 / 2)^2 = 1.
      simp [Finset.sum_range_succ, Nat.pow_succ]
    | succ n =>
      -- Inductive step: use the induction hypothesis to prove the formula for n + 1.
      simp_all [Finset.sum_range_succ, Nat.succ_eq_add_one, Nat.div_eq_of_lt, Nat.mul_add, Nat.add_mul,
        Nat.pow_succ, Nat.mul_one, Nat.add_assoc]
      ring_nf at *
      <;> omega
```