If $r \neq 1$, show that for any positive integer n,
$$a + ar + ar^2 + \ldots + ar^n = \frac{a(r^{n+1}-1)}{r-1}$$

### Lean4 Proof

```lean4
theorem sum_of_geometric_series (a r : ℝ) (n : ℕ) (h : r ≠ 1) : 
  a + ar + ar^2 + ... + ar^n = a * (r^(n+1) - 1) / (r - 1) := by
  have h₁ : a + ar + ar^2 + ... + ar^n = a * (r^(n+1) - 1) / (r - 1) := by
    induction n with
    | zero =>
      -- Base case: n = 0
      simp [mul_comm]
      <;> field_simp [sub_ne_zero.mpr h, sub_ne_zero.mpr h.symm]
      <;> ring
    | succ n ih =>
      -- Inductive step: assume the formula holds for n, prove for n+1
      simp_all [Finset.sum_range_succ, pow_succ, mul_add, mul_comm, mul_left_comm]
      <;> field_simp [sub_ne_zero.mpr h, sub_ne_zero.mpr h.symm] at *
      <;> ring_nf at *
      <;> linarith
  exact h₁
```