 Let's consider the example where $a = 2$, $b = 3$, $k = 2$, $j = 1$, and $n = 4$.

We have $a^k \equiv b^k$ (mod n) since $2^2 \equiv 3^2$ (mod 4), which simplifies to $4 \equiv 9$ (mod 4), which is true because $4 - 9 = -5$ is divisible by 4.

We also have $k \equiv j$ (mod n) since $2 \equiv 1$ (mod 4), which is true because $2 - 1 = 1$ is divisible by 4.

However, $a^j \equiv b^j$ (mod n) does not hold. We have $a^j = 2^1 = 2$ and $b^j = 3^1 = 3$. But $2 \not\equiv 3$ (mod 4), because $2 - 3 = -1$ is not divisible by 4.

So, in this example, $a^k \equiv b^k$ (mod n) and $k \equiv j$ (mod n) do not imply that $a^j \equiv b^j$ (mod n).