 To prove this, we will use the properties of congruences and the given information.

Given:
1. $ab \equiv cd$ (mod n)
2. $b \equiv d$ (mod n)
3. gcd(b, n) = 1

We want to prove: $a \equiv c$ (mod n)

First, we can rewrite the second given as $b - d \equiv 0$ (mod n).

Now, we can multiply both sides of the first given by the multiplicative inverse of b modulo n. Since gcd(b, n) = 1, b has a multiplicative inverse modulo n. Let's call this inverse b'. So, we have:

$ab' \equiv cd'$ (mod n)

Now, we can add $d - d$ to both sides of the congruence:

$ab' + d - d \equiv cd' + d - d$ (mod n)

This simplifies to:

$ab' + (d - d) \equiv cd' + (d - d)$ (mod n)

$ab' \equiv cd'$ (mod n)

Now, we can substitute $b - d$ for $d - d$:

$ab' \equiv cd'$ (mod n)

$ab' \equiv cd' + (b - d)$ (mod n)

$ab' \equiv cd' + b - d$ (mod n)

Now, we can add $d$ to both sides of the congruence:

$ab' + d \equiv cd' + b$ (mod n)

$ab' + d - d \equiv cd' + b - d$ (mod n)

$ab' \equiv cd' + b - d$ (mod n)

Since $b \equiv d$ (mod n), we can substitute $d$ for $b$ in the right side of the congruence:

$ab' \equiv cd' + d - d$ (mod n)

$ab' \equiv cd'$ (mod n)

Now, we can multiply both sides of the congruence by the multiplicative inverse of $d'$ modulo n:

$a \equiv c$ (mod n)

Thus, we have proven that whenever $ab \equiv cd$ (mod n) and $b \equiv d$ (mod n), with gcd(b, n) = 1, then $a \equiv c$ (mod n).