 To prove this, we will use the properties of congruences and the definition of the greatest common divisor (gcd).

First, let's recall the definition of congruence modulo $n$:

If $a \equiv b$ (mod $n$), it means that $n$ divides $a - b$. In other words, $a - b = kn$ for some integer $k$.

Now, let's consider the given congruences:

1. $a \equiv b$ (mod $n_1$)
2. $a \equiv c$ (mod $n_2$)

From these congruences, we can write:

1. $a - b = k_1n_1$ for some integer $k_1$
2. $a - c = k_2n_2$ for some integer $k_2$

We want to prove that $b \equiv c$ (mod $n$), where $n = gcd(n_1, n_2)$.

To do this, we will subtract the second equation from the first:

$(a - b) - (a - c) = k_1n_1 - k_2n_2$

Simplifying, we get:

$c - b = k_1n_1 - k_2n_2$

Now, we need to show that $n$ divides $c - b$. Since $n = gcd(n_1, n_2)$, we know that $n$ divides both $n_1$ and $n_2$. Therefore, $n$ divides any linear combination of $n_1$ and $n_2$, such as $k_1n_1 - k_2n_2$.

So, $n$ divides $c - b$, which means $b \equiv c$ (mod $n$).

Thus, we have proven that if $a \equiv b$ (mod $n_1$) and $a \equiv c$ (mod $n_2$), then $b \equiv c$ (mod $n$), where $n = gcd(n_1, n_2)$.