 We will prove this by induction.

Base case:
For $n=1$, we have $a^{2^1}=a^2$. Since $a$ is an odd integer, $a^2 \equiv 1 \pmod{4}$. Thus, the base case holds.

Inductive step:
Assume that the statement is true for $n=k$, i.e., $a^{2^k} \equiv 1 \pmod{2^{k+2}}$. We want to show that the statement is also true for $n=k+1$.

Consider $a^{2^{k+1}} = a^{2^k \cdot 2} = (a^{2^k})^2$. By the induction hypothesis, $a^{2^k} \equiv 1 \pmod{2^{k+2}}$. Squaring both sides, we get $(a^{2^k})^2 \equiv 1^2 \pmod{2^{k+2}}$. Since $1^2 \equiv 1 \pmod{4}$, we have $(a^{2^k})^2 \equiv 1 \pmod{4}$.

Now, we need to show that $(a^{2^k})^2 \equiv 1 \pmod{2^{k+3}}$. Since $2^{k+2}$ is a factor of $2^{k+3}$, we have $(a^{2^k})^2 \equiv 1 \pmod{2^{k+3}}$ if $(a^{2^k})^2 \equiv 1 \pmod{4}$. Thus, the inductive step holds.

By the principle of mathematical induction, the statement is true for all $n \geq 1$.