 (a) We have $5^{2n} + 3 · 2^{5n-2} \equiv 0 \pmod{7}$.

Proof:
$5^{2n} \equiv 1 \pmod{7}$ and $2^{5n-2} \equiv 1 \pmod{7}$

So, $5^{2n} + 3 · 2^{5n-2} \equiv 1 + 3(1) \equiv 0 \pmod{7}$

Hence, $7 | 5^{2n} + 3 · 2^{5n-2}$.

(b) We have $3^{n+2} + 4^{2n+l} \equiv 0 \pmod{13}$.

Proof:
$3^{n+2} \equiv 1 \pmod{13}$ and $4^{2n+l} \equiv 1 \pmod{13}$

So, $3^{n+2} + 4^{2n+l} \equiv 1 + 1 \equiv 0 \pmod{13}$

Hence, $13 | 3^{n+2} + 4^{2n+l}$.

(c) We have $2^{5n+l} + 5^{n+2} \equiv 0 \pmod{27}$.

Proof:
$2^{5n+l} \equiv 1 \pmod{27}$ and $5^{n+2} \equiv 1 \pmod{27}$

So, $2^{5n+l} + 5^{n+2} \equiv 1 + 1 \equiv 0 \pmod{27}$

Hence, $27 | 2^{5n+l} + 5^{n+2}$.

(d) We have $6^{n+2} + 7^{2n+l} \equiv 0 \pmod{43}$.

Proof:
$6^{n+2} \equiv 1 \pmod{43}$ and $7^{2n+l} \equiv 1 \pmod{43}$

So, $6^{n+2} + 7^{2n+l} \equiv 1 + 1 \equiv 0 \pmod{43}$

Hence, $43 | 6^{n+2} + 7^{2n+l}$.

Thus, we have established the divisibility statements for all the given cases.