 We will use induction to prove this.

Base case: For $n=1$, we have $(-13)^{1+1} = (-13)^2 = 169$ and $(-13)^1 + (-13)^{1-1} = 169$. Thus, the base case holds.

Inductive step: Assume that the statement is true for $n=k$, i.e., $(-13)^{k+1} \equiv (-13)^k + (-13)^{k-1} \pmod{181}$. We need to show that the statement is also true for $n=k+1$, i.e., $(-13)^{k+2} \equiv (-13)^{k+1} + (-13)^k \pmod{181}$.

We can rewrite $(-13)^{k+2}$ as $(-13)^{k+1} \cdot (-13)$. By the induction hypothesis, we have $(-13)^{k+1} \equiv (-13)^k + (-13)^{k-1} \pmod{181}$. Multiplying both sides by $-13$, we get

$(-13)^{k+2} \equiv (-13)^k \cdot (-13) + (-13)^{k-1} \cdot (-13) \pmod{181}$.

Now, we can simplify the right side of the congruence:

$(-13)^k \cdot (-13) + (-13)^{k-1} \cdot (-13) \equiv (-13)^{k+1} + (-13)^k \pmod{181}$.

Thus, we have shown that if the statement is true for $n=k$, it is also true for $n=k+1$. By the principle of mathematical induction, the statement is true for all $n \geq 1$.