 (a) If $a \equiv b$ (mod n) and m | n, then $a \equiv b$ (mod m).

Proof: Since $a \equiv b$ (mod n), we have $a = b + kn$ for some integer k. Since m | n, we can write n = m * t for some integer t. Substituting this into the equation, we get $a = b + k(m*t) = b + (kt)m$. This means $a \equiv b$ (mod m), as required.

(b) If $a \equiv b$ (mod n) and c > 0, then $ca \equiv cb$ (mod en).

Proof: Since $a \equiv b$ (mod n), we have $a = b + kn$ for some integer k. Multiplying both sides by c, we get $ca = cb + kcn$. This means $ca \equiv cb$ (mod en), as required.

(c) If $a \equiv b$ (mod n) and the integers a, b, n are all divisible by d > 0, then $a/d \equiv b/d$ (mod n/d).

Proof: Since $a \equiv b$ (mod n), we have $a = b + kn$ for some integer k. Dividing both sides by d, we get $a/d = b/d + k(n/d)$. This means $a/d \equiv b/d$ (mod n/d), as required.