 (a) A repunit $R_n$ is a number consisting of n ones. So, $R_n = 111...1$ (n times).

We can write $R_n$ as $R_n = \frac{10^n - 1}{9}$.

Now, we want to show that $9 | R_n$ if and only if 9 | n.

First, let's assume that 9 | n. Then, n = 9k for some integer k.

Substitute n = 9k into the expression for $R_n$, we get $R_n = \frac{10^{9k} - 1}{9}$.

Notice that $10^{9k} - 1$ is a difference of two powers, which can be factored as $(10^k - 1)(10^{8k} + 10^{7k} + 10^{6k} + ... + 10^{k} + 1)$.

Since 9 | $(10^k - 1)$, we have $9 | R_n$.

Now, let's assume that $9 | R_n$. Then, $R_n = 9m$ for some integer m.

Substitute $R_n = 9m$ into the expression for $R_n$, we get $9m = \frac{10^n - 1}{9}$.

Multiply both sides by 9, we get $81m = 10^n - 1$.

Rearrange the equation, we get $10^n = 81m + 1$.

Notice that the right side of the equation is 1 more than a multiple of 9, so $10^n$ is 1 more than a multiple of 9.

Since $10^n$ is 1 more than a multiple of 9, n must be a multiple of 9.

Therefore, we have shown that $9 | R_n$ if and only if 9 | n.

(b) We want to show that $11 | R_n$ if and only if n is even.

First, let's assume that n is even. Then, n = 2k for some integer k.

Substitute n = 2k into the expression for $R_n$, we get $R_n = \frac{10^{2k} - 1}{9}$.

Notice that $10^{2k} - 1$ is a difference of two squares, which can be factored as $(10^k + 1)(10^k - 1)$.

Since 11 | $(10^k + 1)$, we have $11 | R_n$.

Now, let's assume that $11 | R_n$. Then, $R_n = 11m$ for some integer m.

Substitute $R_n = 11m$ into the expression for $R_n$, we get $11m = \frac{10^n - 1}{9}$.

Multiply both sides by 9, we get $99m = 10^n - 1$.

Rearrange the equation, we get $10^n = 99m + 1$.

Notice that the right side of the equation is 1 more than a multiple of 11, so $10^n$ is 1 more than a multiple of 11.

Since $10^n$ is 1 more than a multiple of 11, n must be even.

Therefore, we have shown that $11 | R_n$ if and only if n is even.