 We can rewrite the expression as $10^{2p} - 10^p + 1 = (10^p - 1)(10^p - 1) + 1$.

Since $p$ is a prime number greater than 3, we know that $p$ is odd. Therefore, $p$ can be written as $p = 2k + 1$ for some integer $k$.

Now, let's consider the expression $10^p - 1$. We have:

$10^p - 1 = 10^{2k + 1} - 1 = 10^{2k} \cdot 10 - 1 = (10^k)^2 \cdot 10 - 1$.

Notice that $10^k$ is a multiple of 10, so it can be written as $10^k = 10 \cdot m$ for some integer $m$. Substituting this into the expression, we get:

$(10^k)^2 \cdot 10 - 1 = (10 \cdot m)^2 \cdot 10 - 1 = 100m^2 \cdot 10 - 1 = 1000m^2 - 1$.

Now, we can rewrite the original expression as:

$(10^p - 1)(10^p - 1) + 1 = (1000m^2 - 1)(1000m^2 - 1) + 1$.

Expanding this expression, we get:

$(1000m^2 - 1)(1000m^2 - 1) + 1 = 1000^2m^4 - 1000m^2 + 1 + 1 = 1000^2m^4 - 1000m^2 + 2$.

Notice that $1000^2m^4 - 1000m^2 + 2$ is a multiple of 13, since it can be written as $1000(1000m^4 - m^2) + 2$.

Therefore, for any prime $p > 3$, the expression $10^{2p} - 10^p + 1$ is divisible by 13.