 To solve the linear congruence $3x - 7y \equiv 11$ (mod 13), we first need to find the modular inverse of 3 and -7 modulo 13.

The modular inverse of a number $a$ modulo $m$ is a number $b$ such that $ab \equiv 1$ (mod $m$). 

Let's find the modular inverse of 3 modulo 13. We can use the extended Euclidean algorithm to find it.

We start with the equation $13 = 3 \cdot 4 + 1$. Then we rewrite this equation as $1 = 13 - 3 \cdot 4$.

Now we can express 1 as a linear combination of 13 and 3: $1 = 1 \cdot 13 - 3 \cdot 4$.

This means that the modular inverse of 3 modulo 13 is -4, but we need a positive number. Since we are working modulo 13, we can add 13 to -4 to get a positive number: $-4 + 13 = 9$.

So, the modular inverse of 3 modulo 13 is 9.

Now let's find the modular inverse of -7 modulo 13. We can rewrite -7 as 6 modulo 13, so we need to find the modular inverse of 6 modulo 13.

We can use the same method as before. We start with the equation $13 = 6 \cdot 2 + 1$. Then we rewrite this equation as $1 = 13 - 6 \cdot 2$.

Now we can express 1 as a linear combination of 13 and 6: $1 = 1 \cdot 13 - 6 \cdot 2$.

This means that the modular inverse of 6 modulo 13 is -2, but we need a positive number. Since we are working modulo 13, we can add 13 to -2 to get a positive number: $-2 + 13 = 11$.

So, the modular inverse of 6 (or -7) modulo 13 is 11.

Now we can rewrite the linear congruence as $3x \equiv 11$ (mod 13) and $-7y \equiv 11$ (mod 13).

Multiplying both sides of the first congruence by 9 (the modular inverse of 3 modulo 13), we get $x \equiv 33$ (mod 13). Since 33 is congruent to 4 modulo 13, we have $x \equiv 4$ (mod 13).

Multiplying both sides of the second congruence by 11 (the modular inverse of -7 modulo 13), we get $y \equiv 121$ (mod 13). Since 121 is congruent to 3 modulo 13, we have $y \equiv 3$ (mod 13).

So, the solution of the linear congruence is $x \equiv 4$ (mod 13) and $y \equiv 3$ (mod 13).