 (a) 4x +51y = 9.
$4x \equiv 9$ (mod 51) gives x = 15 + 51t, whereas 5$1y \equiv 9$ (mod 4) gives y = 3 + 4s.
Substituting these into the equation, we get:
$4(15 + 51t) + 51(3 + 4s) = 9$
$60 + 204t + 153 + 204s = 9$
$204t + 204s = -102$
$t + s = -1$
So, $s = -1 - t$.

(b) 12x + 25y = 331.
We can use the extended Euclidean algorithm to find the modular inverse of 12 modulo 25.
$25 = 2 \cdot 12 + 1$
$12 = 1 \cdot 1 + 11$
$1 = 12 - 1 \cdot 11$
$1 = 12 - 1 \cdot (25 - 2 \cdot 12)$
$1 = 3 \cdot 12 - 1 \cdot 25$
So, the modular inverse of 12 modulo 25 is 3.

Now, we can find the solution to the equation:
$12x \equiv 331$ (mod 25)
$12x \equiv 11$ (mod 25)
$x \equiv 11 \cdot 3$ (mod 25)
$x \equiv 33$ (mod 25)
$x = 33 + 25t$

Similarly, we can find the solution to the equation:
$25y \equiv 331$ (mod 12)
$25y \equiv 7$ (mod 12)
$y \equiv 7 \cdot 1$ (mod 12)
$y \equiv 7$ (mod 12)
$y = 7 + 12s$

Substituting these into the equation, we get:
$12(33 + 25t) + 25(7 + 12s) = 331$
$396 + 300t + 175 + 300s = 331$
$300t + 300s = -100$
$t + s = -1$
So, $s = -1 - t$.

(c) 5x - 53y = 17.
We can use the extended Euclidean algorithm to find the modular inverse of 5 modulo 53.
$53 = 10 \cdot 5 + 3$
$5 = 1 \cdot 3 + 2$
$3 = 1 \cdot 2 + 1$
$1 = 3 - 1 \cdot 2$
$1 = 3 - 1 \cdot (5 - 1 \cdot 3)$
$1 = 2 \cdot 3 - 1 \cdot 5$
$1 = 2 \cdot (53 - 10 \cdot 5) - 1 \cdot 5$
$1 = 2 \cdot 53 - 21 \cdot 5$
So, the modular inverse of 5 modulo 53 is -21.

Now, we can find the solution to the equation:
$5x \equiv 17$ (mod 53)
$x \equiv 17 \cdot (-21)$ (mod 53)
$x \equiv -357$ (mod 53)
$x \equiv 1$ (mod 53)
$x = 1 + 53t$

Similarly, we can find the solution to the equation:
$-53y \equiv 17$ (mod 5)
$y \equiv 17 \cdot 1$ (mod 5)
$y \equiv 2$ (mod 5)
$y = 2 + 5s$

Substituting these into the equation, we get:
$5(1 + 53t) - 53(2 + 5s) = 17$
$5 + 265t - 106 - 265s = 17$
$265t - 265s = 76$
$t - s = 1$
So, $s = t - 1$.

In conclusion, the solutions to the Diophantine equations are:
(a) $x = 15 + 51t$, $y = 3 + 4s$, with $s = -1 - t$.
(b) $x = 33 + 25t$, $y = 7 + 12s$, with $s = -1 - t$.
(c) $x = 1 + 53t$, $y = 2 + 5s$, with $s = t - 1$.