 We have that
\[t_n = \frac{n(n + 1)}{2}.\]
We want to find when
\[t_1^2 + t_2^2 + \dots + t_n^2\]
is divisible by $t_n$.

We can rewrite the sum as
\[t_1^2 + t_2^2 + \dots + t_n^2 = \frac{1(1+1)^2}{4} + \frac{2(2+1)^2}{4} + \dots + \frac{n(n+1)^2}{4}.\]
This simplifies to
\[t_1^2 + t_2^2 + \dots + t_n^2 = \frac{1^2(1+1) + 2^2(2+1) + \dots + n^2(n+1)}{4}.\]
We can rewrite this as
\[t_1^2 + t_2^2 + \dots + t_n^2 = \frac{1^2(1+1) + 2^2(2+1) + \dots + n^2(n+1)}{4} = \frac{1^3 + 2^3 + \dots + n^3 + 1^2 + 2^2 + \dots + n^2}{4}.\]
We know that
\[1^3 + 2^3 + \dots + n^3 = \left(\frac{n(n+1)}{2}\right)^2 = t_n^2,\]
and
\[1^2 + 2^2 + \dots + n^2 = \frac{n(n+1)(2n+1)}{6}.\]
Therefore,
\[t_1^2 + t_2^2 + \dots + t_n^2 = \frac{t_n^2 + \frac{n(n+1)(2n+1)}{6}}{4}.\]
We want to find when $t_n$ divides this expression.

We can rewrite this as
\[t_1^2 + t_2^2 + \dots + t_n^2 = \frac{t_n^2 + \frac{n(n+1)(2n+1)}{6}}{4} = \frac{t_n^2}{4} + \frac{n(n+1)(2n+1)}{24}.\]
We want to find when $t_n$ divides this expression.

Since $t_n$ is a triangular number, it is of the form $\frac{n(n+1)}{2}$. Therefore, $t_n$ divides $t_n^2$ and $n(n+1)(2n+1)$.

Therefore, $t_n$ divides $t_1^2 + t_2^2 + \dots + t_n^2$ for all $n$.
The answer is $\boxed{all}$.