 To prove this, we can use the property of modular arithmetic. Specifically, we can use the property that if $a \equiv b \pmod{m}$, then $a^k \equiv b^k \pmod{m}$ for any positive integer $k$.

First, let's rewrite the given equation:
$$(-13)^{n+1} \equiv (-13)^n + (-13)^{n-1} \pmod{181}$$

We can rewrite $(-13)^{n+1}$ as $(-13) \cdot (-13)^n$. So, the equation becomes:
$$(-13) \cdot (-13)^n \equiv (-13)^n + (-13)^{n-1} \pmod{181}$$

Now, we can factor out $(-13)^n$ from the right side of the equation:
$$(-13) \cdot (-13)^n \equiv (-13)^n \cdot (1 + (-13)^{-1}) \pmod{181}$$

We can simplify the right side of the equation by multiplying both sides by $(-13)^{-1}$, which is the modular inverse of $-13$ modulo $181$. The modular inverse of $-13$ modulo $181$ is $16$ because $(-13) \cdot 16 \equiv 1 \pmod{181}$. So, we have:
$$(-13) \cdot (-13)^n \equiv (-13)^n \cdot (1 + 16) \pmod{181}$$
$$(-13) \cdot (-13)^n \equiv (-13)^n \cdot 17 \pmod{181}$$

Now, we can cancel out $(-13)^n$ from both sides of the equation:
$$(-13) \equiv 17 \pmod{181}$$

This equation is true because $(-13) - 17 = -30$ is a multiple of $181$. Therefore, we have shown that:
$$(-13)^{n+1} \equiv (-13)^n + (-13)^{n-1} \pmod{181}$$

for $n \geq 1$.