<think>
Okay, so I need to show that for any integer n ≥ 1, the equation (-13)^{n+1} ≡ (-13)^n + (-13)^{n-1} mod 181 holds. Hmm, let me start by recalling some modular arithmetic properties and maybe see if I can manipulate the equation to make it simpler.

First, let me write down the given congruence:

(-13)^{n+1} ≡ (-13)^n + (-13)^{n-1} mod 181.

I notice that both sides have terms with exponents involving n. Maybe I can factor out some common terms on the right-hand side. Let me try that.

On the right-hand side, we have (-13)^n + (-13)^{n-1}. Let me factor out (-13)^{n-1} from both terms:

(-13)^{n-1} [ (-13)^1 + 1 ].

Calculating the bracketed term: (-13) + 1 = -12. So the right-hand side becomes (-13)^{n-1} * (-12).

Therefore, the equation simplifies to:

(-13)^{n+1} ≡ (-13)^{n-1} * (-12) mod 181.

Now, let me look at the left-hand side: (-13)^{n+1}. I can write this as (-13)^{n-1} * (-13)^2. Since exponents add when multiplying, so (-13)^{n-1} * (-13)^2 = (-13)^{n+1}.

Therefore, substituting back into the equation:

(-13)^{n-1} * (-13)^2 ≡ (-13)^{n-1} * (-12) mod 181.

Since (-13)^{n-1} is common on both sides, assuming it's not congruent to 0 mod 181, I can divide both sides by (-13)^{n-1}. However, I need to be careful here. Dividing in modular arithmetic is equivalent to multiplying by the modular inverse. But since 181 is a prime number (I think it is; let me check: 181 is not divisible by 2, 3, 5, 7, 11, 13... sqrt(181) is about 13.4, so primes up to 13. 13*13 is 169, 13*14 is 182, so yes, 181 is prime). Therefore, since (-13) and 181 are coprime (because 13 is less than 181 and 13 doesn't divide 181), so (-13)^{n-1} is invertible mod 181. Therefore, we can safely divide both sides by (-13)^{n-1}.

So dividing both sides by (-13)^{n-1} gives:

(-13)^2 ≡ -12 mod 181.

Calculating (-13)^2: that's 169. So:

169 ≡ -12 mod 181.

Now, let's check if this is true. Let me compute -12 mod 181. Since -12 + 181 = 169. So indeed, -12 ≡ 169 mod 181. Therefore, 169 ≡ -12 mod 181 is true. Therefore, the original equation reduces to a true statement, which means that the original congruence holds for all n ≥ 1.

Wait, so does that mean that the original equation is equivalent to 169 ≡ -12 mod 181, which is true? Therefore, for all n ≥ 1, the congruence holds?

But let me check with a specific example to make sure. Let me take n=1. Then the left-hand side is (-13)^{2} = 169. The right-hand side is (-13)^1 + (-13)^{0} = -13 + 1 = -12. Then 169 ≡ -12 mod 181? As before, yes, because 169 + 12 = 181, so 169 ≡ -12 mod 181. So that works.

Let me check n=2. Left-hand side: (-13)^{3} = -2197. Right-hand side: (-13)^2 + (-13)^1 = 169 -13 = 156. Now, compute -2197 mod 181 and 156 mod 181.

First, compute 156 mod 181 is 156. Now compute -2197 mod 181. Let me divide 2197 by 181 to find the remainder.

First, compute how many times 181 goes into 2197.

Calculate 181 * 12 = 2172. Then 2197 - 2172 = 25. So 2197 = 181*12 + 25. Therefore, -2197 ≡ -25 mod 181. But -25 mod 181 is 181 -25 = 156. Therefore, -2197 ≡ 156 mod 181. Which matches the right-hand side. So that works.

Another check with n=3. Left-hand side: (-13)^4 = 28561. Right-hand side: (-13)^3 + (-13)^2 = -2197 + 169 = -2028. Let me compute both mod 181.

First, compute 28561 mod 181. Let me see if there's a smarter way than dividing 28561 by 181. Alternatively, since we know that (-13)^{n+1} ≡ (-13)^n + (-13)^{n-1} mod 181, and we already checked n=1 and n=2, maybe we can use the recurrence relation.

But let me do it directly. Let me compute (-13)^4 mod 181. Since (-13)^2 is 169 ≡ -12 mod 181. Then (-13)^3 ≡ (-13)^2 * (-13) ≡ (-12)*(-13) mod 181. Let me compute that: (-12)*(-13) = 156. Then (-13)^4 ≡ (-13)^3 * (-13) ≡ 156*(-13) mod 181. Let me compute 156*(-13). 156*13 = 2028. Then 2028 mod 181. Let me divide 2028 by 181.

Earlier, 181*12 = 2172, which is more than 2028. Let me compute 181*11 = 1991. Then 2028 - 1991 = 37. Therefore, 2028 ≡ 37 mod 181. Therefore, (-13)^4 ≡ -37 mod 181? Wait, no. Wait, 156*(-13) = -2028. So -2028 mod 181 is - (2028 mod 181). Since 2028 mod 181 is 37, so -2028 mod 181 is -37 mod 181. Which is 181 - 37 = 144. Therefore, (-13)^4 ≡ 144 mod 181.

Now the right-hand side for n=3 is (-13)^3 + (-13)^2 ≡ 156 + (-12) mod 181? Wait, no. Wait, (-13)^3 is -2197 ≡ 156 mod 181 as before, and (-13)^2 is 169 ≡ -12 mod 181. So adding them: 156 + (-12) = 144 mod 181. Which matches the left-hand side. So that works too.

Therefore, the congruence seems to hold for n=1, 2, 3. So my initial reasoning seems correct. Therefore, the original equation reduces to (-13)^2 ≡ -12 mod 181, which is true because (-13)^2 is 169 and 169 ≡ -12 mod 181 (since 169 + 12 = 181). Therefore, the congruence holds for all n ≥ 1.

But just to make sure, let me think if there's another way to approach this. Maybe by using the concept of linear recursions or something else? The given congruence resembles a linear recurrence relation. For example, if we consider the sequence a_n = (-13)^n mod 181, then the equation is a_{n+1} ≡ a_n + a_{n-1} mod 181. So this is like a Fibonacci-like recurrence. But why is this true?

Well, if we can show that the characteristic equation of this recurrence has roots related to -13? Wait, but maybe that's complicating things. Alternatively, since we have shown that the equation reduces to (-13)^2 ≡ -12 mod 181, which is true, then the recurrence is satisfied for all n because the relation is linear and the initial terms satisfy it. Wait, but actually, the recurrence is valid for all n ≥ 1 if the base case holds. Since we checked n=1 and n=2, and the recurrence is linear, then by induction, it would hold for all n.

But since we have already shown that the equation reduces to a true statement, which is independent of n, then the congruence holds for all n ≥ 1. Therefore, the original statement is proven.

Alternatively, another way to think about it is to note that if we have a_n = (-13)^n, then the given equation is a_{n+1} = a_n + a_{n-1} mod 181. So if we can show that (-13)^{n+1} - (-13)^n - (-13)^{n-1} ≡ 0 mod 181. Factoring out (-13)^{n-1}, we get (-13)^{n-1} [ (-13)^2 - (-13) - 1 ] ≡ 0 mod 181. Therefore, since (-13)^{n-1} is invertible mod 181, this reduces to (-13)^2 - (-13) - 1 ≡ 0 mod 181. Let me compute that:

(-13)^2 - (-13) - 1 = 169 +13 -1 = 181. So 181 ≡ 0 mod 181. Which is true. Therefore, the expression is 0 mod 181. Therefore, the original congruence holds for all n ≥ 1.

Yes, that's another way to see it. So by factoring the expression, we see that the entire expression is a multiple of 181, hence congruent to 0 mod 181. Therefore, the congruence holds.

Therefore, regardless of the value of n, the equation is satisfied because the coefficient in front of (-13)^{n-1} is 181, which is 0 mod 181. Therefore, the original congruence is true for all n ≥ 1.

So, in summary, the key step was to factor the equation and realize that the resulting expression simplifies to 181, which is 0 mod 181, hence proving the congruence holds for all n ≥ 1. The checks with specific values of n also confirm that the congruence is valid. Therefore, the statement is proven.

**Final Answer**
\boxed{(-13)^{n+1} \equiv (-13)^n + (-13)^{n-1} \pmod{181}}
</think>

To prove that for all integers $ n \geq 1 $, the congruence
$$
(-13)^{n+1} \equiv (-13)^n + (-13)^{n-1} \pmod{181}
$$
holds, we proceed by algebraic manipulation and modular arithmetic reasoning.

---

### Step 1: Factor the Right-Hand Side

We begin by factoring the right-hand side of the congruence:

$$
(-13)^n + (-13)^{n-1} = (-13)^{n-1} \cdot [(-13) + 1] = (-13)^{n-1} \cdot (-12)
$$

So the equation becomes:

$$
(-13)^{n+1} \equiv (-13)^{n-1} \cdot (-12) \pmod{181}
$$

---

### Step 2: Express the Left-Hand Side

Now, express the left-hand side using exponent rules:

$$
(-13)^{n+1} = (-13)^{n-1} \cdot (-13)^2
$$

So the equation becomes:

$$
(-13)^{n-1} \cdot (-13)^2 \equiv (-13)^{n-1} \cdot (-12) \pmod{181}
$$

---

### Step 3: Cancel Common Factor

Since $ (-13)^{n-1} $ is invertible modulo 181 (as 181 is prime and $ -13 \not\equiv 0 \pmod{181} $), we can safely divide both sides by $ (-13)^{n-1} $:

$$
(-13)^2 \equiv -12 \pmod{181}
$$

Now compute both sides:

- $ (-13)^2 = 169 $
- $ -12 \equiv 169 \pmod{181} $, since $ 169 + 12 = 181 $

Thus, the congruence:

$$
(-13)^2 \equiv -12 \pmod{181}
$$

is **true**, and this is independent of $ n $.

---

### Step 4: Conclusion

Since the reduced congruence $ (-13)^2 \equiv -12 \pmod{181} $ is true, and the original equation simplifies to it, the original congruence

$$
(-13)^{n+1} \equiv (-13)^n + (-13)^{n-1} \pmod{181}
$$

holds for **all** $ n \geq 1 $, as the reduction is valid for any $ n $, and the result is independent of $ n $.

---

### Final Answer

$$
\boxed{(-13)^{n+1} \equiv (-13)^n + (-13)^{n-1} \pmod{181}}
$$