 To prove this identity, we can use the sum-to-product identities for cosine. The sum-to-product identities are:

1. $\cos{a} + \cos{b} = 2\cos{\frac{a+b}{2}}\cos{\frac{a-b}{2}}$
2. $\cos{a} - \cos{b} = -2\sin{\frac{a+b}{2}}\sin{\frac{a-b}{2}}$

We can rewrite the given expression as:

$\cos{\frac{\pi}{7}}-\cos{\frac{2\pi}{7}}+\cos{\frac{3\pi}{7}} = 2\cos{\frac{\pi}{7}}\cos{\frac{\pi}{7}} - 2\sin{\frac{3\pi}{7}}\sin{\frac{\pi}{7}}$

Now, we can use the Pythagorean identity $\sin^2{x} + \cos^2{x} = 1$ to simplify the expression:

$2\cos^2{\frac{\pi}{7}} - 2\sin^2{\frac{\pi}{7}} = 2(\cos^2{\frac{\pi}{7}} - \sin^2{\frac{\pi}{7}})$

We know that $\cos^2{x} - \sin^2{x} = \cos{2x}$, so we can substitute this into the expression:

$2\cos{2\cdot\frac{\pi}{7}} = 2\cos{\frac{2\pi}{7}}$

Now, we can use the double-angle identity for cosine, which is $\cos{2x} = 2\cos^2{x} - 1$:

$2(2\cos^2{\frac{\pi}{7}} - 1) = 4\cos^2{\frac{\pi}{7}} - 2$

We know that $\cos{\frac{\pi}{7}} = \frac{1}{2}$, so we can substitute this into the expression:

$4\left(\frac{1}{2}\right)^2 - 2 = 4\cdot\frac{1}{4} - 2 = 1 - 2 = -\frac{1}{2}$

However, the given expression is $\cos{\frac{\pi}{7}}-\cos{\frac{2\pi}{7}}+\cos{\frac{3\pi}{7}}$, not $4\cos^2{\frac{\pi}{7}} - 2$. Therefore, the given identity is incorrect.