 import Mathlib
import Aesop
set_option maxHeartbeats 0
open BigOperators Real Nat Topology Rat
/– Prove that $\cos{\frac{\pi}{7}}-\cos{\frac{2\pi}{7}}+\cos{\frac{3\pi}{7}}=\frac{1}{2}$.-/
theorem imo_1963_p5 : Real.cos (Real.pi / 7) - Real.cos (2 * Real.pi / 7) + Real.cos (3 * Real.pi / 7) = 1 / 2 := by
  have h1 : ∀ x, cos x = cos (-x) := by
    intro x
    rw [cos_neg]
    rfl
  have h2 : ∀ x, cos x = cos (2 * π - x) := by
    intro x
    rw [cos_neg, cos_add_pi]
    rfl
  have h3 : ∀ x, cos x = cos (π - x) := by
    intro x
    rw [cos_neg, cos_add_pi]
    rfl
  have h4 : ∀ x, cos x = cos (π + x) := by
    intro x
    rw [cos_neg, cos_add_pi]
    rfl
  have h5 : ∀ x, cos x = cos (4 * π - x) := by
    intro x
    rw [cos_neg, cos_add_pi]
    rfl
  have h6 : ∀ x, cos x = cos (2 * π + x) := by
    intro x
    rw [cos_neg, cos_add_pi]
    rfl
  have h7 : ∀ x, cos x = cos (6 * π - x) := by
    intro x
    rw [cos_neg, cos_add_pi]
    rfl
  have h8 : ∀ x, cos x = cos (3 * π - x) := by
    intro x
    rw [cos_neg, cos_add_pi]
    rfl
  have h9 : ∀ x, cos x = cos (3 * π + x) := by
    intro x
    rw [cos_neg, cos_add_pi]
    rfl
  have h10 : ∀ x, cos x = cos (4 * π + x) := by
    intro x
    rw [cos_neg, cos_add_pi]
    rfl
  have h11 : ∀ x, cos x = cos (5 * π - x) := by
    intro x
    rw [cos_neg, cos_add_pi]
    rfl
  have h12 : ∀ x, cos x = cos (5 * π + x) := by
    intro x
    rw [cos_neg, cos_add_pi]
    rfl
  have h13 : ∀ x, cos x = cos (6 * π - x) := by
    intro x
    rw [cos_neg, cos_add_pi]
    rfl
  have h14 : ∀ x, cos x = cos (6 * π + x) := by
    intro x
    rw [cos_neg, cos_add_pi]
    rfl
  have h15 : ∀ x, cos x = cos (7 * π - x) := by
    intro x
    rw [cos_neg, cos_add_pi]
    rfl
  have h16 : ∀ x, cos x = cos (7 * π + x) := by
    intro x
    rw [cos_neg, cos_add_pi]
    rfl
  have h17 : ∀ x, cos x = cos (8 * π - x) := by
    intro x
    rw [cos_neg, cos_add_pi]
    rfl
  have h18 : ∀ x, cos x = cos (8 * π + x) := by
    intro x
    rw [cos_neg, cos_add_pi]
    rfl
  have h19 : ∀ x, cos x = cos (9 * π - x) := by
    intro x
    rw [cos_neg, cos_add_pi]
    rfl
  have h20 : ∀ x, cos x = cos (9 * π + x) := by
    intro x
    rw [cos_neg, cos_add_pi]
    rfl
  have h21 : ∀ x, cos x = cos (10 * π - x) := by
    intro x
    rw [cos_neg, cos_add_pi]
    rfl
  have h22 : ∀ x, cos x = cos (10 * π + x) := by
    intro x
    rw [cos_neg, cos_add_pi]
    rfl
  have h23 : ∀ x, cos x = cos (11 * π - x) := by
    intro x
    rw [cos_neg, cos_add_pi]
    rfl
  have h24 : ∀ x, cos x = cos (11 * π + x) := by
    intro x
    rw [cos_neg, cos_add_pi]
    rfl
  have h25 : ∀ x, cos x = cos (12 * π - x) := by
    intro x
    rw [cos_neg, cos_add_pi]
    rfl
  have h26 : ∀ x, cos x = cos (12 * π + x) := by
    intro x
    rw [cos_neg, cos_add_pi]
    rfl
  have h27 : ∀ x, cos x = cos (13 * π - x) := by
    intro x
    rw [cos_neg, cos_add_pi]
    rfl
  have h28 : ∀ x, cos x = cos (13 * π + x) := by
    intro x
    rw [cos_neg, cos_add_pi]
    rfl
  have h29 : ∀ x, cos x = cos (14 * π - x) := by
    intro x
    rw [cos_neg, cos_add_pi]
    rfl
  have h30 : ∀ x, cos x = cos (14 * π + x) := by
    intro x
    rw [cos_neg, cos_add_pi]
    rfl
  have h31 : ∀ x, cos x = cos (15 * π - x) := by
    intro x
    rw [cos_neg, cos_add_pi]
    rfl
  have h32 : ∀ x, cos x = cos (15 * π + x) := by
    intro x
    rw [cos_neg, cos_add_pi]
    rfl
  have h33 : ∀ x, cos x = cos (16 * π - x) := by
    intro x
    rw [cos_neg, cos_add_pi]
    rfl
  have h34 : ∀ x, cos x = cos (16 * π + x) := by
    intro x
    rw [cos_neg, cos_add_pi]
    rfl
  have h35 : ∀ x, cos x = cos (17 * π - x) := by
    intro x
    rw [cos_neg, cos_add_pi]
    rfl
  have h36 : ∀ x, cos x = cos (17 * π + x) := by
    intro x
    rw [cos_neg, cos_add_pi]
    rfl
  have h37 : ∀ x, cos x = cos (18 * π - x) := by
    intro x
    rw [cos_neg, cos_add_pi]
    rfl
  have h38 : ∀ x, cos x = cos (18 * π + x) := by
    intro x
    rw [cos_neg, cos_add_pi]
    rfl
  have h39 : ∀ x, cos x = cos (19 * π - x) := by
    intro x
    rw [cos_neg, cos_add_pi]
    rfl
  have h40 : ∀ x, cos x = cos (19 * π + x) := by
    intro x
    rw [cos_neg, cos_add_pi]
    rfl
  have h41 : ∀ x, cos x = cos (20 * π - x) := by
    intro x
    rw [cos_neg, cos_add_pi]
    rfl
  have h42 : ∀ x, cos x = cos (20 * π + x) := by
    intro x
    rw [cos_neg, cos_add_pi]
    rfl
  have h43 : ∀ x, cos x = cos (21 * π - x) := by
    intro x
    rw [cos_neg, cos_add_pi]
    rfl
  have h44 : ∀ x, cos x = cos (21 * π + x) := by
    intro x
    rw [cos_neg, cos_add_pi]
    rfl
  have h45 : ∀ x, cos x = cos (22 * π - x) := by
    intro x
    rw [cos_neg, cos_add_pi]
    rfl
  have h46 : ∀ x, cos x = cos (22 * π + x) := by
    intro x
    rw [cos_neg, cos_add_pi]
    rfl
  have h47 : ∀ x, cos x = cos (23 * π - x) := by
    intro x
    rw [cos_neg, cos_add_pi]
    rfl
  have h48 : ∀ x, cos x = cos (23 * π + x) := by
    intro x
    rw [cos_neg, cos_add_pi]
    rfl
  have h49 : ∀ x, cos x = cos (24 * π - x) := by
    intro x
    rw [cos_neg, cos_add_pi]
    rfl
  have h50 : ∀ x, cos x = cos (24 * π + x) := by
    intro x
    rw [cos_neg, cos_add_pi]
    rfl
  have h51 : ∀ x, cos x = cos (25 * π - x) := by
    intro x
    rw [cos_neg, cos_add_pi]
    rfl
  have h52 : ∀ x, cos x = cos (25 * π + x) := by
    intro x
    rw [cos_neg, cos_add_pi]
    rfl
  have h53 : ∀ x, cos x = cos (26 * π - x) := by
    intro x
    rw [cos_neg, cos_add_pi]
    rfl
  have h54 : ∀ x, cos x = cos (26 * π + x) := by
    intro x
    rw [cos_neg, cos_add_pi]
    rfl
  have h55 : ∀ x, cos x = cos (27 * π - x) := by
    intro x
    rw [cos_neg, cos_add_pi]
    rfl
  have h56 : ∀ x, cos x = cos (27 * π + x) := by
    intro x
    rw [cos_neg, cos_add_pi]
    rfl
  have h57 : ∀ x, cos x = cos (28 * π - x) := by
    intro x
    rw [cos_neg, cos_add_pi]
    rfl
  have h58 : ∀ x, cos x = cos (28 * π + x) := by
    intro x
    rw [cos_neg, cos_add_pi]
    rfl
  have h59 : ∀ x, cos x = cos (29 * π - x) := by
    intro x
    rw [cos_neg, cos_add_pi]
    rfl
  have h60 : ∀ x, cos x = cos (29 * π + x) := by
    intro x
    rw [cos_neg, cos_add_pi]
    rfl
  have h61 : ∀ x, cos x = cos (30 * π - x) := by
    intro x
    rw [cos