<think>
Okay, so I need to show that for any integer n ≥ 1, the congruence (-13)^{n+1} ≡ (-13)^n + (-13)^{n-1} mod 181 holds. Hmm, let me start by recalling some modular arithmetic properties. Maybe I can manipulate the equation algebraically first and then check if it holds modulo 181.

First, let me write down the given congruence:

(-13)^{n+1} ≡ (-13)^n + (-13)^{n-1} mod 181.

I need to verify that this is true for all n ≥ 1. Let me try to simplify the left-hand side (LHS) and the right-hand side (RHS) to see if they are congruent modulo 181.

Starting with the LHS: (-13)^{n+1} can be written as (-13)^n * (-13). Similarly, the RHS is (-13)^n + (-13)^{n-1}. Let me factor out (-13)^{n-1} from the RHS. Let me see:

RHS = (-13)^n + (-13)^{n-1} = (-13)^{n-1} * [(-13) + 1]. Wait, because (-13)^n is (-13)^{n-1} * (-13), right? So factoring out (-13)^{n-1} gives:

(-13)^{n-1} * [(-13) + 1] = (-13)^{n-1} * (-12). 

So the RHS simplifies to (-13)^{n-1} * (-12). 

Now, the LHS is (-13)^{n+1} = (-13)^n * (-13) = (-13)^{n-1} * (-13)^2 * (-13) = (-13)^{n-1} * (-13)^3. Wait, maybe that's complicating things. Let me think again.

Alternatively, since LHS is (-13)^{n+1} and RHS is (-13)^n + (-13)^{n-1}, maybe I can divide both sides by (-13)^{n-1} to simplify? Let's try that.

Dividing both sides by (-13)^{n-1}:

Left side becomes (-13)^{n+1} / (-13)^{n-1} = (-13)^{(n+1)-(n-1)} = (-13)^2 = 169.

Right side becomes [(-13)^n + (-13)^{n-1}] / (-13)^{n-1} = (-13)^n / (-13)^{n-1} + (-13)^{n-1}/(-13)^{n-1} = (-13) + 1 = -12.

So, according to this, we have 169 ≡ -12 mod 181. Is that true? Let me check.

Compute 169 + 12 = 181. Therefore, 169 ≡ -12 mod 181 because 169 + 12 = 181, which is 0 mod 181. Therefore, 169 ≡ -12 mod 181. Therefore, the equation holds. 

Therefore, if we divide both sides by (-13)^{n-1}, which is allowed as long as (-13)^{n-1} is invertible modulo 181. But since 181 is a prime number, and -13 is not a multiple of 181 (since 181 is prime and 13 < 181), so -13 and 181 are coprime. Therefore, (-13)^{n-1} is invertible modulo 181. Therefore, dividing both sides by it is allowed. Therefore, the original congruence is equivalent to 169 ≡ -12 mod 181, which is true because 169 + 12 = 181. Therefore, the original congruence holds for all n ≥ 1.

Wait, but let me check with specific values of n to make sure. Let's take n=1.

For n=1:

LHS: (-13)^{1+1} = (-13)^2 = 169.

RHS: (-13)^1 + (-13)^{0} = -13 + 1 = -12.

Now, check if 169 ≡ -12 mod 181. As before, 169 + 12 = 181, so yes, 169 ≡ -12 mod 181. So that works.

Check n=2:

LHS: (-13)^{3} = (-13)^2 * (-13) = 169 * (-13) = -2197.

RHS: (-13)^2 + (-13)^1 = 169 + (-13) = 156.

Now compute -2197 mod 181 and 156 mod 181.

First, let's compute 181*12 = 2172. 2172 - 2197 = -25. Wait, but that's not helpful. Alternatively, let me compute -2197 divided by 181.

Alternatively, note that 181*12 = 2172. Then 2172 + 181 = 2353. Wait, maybe better to compute 2197 divided by 181.

Let me compute 181 * 12 = 2172. 2197 - 2172 = 25. Therefore, 2197 ≡ 25 mod 181. Therefore, -2197 ≡ -25 mod 181. Which is equivalent to 181 -25 = 156 mod 181. Therefore, LHS is -2197 ≡ 156 mod 181. RHS is 156. Therefore, they are congruent. So that works.

Another check with n=2, LHS ≡ RHS mod 181. So that works.

Another check with n=3:

LHS: (-13)^4 = [(-13)^2]^2 = 169^2. Let me compute 169^2 mod 181.

But 169 ≡ -12 mod 181, so (-12)^2 = 144 mod 181.

RHS: (-13)^3 + (-13)^2 = (-2197) + 169. Earlier we saw that -2197 ≡ 156 mod 181, and 169 is 169. So 156 + 169 = 325. Now compute 325 mod 181. 181*1=181, 325-181=144. Therefore, RHS ≡ 144 mod 181. Which matches the LHS. Therefore, that works.

Therefore, the congruence holds for n=1,2,3. So the general case seems to hold.

Alternatively, maybe I can think of this as a recurrence relation. Let me think.

Let me denote a_n = (-13)^n. Then the given congruence is a_{n+1} ≡ a_n + a_{n-1} mod 181.

But if I look at the recurrence relation a_{n+1} - a_n - a_{n-1} ≡ 0 mod 181. So this is a linear recurrence relation. If I can show that this recurrence holds for the sequence a_n = (-13)^n, then it's proven.

But why would that recurrence hold? Well, if we think of the characteristic equation for the recurrence relation. For a linear recurrence relation like a_{n+1} - a_n - a_{n-1} = 0, the characteristic equation is r^2 - r - 1 = 0. However, our sequence a_n is defined as (-13)^n, so if this sequence satisfies the recurrence, then the characteristic equation must have r = -13 as a root. Let me check.

Let me plug r = -13 into the characteristic equation: (-13)^2 - (-13) - 1 = 169 +13 -1 = 181. Which is 0 mod 181. Therefore, since 181 ≡ 0 mod 181, then r = -13 is indeed a root of the characteristic equation modulo 181. Therefore, the recurrence relation a_{n+1} - a_n - a_{n-1} ≡ 0 mod 181 holds for the sequence a_n = (-13)^n. Therefore, the original congruence is satisfied.

Therefore, this is another way to see it. Since the characteristic equation has r = -13 as a root, the sequence defined by a_n = (-13)^n satisfies the recurrence relation. Therefore, the congruence holds.

Alternatively, since we saw that dividing both sides by (-13)^{n-1} gives 169 ≡ -12 mod 181, which is true because 169 + 12 = 181, which is 0 mod 181. Therefore, the congruence holds for all n ≥ 1.

Therefore, the original statement is proven.

But let me check once more for n=1,2,3 as before, and maybe n=4 to be thorough.

For n=4:

LHS: (-13)^5. Let me compute this mod 181.

Alternatively, since we know that a_{n+1} ≡ a_n + a_{n-1}, so for n=3, a_4 ≡ a_3 + a_2. From previous calculations:

a_3 = (-13)^3 ≡ -2197 ≡ 156 mod 181.

a_2 = 169.

Therefore, a_4 ≡ 156 + 169 = 325 ≡ 325 - 181 = 144 mod 181. Which is same as (-13)^4 ≡ 144 mod 181. Alternatively, (-13)^4 = (169)^2. Since 169 ≡ -12 mod 181, so (-12)^2 = 144 mod 181. Correct.

Now, compute LHS for n=4: (-13)^{5} = (-13)^4 * (-13) ≡ 144 * (-13) mod 181.

Compute 144 * (-13) = -1872. Now compute -1872 mod 181.

First, compute how many times 181 goes into 1872.

Calculate 181 * 10 = 1810. 1872 - 1810 = 62. Therefore, 1872 ≡ 62 mod 181. Therefore, -1872 ≡ -62 mod 181. Which is equivalent to 181 - 62 = 119 mod 181.

Now, compute RHS for n=4: a_4 + a_3 = 144 + 156 = 300. 300 mod 181: 181*1=181, 300 - 181 = 119. Therefore, RHS is 119 mod 181. Which matches LHS. Therefore, congruence holds for n=4.

Therefore, this seems consistent.

Therefore, the conclusion is that the congruence holds for all n ≥ 1 because the equation reduces to 169 ≡ -12 mod 181, which is true, and dividing by (-13)^{n-1} is valid because -13 is invertible mod 181.

Alternatively, another way is to note that the original congruence is equivalent to (-13)^{n+1} - (-13)^n - (-13)^{n-1} ≡ 0 mod 181. Factor out (-13)^{n-1}:

(-13)^{n-1} [ (-13)^2 - (-13) - 1 ] ≡ 0 mod 181.

Compute the bracket term: (-13)^2 - (-13) - 1 = 169 +13 -1 = 181. Therefore, the bracket term is 181, which is 0 mod 181. Therefore, the entire expression is 0 mod 181. Therefore, the congruence holds for all n ≥ 1.

Yes, this is a more straightforward algebraic approach. So, factoring:

(-13)^{n+1} - (-13)^n - (-13)^{n-1} = (-13)^{n-1} [ (-13)^2 - (-13) - 1 ] = (-13)^{n-1} [ 169 +13 -1 ] = (-13)^{n-1} * 181. Therefore, since 181 ≡ 0 mod 181, the entire expression is 0 mod 181. Therefore, the original congruence holds for all n ≥ 1.

This seems like the most straightforward way. Therefore, the answer is proven.

**Final Answer**
\boxed{(-13)^{n+1} \equiv (-13)^n + (-13)^{n-1} \pmod{181}}
</think>

To show that for all integers $ n \geq 1 $, the congruence

$$
(-13)^{n+1} \equiv (-13)^n + (-13)^{n-1} \pmod{181}
$$

holds, we proceed by analyzing the structure of the expression algebraically and verifying its validity under modular arithmetic.

---

### Step 1: Express the Left-Hand Side (LHS)

We begin by expressing the LHS:

$$
(-13)^{n+1} = (-13)^n \cdot (-13)
$$

---

### Step 2: Express the Right-Hand Side (RHS)

We now express the RHS:

$$
(-13)^n + (-13)^{n-1} = (-13)^{n-1} \cdot (-13 + 1) = (-13)^{n-1} \cdot (-12)
$$

---

### Step 3: Compare LHS and RHS

We now compare the two expressions:

- LHS: $ (-13)^{n+1} = (-13)^n \cdot (-13) $
- RHS: $ (-13)^n + (-13)^{n-1} = (-13)^{n-1} \cdot (-12) $

We can factor out $ (-13)^{n-1} $ from both sides to simplify:

$$
\frac{(-13)^{n+1}}{(-13)^{n-1}} = (-13)^2 = 169
$$
$$
\frac{(-13)^n + (-13)^{n-1}}{(-13)^{n-1}} = (-13) + 1 = -12
$$

Thus, the congruence is equivalent to:

$$
169 \equiv -12 \pmod{181}
$$

---

### Step 4: Verify the Congruence

We check whether $ 169 \equiv -12 \pmod{181} $:

$$
169 + 12 = 181 \Rightarrow 169 \equiv -12 \pmod{181}
$$

This is indeed true. Therefore, the original congruence holds for all $ n \geq 1 $, provided that $ (-13)^{n-1} $ is invertible modulo 181.

Since 181 is prime and $ -13 \not\equiv 0 \pmod{181} $, the number $ (-13)^{n-1} $ is invertible modulo 181 for all $ n \geq 1 $. Thus, the division step is valid.

---

### Step 5: General Proof via Factoring

We can also write the original congruence as:

$$
(-13)^{n+1} - (-13)^n - (-13)^{n-1} \equiv 0 \pmod{181}
$$

Factoring out $ (-13)^{n-1} $, we get:

$$
(-13)^{n-1} \left[ (-13)^2 - (-13) - 1 \right] \equiv 0 \pmod{181}
$$

Now compute the bracketed term:

$$
(-13)^2 - (-13) - 1 = 169 + 13 - 1 = 181
$$

So the entire expression becomes:

$$
(-13)^{n-1} \cdot 181 \equiv 0 \pmod{181}
$$

Which is clearly true, since 181 is the modulus. Therefore, the congruence holds for all $ n \geq 1 $.

---

### Final Conclusion

The congruence

$$
(-13)^{n+1} \equiv (-13)^n + (-13)^{n-1} \pmod{181}
$$

is valid for all integers $ n \geq 1 $, as shown through both algebraic manipulation and modular arithmetic verification.

$$
\boxed{(-13)^{n+1} \equiv (-13)^n + (-13)^{n-1} \pmod{181}}
$$