<think>
Okay, so I need to prove that cos(π/7) - cos(2π/7) + cos(3π/7) equals 1/2. Hmm, trigonometric identities can be tricky, especially with angles that are multiples of π/7. Let me think about how to approach this.

First, I remember that sometimes with trigonometric equations involving multiple angles, it's helpful to use complex numbers or roots of unity. Maybe I can relate this to the 7th roots of unity? Let me recall that the 7th roots of unity are solutions to the equation z^7 = 1. These roots are e^(2πik/7) for k = 0, 1, 2, ..., 6. But the angles here are π/7, 2π/7, etc., which are half of those. Maybe I need to consider something else?

Alternatively, perhaps I can use some trigonometric identities to combine these terms. Let me write down the expression again:

cos(π/7) - cos(2π/7) + cos(3π/7). 

I need to show that this equals 1/2. Maybe I can combine the cosines using sum-to-product formulas or something similar. Let me recall that cos A - cos B = -2 sin[(A+B)/2] sin[(A-B)/2]. But here, there are three terms. Maybe I can group them in a way that allows me to apply such identities.

Alternatively, maybe I can consider the sum of cosines with angles in arithmetic progression? Wait, π/7, 2π/7, 3π/7... but the signs are different. The first term is positive, the second is negative, the third is positive. So it's not a straightforward arithmetic progression.

Alternatively, maybe I can think of this as the real part of some complex exponentials. Let me try that approach.

Let me denote z = e^(iπ/7). Then, z^7 = e^(iπ) = -1. So z^14 = 1. Therefore, z is a primitive 14th root of unity. But maybe that's complicating things. Alternatively, since the angles are π/7, 2π/7, etc., which are half of the angles in the 14th roots of unity. Maybe I need to think about that.

Alternatively, perhaps I can use the identity for the sum of cosines. Let me recall that the sum of cos(kπ/n) for certain k can sometimes be evaluated using known formulas. But here, the signs are mixed.

Alternatively, maybe I can square the expression? Let me try that. Let me denote S = cos(π/7) - cos(2π/7) + cos(3π/7). Then, maybe compute S^2 and see if it relates to something?

But that might get complicated. Alternatively, maybe I can use known values or relationships between these cosines. For example, I remember that cos(π/7), cos(3π/7), and cos(5π/7) are related to the roots of some cubic equation. Maybe that's a direction.

Let me recall that cos(π/7), cos(3π/7), and cos(5π/7) are roots of the equation 8x³ - 4x² - 4x + 1 = 0. Wait, is that correct? Let me check. If I consider the minimal polynomial for cos(2π/7), it's a cubic equation. But here, the angles are π/7, 3π/7, 5π/7. Let me verify.

Alternatively, perhaps I can use the identity for multiple angles. For example, using the formula for cos(7θ) and setting θ = π/7. Let me try that.

We know that cos(7θ) = -1 when θ = π/7, since cos(π) = -1. So, expanding cos(7θ) using multiple-angle formulas. Let me recall that cos(7θ) can be expressed in terms of cosθ. But that might be complicated, but maybe manageable.

Alternatively, using De Moivre's theorem: (cosθ + i sinθ)^7 = cos7θ + i sin7θ. Expanding the left side using binomial theorem and equating real parts. Let me try that.

Let me set θ = π/7. Then, cos7θ = cosπ = -1. So, expanding (cosθ + i sinθ)^7:

Using binomial theorem:

cos^7θ + 7cos^6θ(i sinθ) + 21cos^5θ(i sinθ)^2 + 35cos^4θ(i sinθ)^3 + 35cos^3θ(i sinθ)^4 + 21cos^2θ(i sinθ)^5 + 7cosθ(i sinθ)^6 + (i sinθ)^7.

Taking the real part, which is cos7θ = -1. The real parts come from the even powers of i sinθ. Let me compute each term:

Real parts:

cos^7θ + 21cos^5θ(-sin²θ) + 35cos^3θ(sin^4θ) + 7cosθ(-sin^6θ).

So:

cos7θ = cos^7θ - 21cos^5θ sin²θ + 35cos^3θ sin^4θ - 7cosθ sin^6θ = -1.

But this seems complicated. Maybe we can express this in terms of cosθ. Let me recall that sin²θ = 1 - cos²θ, so maybe substitute that in.

But this seems very involved. However, perhaps if I divide both sides by cos^7θ, or something like that. Alternatively, maybe I can write everything in terms of cosθ. Let me denote x = cosθ. Then, sin²θ = 1 - x², sin^4θ = (1 - x²)^2, sin^6θ = (1 - x²)^3.

So substituting:

x^7 - 21x^5(1 - x²) + 35x^3(1 - x²)^2 - 7x(1 - x²)^3 = -1.

Let me expand each term:

First term: x^7.

Second term: -21x^5 + 21x^7.

Third term: 35x^3(1 - 2x² + x^4) = 35x^3 - 70x^5 + 35x^7.

Fourth term: -7x(1 - 3x² + 3x^4 - x^6) = -7x + 21x^3 - 21x^5 + 7x^7.

Now, combining all terms:

x^7 + (-21x^5 + 21x^7) + (35x^3 - 70x^5 + 35x^7) + (-7x + 21x^3 - 21x^5 + 7x^7) = -1.

Let me combine like terms:

First, x^7 terms:

1x^7 + 21x^7 + 35x^7 + 7x^7 = (1 + 21 + 35 + 7)x^7 = 64x^7.

Next, x^5 terms:

-21x^5 -70x^5 -21x^5 = (-21 -70 -21)x^5 = -112x^5.

x^3 terms:

35x^3 + 21x^3 = 56x^3.

x terms:

-7x.

So overall:

64x^7 - 112x^5 + 56x^3 - 7x = -1.

Bring the -1 to the left:

64x^7 - 112x^5 + 56x^3 - 7x + 1 = 0.

Hmm, so we have a 7th-degree equation. But since θ = π/7, x = cos(π/7) is a root of this equation. However, this seems complicated. Maybe there's a way to factor this equation?

Alternatively, maybe we can factor out some terms. Let me check if x = -1 is a root? Plugging x = -1:

64(-1)^7 - 112(-1)^5 + 56(-1)^3 -7(-1) + 1 = -64 + 112 - 56 +7 +1 = (-64 -56) + (112 +7 +1) = -120 + 120 = 0. Oh, so x = -1 is a root. Therefore, we can factor (x + 1) from the polynomial.

Let me perform polynomial division or factor it out. Let me write the polynomial as:

64x^7 - 112x^5 + 56x^3 - 7x + 1.

Let me note that the polynomial is of degree 7, and we have a root at x = -1. Let me use synthetic division. But synthetic division with polynomials of higher degrees is a bit tedious. Alternatively, maybe factor (x + 1) out.

Alternatively, since we know that x = cos(π/7) is a root, but maybe there are other roots. However, this seems too involved. Maybe there's another approach.

Alternatively, since we have the equation for cos(7θ) = -1, which is satisfied by θ = π/7, 3π/7, 5π/7, etc. But maybe this is leading me somewhere.

Alternatively, maybe I can consider the minimal polynomial for cos(π/7). I remember that cos(π/7), cos(3π/7), cos(5π/7) are roots of the cubic equation 8x³ - 4x² - 4x + 1 = 0. Let me check that.

Let me suppose that the minimal polynomial is cubic. Let me try to derive it.

Let me recall that for θ = π/7, 3π/7, 5π/7, cos(7θ) = cos(π) = -1. So, using the identity for cos(7θ) in terms of cosθ. Let me use the formula for cos(7θ). Alternatively, using the multiple-angle formula.

Alternatively, using the identity that relates cos(7θ) to cosθ. Let me recall that cos(7θ) can be expressed as 64cos^7θ - 112cos^5θ + 56cos^3θ - 7cosθ. Wait, that's the same as the equation we had earlier. So:

cos(7θ) = 64cos^7θ - 112cos^5θ + 56cos^3θ - 7cosθ.

But since cos(7θ) = -1 when θ = π/7, so:

64x^7 - 112x^5 + 56x^3 - 7x = -1, where x = cosθ. Therefore:

64x^7 - 112x^5 + 56x^3 - 7x + 1 = 0.

As before. Since θ = π/7, 3π/7, 5π/7, etc., are solutions. But since cos(π - θ) = -cosθ, so cos(5π/7) = -cos(2π/7), and cos(3π/7) is positive. Wait, maybe the roots of this equation are cos(π/7), cos(3π/7), cos(5π/7), and also cos(π), which is -1, and others? But since cos(7θ) = -1, θ can be π/7 + 2πk/7, etc. But maybe the equation factors into (x + 1)(something) = 0.

Earlier, we saw that x = -1 is a root. Let me factor (x + 1) out of the polynomial 64x^7 - 112x^5 + 56x^3 - 7x + 1.

Let me write the polynomial as:

64x^7 + 0x^6 -112x^5 + 0x^4 + 56x^3 + 0x^2 -7x + 1.

Divide by (x + 1). Let me use polynomial long division.

Dividing 64x^7 - 112x^5 + 56x^3 -7x +1 by (x + 1). Let me note that the polynomial is missing some terms. Let me write all coefficients:

Degree 7: 64

Degree 6: 0

Degree 5: -112

Degree 4: 0

Degree 3: 56

Degree 2: 0

Degree 1: -7

Degree 0: 1

Dividing by (x + 1). Let me perform the division.

First term: 64x^7 divided by x is 64x^6. Multiply (x + 1) by 64x^6: 64x^7 + 64x^6. Subtract this from the original polynomial:

(64x^7 + 0x^6 -112x^5 + 0x^4 + 56x^3 + 0x^2 -7x + 1) - (64x^7 + 64x^6) = -64x^6 -112x^5 + 0x^4 + 56x^3 + 0x^2 -7x +1.

Next term: -64x^6 divided by x is -64x^5. Multiply (x + 1) by -64x^5: -64x^6 -64x^5. Subtract:

(-64x^6 -112x^5 + 0x^4 + 56x^3 + 0x^2 -7x +1) - (-64x^6 -64x^5) = (-112x^5 + 64x^5) + 0x^4 + 56x^3 + ... = -48x^5 + 0x^4 + 56x^3 + 0x^2 -7x +1.

Next term: -48x^5 / x = -48x^4. Multiply (x + 1) by -48x^4: -48x^5 -48x^4. Subtract:

(-48x^5 + 0x^4 + 56x^3 + 0x^2 -7x +1) - (-48x^5 -48x^4) = 0x^5 + 48x^4 + 56x^3 + 0x^2 -7x +1.

Next term: 48x^4 / x = 48x^3. Multiply (x + 1) by 48x^3: 48x^4 + 48x^3. Subtract:

(48x^4 + 56x^3 + 0x^2 -7x +1) - (48x^4 + 48x^3) = 8x^3 + 0x^2 -7x +1.

Next term: 8x^3 / x = 8x^2. Multiply (x + 1) by 8x^2: 8x^3 + 8x^2. Subtract:

(8x^3 + 0x^2 -7x +1) - (8x^3 + 8x^2) = -8x^2 -7x +1.

Next term: -8x^2 / x = -8x. Multiply (x + 1) by -8x: -8x^2 -8x. Subtract:

(-8x^2 -7x +1) - (-8x^2 -8x) = (0x^2) + x +1.

Next term: x / x = 1. Multiply (x + 1) by 1: x + 1. Subtract:

(x +1) - (x +1) = 0.

So the division gives us:

Quotient: 64x^6 -64x^5 -48x^4 +48x^3 +8x^2 -8x +1.

Therefore, the original polynomial factors as (x + 1)(64x^6 -64x^5 -48x^4 +48x^3 +8x^2 -8x +1) = 0.

Now, since we are interested in cos(π/7), cos(3π/7), cos(5π/7), which are not equal to -1, we can focus on the 6th-degree polynomial:

64x^6 -64x^5 -48x^4 +48x^3 +8x^2 -8x +1 = 0.

But this still seems complicated. However, maybe this polynomial can be factored further. Let me check if it factors into lower-degree polynomials.

Alternatively, note that cos(π/7), cos(3π/7), cos(5π/7) are roots of this equation, but since cos(5π/7) = -cos(2π/7), maybe there's some symmetry here.

Alternatively, perhaps this 6th-degree polynomial can be factored into two cubics. Let me try to factor it as (ax³ + bx² + cx + d)(ex³ + fx² + gx + h). Given the coefficients, maybe with some symmetry.

Alternatively, since the original equation was for cos(7θ) = -1, which has solutions θ = π/7, 3π/7, 5π/7, and also θ = π - π/7 = 6π/7, etc. But cos(6π/7) = -cos(π/7), cos(4π/7) = -cos(3π/7), cos(2π/7) = -cos(5π/7). Therefore, the roots of the equation cos(7θ) = -1 are θ = π/7 + 2πk/7, which gives angles π/7, 3π/7, 5π/7, 7π/7=π, 9π/7, 11π/7, 13π/7. However, cos(π) = -1, which we already considered. The other angles have cosines that are either cos(π/7), cos(3π/7), cos(5π/7), or their negatives.

Therefore, the equation 64x^7 - 112x^5 + 56x^3 - 7x + 1 = 0 factors as (x + 1)(something) = 0, where the something is a 6th-degree polynomial whose roots are cos(π/7), cos(3π/7), cos(5π/7), -cos(π/7), -cos(3π/7), -cos(5π/7). Therefore, if we let y = x, then the 6th-degree polynomial is (y - cos(π/7))(y + cos(π/7))(y - cos(3π/7))(y + cos(3π/7))(y - cos(5π/7))(y + cos(5π/7)).

But this is equal to [(y² - cos²(π/7))(y² - cos²(3π/7))(y² - cos²(5π/7))]. Therefore, the 6th-degree polynomial is the product of three quadratic factors. Therefore, if I can find those quadratics, maybe I can find the cubic equation for cos(π/7), cos(3π/7), cos(5π/7).

Alternatively, since the original equation is symmetric, maybe the 6th-degree polynomial can be written as (something)^2? Not sure.

Alternatively, maybe I can consider that the minimal polynomial for cos(π/7) is a cubic. Let me check. Suppose that the roots are cos(π/7), cos(3π/7), cos(5π/7). Let me denote them as α, β, γ. Then, if I can find a cubic equation with roots α, β, γ.

Let me consider that the 6th-degree polynomial is [(y² - α²)(y² - β²)(y² - γ²)]. Therefore, if I can find this product, then maybe I can find the cubic equation.

Alternatively, since α + β + γ, αβ + αγ + βγ, and αβγ can be found using Vieta's formula. But how?

Alternatively, maybe I can use known values. Wait, I remember that cos(π/7) + cos(3π/7) + cos(5π/7) = 1/2. Wait, but that's similar to our original problem. Wait, but in our original problem, we have cos(π/7) - cos(2π/7) + cos(3π/7). Let me check if there's a relationship.

Alternatively, maybe I can compute the sum S = cos(π/7) - cos(2π/7) + cos(3π/7). Let me try to compute this numerically to check if it's indeed 1/2. Let me compute approximate values:

cos(π/7) ≈ cos(25.714°) ≈ 0.90097

cos(2π/7) ≈ cos(51.428°) ≈ 0.62349

cos(3π/7) ≈ cos(77.142°) ≈ 0.2225

So S ≈ 0.90097 - 0.62349 + 0.2225 ≈ 0.90097 - 0.62349 = 0.27748 + 0.2225 ≈ 0.49998 ≈ 0.5. So that's approximately 1/2. So that checks out. Therefore, the identity is correct.

But how to prove it?

Alternatively, since I know that cos(π/7) + cos(3π/7) + cos(5π/7) = 1/2. Wait, let me check that. If I compute cos(π/7) + cos(3π/7) + cos(5π/7):

cos(π/7) ≈ 0.90097, cos(3π/7) ≈ 0.2225, cos(5π/7) ≈ cos(π - 2π/7) = -cos(2π/7) ≈ -0.62349. Therefore, sum ≈ 0.90097 + 0.2225 - 0.62349 ≈ 0.90097 + 0.2225 = 1.12347 - 0.62349 ≈ 0.49998 ≈ 0.5. So that's also 1/2. Therefore, cos(π/7) + cos(3π/7) - cos(2π/7) = 1/2. Which is exactly our original expression! Because cos(π/7) - cos(2π/7) + cos(3π/7) is the same as cos(π/7) + cos(3π/7) - cos(2π/7). Therefore, if I can show that cos(π/7) + cos(3π/7) - cos(2π/7) = 1/2, which is equivalent to the given identity.

But how to prove that cos(π/7) + cos(3π/7) - cos(2π/7) = 1/2?

Alternatively, since we know that cos(π/7) + cos(3π/7) + cos(5π/7) = 1/2, and cos(5π/7) = -cos(2π/7), so substituting that in, we get:

cos(π/7) + cos(3π/7) - cos(2π/7) = 1/2. Which is exactly our expression. Therefore, if we can show that cos(π/7) + cos(3π/7) + cos(5π/7) = 1/2, then we are done. Therefore, the problem reduces to proving that sum equals 1/2.

So, how to prove that cos(π/7) + cos(3π/7) + cos(5π/7) = 1/2?

Well, maybe using the same approach as before, with the equation for cos(7θ) = -1. Let me think.

Alternatively, since we have the minimal polynomial for cos(π/7), which is a cubic equation. Let me try to find that.

Earlier, we had the equation for cos(7θ) = -1, which led us to the polynomial equation. However, we can consider that cos(π/7), cos(3π/7), cos(5π/7) are roots of a cubic equation. Let me denote x = cosθ, where θ = π/7, 3π/7, 5π/7. Then, using the identity for cos(7θ) = -1.

Alternatively, using the identity that relates cos(7θ) to cosθ. But earlier, we had:

cos(7θ) = 64x^7 - 112x^5 + 56x^3 - 7x, where x = cosθ. And since cos(7θ) = -1, then:

64x^7 - 112x^5 + 56x^3 - 7x + 1 = 0.

But we also factored this as (x + 1)(something) = 0. Therefore, the other roots are solutions to the 6th-degree equation. However, if we consider that cos(π/7), cos(3π/7), cos(5π/7) are roots of the cubic equation, then maybe we can find that equation.

Alternatively, perhaps we can use the fact that cos(π/7), cos(3π/7), cos(5π/7) are roots of the equation 8x³ - 4x² - 4x + 1 = 0. Let me check if this is true.

Let me suppose that this cubic equation is satisfied by these cosines. Let me take x = cos(π/7). Let me compute 8x³ - 4x² - 4x + 1.

But without knowing the exact value, it's hard to compute. Alternatively, maybe I can use the previous polynomial. Since we have the 6th-degree polynomial, which is [(y² - α²)(y² - β²)(y² - γ²)] where α, β, γ are cos(π/7), cos(3π/7), cos(5π/7). Therefore, expanding this product:

(y² - α²)(y² - β²)(y² - γ²) = y^6 - (α² + β² + γ²)y^4 + (α²β² + α²γ² + β²γ²)y² - α²β²γ².

Therefore, comparing with the 6th-degree polynomial we had earlier: 64x^6 -64x^5 -48x^4 +48x^3 +8x^2 -8x +1 = 0. Wait, but this seems different from the expansion above. However, if we factor out the 64, maybe?

Wait, the polynomial we had was:

64x^6 -64x^5 -48x^4 +48x^3 +8x^2 -8x +1 = 0.

But according to the expansion above, it should be:

(y² - α²)(y² - β²)(y² - γ²) = y^6 - (α² + β² + γ²)y^4 + (α²β² + α²γ² + β²γ²)y² - α²β²γ².

But our polynomial is not in the form of y^6 + ... so perhaps there is a scaling factor. However, since we have the 6th-degree polynomial as 64x^6 - ... , maybe it's 64 times the product above?

Alternatively, maybe I need to consider that the minimal polynomial for cos(π/7) is a cubic, and the 6th-degree polynomial is the square of that? Not sure.

Alternatively, maybe I can use the identity that we derived earlier: cos(π/7) + cos(3π/7) + cos(5π/7) = 1/2. If I can prove that, then we are done.

Alternatively, let me consider using complex numbers. Let me consider the sum S = cos(π/7) + cos(3π/7) + cos(5π/7). Let me write this as the real part of the sum of e^(iπ/7) + e^(i3π/7) + e^(i5π/7).

Let me compute this sum. Let me denote ω = e^(iπ/7). Then, ω^7 = e^(iπ) = -1. Therefore, ω^14 = 1. Therefore, ω is a primitive 14th root of unity.

Therefore, the sum is ω + ω^3 + ω^5. Let me compute this sum. Let me note that ω^k for k = 1, 3, 5 are the roots of some equation.

Alternatively, note that the sum of all 14th roots of unity is 0. Therefore, the sum of all ω^k from k=0 to 13 is 0. Therefore, the sum from k=0 to 13 of ω^k = 0. Therefore, the sum from k=1 to 13 of ω^k = -1. Therefore, we can split this sum into even and odd exponents.

But maybe not helpful. Alternatively, note that ω^7 = -1, so ω^k for k=1,...,13 can be grouped as ω, ω^2, ..., ω^6, ω^7=-1, ω^8=-ω, ω^9=-ω^2, ..., ω^13=-ω^6.

Therefore, the sum from k=1 to 13 of ω^k = (ω + ω^2 + ... + ω^6) + (-1) + (-ω - ω^2 - ... - ω^6) = 0. Therefore, the sum of ω + ω^2 + ... + ω^6 = 1/2. Wait, let me check:

Let me denote S = ω + ω^2 + ... + ω^6. Then, the sum from k=1 to 6 of ω^k + sum from k=8 to 13 of ω^k = S + (-ω - ω^2 - ... - ω^6) = S - S = 0. But we also have that the total sum from k=1 to 13 is -1. Therefore, S + (-S) + (-1) = -1, which is consistent. Therefore, this doesn't help directly.

But if I consider the sum of ω + ω^3 + ω^5. Let me denote this as T. Then, note that ω^7 = -1, so ω^k for k=7, 8,... can be expressed in terms of lower exponents. But how does this help?

Alternatively, note that T = ω + ω^3 + ω^5. Let me compute T + T* where T* is the complex conjugate. Since ω is e^(iπ/7), then T* = e^(-iπ/7) + e^(-i3π/7) + e^(-i5π/7) = cos(π/7) + cos(3π/7) + cos(5π/7) = S. Therefore, T + T* = 2S. Also, T * T* = |T|^2.

But maybe I can compute T^2 or something else. Alternatively, note that T is related to the sum of certain roots of unity.

Alternatively, note that ω, ω^3, ω^5 are roots of the equation x^3 + x^2 - 2x -1 = 0. Wait, is that true? Let me check. If I consider the minimal polynomial for ω^k where k is odd. But I need to think.

Alternatively, since ω^7 = -1, then ω^14 = 1. Therefore, the minimal polynomial for ω is x^14 - 1 = 0, but since ω is a primitive 14th root of unity, its minimal polynomial is the 14th cyclotomic polynomial. The 14th cyclotomic polynomial is Φ₁₄(x) = x^6 - x^5 + x^4 - x^3 + x^2 - x + 1. Therefore, ω satisfies Φ₁₄(ω) = 0. Therefore, ω^6 - ω^5 + ω^4 - ω^3 + ω^2 - ω + 1 = 0. Therefore, rearranged:

ω^6 + ω^4 + ω^2 + 1 = ω^5 + ω^3 + ω.

Therefore, the sum of ω^6 + ω^4 + ω^2 + 1 equals the sum of ω^5 + ω^3 + ω. Therefore, if I denote S1 = ω + ω^3 + ω^5 and S2 = ω^2 + ω^4 + ω^6, then S1 + 1 = S2. But from the equation above, S1 + 1 = S2.

But also, the sum of all roots of Φ₁₄(x) is 0, since the sum of roots of cyclotomic polynomials is μ(14) where μ is Möbius function. Wait, the sum of roots of Φ_n(x) is μ(n). For n=14, μ(14) = μ(2*7) = μ(2)μ(7) = (-1)(-1) = 1. Wait, but Φ₁₄(x) is degree 6, so the sum of roots is 1. Therefore, the sum of ω, ω^3, ω^5, ω^7, ω^9, ω^11, ω^13? Wait, no, Φ₁₄(x) is the minimal polynomial for primitive 14th roots of unity. The primitive 14th roots of unity are e^(2πik/14) where k is coprime to 14, i.e., k=1,3,5,9,11,13. Therefore, the roots are ω^2, ω^6, ω^10, ω^12, ω^14=1? Wait, no, ω = e^(iπ/7) = e^(i2π/14). Therefore, the primitive 14th roots of unity are e^(i2πk/14) where k=1,3,5,9,11,13. Therefore, these correspond to exponents 1,3,5,9,11,13. Therefore, the sum of these roots is μ(14) = 1. Therefore:

ω + ω^3 + ω^5 + ω^9 + ω^11 + ω^13 = 1.

But ω^9 = ω^(7 + 2) = ω^7 * ω^2 = -ω^2. Similarly, ω^11 = ω^(7 + 4) = -ω^4, ω^13 = ω^(7 + 6) = -ω^6. Therefore, the sum becomes:

ω + ω^3 + ω^5 - ω^2 - ω^4 - ω^6 = 1.

Rearranged:

(ω - ω^2) + (ω^3 - ω^4) + (ω^5 - ω^6) = 1.

But this seems complicated. However, note that earlier we had S1 = ω + ω^3 + ω^5 and S2 = ω^2 + ω^4 + ω^6. Therefore, the equation becomes S1 - S2 = 1.

But earlier, from the cyclotomic polynomial equation, we had S1 + 1 = S2. Therefore, combining S1 - S2 = 1 and S1 + 1 = S2:

From S1 + 1 = S2, substitute into S1 - S2 = 1:

S1 - (S1 + 1) = 1 => -1 = 1? Wait, that can't be. There must be a mistake here.

Wait, let me check again. From the cyclotomic polynomial equation:

We had ω^6 - ω^5 + ω^4 - ω^3 + ω^2 - ω + 1 = 0.

Rearranged:

(ω^6 + ω^4 + ω^2 + 1) = (ω^5 + ω^3 + ω).

Which is S2 + 1 = S1.

But from the sum of roots of Φ₁₄(x) = 1, we have S1 - S2 = 1.

Therefore, we have two equations:

1. S2 + 1 = S1

2. S1 - S2 = 1

Substituting equation 1 into equation 2: (S2 + 1) - S2 = 1 => 1 = 1. Which is consistent. Therefore, these equations are not independent. Therefore, we can't get more information from them.

But we need to find S = Re(T) = cos(π/7) + cos(3π/7) + cos(5π/7) = Re(S1). Since S1 = ω + ω^3 + ω^5, and T = S1, then Re(S1) = S.

But how to find Re(S1)? Let me think. Maybe compute |S1|^2?

Let me compute |S1|^2 = S1 * S1* = (ω + ω^3 + ω^5)(ω^{-1} + ω^{-3} + ω^{-5}) = (ω + ω^3 + ω^5)(ω^{-1} + ω^{-3} + ω^{-5}).

Since ω^7 = -1, ω^{-1} = ω^6, ω^{-3} = ω^4, ω^{-5} = ω^2. Therefore:

|S1|^2 = (ω + ω^3 + ω^5)(ω^6 + ω^4 + ω^2) = (ω + ω^3 + ω^5)(ω^2 + ω^4 + ω^6).

But earlier, we have S1 - S2 = 1, and S2 + 1 = S1. Therefore, S1 = S2 + 1. Also, S2 = ω^2 + ω^4 + ω^6.

But let me compute (ω + ω^3 + ω^5)(ω^2 + ω^4 + ω^6). Let me expand this product:

Multiply term by term:

ω*ω^2 + ω*ω^4 + ω*ω^6 + ω^3*ω^2 + ω^3*ω^4 + ω^3*ω^6 + ω^5*ω^2 + ω^5*ω^4 + ω^5*ω^6.

Simplify exponents:

ω^3 + ω^5 + ω^7 + ω^5 + ω^7 + ω^9 + ω^7 + ω^9 + ω^{11}.

Now, simplify each term:

ω^3 + ω^5 + (-1) + ω^5 + (-1) + ω^9 + (-1) + ω^9 + ω^{11}.

But ω^7 = -1, ω^9 = ω^7 * ω^2 = -ω^2, ω^{11} = ω^7 * ω^4 = -ω^4.

Therefore, substituting:

ω^3 + ω^5 -1 + ω^5 -1 -ω^2 -1 -ω^2 + (-ω^4).

Simplify:

Combine like terms:

ω^3 + (ω^5 + ω^5) + (-1 -1 -1) + (-ω^2 - ω^2) + (-ω^4).

Which is:

ω^3 + 2ω^5 - 3 - 2ω^2 - ω^4.

Now, rearrange:

-3 + ω^3 - ω^4 + 2ω^5 - 2ω^2.

Hmm, not sure if this helps. But maybe we can use the earlier equation S1 - S2 = 1. Recall that S1 = ω + ω^3 + ω^5 and S2 = ω^2 + ω^4 + ω^6. Therefore, S1 - S2 = (ω - ω^2) + (ω^3 - ω^4) + (ω^5 - ω^6) = 1. But I don't know if that helps here.

Alternatively, maybe I can find |S1|^2 in terms of S1 and S2. But this seems complicated.

Alternatively, since we have that S1 + 1 = S2, then S2 = S1 + 1. Also, from the sum of roots, S1 - S2 = 1, which is S1 - (S1 + 1) = -1 = 1? No, that contradicts. Wait, earlier we had S1 - S2 = 1 and S2 + 1 = S1, which gives S1 - S2 = 1 and S2 = S1 - 1. Therefore, substituting into S1 - S2 = 1: S1 - (S1 - 1) = 1 => 1 = 1. So it's consistent.

But how to find S = Re(S1). Let me think. Let me denote S = Re(S1) = cos(π/7) + cos(3π/7) + cos(5π/7). Also, since S1 = ω + ω^3 + ω^5, then the imaginary part of S1 is Im(S1) = sin(π/7) + sin(3π/7) + sin(5π/7). Let me denote this as I.

Therefore, |S1|^2 = S² + I².

But earlier, we computed |S1|^2 as -3 + ω^3 - ω^4 + 2ω^5 - 2ω^2. But this seems messy. Maybe there's another way.

Alternatively, since we know that S1 + 1 = S2, and S1 - S2 = 1, which gives S1 = S2 + 1 and S1 - S2 = 1, which is consistent. But we need another relation.

Alternatively, maybe we can use the equation from the cyclotomic polynomial. Recall that ω^6 - ω^5 + ω^4 - ω^3 + ω^2 - ω + 1 = 0. Let me write this as:

(ω^6 + ω^4 + ω^2 + 1) = (ω^5 + ω^3 + ω).

Which is S2 + 1 = S1. Which we already know.

Alternatively, maybe consider that S1 is a complex number, and we can find its magnitude or something else.

Alternatively, let me consider that the real part of S1 is S = cos(π/7) + cos