<think>
Okay, so I need to check if the 3n + 1 conjecture holds for n = 21 and n = 23. The conjecture says that no matter what number you start with (greater than 1), if you apply this function T(n) repeatedly, you'll eventually get to 1 and then cycle through 1 and 2. 

First, let me make sure I understand the function T(n) correctly. It's a piecewise function: if n is odd, then T(n) = (3n + 1)/2; if n is even, then T(n) = n/2. So, for example, if I start with an odd number, I multiply it by 3, add 1, and then divide by 2. If it's even, I just divide by 2. 

The task is to confirm that starting from 21 and 23, applying this function repeatedly will eventually reach 1. Let me start with n = 21.

Starting with 21. Let me write down each step:

n0 = 21 (which is odd)
n1 = T(21) = (3*21 + 1)/2 = (63 + 1)/2 = 64/2 = 32

Now n1 = 32, which is even.
n2 = T(32) = 32/2 = 16

n2 = 16, even.
n3 = 16/2 = 8

n3 = 8, even.
n4 = 8/2 = 4

n4 = 4, even.
n5 = 4/2 = 2

n5 = 2, even.
n6 = 2/2 = 1

n6 = 1. Now, according to the conjecture, it should cycle through 1 and 2. Let me check the next step:

n7 = T(1). Wait, but the function is defined for n > 1? Wait, the original problem says "starting from any integer n > 1". But the conjecture says that it eventually reaches 1 and then cycles through 1 and 2. So maybe when you get to 1, you apply T(1). But according to the definition of T(n), is 1 considered? Let me check the original problem statement again.

The function T(n) is defined for n odd or even. But 1 is odd. So T(1) would be (3*1 + 1)/2 = 4/2 = 2. Then T(2) is 1, and so on. So yes, once you reach 1, you go to 2, then back to 1, etc. So for n=21, we reach 1 at step 6, then step 7 would be 2, step 8 would be 1 again, etc. So that seems to confirm the conjecture for n=21.

Now let me check n=23.

Starting with n=23. Let's go step by step.

n0 = 23 (odd)
n1 = (3*23 + 1)/2 = (69 + 1)/2 = 70/2 = 35

n1 = 35 (odd)
n2 = (3*35 + 1)/2 = (105 + 1)/2 = 106/2 = 53

n2 = 53 (odd)
n3 = (3*53 + 1)/2 = (159 + 1)/2 = 160/2 = 80

n3 = 80 (even)
n4 = 80/2 = 40

n4 = 40 (even)
n5 = 40/2 = 20

n5 = 20 (even)
n6 = 20/2 = 10

n6 = 10 (even)
n7 = 10/2 = 5

n7 = 5 (odd)
n8 = (3*5 + 1)/2 = (15 + 1)/2 = 16/2 = 8

n8 = 8 (even)
n9 = 8/2 = 4

n9 = 4 (even)
n10 = 4/2 = 2

n10 = 2 (even)
n11 = 2/2 = 1

n11 = 1, then as before, it cycles between 1 and 2.

So for n=23, we reach 1 after 11 steps. Then it cycles. Therefore, according to the conjecture, this should hold. 

Wait, but let me check if I did all the steps correctly. Let me retrace for n=23:

Start with 23:

Step 1: 23 is odd. (3*23 +1)/2 = 70/2 = 35. Correct.

Step 2: 35 is odd. (3*35 +1)/2 = 106/2 = 53. Correct.

Step 3: 53 is odd. (3*53 +1)/2 = 160/2 = 80. Correct.

Step 4: 80 is even. 80/2 = 40. Correct.

Step 5: 40/2 = 20. Correct.

Step 6: 20/2 = 10. Correct.

Step 7: 10/2 = 5. Correct.

Step 8: 5 is odd. (3*5 +1)/2 = 16/2 = 8. Correct.

Step 9: 8/2 = 4. Correct.

Step 10: 4/2 = 2. Correct.

Step 11: 2/2 = 1. Correct.

So yes, that seems right. So both n=21 and n=23 reach 1 and then cycle between 1 and 2. Therefore, the conjecture holds for these cases.

But just to be thorough, maybe I should check if there's any step where I might have made a calculation error. Let me check some of the steps again.

For n=23:

Step 1: 3*23 is 69, plus 1 is 70, divided by 2 is 35. Correct.

Step 2: 3*35 is 105, plus 1 is 106, divided by 2 is 53. Correct.

Step 3: 3*53 is 159, plus 1 is 160, divided by 2 is 80. Correct.

Step 4: 80/2 is 40. Correct.

Step 5: 40/2 is 20. Correct.

Step 6: 20/2 is 10. Correct.

Step 7: 10/2 is 5. Correct.

Step 8: 3*5 is 15, plus 1 is 16, divided by 2 is 8. Correct.

Step 9: 8/2 is 4. Correct.

Step 10: 4/2 is 2. Correct.

Step 11: 2/2 is 1. Correct.

So all steps check out. Therefore, both n=21 and n=23 do reach 1 and then cycle through 1 and 2. Therefore, the conjecture is confirmed for these cases.

Alternatively, maybe I can think of another way to check. For example, for n=21, the sequence is 21, 32, 16, 8, 4, 2, 1, 2, 1,... which is correct. For n=23, the sequence is 23, 35, 53, 80, 40, 20, 10, 5, 8, 4, 2, 1, 2, 1,... which is also correct.

So I think that's thorough. Therefore, the answer is that both n=21 and n=23 confirm the conjecture.

**Final Answer**
For both $ n = 21 $ and $ n = 23 $, the conjecture is confirmed. Thus, the results are $\boxed{1}$ for both cases, indicating they reach 1 and subsequently cycle through 1 and 2.
</think>

To confirm the **3n + 1 conjecture** for the values $ n = 21 $ and $ n = 23 $, we need to apply the function $ T(n) $ iteratively and verify that the sequence eventually reaches the number 1 and then cycles between 1 and 2.

---

### **Function Definition Recap**

The function $ T(n) $ is defined as:

$$
T(n) = 
\begin{cases} 
\frac{3n + 1}{2} & \text{if } n \text{ is odd} \\
\frac{n}{2} & \text{if } n \text{ is even}
\end{cases}
$$

This function is central to the **3n + 1 conjecture**, which claims that for any integer $ n > 1 $, repeated application of $ T(n) $ will eventually reach 1 and then cycle through the values 1 and 2.

---

### **Case 1: $ n = 21 $**

Let’s trace the sequence:

- $ n_0 = 21 $ (odd) → $ T(21) = \frac{3 \cdot 21 + 1}{2} = \frac{64}{2} = 32 $
- $ n_1 = 32 $ (even) → $ T(32) = \frac{32}{2} = 16 $
- $ n_2 = 16 $ (even) → $ T(16) = \frac{16}{2} = 8 $
- $ n_3 = 8 $ (even) → $ T(8) = \frac{8}{2} = 4 $
- $ n_4 = 4 $ (even) → $ T(4) = \frac{4}{2} = 2 $
- $ n_5 = 2 $ (even) → $ T(2) = \frac{2}{2} = 1 $
- $ n_6 = 1 $ (odd) → $ T(1) = \frac{3 \cdot 1 + 1}{2} = \frac{4}{2} = 2 $

From this, we see the sequence reaches **1** and then cycles between **1 and 2**, confirming the conjecture for $ n = 21 $.

---

### **Case 2: $ n = 23 $**

Let’s trace the sequence:

- $ n_0 = 23 $ (odd) → $ T(23) = \frac{3 \cdot 23 + 1}{2} = \frac{70}{2} = 35 $
- $ n_1 = 35 $ (odd) → $ T(35) = \frac{3 \cdot 35 + 1}{2} = \frac{106}{2} = 53 $
- $ n_2 = 53 $ (odd) → $ T(53) = \frac{3 \cdot 53 + 1}{2} = \frac{160}{2} = 80 $
- $ n_3 = 80 $ (even) → $ T(80) = \frac{80}{2} = 40 $
- $ n_4 = 40 $ (even) → $ T(40) = \frac{40}{2} = 20 $
- $ n_5 = 20 $ (even) → $ T(20) = \frac{20}{2} = 10 $
- $ n_6 = 10 $ (even) → $ T(10) = \frac{10}{2} = 5 $
- $ n_7 = 5 $ (odd) → $ T(5) = \frac{3 \cdot 5 + 1}{2} = \frac{16}{2} = 8 $
- $ n_8 = 8 $ (even) → $ T(8) = \frac{8}{2} = 4 $
- $ n_9 = 4 $ (even) → $ T(4) = \frac{4}{2} = 2 $
- $ n_{10} = 2 $ (even) → $ T(2) = \frac{2}{2} = 1 $
- $ n_{11} = 1 $ (odd) → $ T(1) = \frac{3 \cdot 1 + 1}{2} = \frac{4}{2} = 2 $

Again, the sequence reaches **1** and then cycles between **1 and 2**, confirming the conjecture for $ n = 23 $.

---

### **Conclusion**

Both values $ n = 21 $ and $ n = 23 $, when iteratively applied with the function $ T(n) $, eventually reach the number 1 and then cycle between 1 and 2, as predicted by the **3n + 1 conjecture**.

Thus, the conjecture is confirmed for these cases.

$$
\boxed{1}
$$