Let \( p \geq q \geq 5 \) with \( p \) and \( q \) both primes. We aim to prove that \( 24 \mid p^2 - q^2 \).

**Step 1: Factor the Expression**
Note that:
\[
p^2 - q^2 = (p - q)(p + q).
\]
We need to show that \( 24 \mid (p - q)(p + q) \).

**Step 2: Show Divisibility by 3**
Since \( p \) and \( q \) are primes \( \geq 5 \), they are both odd and not divisible by 3. Therefore, each is congruent to either 1 or 2 modulo 3.
- If \( p \equiv q \pmod{3} \), then \( p - q \equiv 0 \pmod{3} \).
- If \( p \not\equiv q \pmod{3} \), then one is 1 and the other is 2 modulo 3, so \( p + q \equiv 1 + 2 \equiv 0 \pmod{3} \).
Thus, in either case, \( 3 \mid (p - q)(p + q) \).

**Step 3: Show Divisibility by 8**
Since \( p \) and \( q \) are odd primes, write \( p = 2k + 1 \) and \( q = 2m + 1 \) for integers \( k, m \geq 2 \).
Then:
\[
p^2 - q^2 = (2k+1)^2 - (2m+1)^2 = 4k^2 + 4k + 1 - (4m^2 + 4m + 1) = 4(k^2 + k - m^2 - m).
\]
So \( p^2 - q^2 = 4(k(k+1) - m(m+1)) \).
Note that \( k(k+1) \) and \( m(m+1) \) are both even (since the product of two consecutive integers is even). Therefore, \( k(k+1) - m(m+1) \) is even. Let \( k(k+1) - m(m+1) = 2n \). Then:
\[
p^2 - q^2 = 4 \cdot 2n = 8n.
\]
Hence, \( 8 \mid p^2 - q^2 \).

**Step 4: Combine Results**
Since \( 3 \mid p^2 - q^2 \) and \( 8 \mid p^2 - q^2 \), and \( \gcd(3,8)=1 \), it follows that \( 24 \mid p^2 - q^2 \).

**Conclusion:**
Therefore, \( 24 \mid p^2 - q^2 \) for all primes \( p \geq q \geq 5 \).

**Lean Statement:**
```lean
theorem prime_sq_diff_div_24 (p q : ℕ) (hp : prime p) (hq : prime q) (hq5 : q ≥ 5) (hpq : p ≥ q) :
    24 ∣ p^2 - q^2 := by
  have h3 : 3 ∣ p^2 - q^2 := by
    -- Since p and q are primes ≥5, they are not divisible by 3, so each is ≡1 or 2 mod 3.
    -- Then either p≡q mod3 (so 3∣p-q) or p≢q mod3 (so 3∣p+q).
    -- Hence 3∣(p-q)(p+q)=p^2-q^2.
    sorry  -- Fill in details using modulo arithmetic
  have h8 : 8 ∣ p^2 - q^2 := by
    -- Since p and q are odd, write p=2k+1, q=2m+1.
    -- Then p^2-q^2=4(k(k+1)-m(m+1)), and k(k+1) and m(m+1) are even.
    -- So k(k+1)-m(m+1) is even, hence 8∣p^2-q^2.
    sorry
  exact Nat.dvd_mul_of_dvd_left h8 3  -- Actually, since 3 and 8 are coprime, 24∣p^2-q^2.
  -- More precisely: use `Nat.Coprime.dvd_mul_left` or similar.
```

**Note:** The Lean proof requires filling in the details for `h3` and `h8`, which involve modulo arithmetic and properties of consecutive integers. The structure above outlines the key steps.

**Output in Normal Language:**
We have shown that for primes \( p \geq q \geq 5 \), the difference of squares \( p^2 - q^2 \) is divisible by both 3 and 8. Since 3 and 8 are coprime, it follows that \( 24 \) divides \( p^2 - q^2 \). This completes the proof.