I will solve both parts step by step.

### (a) Proof that if p is prime and p | aⁿ, then pⁿ | aⁿ

**Proof:**
Let p be a prime and assume p | aⁿ.

By the Fundamental Theorem of Arithmetic, we can write the prime factorization of a as:
a = p₁^α₁ × p₂^α₂ × ... × pₖ^αₖ

Then aⁿ = p₁^(nα₁) × p₂^(nα₂) × ... × pₖ^(nαₖ)

Since p | aⁿ and p is prime, p must be one of the primes pᵢ in the factorization. Without loss of generality, let p = p₁.

This means that the exponent of p in aⁿ must be at least 1, so nα₁ ≥ 1 ⇒ α₁ ≥ 1/n.

Since α₁ must be a non-negative integer, α₁ ≥ 1 (since 1/n < 1 for n ≥ 2, and the smallest positive integer is 1).

Therefore, the exponent of p in aⁿ is nα₁ ≥ n × 1 = n.

This means pⁿ | aⁿ. QED.

**Lean 4 statement:**
```lean
theorem part_a (p : ℕ) (hp : Nat.Prime p) (a n : ℕ) (h : p ∣ a ^ n) : p ^ n ∣ a ^ n := by
  -- Proof would use properties of prime factorization
  -- This would typically be proven using the multiplicity of primes
  sorry
```

### (b) Possible values of gcds when gcd(a, b) = p (prime)

Given: gcd(a, b) = p, where p is prime

Let a = p × a₁ and b = p × b₁, where gcd(a₁, b₁) = 1

**1. gcd(a², b²):**
a² = p² × a₁²  
b² = p² × b₁²  
gcd(a², b²) = p² × gcd(a₁², b₁²)

Since gcd(a₁, b₁) = 1, we have gcd(a₁², b₁²) = 1  
∴ gcd(a², b²) = p²

**2. gcd(a², b):**
a² = p² × a₁²  
b = p × b₁  
gcd(a², b) = p × gcd(p × a₁², b₁)

Since gcd(a₁, b₁) = 1, we consider two cases:
- If p ∤ b₁, then gcd(p × a₁², b₁) = 1 ⇒ gcd(a², b) = p
- If p | b₁, then b₁ = p × b₂, so gcd(p × a₁², p × b₂) = p × gcd(a₁², b₂)

But since gcd(a₁, b₁) = 1 and b₁ = p × b₂, we have gcd(a₁, p) = 1, so gcd(a₁², b₂) = 1  
∴ gcd(a², b) = p²

So possible values: p or p²

**3. gcd(a³, b²):**
a³ = p³ × a₁³  
b² = p² × b₁²  
gcd(a³, b²) = p² × gcd(p × a₁³, b₁²)

Since gcd(a₁, b₁) = 1, we consider:
- If p ∤ b₁, then gcd(p × a₁³, b₁²) = 1 ⇒ gcd(a³, b²) = p²
- If p | b₁, then b₁ = p × b₂, b₁² = p² × b₂²  
  gcd(p × a₁³, p² × b₂²) = p × gcd(a₁³, p × b₂²)
  
  Since gcd(a₁, b₁) = 1 and b₁ = p × b₂, we have gcd(a₁, p) = 1, so gcd(a₁³, p) = 1  
  ∴ gcd(a₁³, p × b₂²) = gcd(a₁³, b₂²) (since gcd(a₁³, p) = 1)
  
  And since gcd(a₁, b₂) = 1 (from gcd(a₁, b₁) = 1 and b₁ = p × b₂), we have gcd(a₁³, b₂²) = 1  
  ∴ gcd(a³, b²) = p³

So possible values: p² or p³

**Summary:**
- gcd(a², b²) = p² (only possible value)
- gcd(a², b) = p or p²
- gcd(a³, b²) = p² or p³

**Lean 4 statements:**
```lean
theorem part_b1 (a b p : ℕ) (hp : Nat.Prime p) (h : Nat.gcd a b = p) : 
    Nat.gcd (a ^ 2) (b ^ 2) = p ^ 2 := by
  sorry

theorem part_b2 (a b p : ℕ) (hp : Nat.Prime p) (h : Nat.gcd a b = p) : 
    Nat.gcd (a ^ 2) b = p ∨ Nat.gcd (a ^ 2) b = p ^ 2 := by
  sorry

theorem part_b3 (a b p : ℕ) (hp : Nat.Prime p) (h : Nat.gcd a b = p) : 
    Nat.gcd (a ^ 3) (b ^ 2) = p ^ 2 ∨ Nat.gcd (a ^ 3) (b ^ 2) = p ^ 3 := by
  sorry
```

**Normal language output:**
For part (a): If a prime p divides aⁿ, then pⁿ must divide aⁿ.

For part (b) with gcd(a, b) = p (prime):
- gcd(a², b²) is always exactly p²
- gcd(a², b) can be either p or p²
- gcd(a³, b²) can be either p² or p³