Let \( n \) be a square-full positive integer. This means that for every prime \( p \) dividing \( n \), we have \( p^2 \mid n \).

We aim to show that \( n \) can be written in the form \( n = a^2 b^3 \), where \( a \) and \( b \) are positive integers.

**Proof:**

Let \( n \) have the prime factorization:
\[
n = p_1^{e_1} p_2^{e_2} \cdots p_k^{e_k}
\]
Since \( n \) is square-full, for each \( i \), \( e_i \geq 2 \).

Now, for each exponent \( e_i \), we can write it as:
\[
e_i = 2q_i + r_i
\]
where \( r_i \in \{0, 1\} \). However, since \( e_i \geq 2 \), if \( e_i \) is even, \( r_i = 0 \); if \( e_i \) is odd, \( r_i = 1 \) and \( e_i \geq 3 \) (because if \( e_i = 1 \), it would not satisfy \( e_i \geq 2 \), so the smallest odd exponent is 3).

Actually, a better approach is to express each exponent \( e_i \) in terms of multiples of 2 and 3. Note that every integer \( \geq 2 \) can be written as \( 2x + 3y \) for nonnegative integers \( x, y \). For example:
- \( 2 = 2 \cdot 1 + 3 \cdot 0 \)
- \( 3 = 2 \cdot 0 + 3 \cdot 1 \)
- \( 4 = 2 \cdot 2 + 3 \cdot 0 \) or \( 2 \cdot 0 + 3 \cdot 1 + 1 \), but wait, we need nonnegative integers. Actually, \( 4 = 2 \cdot 2 + 3 \cdot 0 \).
- \( 5 = 2 \cdot 1 + 3 \cdot 1 \)
- \( 6 = 2 \cdot 0 + 3 \cdot 2 \) or \( 2 \cdot 3 + 3 \cdot 0 \), etc.

In fact, by the coin problem, since 2 and 3 are coprime, every integer \( \geq 2 \) can be expressed as \( 2x + 3y \) with \( x, y \geq 0 \). So for each \( e_i \geq 2 \), there exist nonnegative integers \( x_i, y_i \) such that:
\[
e_i = 2x_i + 3y_i
\]

Now, define:
\[
a = \prod_{i=1}^k p_i^{x_i}, \quad b = \prod_{i=1}^k p_i^{y_i}
\]
Then:
\[
a^2 b^3 = \left( \prod_{i=1}^k p_i^{x_i} \right)^2 \cdot \left( \prod_{i=1}^k p_i^{y_i} \right)^3 = \prod_{i=1}^k p_i^{2x_i + 3y_i} = \prod_{i=1}^k p_i^{e_i} = n
\]

Thus, \( n = a^2 b^3 \), as required.

**Conclusion:**
Every square-full number \( n \) can be written in the form \( n = a^2 b^3 \) for positive integers \( a \) and \( b \).

---

**Lean Statement:**
```lean
theorem square_full_iff_exists_a_b (n : ℕ) (h : n > 0) :
  (∀ p : ℕ, p.prime → p ∣ n → p^2 ∣ n) ↔ ∃ (a b : ℕ), a > 0 ∧ b > 0 ∧ n = a^2 * b^3 := by
  constructor
  · intro hsq
    -- Get the prime factorization of n
    rcases exists_prime_factorization n h with ⟨f, hf⟩
    have := hf
    -- For each prime in the support, the exponent is at least 2
    have hex : ∀ p, p.prime → f p ≥ 2 := by
      intro p hp
      have := hsq p hp (hfac.dvd_of_mem_support hf hp)
      -- Then the exponent must be at least 2
      ...
    -- Now, for each exponent e, write e = 2x + 3y with x,y nonnegative
    -- Define a and b accordingly
    let a := ∏ p in f.support, p ^ (x p)
    let b := ∏ p in f.support, p ^ (y p)
    have ha : a > 0 := ...
    have hb : b > 0 := ...
    have hn : n = a^2 * b^3 := by
      simp [a, b]
      apply factorization_eq_prod_pow_eq n (a^2 * b^3) ...
    exact ⟨a, b, ha, hb, hn⟩
  · intro ⟨a, b, ha, hb, hn⟩
    intro p hp hpd
    rw [hn] at hpd
    -- Since p divides a^2 * b^3, it divides a or b
    rcases hp.dvd_mul.mp hpd with (h | h)
    · have := hp.dvd_pow.mp h
      exact pow_two_dvd_pow_two (by omega)
    · have := hp.dvd_pow.mp h
      -- But then p^2 divides b^3? Actually, if p divides b, then since b^3 = b * b^2, p^2 divides b^3 if the exponent in b is at least 1?
      -- More carefully: if p ∣ b, then let k be the exponent of p in b. Then in b^3, the exponent is 3k ≥ 3 (if k≥1) so p^2 ∣ b^3.
      ...
```

Note: The Lean proof sketch above outlines the structure. The actual implementation would require more details, such as handling the factorization and the decomposition of exponents. The key step is to use the fact that every exponent \( e \geq 2 \) can be written as \( 2x + 3y \) with \( x, y \geq 0 \), which can be proven by induction or using the fact that 2 and 3 generate all integers beyond 1.

---

**Output in normal language:**
We have shown that if \( n \) is square-full (meaning every prime factor appears with exponent at least 2), then its prime exponents \( e_i \) (all \( \geq 2 \)) can each be expressed as \( e_i = 2x_i + 3y_i \) for nonnegative integers \( x_i, y_i \). By setting \( a = \prod p_i^{x_i} \) and \( b = \prod p_i^{y_i} \), we obtain \( n = a^2 b^3 \). Thus, every square-full number can be written in the form \( a^2 b^3 \).