 To prove the formula using mathematical induction, we need to follow these steps:

1. Base case: Show that the formula holds for the smallest value of n, which is 1 in this case.
2. Inductive step: Assume the formula holds for some arbitrary value of n, and then show that it also holds for n+1.

Let's start with the base case:

For n = 1, the left side of the formula is $1(1!) = 1$, and the right side is $(1+1)! - 1 = 2! - 1 = 2 - 1 = 1$. So, the formula holds for n = 1.

Now, let's assume the formula holds for some arbitrary value of n, and then show that it also holds for n+1.

Assume the formula holds for n:
$$1(1!) + 2(2!) + 3(3!) + \ldots + n(n!) = (n + 1)! - 1$$

Now, we want to show that the formula holds for n+1:
$$1(1!) + 2(2!) + 3(3!) + \ldots + n(n!) + (n+1)((n+1)!) = ((n+1) + 1)! - 1$$

We can rewrite the left side of the equation as:
$$(1(1!) + 2(2!) + 3(3!) + \ldots + n(n!)) + (n+1)((n+1)!) = ((n+1) + 1)! - 1$$

Using the assumption that the formula holds for n, we can substitute $(n + 1)! - 1$ for the sum of the first n terms:
$$(n + 1)! - 1 + (n+1)((n+1)!) = ((n+1) + 1)! - 1$$

Now, let's simplify the left side of the equation:
$$(n + 1)! + (n+1)((n+1)!) - 1 = ((n+1) + 1)! - 1$$

Factor out $(n+1)!$ from the first two terms:
$$(n + 1)!(1 + (n+1)) - 1 = ((n+1) + 1)! - 1$$

Simplify the expression inside the parentheses:
$$(n + 1)!(n+2) - 1 = ((n+1) + 1)! - 1$$

Now, let's simplify the right side of the equation:
$$(n + 2)! - 1 = (n+2)! - 1$$

Since both sides of the equation are equal, we have shown that if the formula holds for n, it also holds for n+1.

Therefore, by mathematical induction, the formula holds for all n $\geq{1}$:
$$1(1!) + 2(2!) + 3(3!) + \ldots + n(n!) = (n + 1)! - 1$$