 a) We can prove this by induction.

Base case: For $n=1$, we have $2 = \frac{2!}{1!}$, which is true.

Inductive step: Assume the statement is true for $n=k$, i.e.,
$$2 · 6 · 10 · 14 · · · · · (4k - 2) = \frac{(2k)!}{k!}.$$
We want to show that the statement is true for $n=k+1$, i.e.,
$$2 · 6 · 10 · 14 · · · · · (4k - 2) · 4(2k+1) = \frac{(2k+2)!}{(k+1)!}.$$

Multiplying both sides of the inductive hypothesis by $4(2k+1)$, we get
$$2 · 6 · 10 · 14 · · · · · (4k - 2) · 4(2k+1) = \frac{(2k)!}{k!} \cdot 4(2k+1).$$

Now, we can simplify the right side:
$$\frac{(2k)!}{k!} \cdot 4(2k+1) = \frac{(2k)! \cdot 4(2k+1)}{k!} = \frac{(2k)! \cdot 4 \cdot (2k+1)}{k!} = \frac{(2k)! \cdot 2 \cdot 2 \cdot (2k+1)}{k!} = \frac{(2k)! \cdot 2 \cdot (2k+2)}{k!} = \frac{(2k)! \cdot 2 \cdot (2k+2) \cdot (k+1)}{(k+1)!} = \frac{(2k+2)!}{(k+1)!}.$$

Thus, the statement is true for $n=k+1$.

By induction, the statement is true for all $n \geq 1$.

b) Using the result from part (a), we have
$$2^n(n!)^2 = 2^n \cdot n! \cdot n! = 2^n \cdot n! \cdot (2n)! \cdot \frac{1}{(2n)!} = (2n)! \cdot \frac{2^n \cdot n!}{(2n)!} \leq (2n)!.$$

Since $\frac{2^n \cdot n!}{(2n)!} \leq 1$ for all $n \geq 1$, we have $2^n(n!)^2 \leq (2n)!$ for all $n \geq 1$.