 To prove that n! > $n^2$ for every integer n $\geq{4}$, we can use induction.

Base case: For n = 4, we have 4! = 24 and $4^2$ = 16. Since 24 > 16, the base case holds.

Inductive step: Assume that the inequality holds for some integer k ≥ 4, i.e., k! > $k^2$. We want to show that (k+1)! > $(k+1)^2$.

(k+1)! = (k+1) * k! > (k+1) * $k^2$ (by the inductive hypothesis)

Now, we need to show that (k+1) * $k^2$ > $(k+1)^2$.

(k+1) * $k^2$ - $(k+1)^2$ = (k+1) * ($k^2$ - (k+1)) = (k+1) * ($k^2$ - k - 1)

Since k ≥ 4, we have k+1 ≥ 5 and $k^2$ - k - 1 ≥ 15. Therefore, (k+1) * ($k^2$ - k - 1) ≥ 5 * 15 = 75 > 0.

Thus, (k+1)! > $(k+1)^2$.

By induction, n! > $n^2$ for every integer n ≥ 4.

Now, to prove that n! - n^3 for every integer n ≥ 6, we can use the same induction method.

Base case: For n = 6, we have 6! = 720 and $6^3$ = 216. Since 720 > 216, the base case holds.

Inductive step: Assume that the inequality holds for some integer k ≥ 6, i.e., k! > $k^3$. We want to show that (k+1)! > $(k+1)^3$.

(k+1)! = (k+1) * k! > (k+1) * $k^3$ (by the inductive hypothesis)

Now, we need to show that (k+1) * $k^3$ > $(k+1)^3$.

(k+1) * $k^3$ - $(k+1)^3$ = (k+1) * ($k^3$ - (k+1)^2)

Since k ≥ 6, we have k+1 ≥ 7 and $k^3$ - (k+1)^2 ≥ 0 (as the function is increasing for k ≥ 6). Therefore, (k+1) * ($k^3$ - (k+1)^2) ≥ 7 * 0 = 0.

Thus, (k+1)! > $(k+1)^3$.

By induction, n! - n^3 for every integer n ≥ 6.