 To prove this, we can use mathematical induction.

Base case (n = 1):
$$a + ar = a(1 + r) = \frac{a(r^2 - 1)}{r - 1} = \frac{a(r - 1)(r + 1)}{r - 1} = a(r + 1)$$

Inductive step:
Assume the statement is true for n = k, i.e.,
$$a + ar + ar^2 + \ldots + ar^k = \frac{a(r^{k+1}-1)}{r-1}$$

Now, we need to prove that the statement is true for n = k + 1.

Consider the left-hand side of the equation for n = k + 1:
$$a + ar + ar^2 + \ldots + ar^k + ar^{k+1}$$

We can rewrite this as:
$$(a + ar + ar^2 + \ldots + ar^k) + ar^{k+1}$$

By the inductive hypothesis, we can substitute the right-hand side of the equation for n = k:
$$\frac{a(r^{k+1}-1)}{r-1} + ar^{k+1}$$

Now, we can factor out a common term of $ar^{k+1}$:
$$ar^{k+1}\left(\frac{1}{r-1} + 1\right)$$

Simplify the expression inside the parentheses:
$$ar^{k+1}\left(\frac{1 + r - 1}{r - 1}\right)$$

$$ar^{k+1}\left(\frac{r}{r - 1}\right)$$

$$ar^{k+1}\left(\frac{r^{k+1} - 1}{r^{k+1} - r}\right)$$

$$ar^{k+1}\left(\frac{r^{k+1} - 1}{r(r^k - 1)}\right)$$

$$a\left(\frac{r^{k+2} - r}{r^k - 1}\right)$$

$$a\left(\frac{r^{k+2} - 1}{r^k - 1}\right)$$

This is the right-hand side of the equation for n = k + 1.

Thus, by mathematical induction, the statement is true for any positive integer n.