 We will prove this by induction.

Base Case:
For $n=1$, we have $a_1 = 5 \cdot 2^1 + 1 = 11$, which is true.
For $n=2$, we have $a_2 = 5 \cdot 2^2 + 1 = 21$, which is also true.

Inductive Step:
Assume that the formula holds for $n=k$ and $n=k-1$, i.e.,
$$a_k = 5 \cdot 2^k + 1 \hspace{20pt} and \hspace{20pt} a_{k-1} = 5 \cdot 2^{k-1} + 1$$

We need to prove that the formula holds for $n=k+1$, i.e.,
$$a_{k+1} = 5 \cdot 2^{k+1} + 1$$

Using the recursive formula, we have
$$a_{k+1} = 3a_k - 2a_{k-1}$$

Substituting the assumed formulas, we get
$$a_{k+1} = 3(5 \cdot 2^k + 1) - 2(5 \cdot 2^{k-1} + 1)$$

Expanding and simplifying, we get
$$a_{k+1} = 15 \cdot 2^k + 3 - 10 \cdot 2^{k-1} - 2$$

Combining like terms, we get
$$a_{k+1} = 15 \cdot 2^k - 10 \cdot 2^{k-1} + 1$$

Factoring out a $2^{k-1}$ term, we get
$$a_{k+1} = 2^{k-1}(15 \cdot 2 - 10) + 1$$

Simplifying further, we get
$$a_{k+1} = 2^{k-1}(25) + 1$$

Finally, we can rewrite this as
$$a_{k+1} = 5 \cdot 2^{k+1} + 1$$

Thus, the formula holds for $n=k+1$.

By induction, the formula $a_n = 5 \cdot 2^n + 1$ holds for all $n \geq 1$.