 To use the Second Principle of Finite Induction, we need to prove two things:

1. The base case: The statement is true for $n = 1$.
2. The induction step: If the statement is true for $n = k$, then it is also true for $n = k + 1$.

Let's start with the base case:

For $n = 1$, we have:
$$a^1 - 1 = (a - 1)(a^{1-1}) = a - 1$$

So, the base case is true.

Now, let's move on to the induction step. We assume that the statement is true for $n = k$, i.e.,
$$a^k - 1 = (a - 1)(a^{k-1} + a^{k-2} + a^{k-3} + \ldots + a + 1)$$

We want to show that the statement is also true for $n = k + 1$, i.e.,
$$a^{k+1} - 1 = (a - 1)(a^{k} + a^{k-1} + a^{k-2} + \ldots + a + 1)$$

To prove this, we can multiply the assumed equation by $a$ and then subtract 1 from both sides:

$$a \cdot (a^k - 1) - 1 = a \cdot (a - 1)(a^{k-1} + a^{k-2} + a^{k-3} + \ldots + a + 1) - 1$$

Simplify the left side:

$$a^{k+1} - a - 1 = a \cdot (a - 1)(a^{k-1} + a^{k-2} + a^{k-3} + \ldots + a + 1) - 1$$

Now, we can factor out $(a - 1)$ from the right side:

$$a^{k+1} - a - 1 = (a - 1)(a \cdot (a^{k-1} + a^{k-2} + a^{k-3} + \ldots + a + 1) - 1)$$

Finally, we can rewrite the right side as:

$$a^{k+1} - a - 1 = (a - 1)(a^{k} + a^{k-1} + a^{k-2} + \ldots + a + 1)$$

This is exactly what we wanted to prove. Therefore, by the Second Principle of Finite Induction, the statement is true for all $n \geq 1$.