 (a) Base case: For $n=1$, we have $1 = \frac{1(1+1)}{2} = 1$. So the formula holds for $n=1$.

Inductive step: Assume the formula holds for $n=k$, i.e., $1 + 2 + 3 + \ldots + k = \frac{k(k+1)}{2}$. We want to show that the formula also holds for $n=k+1$, i.e., $1 + 2 + 3 + \ldots + k + (k+1) = \frac{(k+1)(k+2)}{2}$.

We can rewrite the left-hand side of the equation as $\frac{k(k+1)}{2} + (k+1)$ (by the assumption of the inductive step).

Now, we can factor out $(k+1)$ to get $\frac{k(k+1)}{2} + (k+1) = (k+1)(\frac{k}{2} + 1) = (k+1)\frac{k+2}{2}$.

This is exactly the right-hand side of the equation we want to prove, so the formula holds for $n=k+1$.

By mathematical induction, the formula $1 + 2 + 3 + \ldots + n = \frac{n(n+1)}{2}$ holds for all $n \geq 1$.

(b) Base case: For $n=1$, we have $1 = 1^2 = 1$. So the formula holds for $n=1$.

Inductive step: Assume the formula holds for $n=k$, i.e., $1 + 3 + 5 + \ldots + (2k - 1) = k^2$. We want to show that the formula also holds for $n=k+1$, i.e., $1 + 3 + 5 + \ldots + (2k - 1) + (2(k+1) - 1) = (k+1)^2$.

We can rewrite the left-hand side of the equation as $k^2 + (2(k+1) - 1)$ (by the assumption of the inductive step).

Now, we can simplify the right-hand side of the equation to get $(k+1)^2 = k^2 + 2k + 1$.

We can see that $k^2 + (2(k+1) - 1) = k^2 + 2k + 1$, so the formula holds for $n=k+1$.

By mathematical induction, the formula $1 + 3 + 5 + \ldots + (2n - 1) = n^2$ holds for all $n \geq 1$.

(c) Base case: For $n=1$, we have $1 · 2 = \frac{1(1+1)(1+2)}{3} = 2$. So the formula holds for $n=1$.

Inductive step: Assume the formula holds for $n=k$, i.e., $1 · 2 + 2 · 3 + 3 · 4 + \ldots + k(k + 1) = \frac{k(k+1)(k+2)}{3}$. We want to show that the formula also holds for $n=k+1$, i.e., $1 · 2 + 2 · 3 + 3 · 4 + \ldots + k(k + 1) + (k+1)(k+2) = \frac{(k+1)(k+2)(k+3)}{3}$.

We can rewrite the left-hand side of the equation as $\frac{k(k+1)(k+2)}{3} + (k+1)(k+2)$ (by the assumption of the inductive step).

Now, we can factor out $(k+1)(k+2)$ to get $\frac{k(k+1)(k+2)}{3} + (k+1)(k+2) = (k+1)(k+2)(\frac{k}{3} + 1) = (k+1)(k+2)\frac{k+3}{3}$.

This is exactly the right-hand side of the equation we want to prove, so the formula holds for $n=k+1$.

By mathematical induction, the formula $1 · 2 + 2 · 3 + 3 · 4 + \ldots + n(n + 1) = \frac{n(n+1)(n+2)}{3}$ holds for all $n \geq 1$.

(d) Base case: For $n=1$, we have $1^2 = \frac{1(2*1-1)(2*1+1)}{3} = 1$. So the formula holds for $n=1$.

Inductive step: Assume the formula holds for $n=k$, i.e., $1^2 + 3^2 + 5^2 + \ldots + (2k - 1)^2 = \frac{k(2k-1)(2k+1)}{3}$. We want to show that the formula also holds for $n=k+1$, i.e., $1^2 + 3^2 + 5^2 + \ldots + (2k - 1)^2 + (2(k+1) - 1)^2 = \frac{(k+1)(2(k+1)-1)(2(k+1)+1)}{3}$.

We can rewrite the left-hand side of the equation as $\frac{k(2k-1)(2k+1)}{3} + (2(k+1) - 1)^2$ (by the assumption of the inductive step).

Now, we can simplify the right-hand side of the equation to get $\frac{(k+1)(2(k+1)-1)(2(k+1)+1)}{3} = \frac{(k+1)(2k+1)(2k+3)}{3}$.

We can see that $\frac{k(2k-1)(2k+1)}{3} + (2(k+1) - 1)^2 = \frac{(k+1)(2k+1)(2k+3)}{3}$, so the formula holds for $n=k+1$.

By mathematical induction, the formula $1^2 + 3^2 + 5^2 + \ldots + (2n - 1)^2 = \frac{n(2n-1)(2n+1)}{3}$ holds for all $n \geq 1$.

(e) Base case: For $n=1$, we have $1^3 = [\frac{1(1+1)}{2}]^2 = 1$. So the formula holds for $n=1$.

Inductive step: Assume the formula holds for $n=k$, i.e., $1^3 + 2^3 + 3^3 + \ldots + k^3 = [\frac{k(k+1)}{2}]^2$. We want to show that the formula also holds for $n=k+1$, i.e., $1^3 + 2^3 + 3^3 + \ldots + k^3 + (k+1)^3 = [\frac{(k+1)(k+2)}{2}]^2$.

We can rewrite the left-hand side of the equation as $[\frac{k(k+1)}{2}]^2 + (k+1)^3$ (by the assumption of the inductive step).

Now, we can factor out $(k+1)^2$ to get $[\frac{k(k+1)}{2}]^2 + (k+1)^3 = (k+1)^2[\frac{k^2}{4} + k + 1] = (k+1)^2[\frac{k^2+4k+4}{4}] = (k+1)^2[\frac{(k+2)^2}{4}]$.

This is exactly the right-hand side of the equation we want to prove, so the formula holds for $n=k+1$.

By mathematical induction, the formula $1^3 + 2^3 + 3^3 + \ldots + n^3 = [\frac{n(n+1)}{2}]^2$ holds for all $n \geq 1$.