 To prove that the cube of any integer can be written as the difference of two squares, we will use the hint provided and the formula for the sum of consecutive cubes.

The hint suggests that we can express $n^3$ as the difference of two sums of consecutive cubes. The sum of consecutive cubes from $1$ to $n$ can be expressed as:

$$1^3 + 2^3 + \ldots + n^3 = (1 + 2 + \ldots + n)^2 = \left(\frac{n(n+1)}{2}\right)^2 = \left(\frac{n^2 + n}{2}\right)^2$$

Now, let's consider the sum of consecutive cubes from $1$ to $n-1$:

$$1^3 + 2^3 + \ldots + (n-1)^3 = \left(\frac{(n-1)(n-1+1)}{2}\right)^2 = \left(\frac{(n-1)n}{2}\right)^2$$

Now, we can express $n^3$ as the difference of these two sums:

$$n^3 = (1^3 + 2^3 + \ldots + n^3) - (1^3 + 2^3 + \ldots + (n - 1)^3)$$

Substituting the expressions for the sums of consecutive cubes, we get:

$$n^3 = \left(\frac{n^2 + n}{2}\right)^2 - \left(\frac{(n-1)n}{2}\right)^2$$

Now, let's simplify the right side of the equation:

$$n^3 = \frac{n^4 + 2n^3 + n^2}{4} - \frac{n^4 - 2n^3 + n^2}{4}$$

Combining the terms, we get:

$$n^3 = \frac{4n^3}{4} = n^3$$

Thus, we have shown that the cube of any integer $n$ can be expressed as the difference of two squares:

$$n^3 = \left(\frac{n^2 + n}{2}\right)^2 - \left(\frac{(n-1)n}{2}\right)^2$$

This completes the proof.