 To establish the Bernoulli inequality, we will use mathematical induction.

Base case (n = 1):
For n = 1, the inequality becomes:
$$(1 + a)^1 \geq{1 + a}$$
which is true since $(1 + a)^1 = 1 + a$.

Inductive step:
Assume the inequality holds for some positive integer k, i.e.,
$$(1 + a)^k \geq{1 + ka}$$

Now, we need to show that the inequality holds for k + 1.

Multiply both sides of the inequality by $(1 + a)$:
$$(1 + a)^{k+1} \geq{(1 + ka)(1 + a)}$$

Expanding the right side, we get:
$$(1 + ka)(1 + a) = 1 + a + ka + kaa$$

Since $1 + a > 0$, we can divide both sides of the inequality by $(1 + a)$:
$$(1 + a)^{k+1} \geq{1 + (k + 1)a + kaa}$$

Now, we need to show that $1 + (k + 1)a + kaa \geq{1 + (k + 1)a}$.

Subtracting $1 + (k + 1)a$ from both sides, we get:
$$kaa \geq{0}$$

Since $a > -1$, $ka > -k$, and thus $kaa > -ka$. Therefore, $kaa \geq{0}$.

Thus, the inequality holds for k + 1, and by mathematical induction, the Bernoulli inequality is established for all $n \geq{1}$.