 (a) For the first part, we will first prove the base case, which is when $n = 1$. We have $\frac{1}{1^2} = 1$ and $2 - \frac{1}{1} = 1$. So, the base case holds.

Now, we will assume that the statement is true for $n = k$, i.e., $\frac{1}{1^2} + \frac{1}{2^2} + \frac{1}{3^2} + \ldots + \frac{1}{k^2} \leq 2 - \frac{1}{k}$.

We need to prove that the statement is true for $n = k + 1$, i.e., $\frac{1}{1^2} + \frac{1}{2^2} + \frac{1}{3^2} + \ldots + \frac{1}{k^2} + \frac{1}{(k + 1)^2} \leq 2 - \frac{1}{k + 1}$.

We know that $\frac{1}{(k + 1)^2} \leq \frac{1}{k(k + 1)} = \frac{1}{k} - \frac{1}{k + 1}$ (since $\frac{1}{(k + 1)^2}$ is a decreasing function of $k$).

So, we can write $\frac{1}{1^2} + \frac{1}{2^2} + \frac{1}{3^2} + \ldots + \frac{1}{k^2} + \frac{1}{(k + 1)^2} \leq 2 - \frac{1}{k} + \frac{1}{k} - \frac{1}{k + 1} = 2 - \frac{1}{k + 1}$.

Thus, the statement is true for $n = k + 1$ if it is true for $n = k$. Since we have proved the base case, by mathematical induction, the statement is true for all $n \geq 1$.

(b) For the second part, we will first prove the base case, which is when $n = 1$. We have $\frac{1}{2} = \frac{1}{2}$ and $2 - \frac{1 + 2}{2^1} = 2 - \frac{3}{2} = \frac{1}{2}$. So, the base case holds.

Now, we will assume that the statement is true for $n = k$, i.e., $\frac{1}{2} + \frac{2}{2^2} + \frac{3}{2^3} + \ldots + \frac{k}{2^k} = 2 - \frac{k + 2}{2^k}$.

We need to prove that the statement is true for $n = k + 1$, i.e., $\frac{1}{2} + \frac{2}{2^2} + \frac{3}{2^3} + \ldots + \frac{k}{2^k} + \frac{k + 1}{2^{k + 1}} = 2 - \frac{k + 3}{2^{k + 1}}$.

We know that $\frac{k + 1}{2^{k + 1}} = \frac{1}{2} - \frac{k + 2}{2^{k + 1}}$.

So, we can write $\frac{1}{2} + \frac{2}{2^2} + \frac{3}{2^3} + \ldots + \frac{k}{2^k} + \frac{k + 1}{2^{k + 1}} = 2 - \frac{k + 2}{2^k} + \frac{1}{2} - \frac{k + 2}{2^{k + 1}} = 2 - \frac{k + 3}{2^{k + 1}}$.

Thus, the statement is true for $n = k + 1$ if it is true for $n = k$. Since we have proved the base case, by mathematical induction, the statement is true for all $n \geq 1$.