 (a) To derive Newton's identity, we start with the definition of binomial coefficients:

$$\binom{n}{k} = \frac{n!}{k!(n-k)!}$$

Now, we can rewrite the right-hand side of the identity as:

$$\binom{n}{r}\binom{n-r}{k-r} = \frac{n!}{r!(n-r)!} \cdot \frac{(n-r)!}{(k-r)!(n-k)!}$$

Simplifying the expression, we get:

$$\frac{n!}{r!(n-r)!} \cdot \frac{(n-r)!}{(k-r)!(n-k)!} = \frac{n!}{r!(k-r)!(n-k)!}$$

Now, we can rewrite the left-hand side of the identity as:

$$\binom{n}{k}\binom{k}{r} = \frac{n!}{k!(n-k)!} \cdot \frac{k!}{r!(k-r)!}$$

Simplifying the expression, we get:

$$\frac{n!}{k!(n-k)!} \cdot \frac{k!}{r!(k-r)!} = \frac{n!}{r!(k-r)!(n-k)!}$$

Comparing the expressions on both sides of the identity, we can see that they are equal:

$$\frac{n!}{k!(n-k)!} \cdot \frac{k!}{r!(k-r)!} = \frac{n!}{r!(k-r)!(n-k)!}$$

Thus, we have derived Newton's identity:

$$\binom{n}{k}\binom{k}{r}=\binom{n}{r}\binom{n-r}{k-r} \hspace{24pt} n\geq{k}\geq{r}\geq{0}$$

(b) To express $\binom{n}{k}$ in terms of its predecessor, we can use Newton's identity with $r=k-1$:

$$\binom{n}{k}\binom{k}{k-1}=\binom{n}{k-1}\binom{n-(k-1)}{k-(k-1)}$$

Simplifying the expression, we get:

$$\binom{n}{k}\cdot\frac{k}{k-1}=\binom{n}{k-1}\cdot\frac{n-k+1}{1}$$

Now, we can solve for $\binom{n}{k}$:

$$\binom{n}{k} = \frac{n-k+1}{k}\binom{n}{k-1} \hspace{24pt} n\geq{k}\geq{1}$$