 (a) We will prove this by induction.

Base case: For $n=2$, we have $\binom{2}{2} = 1$ and $\binom{3}{3} = 1$, so the equation holds.

Inductive step: Assume the equation holds for $n=k$, i.e.,
$$\binom{2}{2} + \binom{3}{2} + \binom{4}{2} + \ldots + \binom{k}{2} = \binom{k+1}{3}$$
We want to show that the equation also holds for $n=k+1$, i.e.,
$$\binom{2}{2} + \binom{3}{2} + \binom{4}{2} + \ldots + \binom{k}{2} + \binom{k+1}{2} = \binom{k+2}{3}$$

By the Pascal's identity, we have $\binom{k+1}{2} + \binom{k+1}{3} = \binom{k+2}{3}$.

Therefore, we can rewrite the right-hand side of the equation for $n=k+1$ as
$$\binom{k+1}{2} + \binom{k+1}{3} = \binom{k+2}{3}$$

By the inductive hypothesis, the left-hand side of the equation for $n=k+1$ is
$$\binom{2}{2} + \binom{3}{2} + \binom{4}{2} + \ldots + \binom{k}{2} + \binom{k+1}{2} = \binom{k+1}{3} + \binom{k+1}{2}$$

So, the equation holds for $n=k+1$ if and only if
$$\binom{k+1}{3} + \binom{k+1}{2} = \binom{k+2}{3}$$

This is true by the Pascal's identity, so the equation holds for $n=k+1$.

By the principle of mathematical induction, the equation holds for all $n \geq 2$.

(b) From the relation $m^2 = 2\binom{m}{2} + m$ for $m \geq 2$, we have
$$1^2 + 2^2 + 3^2 + \ldots + n^2 = 2\left(\binom{2}{2} + \binom{3}{2} + \binom{4}{2} + \ldots + \binom{n}{2}\right) + (1+2+3+\ldots+n)$$

By part (a), we know that $\binom{2}{2} + \binom{3}{2} + \binom{4}{2} + \ldots + \binom{n}{2} = \binom{n+1}{3}$.

And by the formula for the sum of an arithmetic series, we have $1+2+3+\ldots+n = \frac{n(n+1)}{2}$.

Substituting these into the equation above, we get
$$1^2 + 2^2 + 3^2 + \ldots + n^2 = 2\binom{n+1}{3} + \frac{n(n+1)}{2}$$

By the Pascal's identity, we have $2\binom{n+1}{3} = \binom{n+2}{3}$.

So, we can rewrite the equation as
$$1^2 + 2^2 + 3^2 + \ldots + n^2 = \binom{n+2}{3} + \frac{n(n+1)}{2}$$

By the formula for the sum of an arithmetic series, we have $\binom{n+2}{3} = \frac{n(n+1)(n+2)}{6}$.

Substituting this into the equation above, we get
$$1^2 + 2^2 + 3^2 + \ldots + n^2 = \frac{n(n+1)(n+2)}{6} + \frac{n(n+1)}{2}$$

Combining the fractions, we get
$$1^2 + 2^2 + 3^2 + \ldots + n^2 = \frac{n(n+1)(2n+1)}{6}$$

(c) We can rewrite the left-hand side of the equation in part (a) as
$$1·2 + 2·3 + \ldots + n(n+1) = \sum_{i=1}^{n} i(i+1)$$

By the formula for the sum of an arithmetic series, we have $1+2+3+\ldots+n = \frac{n(n+1)}{2}$.

So, we can rewrite the left-hand side of the equation as
$$\sum_{i=1}^{n} i(i+1) = \sum_{i=1}^{n} i + \sum_{i=1}^{n} i^2$$

By the formula for the sum of an arithmetic series, we have $\sum_{i=1}^{n} i = \frac{n(n+1)}{2}$.

And by the formula in part (b), we have $\sum_{i=1}^{n} i^2 = \frac{n(n+1)(2n+1)}{6}$.

Substituting these into the equation above, we get
$$\sum_{i=1}^{n} i(i+1) = \frac{n(n+1)}{2} + \frac{n(n+1)(2n+1)}{6}$$

Combining the fractions, we get
$$\sum_{i=1}^{n} i(i+1) = \frac{n(n+1)(n+2)}{3}$$

So, the formula holds.