 To prove these statements, we will use the properties of binomial coefficients and the concept of mathematical induction.

(a) $\binom{n}{r} < \binom{n}{r+1}$ if and only if $0 \leq r < \frac{1}{2}(n - 1)$

Proof:

We will use the property of binomial coefficients that $\binom{n}{r} = \frac{n!}{r!(n-r)!}$, where $n!$ denotes the factorial of $n$.

Let's first consider the case when $0 \leq r < \frac{1}{2}(n - 1)$. 

We have $\binom{n}{r} = \frac{n!}{r!(n-r)!}$ and $\binom{n}{r+1} = \frac{n!}{(r+1)!(n-r-1)!}$.

Now, let's compare these two expressions:

$\frac{n!}{r!(n-r)!} < \frac{n!}{(r+1)!(n-r-1)!}$

We can simplify this inequality by multiplying both sides by $r!(n-r)!(n-r)$:

$n(n-1)(n-2)...(n-r+1) < (n-r)(n-r-1)...(n-r-r+1)$

This inequality is true because the left side of the inequality has $r$ terms, while the right side has $r+1$ terms. Since $0 \leq r < \frac{1}{2}(n - 1)$, the left side is less than the right side.

Now, let's consider the case when $r \geq \frac{1}{2}(n - 1)$. 

We have $\binom{n}{r} = \frac{n!}{r!(n-r)!}$ and $\binom{n}{r+1} = \frac{n!}{(r+1)!(n-r-1)!}$.

Now, let's compare these two expressions:

$\frac{n!}{r!(n-r)!} > \frac{n!}{(r+1)!(n-r-1)!}$

We can simplify this inequality by multiplying both sides by $r!(n-r)!(n-r)$:

$n(n-1)(n-2)...(n-r+1) > (n-r)(n-r-1)...(n-r-r+1)$

This inequality is false because the left side of the inequality has $r$ terms, while the right side has $r+1$ terms. Since $r \geq \frac{1}{2}(n - 1)$, the left side is greater than the right side.

Therefore, we have shown that $\binom{n}{r} < \binom{n}{r+1}$ if and only if $0 \leq r < \frac{1}{2}(n - 1)$.

(b) $\binom{n}{r} > \binom{n}{r+1}$ if and only if $n - 1 \geq r > \frac{1}{2}(n - 1)$

Proof:

We will use the property of binomial coefficients that $\binom{n}{r} = \frac{n!}{r!(n-r)!}$.

Let's first consider the case when $n - 1 \geq r > \frac{1}{2}(n - 1)$. 

We have $\binom{n}{r} = \frac{n!}{r!(n-r)!}$ and $\binom{n}{r+1} = \frac{n!}{(r+1)!(n-r-1)!}$.

Now, let's compare these two expressions:

$\frac{n!}{r!(n-r)!} > \frac{n!}{(r+1)!(n-r-1)!}$

We can simplify this inequality by multiplying both sides by $r!(n-r)!(n-r)$:

$n(n-1)(n-2)...(n-r+1) > (n-r)(n-r-1)...(n-r-r+1)$

This inequality is true because the left side of the inequality has $r$ terms, while the right side has $r+1$ terms. Since $n - 1 \geq r > \frac{1}{2}(n - 1)$, the left side is greater than the right side.

Now, let's consider the case when $r \leq \frac{1}{2}(n - 1)$. 

We have $\binom{n}{r} = \frac{n!}{r!(n-r)!}$ and $\binom{n}{r+1} = \frac{n!}{(r+1)!(n-r-1)!}$.

Now, let's compare these two expressions:

$\frac{n!}{r!(n-r)!} < \frac{n!}{(r+1)!(n-r-1)!}$

We can simplify this inequality by multiplying both sides by $r!(n-r)!(n-r)$:

$n(n-1)(n-2)...(n-r+1) < (n-r)(n-r-1)...(n-r-r+1)$

This inequality is false because the left side of the inequality has $r$ terms, while the right side has $r+1$ terms. Since $r \leq \frac{1}{2}(n - 1)$, the left side is less than the right side.

Therefore, we have shown that $\binom{n}{r} > \binom{n}{r+1}$ if and only if $n - 1 \geq r > \frac{1}{2}(n - 1)$.

(c) $\binom{n}{r} = \binom{n}{r+1}$ if and only if $n$ is an odd integer, and $r = \frac{1}{2}(n - 1)$

Proof:

We will use the property of binomial coefficients that $\binom{n}{r} = \frac{n!}{r!(n-r)!}$.

Let's consider the case when $\binom{n}{r} = \binom{n}{r+1}$.

We have $\frac{n!}{r!(n-r)!} = \frac{n!}{(r+1)!(n-r-1)!}$.

We can simplify this equation by multiplying both sides by $r!(n-r)!(n-r)$:

$n(n-1)(n-2)...(n-r+1) = (n-r)(n-r-1)...(n-r-r+1)$

This equation is true if and only if $n$ is an odd integer, and $r = \frac{1}{2}(n - 1)$.

Therefore, we have shown that $\binom{n}{r} = \binom{n}{r+1}$ if and only if $n$ is an odd integer, and $r = \frac{1}{2}(n - 1)$.