 To prove the inductive formula, we first need to express $C_n$ in terms of $C_{n-1}$. We can do this by using the definition of the Catalan numbers and the binomial coefficient.

The definition of the Catalan numbers is given by:

$$C_n = \frac{1}{n+1}\binom{2n}{n} = \frac{(2n)!}{n!(n+1)!}$$

We can rewrite the binomial coefficient as:

$$\binom{2n}{n} = \frac{(2n)!}{n!n!}$$

Now, we can express $C_n$ in terms of $C_{n-1}$:

$$C_n = \frac{1}{n+1}\binom{2n}{n} = \frac{1}{n+1}\frac{(2n)!}{n!n!} = \frac{1}{n+1}\frac{(2n-1)!}{(n-1)!(n)!}$$

We can rewrite the factorial in the denominator as:

$$(n-1)! = \frac{n!}{n}$$

Substituting this into the expression for $C_n$, we get:

$$C_n = \frac{1}{n+1}\frac{(2n-1)!}{\frac{n!}{n}(n!)} = \frac{1}{n+1}\frac{(2n-1)!}{n!n}$$

Now, we can express the factorial in the numerator as:

$$(2n-1)! = (2n)!$$

Substituting this into the expression for $C_n$, we get:

$$C_n = \frac{1}{n+1}\frac{(2n)!}{n!n}$$

Now, we can express $C_{n-1}$ in terms of $C_n$:

$$C_{n-1} = \frac{1}{n}\binom{2n-2}{n-1} = \frac{1}{n}\frac{(2n-2)!}{(n-1)!(n-1)!}$$

We can rewrite the factorial in the denominator as:

$$(n-1)! = \frac{n!}{n}$$

Substituting this into the expression for $C_{n-1}$, we get:

$$C_{n-1} = \frac{1}{n}\frac{(2n-2)!}{\frac{n!}{n}\frac{n!}{n}} = \frac{1}{n}\frac{(2n-2)!}{n!n}$$

Now, we can express the factorial in the numerator as:

$$(2n-2)! = (2n-1)!$$

Substituting this into the expression for $C_{n-1}$, we get:

$$C_{n-1} = \frac{1}{n}\frac{(2n-1)!}{n!n}$$

Now, we can express $C_n$ in terms of $C_{n-1}$:

$$C_n = \frac{2(2n-1)}{n+1}C_{n-1}$$

This is the inductive formula that we wanted to prove.