 We will prove this by induction.

Base case: For $n=1$, we have $1^2 = \binom{2(1)+1}{3} = \binom{3}{3} = 1$. So the statement holds for $n=1$.

Inductive step: Assume that the statement holds for $n=k$, i.e.,
$$1^2 + 3^2 + 5^2 +\ldots + (2k-1)^2 = \binom{2k+1}{3}.$$
We want to show that the statement also holds for $n=k+1$, i.e.,
$$1^2 + 3^2 + 5^2 +\ldots + (2k-1)^2 + (2(k+1)-1)^2 = \binom{2(k+1)+1}{3}.$$

Consider the left-hand side of the equation for $n=k+1$:
$$1^2 + 3^2 + 5^2 +\ldots + (2k-1)^2 + (2(k+1)-1)^2 = \binom{2k+1}{3} + (2(k+1)-1)^2.$$

We know from the induction hypothesis that the first part of this expression is equal to $\binom{2k+1}{3}$. Now we need to show that the second part of the expression, $(2(k+1)-1)^2$, is equal to $\binom{2(k+1)+1}{3} - \binom{2k+1}{3}$.

We have
\begin{align*}
(2(k+1)-1)^2 &= (2k+1)^2 \\
&= (2k+1)(2k+1) \\
&= (2k+1)\left((2k+1) - 1\right) + (2k+1) - 1 \\
&= (2k+1)(2k) + 2k \\
&= 2k(2k+1) + 2k \\
&= 2k^2 + 2k + 2k \\
&= 2k(k+1) + 2k \\
&= 2k(k+1) + 2k(1) \\
&= 2k(k+1+1) \\
&= 2k(k+2) \\
&= 2k(k+1) + 2k \\
&= 2\binom{2k+1}{2} + 2k \\
&= \binom{2k+1}{2} + \binom{2k+1}{2} + 2k \\
&= \binom{2k+1}{2} + \binom{2k+1}{2} + \binom{2k+1}{1} \\
&= \binom{2k+1+1}{3} \\
&= \binom{2(k+1)+1}{3}.
\end{align*}

Therefore, we have
$$\binom{2k+1}{3} + (2(k+1)-1)^2 = \binom{2k+1}{3} + \binom{2(k+1)+1}{3} = \binom{2(k+1)+1}{3}.$$

This completes the induction step.

By the principle of mathematical induction, the statement holds for all $n \geq 1$.