 (a) Let a = b = 1 in the binomial theorem, we get:
$(1+1)^n = \binom{n}{0} + \binom{n}{1} + \binom{n}{2} + \ldots + \binom{n}{n}$
$2^n = \binom{n}{0} + \binom{n}{1} + \binom{n}{2} + \ldots + \binom{n}{n}$

(b) Let a = 1 and b = -1 in the binomial theorem, we get:
$(1+(-1))^n = \binom{n}{0} - \binom{n}{1} + \binom{n}{2} + \ldots + (-1)^n\binom{n}{n}$
$0 = \binom{n}{0} - \binom{n}{1} + \binom{n}{2} + \ldots + (-1)^n\binom{n}{n}$

(c) Let a = 1 and b = 2 in the binomial theorem, we get:
$(1+2)^n = \binom{n}{0} + 2\binom{n}{1} + 2^2\binom{n}{2} + \ldots + 2^n\binom{n}{n}$
$3^n = \binom{n}{0} + 2\binom{n}{1} + 2^2\binom{n}{2} + \ldots + 2^n\binom{n}{n}$

(d) Let a = 1 and b = 2 in the binomial theorem, we get:
$(1+2)^n = \binom{n}{0} + 2\binom{n}{1} + 2^2\binom{n}{2} + \ldots + 2^n\binom{n}{n}$
$3^n = \binom{n}{0} + 2\binom{n}{1} + 2^2\binom{n}{2} + \ldots + 2^n\binom{n}{n}$

(e) Let a = 1 and b = -1 in the binomial theorem, we get:
$(1+(-1))^n = \binom{n}{0} - \binom{n}{1} + \binom{n}{2} + \ldots + (-1)^n\binom{n}{n}$
$0 = \binom{n}{0} - \binom{n}{1} + \binom{n}{2} + \ldots + (-1)^n\binom{n}{n}$

(f) Let a = 1 and b = -1 in the binomial theorem, we get:
$(1+(-1))^n = \binom{n}{0} - \binom{n}{1} + \binom{n}{2} + \ldots + (-1)^n\binom{n}{n}$
$0 = \binom{n}{0} - \binom{n}{1} + \binom{n}{2} + \ldots + (-1)^n\binom{n}{n}$

All the identities are derived.