I'll verify these relations step by step.

First, recall the formulas:
- Triangular numbers: \( t_n = \frac{n(n+1)}{2} \)
- Square numbers: \( n^2 \)
- Pentagonal numbers: \( p_n = \frac{n(3n-1)}{2} \)

Now let's verify each relation:

**(a) \( p_n = t_{n-1} + n^2 \)**

Left side: \( p_n = \frac{n(3n-1)}{2} \)

Right side: \( t_{n-1} + n^2 = \frac{(n-1)n}{2} + n^2 = \frac{n(n-1) + 2n^2}{2} = \frac{n^2 - n + 2n^2}{2} = \frac{3n^2 - n}{2} = \frac{n(3n-1)}{2} \)

✅ Both sides are equal.

**(b) \( p_n = 3t_{n-1} + n = 2t_{n-1} + t_n \)**

First equality: \( p_n = 3t_{n-1} + n \)

Left side: \( p_n = \frac{n(3n-1)}{2} \)

Right side: \( 3t_{n-1} + n = 3 \cdot \frac{(n-1)n}{2} + n = \frac{3n(n-1)}{2} + n = \frac{3n^2 - 3n + 2n}{2} = \frac{3n^2 - n}{2} = \frac{n(3n-1)}{2} \)

✅ First equality holds.

Second equality: \( p_n = 2t_{n-1} + t_n \)

Left side: \( p_n = \frac{n(3n-1)}{2} \)

Right side: \( 2t_{n-1} + t_n = 2 \cdot \frac{(n-1)n}{2} + \frac{n(n+1)}{2} = n(n-1) + \frac{n(n+1)}{2} = \frac{2n(n-1) + n(n+1)}{2} = \frac{2n^2 - 2n + n^2 + n}{2} = \frac{3n^2 - n}{2} = \frac{n(3n-1)}{2} \)

✅ Second equality holds.

All relations are verified to be true for n ≥ 2.

```lean
theorem pentagonal_relations (n : ℕ) (h : n ≥ 2) :
    -- (a) pₙ = tₙ₋₁ + n²
    (pentagonal n = triangular (n-1) + n^2) ∧
    -- (b) pₙ = 3tₙ₋₁ + n = 2tₙ₋₁ + tₙ
    (pentagonal n = 3 * triangular (n-1) + n) ∧
    (pentagonal n = 2 * triangular (n-1) + triangular n) := by
  -- Define the number formulas
  have triangular_eq : ∀ k, triangular k = k*(k+1)/2 := by
    intro k; exact rfl
  have pentagonal_eq : ∀ k, pentagonal k = k*(3*k-1)/2 := by
    intro k; exact rfl
  
  -- Prove each equality through algebraic manipulation
  constructor
  · -- Part (a)
    rw [pentagonal_eq, triangular_eq, show (n-1)*n/2 + n^2 = n*(3*n-1)/2 by ring]
  constructor
  · -- First part of (b)
    rw [pentagonal_eq, triangular_eq, show 3*((n-1)*n/2) + n = n*(3*n-1)/2 by ring]
  · -- Second part of (b)
    rw [pentagonal_eq, triangular_eq, triangular_eq, show 2*((n-1)*n/2) + (n*(n+1)/2) = n*(3*n-1)/2 by ring]
```

**Verification Summary:**

All three relations between pentagonal, square, and triangular numbers have been algebraically verified:
- (a) Pentagonal number equals previous triangular number plus square number
- (b) Pentagonal number equals three times previous triangular number plus n, and also equals twice previous triangular number plus current triangular number

These identities hold for all integers n ≥ 2.