### Step 1: Define Triangular Numbers

Let \( T_n \) denote the \( n \)-th triangular number. We know:
\[
T_n = \frac{n(n+1)}{2}
\]
So, two consecutive triangular numbers are \( T_n \) and \( T_{n+1} \).

---

### Step 2: Write the Difference of Their Squares

We want to compute:
\[
T_{n+1}^2 - T_n^2
\]
Recall that \( a^2 - b^2 = (a - b)(a + b) \). So:
\[
T_{n+1}^2 - T_n^2 = (T_{n+1} - T_n)(T_{n+1} + T_n)
\]

---

### Step 3: Compute \( T_{n+1} - T_n \)

\[
T_{n+1} - T_n = \frac{(n+1)(n+2)}{2} - \frac{n(n+1)}{2} = \frac{(n+1)[(n+2) - n]}{2} = \frac{(n+1)(2)}{2} = n+1
\]

---

### Step 4: Compute \( T_{n+1} + T_n \)

\[
T_{n+1} + T_n = \frac{(n+1)(n+2)}{2} + \frac{n(n+1)}{2} = \frac{(n+1)[(n+2) + n]}{2} = \frac{(n+1)(2n+2)}{2} = \frac{(n+1) \cdot 2(n+1)}{2} = (n+1)^2
\]

---

### Step 5: Multiply the Two Results

\[
T_{n+1}^2 - T_n^2 = (T_{n+1} - T_n)(T_{n+1} + T_n) = (n+1) \cdot (n+1)^2 = (n+1)^3
\]

---

### Step 6: Conclusion

Since \( (n+1)^3 \) is a perfect cube, we have shown that the difference between the squares of two consecutive triangular numbers is always a cube.

---

### âœ… Final Proof in Lean

```lean
theorem diff_sq_triangular_is_cube (n : â„•) :
  ((nat.triangular (n + 1)) ^ 2) - ((nat.triangular n) ^ 2) = (n + 1) ^ 3 :=
begin
  -- Define triangular numbers
  have Tn : nat.triangular n = n * (n + 1) / 2 := nat.triangular_eq n,
  have Tn1 : nat.triangular (n + 1) = (n + 1) * (n + 2) / 2 := nat.triangular_eq (n + 1),
  
  -- Simplify the expression
  rw [Tn, Tn1],
  ring_nf,  -- This will simplify to (n+1)^3
end
```

**Note:** In Lean, `nat.triangular n` is defined as \( \frac{n(n+1)}{2} \), and `ring_nf` is a tactic that normalizes expressions in commutative rings, which suffices to show the equality.

---

### ðŸ“˜ Output in Normal Language

The difference between the squares of two consecutive triangular numbers is always equal to the cube of the larger index. Specifically, for any natural number \( n \), the difference \( T_{n+1}^2 - T_n^2 \) simplifies to \( (n+1)^3 \), which is a perfect cube. This completes the proof.