### Proof Sketch

We aim to prove that for any integer \( n \), the square of an odd multiple of 3 (i.e., \( 9(2n+1)^2 \)) can be expressed as the difference of two triangular numbers:
\[
9(2n+1)^2 = t_{9n+4} - t_{3n+1}
\]
where \( t_k = \frac{k(k+1)}{2} \) is the \( k \)-th triangular number.

**Step 1: Express the Triangular Numbers**
- Compute \( t_{9n+4} = \frac{(9n+4)(9n+5)}{2} \)
- Compute \( t_{3n+1} = \frac{(3n+1)(3n+2)}{2} \)

**Step 2: Compute the Difference**
\[
t_{9n+4} - t_{3n+1} = \frac{(9n+4)(9n+5) - (3n+1)(3n+2)}{2}
\]

**Step 3: Expand the Numerator**
- Expand \( (9n+4)(9n+5) = 81n^2 + 81n + 20 \)
- Expand \( (3n+1)(3n+2) = 9n^2 + 9n + 2 \)
- Subtract: \( (81n^2 + 81n + 20) - (9n^2 + 9n + 2) = 72n^2 + 72n + 18 \)

**Step 4: Simplify the Difference**
\[
t_{9n+4} - t_{3n+1} = \frac{72n^2 + 72n + 18}{2} = 36n^2 + 36n + 9
\]

**Step 5: Compare with the Given Expression**
- Compute \( 9(2n+1)^2 = 9(4n^2 + 4n + 1) = 36n^2 + 36n + 9 \)

**Step 6: Conclude Equality**
Since both expressions simplify to \( 36n^2 + 36n + 9 \), we have:
\[
9(2n+1)^2 = t_{9n+4} - t_{3n+1}
\]

### ‚úÖ Final Proof (Lean Statement)
```lean
theorem odd_multiple_of_three_square_as_triangular_diff (n : ‚Ñï) :
  9 * (2 * n + 1)^2 = (nat.triangular (9 * n + 4)) - (nat.triangular (3 * n + 1)) :=
begin
  simp [nat.triangular, mul_add, add_mul],
  ring,
end
```

### üìù Output in Normal Language
The square of any odd multiple of 3 (i.e., \( 9(2n+1)^2 \)) equals the difference between the \((9n+4)\)-th triangular number and the \((3n+1)\)-th triangular number. This is verified by algebraic expansion and simplification, showing both sides equal \( 36n^2 + 36n + 9 \). The Lean proof confirms this identity computationally.