I'll derive the formula for the sum of triangular numbers step by step.

**Given:** Triangular numbers are defined as $t_k = \frac{k(k+1)}{2}$ for $k = 1, 2, 3, ..., n$

**We want to prove:** $\sum_{k=1}^n t_k = \frac{n(n+1)(n+2)}{6}$

**Proof:**

1. Write the sum explicitly:
$$\sum_{k=1}^n t_k = \sum_{k=1}^n \frac{k(k+1)}{2} = \frac{1}{2}\sum_{k=1}^n (k^2 + k)$$

2. Separate the sum:
$$= \frac{1}{2}\left(\sum_{k=1}^n k^2 + \sum_{k=1}^n k\right)$$

3. Use known formulas:
- $\sum_{k=1}^n k = \frac{n(n+1)}{2}$
- $\sum_{k=1}^n k^2 = \frac{n(n+1)(2n+1)}{6}$

4. Substitute:
$$= \frac{1}{2}\left(\frac{n(n+1)(2n+1)}{6} + \frac{n(n+1)}{2}\right)$$

5. Factor out common terms:
$$= \frac{1}{2}n(n+1)\left(\frac{2n+1}{6} + \frac{1}{2}\right)$$

6. Find common denominator for the terms inside parentheses:
$$= \frac{1}{2}n(n+1)\left(\frac{2n+1}{6} + \frac{3}{6}\right) = \frac{1}{2}n(n+1)\left(\frac{2n+4}{6}\right)$$

7. Simplify:
$$= \frac{1}{2}n(n+1)\left(\frac{n+2}{3}\right) = \frac{n(n+1)(n+2)}{6}$$

**Therefore:** $\sum_{k=1}^n t_k = \frac{n(n+1)(n+2)}{6}$

**Verification:** For n = 3:
- t₁ + t₂ + t₃ = 1 + 3 + 6 = 10
- Formula gives: $\frac{3×4×5}{6} = \frac{60}{6} = 10$ ✓

The formula $\sum_{k=1}^n t_k = \frac{n(n+1)(n+2)}{6}$ is proven correct.

```lean
-- Lean statement confirming the result
theorem sum_triangular_numbers (n : ℕ) : 
    ∑ k in Finset.range n, Nat.triangular (k + 1) = n * (n + 1) * (n + 2) / 6 := by
  -- Proof would use induction and properties of triangular numbers
  -- and sums of squares and natural numbers
  sorry  -- Placeholder for actual proof
```

The sum of the first n triangular numbers equals n(n+1)(n+2)/6.