I will prove the formula \( p_n = \frac{n(3n-1)}{2} \) for all \( n \geq 1 \) by mathematical induction.

**Base Case (n = 1):**
\[
p_1 = \frac{1 \cdot (3 \cdot 1 - 1)}{2} = \frac{1 \cdot (3 - 1)}{2} = \frac{2}{2} = 1
\]
This matches the given \( p_1 = 1 \).

**Inductive Step:**
Assume the formula holds for \( n = k \), i.e.,
\[
p_k = \frac{k(3k - 1)}{2}
\]
We want to show it holds for \( n = k+1 \), i.e.,
\[
p_{k+1} = \frac{(k+1)(3(k+1) - 1)}{2} = \frac{(k+1)(3k + 2)}{2}
\]

From the recurrence relation:
\[
p_{k+1} = p_k + (3(k+1) - 2) = p_k + (3k + 3 - 2) = p_k + (3k + 1)
\]

Substitute the inductive hypothesis:
\[
p_{k+1} = \frac{k(3k - 1)}{2} + (3k + 1) = \frac{k(3k - 1) + 2(3k + 1)}{2}
\]
\[
= \frac{3k^2 - k + 6k + 2}{2} = \frac{3k^2 + 5k + 2}{2}
\]

Now, factor the numerator:
\[
3k^2 + 5k + 2 = (k+1)(3k+2)
\]
So,
\[
p_{k+1} = \frac{(k+1)(3k+2)}{2}
\]
which is exactly the desired formula for \( n = k+1 \).

By mathematical induction, the formula \( p_n = \frac{n(3n-1)}{2} \) holds for all \( n \geq 1 \).

---

**Lean 4 Statement:**
```lean
theorem pentagonal_number_formula (n : ℕ) (h : n ≥ 1) : p n = (n * (3 * n - 1)) / 2 := by
  -- Here p is defined with p 1 = 1 and the recurrence relation for n ≥ 2.
  -- The proof would use induction and the recurrence.
  -- (Actual Lean code would require defining the function p first.)
```

**Output in Normal Language:**
The pentagonal number \( p_n \) is given by the formula \( \frac{n(3n-1)}{2} \) for all \( n \geq 1 \). This is proven by induction: the base case \( n=1 \) holds, and assuming it holds for \( n=k \), it also holds for \( n=k+1 \) using the recurrence relation \( p_{k+1} = p_k + (3(k+1)-2) \). Thus, the formula is valid for all positive integers \( n \).