### Step-by-Step Proof:

We aim to prove that for every integer \( n \geq 1 \), the expression \( \frac{n(n + 1)(2n + 1)}{6} \) is an integer.

#### 1. **Recognize the Formula**:
This expression is known to be the formula for the sum of the first \( n \) squares:
\[
1^2 + 2^2 + \cdots + n^2 = \frac{n(n + 1)(2n + 1)}{6}.
\]
Since the sum of integers (squares) is an integer, the result must be an integer.

#### 2. **Alternate Approach: Divisibility Argument**:
To explicitly show divisibility by 6, note that \( n(n+1)(2n+1) \) must be divisible by 6. Since 6 = 2 × 3, we show divisibility by 2 and 3.

- **Divisibility by 2**: Among \( n \) and \( n+1 \), one is even, so their product is divisible by 2.
- **Divisibility by 3**: Consider \( n \) modulo 3:
  - If \( n \equiv 0 \pmod{3} \), then \( n \) is divisible by 3.
  - If \( n \equiv 1 \pmod{3} \), then \( 2n+1 \equiv 2\cdot1 + 1 = 3 \equiv 0 \pmod{3} \).
  - If \( n \equiv 2 \pmod{3} \), then \( n+1 \equiv 2+1 = 3 \equiv 0 \pmod{3} \).
In all cases, \( n(n+1)(2n+1) \) is divisible by 3.

Thus, \( n(n+1)(2n+1) \) is divisible by both 2 and 3, hence by 6. Therefore, \( \frac{n(n+1)(2n+1)}{6} \) is an integer.

#### 3. **Conclusion**:
For every integer \( n \geq 1 \), \( \frac{n(n+1)(2n+1)}{6} \) is an integer.

---

### Lean 4 Statement:
```lean
theorem sum_of_squares_integer (n : ℕ) : ∃ k : ℕ, (n * (n + 1) * (2 * n + 1)) / 6 = k := by
  have h : (6 : ℕ) ∣ n * (n + 1) * (2 * n + 1) := by
    -- Proof that 2 ∣ n*(n+1)*(2n+1)
    have h2 : 2 ∣ n * (n + 1) := by
      have : 2 ∣ n * (n + 1) := by
        exact by simp [mul_comm, show 2 ∣ n * (n+1) from ?_] -- Alternatively, use that one of n, n+1 is even.
      sorry  -- Fill in with detailed proof for divisibility by 2
    -- Proof that 3 ∣ n*(n+1)*(2n+1)
    have h3 : 3 ∣ n * (n + 1) * (2 * n + 1) := by
      sorry  -- Based on the modulo argument above
    exact Nat.dvd_mul_of_dvd_mul h2 h3?  -- Actually need to combine divisibility by 2 and 3. Alternatively, use `Nat.dvd_gcd` or show directly.
  -- Since 6 divides the numerator, the division is exact.
  exact ⟨(n * (n + 1) * (2 * n + 1)) / 6, rfl⟩
```
*Note: The Lean proof above is a sketch. A complete Lean proof would require filling in the divisibility details, possibly using tactics like `omega` or case analysis on `n % 3`.*

---

### Output in Normal Language:
For every integer \( n \geq 1 \), the expression \( \frac{n(n+1)(2n+1)}{6} \) is an integer. This is because it equals the sum of the squares of the first \( n \) natural numbers, which is an integer. Alternatively, one can show that \( n(n+1)(2n+1) \) is always divisible by 6 due to divisibility by 2 (since either \( n \) or \( n+1 \) is even) and by 3 (by checking cases modulo 3). Hence, the division by 6 yields an integer result.