Let's verify each statement step by step.

### (a) Verify: \(2 \mid a(a+1)\) and \(3 \mid a(a+1)(a+2)\)

1. **\(2 \mid a(a+1)\)**:
   - Among any two consecutive integers, one must be even (divisible by 2).
   - Therefore, \(a(a+1)\) is always divisible by 2.

2. **\(3 \mid a(a+1)(a+2)\)**:
   - Among any three consecutive integers, one must be divisible by 3.
   - Therefore, \(a(a+1)(a+2)\) is always divisible by 3.

**Conclusion**: Both statements are true for any integer \(a\).

---

### (b) Verify: \(3 \mid a(2a^2 + 7)\)

We need to show that \(a(2a^2 + 7)\) is divisible by 3 for all integers \(a\).

Consider \(a\) modulo 3:

- If \(a \equiv 0 \pmod{3}\), then \(a(2a^2 + 7) \equiv 0 \cdot (2 \cdot 0 + 7) \equiv 0 \pmod{3}\).
- If \(a \equiv 1 \pmod{3}\), then:
  \(2a^2 + 7 \equiv 2(1)^2 + 7 \equiv 2 + 7 \equiv 9 \equiv 0 \pmod{3}\),
  so \(a(2a^2 + 7) \equiv 1 \cdot 0 \equiv 0 \pmod{3}\).
- If \(a \equiv 2 \pmod{3}\), then:
  \(2a^2 + 7 \equiv 2(4) + 7 \equiv 8 + 7 \equiv 15 \equiv 0 \pmod{3}\),
  so \(a(2a^2 + 7) \equiv 2 \cdot 0 \equiv 0 \pmod{3}\).

In all cases, \(a(2a^2 + 7) \equiv 0 \pmod{3}\).

**Conclusion**: \(3 \mid a(2a^2 + 7)\) for any integer \(a\).

---

### (c) If \(a\) is odd, then \(32 \mid (a^2 + 3)(a^2 + 7)\)

Let \(a\) be odd. Write \(a = 2k + 1\) for some integer \(k\).

Then:
\[
a^2 = (2k+1)^2 = 4k^2 + 4k + 1 = 4k(k+1) + 1.
\]
Since \(k(k+1)\) is even (as one of \(k\) or \(k+1\) is even), let \(k(k+1) = 2m\) for some integer \(m\). Then:
\[
a^2 = 4 \cdot 2m + 1 = 8m + 1.
\]
So:
\[
a^2 + 3 = 8m + 1 + 3 = 8m + 4 = 4(2m + 1),
\]
\[
a^2 + 7 = 8m + 1 + 7 = 8m + 8 = 8(m + 1).
\]
Therefore:
\[
(a^2 + 3)(a^2 + 7) = [4(2m+1)] \cdot [8(m+1)] = 32 \cdot (2m+1)(m+1).
\]
This is clearly divisible by 32.

**Conclusion**: If \(a\) is odd, then \(32 \mid (a^2 + 3)(a^2 + 7)\).

---

### Summary of Results:
- (a) True: \(2 \mid a(a+1)\) and \(3 \mid a(a+1)(a+2)\) for any integer \(a\).
- (b) True: \(3 \mid a(2a^2 + 7)\) for any integer \(a\).
- (c) True: If \(a\) is odd, then \(32 \mid (a^2 + 3)(a^2 + 7)\).

All statements are verified.

---

### Lean 4 Statements:

```lean
theorem part_a (a : ℤ) : 2 ∣ a * (a + 1) := by
  have : Even (a * (a + 1)) := by
    rcases em (Even a) with (⟨k, hk⟩ | h)
    · exact ⟨k * (2*k + 1), by linear_combination [hk]⟩
    · have : Even (a + 1) := by
        rcases odd_iff.mp (odd_iff_not_even.mpr h) with ⟨k, hk⟩
        exact ⟨k+1, by linear_combination [hk]⟩
      rcases this with ⟨k, hk⟩
      exact ⟨k * (2*k - 1), by linear_combination [hk]⟩
  exact this

theorem part_a2 (a : ℤ) : 3 ∣ a * (a + 1) * (a + 2) := by
  have : ∃ k : ℤ, a * (a + 1) * (a + 2) = 3 * k := by
    apply int.mod_three_cases a
    · intro h
      exact ⟨(a/3)*(a/3+1)*(a/3+2), by linear_combination [h]⟩
    · intro h
      obtain ⟨k, hk⟩ := h
      exact ⟨(3*k+1)*k*(k+1), by linear_combination [hk]⟩
    · intro h
      obtain ⟨k, hk⟩ := h
      exact ⟨(3*k+2)*k*(k+1), by linear_combination [hk]⟩
  exact this

theorem part_b (a : ℤ) : 3 ∣ a * (2 * a ^ 2 + 7) := by
  apply int.mod_three_cases a
  · intro h
    exact ⟨(a/3)*(2*(a/3)^2+7), by linear_combination [h]⟩
  · intro h
    obtain ⟨k, hk⟩ := h
    have : 2*(3*k+1)^2 + 7 = 3*(6*k^2+4*k+3) := by ring
    exact ⟨(3*k+1)*(6*k^2+4*k+3), by linear_combination [hk, this]⟩
  · intro h
    obtain ⟨k, hk⟩ := h
    have : 2*(3*k+2)^2 + 7 = 3*(6*k^2+8*k+5) := by ring
    exact ⟨(3*k+2)*(6*k^2+8*k+5), by linear_combination [hk, this]⟩

theorem part_c (a : ℤ) (h : Odd a) : 32 ∣ (a ^ 2 + 3) * (a ^ 2 + 7) := by
  rcases h with ⟨k, rfl⟩
  have h1 : (2*k+1)^2 + 3 = 4*(2*k^2+2*k+1) := by ring
  have h2 : (2*k+1)^2 + 7 = 8*(k+1) := by ring
  rw [h1, h2]
  ring_nf
  exact ⟨(2*k^2+2*k+1)*(k+1), by ring⟩
```

Note: The above Lean code uses some auxiliary lemmas (e.g., `int.mod_three_cases`, `odd_iff`, etc.) which are not built-in. In practice, you might need to define these or use existing library results. The proofs are written to reflect the mathematical reasoning.

---

### Output in Normal Language:
- (a) For any integer \(a\), the product \(a(a+1)\) is always divisible by 2, and \(a(a+1)(a+2)\) is always divisible by 3.
- (b) For any integer \(a\), the expression \(a(2a^2 + 7)\) is always divisible by 3.
- (c) If \(a\) is odd, then \((a^2 + 3)(a^2 + 7)\) is divisible by 32.

All statements are true.