### Proof in Lean 4

```lean
theorem odd_square_form (a : ℤ) (ha : Odd a) : ∃ (k : ℤ), a^2 = 8*k + 1 := by
  rcases ha with ⟨x, rfl⟩
  use 2*x^2 + x
  ring_nf

theorem part_b (a : ℤ) (ha : Odd a) : 24 ∣ a * (a^2 - 1) := by
  -- Factor the expression: a(a² - 1) = (a-1)a(a+1) - three consecutive integers
  have hprod := a * (a^2 - 1)
  have hfact : a * (a^2 - 1) = (a - 1) * a * (a + 1) := by ring
  
  -- Among three consecutive integers, one is divisible by 3
  have h3 : 3 ∣ (a - 1) * a * (a + 1) := by
    have : ∃ (b : ℤ), 3 ∣ a + b ∧ (b = -1 ∨ b = 0 ∨ b = 1) := by
      have := Int.mod_eq_zero_or_eq_one_or_eq_two (a % 3)
      omega
    rcases this with ⟨b, hb, hbval⟩
    rcases hbval with (rfl|rfl|rfl)
    · exact ⟨a - 1, by ring⟩
    · exact ⟨a, by ring⟩
    · exact ⟨a + 1, by ring⟩
  
  -- Since a is odd, a² ≡ 1 mod 8, so a(a² - 1) ≡ 0 mod 8
  have h8 : 8 ∣ a * (a^2 - 1) := by
    rcases odd_square_form a ha with ⟨k, hk⟩
    rw [hk]
    have : a * (8*k + 1 - 1) = 8*(a*k) := by ring
    exact ⟨a*k, by ring⟩
  
  -- Since 3 and 8 are coprime, their product divides a(a² - 1)
  exact Nat.dvd_gcd h3 h8 |>.trans (by norm_num)
```

### Proof Explanation

**Assertion**: If \( a \) is an odd integer, then \( 24 \mid a(a^2 - 1) \).

**Proof**:

1. **Factorization**:  
   Note that \( a(a^2 - 1) = (a-1)a(a+1) \). This is the product of three consecutive integers.

2. **Divisibility by 3**:  
   Among any three consecutive integers, exactly one is divisible by 3. Therefore, \( 3 \mid (a-1)a(a+1) \).

3. **Divisibility by 8**:  
   Since \( a \) is odd, we can write \( a = 2k + 1 \) for some integer \( k \). Then:
   \[
   a^2 = (2k + 1)^2 = 4k(k + 1) + 1.
   \]
   Since \( k(k+1) \) is even (as one of \( k \) or \( k+1 \) is even), \( 4k(k+1) \) is divisible by 8. Thus, \( a^2 \equiv 1 \pmod{8} \), so \( a^2 - 1 \equiv 0 \pmod{8} \). Hence, \( 8 \mid a(a^2 - 1) \).

4. **Combining Results**:  
   Since \( \gcd(3, 8) = 1 \), and both 3 and 8 divide \( a(a^2 - 1) \), their product \( 24 \) also divides \( a(a^2 - 1) \).

✅ Therefore, \( 24 \mid a(a^2 - 1) \) for any odd integer \( a \).

### Output in Normal Language

If \( a \) is an odd integer, then \( a(a^2 - 1) \) is divisible by 24. This follows because:
- The product \( (a-1)a(a+1) \) of three consecutive integers is always divisible by 3.
- For odd \( a \), \( a^2 \equiv 1 \pmod{8} \), so \( a^2 - 1 \) is divisible by 8, making \( a(a^2 - 1) \) divisible by 8.
- Since 3 and 8 are coprime, their product 24 divides \( a(a^2 - 1) \).

Thus, the assertion is proven.