### Step 1: Understand the Problem

We are to prove:  
If \( a \) is an integer not divisible by 2 or 3, then \( 24 \mid (a^2 + 23) \).

This means \( a \) is odd and not divisible by 3. So \( a \equiv \pm1 \pmod{6} \).

We need to show \( a^2 + 23 \equiv 0 \pmod{24} \).

---

### Step 2: Reformulate Modulo 24

Since \( 24 = 8 \cdot 3 \), we check modulo 8 and modulo 3.

We need:
1. \( a^2 + 23 \equiv 0 \pmod{8} \)
2. \( a^2 + 23 \equiv 0 \pmod{3} \)

---

### Step 3: Check Modulo 3

Given \( a \not\equiv 0 \pmod{3} \), so \( a \equiv \pm1 \pmod{3} \).

Then \( a^2 \equiv 1 \pmod{3} \).

So \( a^2 + 23 \equiv 1 + 23 \equiv 24 \equiv 0 \pmod{3} \). ✅

---

### Step 4: Check Modulo 8

Given \( a \) is odd, so \( a \equiv \pm1, \pm3 \pmod{8} \).

Check each case:

- If \( a \equiv 1 \pmod{8} \):  
  \( a^2 \equiv 1 \), so \( a^2 + 23 \equiv 1 + 23 = 24 \equiv 0 \pmod{8} \)

- If \( a \equiv 3 \pmod{8} \):  
  \( a^2 \equiv 9 \equiv 1 \), so \( a^2 + 23 \equiv 1 + 23 = 24 \equiv 0 \pmod{8} \)

- If \( a \equiv 5 \equiv -3 \pmod{8} \):  
  \( a^2 \equiv 9 \equiv 1 \), so \( a^2 + 23 \equiv 1 + 23 = 24 \equiv 0 \pmod{8} \)

- If \( a \equiv 7 \equiv -1 \pmod{8} \):  
  \( a^2 \equiv 49 \equiv 1 \), so \( a^2 + 23 \equiv 1 + 23 = 24 \equiv 0 \pmod{8} \)

So in all cases, \( a^2 + 23 \equiv 0 \pmod{8} \). ✅

---

### Step 5: Combine Using CRT

Since \( \gcd(8,3)=1 \), and:
- \( a^2 + 23 \equiv 0 \pmod{8} \)
- \( a^2 + 23 \equiv 0 \pmod{3} \)

Then \( a^2 + 23 \equiv 0 \pmod{24} \).

---

### ✅ Final Proof

Let \( a \) be an integer not divisible by 2 or 3. Then \( a \) is odd and \( a \not\equiv 0 \pmod{3} \).

- **Modulo 3**: Since \( a \equiv \pm1 \pmod{3} \), \( a^2 \equiv 1 \), so \( a^2 + 23 \equiv 24 \equiv 0 \pmod{3} \).
- **Modulo 8**: Since \( a \) is odd, \( a \equiv \pm1, \pm3 \pmod{8} \). In all cases, \( a^2 \equiv 1 \pmod{8} \), so \( a^2 + 23 \equiv 24 \equiv 0 \pmod{8} \).

By the Chinese Remainder Theorem, \( a^2 + 23 \equiv 0 \pmod{24} \), i.e., \( 24 \mid (a^2 + 23) \).

---

### Lean 4 Statement

```lean
theorem problem_d (a : ℤ) (h2 : ¬(2 ∣ a)) (h3 : ¬(3 ∣ a)) : 24 ∣ (a^2 + 23) := by
  have h24 : 24 = 8 * 3 := by norm_num
  rw [h24]
  apply Nat.Coprime.dvd_of_dvd_mul_left (show Nat.Coprime 8 3 from by norm_num)
  constructor
  · -- Show 8 ∣ a^2 + 23
    have h_odd : a % 2 = 1 := by
      have := mod_two_eq_zero_or_one a
      rcases this with h | h
      · exfalso; exact h2 (dvd_mod_eq_zero_of_dvd (by exact ⟨2, by ring⟩) ?_)
        simp [h]
      · exact h
    have : a^2 % 8 = 1 := by
      -- Since a is odd, a ≡ ±1, ±3 mod 8, and squaring gives 1 mod 8.
      -- Alternatively, use that for odd a, a^2 ≡ 1 mod 8.
      zmod_trick   -- Or casewise as above
    simp [show (a^2 + 23) % 8 = 0 from ?_]   -- Details omitted for brevity
  · -- Show 3 ∣ a^2 + 23
    have : a % 3 ≠ 0 := by
      intro h; apply h3; exact dvd_of_mod_eq_zero h
    have : a^2 % 3 = 1 := by
      -- Since a ≢ 0 mod 3, a ≡ ±1 mod 3, so a^2 ≡ 1 mod 3.
      zmod_trick
    simp [show (a^2 + 23) % 3 = 0 from ?_]
```

*Note: The Lean proof uses tactics like `zmod_trick` or explicit case analysis modulo 8 and 3. The above is a sketch; a full Lean proof would require more detailed steps.*