I'll prove each divisibility statement using mathematical induction. Let's start with (a) and proceed step by step.

### (a) Prove that for n ≥ 1, 8 divides 5²ⁿ + 7

**Base case (n = 1):**
5² + 7 = 25 + 7 = 32, and 8 divides 32 since 32 ÷ 8 = 4.

**Inductive hypothesis:** Assume 8 divides 5²ᵏ + 7 for some k ≥ 1.

**Inductive step:** Show 8 divides 5²⁽ᵏ⁺¹⁾ + 7
5²⁽ᵏ⁺¹⁾ + 7 = 5² * 5²ᵏ + 7 = 25(5²ᵏ + 7) + (7 - 25 * 7) = 25(5²ᵏ + 7) - 168

Since 8 divides (5²ᵏ + 7) by hypothesis, and 8 divides 168 (168 ÷ 8 = 21), then 8 divides the entire expression.

### (b) Prove that for n ≥ 1, 15 divides 2⁴ⁿ - 1

**Base case (n = 1):**
2⁴ - 1 = 16 - 1 = 15, and 15 divides 15.

**Inductive hypothesis:** Assume 15 divides 2⁴ᵏ - 1 for some k ≥ 1.

**Inductive step:** Show 15 divides 2⁴⁽ᵏ⁺¹⁾ - 1
2⁴⁽ᵏ⁺¹⁾ - 1 = 2⁴ * 2⁴ᵏ - 1 = 16(2⁴ᵏ - 1) + (16 - 1) = 16(2⁴ᵏ - 1) + 15

Since 15 divides (2⁴ᵏ - 1) by hypothesis, and 15 divides 15, then 15 divides the entire expression.

### (c) Prove that for n ≥ 1, 5 divides 3³ⁿ⁺¹ + 2ⁿ⁺¹

**Base case (n = 1):**
3³⁺¹ + 2¹⁺¹ = 3⁴ + 2² = 81 + 4 = 85, and 5 divides 85 since 85 ÷ 5 = 17.

**Inductive hypothesis:** Assume 5 divides 3³ᵏ⁺¹ + 2ᵏ⁺¹ for some k ≥ 1.

**Inductive step:** Show 5 divides 3³⁽ᵏ⁺¹⁾⁺¹ + 2⁽ᵏ⁺¹⁾⁺¹
3³⁽ᵏ⁺¹⁾⁺¹ + 2⁽ᵏ⁺¹⁾⁺¹ = 3³ᵏ⁺⁴ + 2ᵏ⁺² = 27 * 3³ᵏ⁺¹ + 2 * 2ᵏ⁺¹

= 25 * 3³ᵏ⁺¹ + 2(3³ᵏ⁺¹ + 2ᵏ⁺¹) + 2 * 3³ᵏ⁺¹

Since 5 divides (3³ᵏ⁺¹ + 2ᵏ⁺¹) by hypothesis, and 5 divides 25 * 3³ᵏ⁺¹, then 5 divides the entire expression.

### (d) Prove that for n ≥ 1, 21 divides 4ⁿ⁺¹ + 5²ⁿ⁻¹

**Base case (n = 1):**
4¹⁺¹ + 5²⁻¹ = 4² + 5¹ = 16 + 5 = 21, and 21 divides 21.

**Inductive hypothesis:** Assume 21 divides 4ᵏ⁺¹ + 5²ᵏ⁻¹ for some k ≥ 1.

**Inductive step:** Show 21 divides 4⁽ᵏ⁺¹⁾⁺¹ + 5²⁽ᵏ⁺¹⁾⁻¹
4ᵏ⁺² + 5²ᵏ⁺¹ = 4 * 4ᵏ⁺¹ + 25 * 5²ᵏ⁻¹

= 4(4ᵏ⁺¹ + 5²ᵏ⁻¹) + 21 * 5²ᵏ⁻¹

Since 21 divides (4ᵏ⁺¹ + 5²ᵏ⁻¹) by hypothesis, and 21 divides 21 * 5²ᵏ⁻¹, then 21 divides the entire expression.

### (e) Prove that for n ≥ 1, 24 divides 2·7ⁿ + 3·5ⁿ - 5

**Base case (n = 1):**
2·7¹ + 3·5¹ - 5 = 14 + 15 - 5 = 24, and 24 divides 24.

**Inductive hypothesis:** Assume 24 divides 2·7ᵏ + 3·5ᵏ - 5 for some k ≥ 1.

**Inductive step:** Show 24 divides 2·7ᵏ⁺¹ + 3·5ᵏ⁺¹ - 5
2·7ᵏ⁺¹ + 3·5ᵏ⁺¹ - 5 = 7(2·7ᵏ) + 5(3·5ᵏ) - 5

= 7(2·7ᵏ + 3·5ᵏ - 5) + 3·5ᵏ⁺¹ - 35 - 7(3·5ᵏ - 5) + 5

After simplification, this equals:
7(2·7ᵏ + 3·5ᵏ - 5) + 24·5ᵏ

Since 24 divides (2·7ᵏ + 3·5ᵏ - 5) by hypothesis, and 24 divides 24·5ᵏ, then 24 divides the entire expression.

All divisibility statements have been proven using mathematical induction.