### Step 1: Understand the Definition of gcd

The greatest common divisor (gcd) of two integers \(a\) and \(b\) (not both zero) is defined as the largest positive integer that divides both \(a\) and \(b\). Importantly, the gcd is always positive.

### Step 2: Analyze the Effect of Negation on Divisors

Notice that for any integer \(d\):
- \(d\) divides \(a\) if and only if \(d\) divides \(-a\).
- Similarly, \(d\) divides \(b\) if and only if \(d\) divides \(-b\).

This is because if \(d \mid a\), then \(a = d \cdot k\) for some integer \(k\), so \(-a = d \cdot (-k)\), meaning \(d \mid (-a)\). The converse holds similarly.

Therefore, the set of common divisors of \(a\) and \(b\) is exactly the same as the common divisors of:
- \(-a\) and \(b\),
- \(a\) and \(-b\),
- \(-a\) and \(-b\).

### Step 3: Conclude the gcd Equality

Since the sets of common divisors are identical, the largest common divisor (the gcd) must be the same in all cases. Hence:
\[
\gcd(a, b) = \gcd(-a, b) = \gcd(a, -b) = \gcd(-a, -b)
\]

### Step 4: Formal Proof Sketch

Let \(d = \gcd(a, b)\). Then:
- \(d \mid a\) and \(d \mid b\).
- By the above, \(d \mid (-a)\) and \(d \mid (-b)\).
- So \(d\) is a common divisor of all pairs: \((a,b), (-a,b), (a,-b), (-a,-b)\).

Moreover, if \(d'\) is any common divisor of (say) \((-a, b)\), then \(d' \mid a\) and \(d' \mid b\), so \(d' \leq d\). Thus, \(d\) is the greatest common divisor for all these pairs.

### Step 5: Lean Statement

In Lean, we can state this as:

```lean
theorem gcd_neg (a b : ℤ) (h : ¬(a = 0 ∧ b = 0)) : 
  gcd a b = gcd (-a) b ∧ gcd a b = gcd a (-b) ∧ gcd a b = gcd (-a) (-b) := by
  have h1 : gcd a b = gcd (-a) b := by
    apply gcd_eq_gcd_neg_left a b
  have h2 : gcd a b = gcd a (-b) := by
    apply gcd_eq_gcd_neg_right a b
  have h3 : gcd a b = gcd (-a) (-b) := by
    rw [h1, gcd_neg_right]
  exact ⟨h1, h2, h3⟩
```

Note: This uses existing Lean lemmas like `gcd_eq_gcd_neg_left` and `gcd_neg_right` from `Mathlib.Data.Int.GCD`.

### Step 6: Output in Normal Language

The greatest common divisor of two integers \(a\) and \(b\) (not both zero) remains unchanged if we replace one or both of them with their negatives. That is:
\[
\gcd(a, b) = \gcd(-a, b) = \gcd(a, -b) = \gcd(-a, -b)
\]
This is because the set of common divisors of \(a\) and \(b\) is the same as that of \(-a\) and \(b\), etc., so the largest common divisor (which is positive) is identical in all cases.

---

**Final Answer:**
\[
\gcd(a, b) = \gcd(-a, b) = \gcd(a, -b) = \gcd(-a, -b)
\]