Let \( a \) be an odd integer. We aim to show that
\[
a^2 + (a+2)^2 + (a+4)^2 + 1
\]
is divisible by 12.

First, expand each square:
\[
a^2 + (a+2)^2 + (a+4)^2 + 1 = a^2 + (a^2 + 4a + 4) + (a^2 + 8a + 16) + 1
\]
Combine like terms:
\[
= a^2 + a^2 + 4a + 4 + a^2 + 8a + 16 + 1 = 3a^2 + 12a + 21
\]
So the expression simplifies to:
\[
3a^2 + 12a + 21
\]

We want to show that \( 3a^2 + 12a + 21 \) is divisible by 12. Note that 12a is divisible by 12, so we focus on \( 3a^2 + 21 \). Factor out 3:
\[
3a^2 + 12a + 21 = 3(a^2 + 4a + 7)
\]
Thus, we need to show that \( a^2 + 4a + 7 \) is divisible by 4 (since \( 3 \times 4 = 12 \)).

Now, since \( a \) is odd, write \( a = 2k + 1 \) for some integer \( k \). Substitute:
\[
a^2 + 4a + 7 = (2k+1)^2 + 4(2k+1) + 7 = (4k^2 + 4k + 1) + (8k + 4) + 7 = 4k^2 + 12k + 12
\]
Factor:
\[
= 4(k^2 + 3k + 3)
\]
This is clearly divisible by 4. Therefore, \( a^2 + 4a + 7 \) is divisible by 4, and so \( 3(a^2 + 4a + 7) \) is divisible by 12.

Hence, \( a^2 + (a+2)^2 + (a+4)^2 + 1 \) is divisible by 12 for any odd integer \( a \).

**Lean 4 Statement:**
```lean
theorem odd_squares_plus_one_divisible_by_12 (a : ℤ) (ha : a % 2 = 1) :
    12 ∣ (a^2 + (a + 2)^2 + (a + 4)^2 + 1) := by
  have h : a^2 + (a + 2)^2 + (a + 4)^2 + 1 = 3 * (a^2 + 4 * a + 7) := by
    ring
  rw [h]
  have : a^2 + 4 * a + 7 = 4 * (k^2 + 3 * k + 3) := by
    obtain ⟨k, rfl⟩ := Int.exists_eq_add_of_ne_zero (by omega)  -- Since a is odd, write a = 2*k + 1
    ring
  rw [this]
  ring
  exact ⟨k^2 + 3 * k + 3, by ring⟩
```

**Output in Normal Language:**
The expression \( a^2 + (a+2)^2 + (a+4)^2 + 1 \) simplifies to \( 3a^2 + 12a + 21 \). Since \( a \) is odd, we write \( a = 2k + 1 \). Substituting gives \( 4k^2 + 12k + 12 \), which is \( 4(k^2 + 3k + 3) \). Thus, the original expression becomes \( 3 \times 4(k^2 + 3k + 3) = 12(k^2 + 3k + 3) \), clearly divisible by 12. Therefore, the statement holds for all odd integers \( a \).