### Proof in Lean 4

```lean
import Mathlib.Data.Int.GCD
import Mathlib.Tactic

theorem part_a (a b c : ℤ) : 
    (∃ x y : ℤ, c = a * x + b * y) ↔ (Int.gcd a b ∣ c) := by
  constructor
  · intro ⟨x, y, h⟩
    have hgcd : (Int.gcd a b : ℤ) ∣ a ∧ (Int.gcd a b : ℤ) ∣ b := by
      exact ⟨Int.gcd_dvd_left a b, Int.gcd_dvd_right a b⟩
    rcases hgcd with ⟨ha, hb⟩
    rw [h]
    exact ⟨x, y, by
      calc
        a * x + b * y = x * a + y * b := by ring
        _ = x * ((Int.gcd a b) * (a / Int.gcd a b)) + y * ((Int.gcd a b) * (b / Int.gcd a b)) := by
          rw [Int.mul_ediv_cancel' ha, Int.mul_ediv_cancel' hb]
        _ = (Int.gcd a b) * (x * (a / Int.gcd a b) + y * (b / Int.gcd a b)) := by ring⟩
  · intro h
    exact Int.exists_gcd_eq h

theorem part_b (a b x y : ℤ) (h : a * x + b * y = Int.gcd a b) :
    Int.gcd x y = 1 := by
  have hgcd := Int.gcd_eq_gcd_ab a b
  have : Int.gcd a b ∣ Int.gcd x y := by
    rw [← h]
    exact Int.dvd_gcd (Int.dvd_mul_right x) (Int.dvd_mul_right y)
  have : Int.gcd x y ∣ Int.gcd a b :=
    Int.gcd_dvd_gcd (by rfl) (by rfl) (Int.gcd_dvd_left x y) (Int.gcd_dvd_right x y)
  have : Int.gcd x y = Int.gcd a b :=
    Int.dvd_antisymm ‹Int.gcd x y ∣ Int.gcd a b› ‹Int.gcd a b ∣ Int.gcd x y›
  rw [this] at *
  exact Int.gcd_eq_one_of_dvd_of_dvd (Int.gcd_dvd_left a b) (Int.gcd_dvd_right a b) h
```

### Explanation in Normal Language

**(a) Proof that ∃ integers x,y such that c = ax + by ↔ gcd(a,b) divides c**

**Forward direction (→):**
If there exist integers x and y such that c = ax + by, then since gcd(a,b) divides both a and b, it must also divide any linear combination of a and b. Therefore gcd(a,b) divides c.

**Backward direction (←):**
If gcd(a,b) divides c, then by Bézout's identity (which guarantees the existence of integers x,y such that gcd(a,b) = ax + by), we can scale this identity appropriately to obtain c = ax + by for some integers x,y.

**(b) Proof that if ax + by = gcd(a,b), then gcd(x,y) = 1**

Let d = gcd(x,y). Then d divides both x and y, so d divides any linear combination of x and y. In particular, d divides ax + by = gcd(a,b). But gcd(a,b) also divides both a and b, and therefore divides any linear combination of a and b. This creates a mutual divisibility relationship that forces d = gcd(a,b).

However, since d divides gcd(a,b) and gcd(a,b) divides d, we must have d = gcd(a,b). But then from ax + by = gcd(a,b) = d, and since d divides both x and y, the only possibility is that d = 1 (otherwise the equation would represent a nontrivial common factor).

More precisely: if d > 1, then we could divide both sides by d to get a smaller representation, contradicting the minimality of the gcd representation. Therefore gcd(x,y) must be 1.

The Lean proof formalizes this reasoning using the properties of gcd and divisibility in the integers.