Let's break down the problem into two parts:

1. **Prove that if \(a\) and \(b\) are integers, not both zero, then \(\gcd(2a - 3b, 4a - 5b)\) divides \(b\).**
2. **Hence, show that \(\gcd(2a + 3, 4a + 5) = 1\).**

---

### Part 1: Prove that \(\gcd(2a - 3b, 4a - 5b)\) divides \(b\)

Let \(d = \gcd(2a - 3b, 4a - 5b)\). Then \(d\) divides any integer linear combination of \(2a - 3b\) and \(4a - 5b\). In particular, we can eliminate \(a\):

Compute:
\[
2 \cdot (4a - 5b) - 4 \cdot (2a - 3b) = (8a - 10b) - (8a - 12b) = 2b.
\]
So,
\[
d \mid 2b.
\]
Similarly, eliminate \(b\):
Multiply the first expression by 5 and the second by 3:
\[
5(2a - 3b) - 3(4a - 5b) = (10a - 15b) - (12a - 15b) = -2a.
\]
So,
\[
d \mid 2a.
\]
Therefore, \(d \mid \gcd(2a, 2b) = 2 \gcd(a, b)\). However, we can get a more precise relation.

Alternatively, we can express \(d\) in terms of \(b\):
From \(d \mid 2b\), we know \(d\) divides \(2b\). But we want to show \(d \mid b\). Note that \(d\) might share a factor with 2.

Actually, we can show that \(d\) divides \(b\) directly. Consider:
\[
(4a - 5b) - 2 \cdot (2a - 3b) = (4a - 5b) - (4a - 6b) = b.
\]
So,
\[
d \mid b.
\]
This is straightforward! Therefore, \(\gcd(2a - 3b, 4a - 5b) \mid b\).

---

### Part 2: Hence, show that \(\gcd(2a + 3, 4a + 5) = 1\)

Now, set \(b = -1\). Then:
\[
2a - 3b = 2a - 3(-1) = 2a + 3,
\]
\[
4a - 5b = 4a - 5(-1) = 4a + 5.
\]
So,
\[
\gcd(2a + 3, 4a + 5) = \gcd(2a - 3(-1), 4a - 5(-1)).
\]
From Part 1, this gcd divides \(b = -1\). Therefore, it divides \(1\). Hence,
\[
\gcd(2a + 3, 4a + 5) = 1.
\]

---

### **Lean Statement**

To formalize this in Lean:

```lean
theorem gcd_divides_b (a b : ℤ) (h : ¬(a = 0 ∧ b = 0)) : 
  gcd (2*a - 3*b) (4*a - 5*b) ∣ b := by
  let d := gcd (2*a - 3*b) (4*a - 5*b)
  have h1 : d ∣ (2*a - 3*b) := gcd_dvd_left _ _
  have h2 : d ∣ (4*a - 5*b) := gcd_dvd_right _ _
  have comb : d ∣ b := by
    have : (4*a - 5*b) - 2*(2*a - 3*b) = b := by ring
    exact dvd_of_dvd_sub (dvd_mul_of_dvd_right h1 2) (by
      rw [this]
      exact h2)
  exact comb

theorem gcd_2a_3_4a_5_eq_one (a : ℤ) : gcd (2*a + 3) (4*a + 5) = 1 := by
  have h : gcd (2*a + 3) (4*a + 5) ∣ (-1) := by
    have := gcd_divides_b a (-1) (by simp [ne_of_gt?])
    simpa [show (2*a - 3*(-1 : ℤ)) = 2*a + 3 by ring, 
            show (4*a - 5*(-1 : ℤ)) = 4*a + 5 by ring] at this
  exact nat.dvd_one.mp (int.nat_abs_dvd_nat_abs.mpr h)
```

**Note:** The Lean proof uses the fact that if \(d \mid -1\), then \(d = \pm 1\), so the gcd is 1. The `gcd` in Lean for integers returns a nonnegative value, so it is 1.

---

### **Output in Normal Language**

1. **Proof that \(\gcd(2a - 3b, 4a - 5b)\) divides \(b\):**
   Let \(d = \gcd(2a - 3b, 4a - 5b)\). Then \(d\) divides both \(2a - 3b\) and \(4a - 5b\). Consider the linear combination:
   \[
   (4a - 5b) - 2 \cdot (2a - 3b) = 4a - 5b - 4a + 6b = b.
   \]
   Therefore, \(d\) divides \(b\).

2. **Hence, \(\gcd(2a + 3, 4a + 5) = 1\):**
   Set \(b = -1\). Then:
   \[
   2a - 3b = 2a + 3, \quad 4a - 5b = 4a + 5.
   \]
   By the above result, \(\gcd(2a + 3, 4a + 5)\) divides \(b = -1\). Since the gcd must be positive, it divides 1. Therefore, \(\gcd(2a + 3, 4a + 5) = 1\).

This completes the proof.