### Step 1: Understand the Problem

We wish to show that for any integer \( n \), the number  
\[
(n+1)^3 - n^3
\]  
is **never divisible by 2**. That is, it is always **odd**.

---

### Step 2: Expand the Expression

Expand \( (n+1)^3 \):
\[
(n+1)^3 = n^3 + 3n^2 + 3n + 1
\]

Now subtract \( n^3 \):
\[
(n+1)^3 - n^3 = (n^3 + 3n^2 + 3n + 1) - n^3 = 3n^2 + 3n + 1
\]

So,
\[
(n+1)^3 - n^3 = 3n(n + 1) + 1
\]

---

### Step 3: Analyze Modulo 2

We want to show that \( 3n(n+1) + 1 \) is **never divisible by 2**, i.e., it is **odd**.

Note:
- \( 3 \equiv 1 \pmod{2} \), so \( 3n(n+1) \equiv n(n+1) \pmod{2} \).
- Therefore, \( 3n(n+1) + 1 \equiv n(n+1) + 1 \pmod{2} \).

Now, observe that for any integer \( n \), one of \( n \) or \( n+1 \) is **even**. Hence, \( n(n+1) \) is even, i.e.,  
\[
n(n+1) \equiv 0 \pmod{2}
\]

So,
\[
n(n+1) + 1 \equiv 0 + 1 = 1 \pmod{2}
\]

Thus, \( (n+1)^3 - n^3 \equiv 1 \pmod{2} \), meaning it is **always odd**, and therefore **never divisible by 2**.

---

### Step 4: Formal Proof in Lean

```lean
theorem cube_diff_odd (n : ℤ) : ¬ (2 ∣ (n + 1)^3 - n^3) := by
  have h : (n + 1)^3 - n^3 = 3 * n * (n + 1) + 1 := by
    ring
  rw [h]
  intro hdiv
  have : 2 ∣ 3 * n * (n + 1) + 1 := hdiv
  have : 2 ∣ 3 * n * (n + 1) := by
    have : 2 ∣ n * (n + 1) := by
      have : Even (n * (n + 1)) := by
        exact Int.even_mul_succ_self n
      rcases this with ⟨k, hk⟩
      exact ⟨k, hk⟩
    have : 2 ∣ 3 * (n * (n + 1)) :=
      this.mul_left 3
    rwa [show (3 : ℤ) * n * (n + 1) = 3 * (n * (n + 1)) by ring] at this
  have : 2 ∣ 1 :=
    Int.dvd_add_of_dvd_of_dvd_right this hdiv
  have : ¬ (2 : ℤ) ∣ 1 := by
    decide
  contradiction
```

**Explanation of the Lean proof:**
1. We compute \( (n+1)^3 - n^3 = 3n(n+1) + 1 \) using `ring`.
2. Assume for contradiction that \( 2 \mid 3n(n+1) + 1 \).
3. Note that \( 2 \mid n(n+1) \) because one of \( n \) or \( n+1 \) is even (proven by `Int.even_mul_succ_self`).
4. Then \( 2 \mid 3 \cdot n(n+1) \), so \( 2 \mid (3n(n+1) + 1 - 3n(n+1)) = 1 \), which is false.
5. Hence, the assumption is false, and \( 2 \nmid (n+1)^3 - n^3 \).

---

### Step 5: Conclusion in Normal Language

The difference between two consecutive cubes, \( (n+1)^3 - n^3 \), simplifies to \( 3n(n+1) + 1 \). Since \( n(n+1) \) is always even (as one of \( n \) or \( n+1 \) is even), \( 3n(n+1) \) is also even. Adding 1 to an even number yields an odd number. Therefore, \( (n+1)^3 - n^3 \) is always odd and never divisible by 2.

This holds for all integers \( n \). ✅