Let's analyze and prove the statement:

**Statement:** If \( a \mid bc \), then \( a \mid \gcd(a, b) \cdot \gcd(a, c) \).

---

### Step 1: Understand the Notation and Given
- \( a \mid bc \) means \( a \) divides \( b \cdot c \).
- We need to show that \( a \) divides the product \( \gcd(a, b) \cdot \gcd(a, c) \).

---

### Step 2: Express gcds in Terms of a
Let:
- \( d = \gcd(a, b) \)
- \( e = \gcd(a, c) \)

Then we can write:
- \( a = d \cdot a_1 \), and \( b = d \cdot b_1 \), with \( \gcd(a_1, b_1) = 1 \).
- \( a = e \cdot a_2 \), and \( c = e \cdot c_1 \), with \( \gcd(a_2, c_1) = 1 \).

Note: Since \( d \mid a \) and \( e \mid a \), we have \( a_1 = \frac{a}{d} \) and \( a_2 = \frac{a}{e} \).

---

### Step 3: Use the Given \( a \mid bc \)
Given \( a \mid bc \), so:
\[
bc = a \cdot k = (d \cdot a_1) \cdot k \quad \text{for some integer } k.
\]
But \( b = d \cdot b_1 \), so:
\[
(d \cdot b_1) \cdot c = d \cdot a_1 \cdot k \implies b_1 c = a_1 k.
\]
So \( a_1 \mid b_1 c \). But since \( \gcd(a_1, b_1) = 1 \), we must have \( a_1 \mid c \).

Similarly, we can write \( c = e \cdot c_1 \), and since \( a_1 \mid c \), we have \( a_1 \mid e \cdot c_1 \). But \( \gcd(a_1, c_1) = 1 \) (why? because \( \gcd(a_1, b_1)=1 \) and \( a_1 \mid c \), but actually we need to be careful).

Alternatively, we can proceed as:

Since \( a_1 \mid c \), and \( e = \gcd(a, c) \), we note that \( a_1 \mid a \) and \( a_1 \mid c \), so \( a_1 \mid \gcd(a, c) = e \).

So \( a_1 \mid e \).

Therefore, \( e = a_1 \cdot t \) for some integer \( t \).

Now recall \( a = d \cdot a_1 \), and \( e = a_1 \cdot t \).

Then:
\[
d \cdot e = d \cdot (a_1 \cdot t) = (d \cdot a_1) \cdot t = a \cdot t.
\]
So \( a \mid d \cdot e \), i.e., \( a \mid \gcd(a, b) \cdot \gcd(a, c) \).

---

### Step 4: Write the Proof Concisely

**Proof:**
Let \( d = \gcd(a, b) \) and \( e = \gcd(a, c) \). Then we can write:
- \( a = d \cdot a_1 \), \( b = d \cdot b_1 \) with \( \gcd(a_1, b_1) = 1 \).
- \( a = e \cdot a_2 \), \( c = e \cdot c_1 \) with \( \gcd(a_2, c_1) = 1 \).

Given \( a \mid bc \), we have:
\[
bc = a \cdot k = (d \cdot a_1) \cdot k.
\]
Substitute \( b = d \cdot b_1 \):
\[
(d \cdot b_1) \cdot c = d \cdot a_1 \cdot k \implies b_1 c = a_1 k.
\]
So \( a_1 \mid b_1 c \). Since \( \gcd(a_1, b_1) = 1 \), it follows that \( a_1 \mid c \).

Now, since \( a_1 \mid a \) and \( a_1 \mid c \), we have \( a_1 \mid \gcd(a, c) = e \). So \( e = a_1 \cdot t \) for some integer \( t \).

Then:
\[
d \cdot e = d \cdot (a_1 \cdot t) = (d \cdot a_1) \cdot t = a \cdot t.
\]
Therefore, \( a \mid d \cdot e \), i.e., \( a \mid \gcd(a, b) \cdot \gcd(a, c) \). ∎

---

### Step 5: Output in Normal Language

**If \( a \) divides \( b \cdot c \), then \( a \) also divides the product of the greatest common divisor of \( a \) and \( b \) and the greatest common divisor of \( a \) and \( c \).**

This is proven by expressing \( a \) in terms of its gcd with \( b \) and \( c \), and using the given divisibility condition to show that a component of \( a \) must divide the gcd with \( c \), leading to the result.

---

**Lean Statement** (for verification in Lean):
```lean
theorem gcd_product_div (a b c : ℤ) (h : a ∣ b * c) : a ∣ (nat.gcd a.nat_abs b.nat_abs).gcd (nat.gcd a.nat_abs c.nat_abs) :=
by
  -- Proof would involve integer gcd properties and the above reasoning.
  -- Actual Lean proof might be more involved due to nat vs int.
  sorry
```
*Note: The exact Lean formulation may require handling absolute values and nonnegative gcds. The concept is translated, but the actual proof in Lean would use properties of `gcd` and divisibility.*