Let's analyze the statement: "If \( a \mid (b + c) \), then either \( a \mid b \) or \( a \mid c \)."

We need to prove or disprove this.

**Disproof by Counterexample:**
Let \( a = 2 \), \( b = 1 \), \( c = 1 \).
Then \( b + c = 2 \), so \( 2 \mid 2 \), meaning \( a \mid (b + c) \).
However, \( 2 \nmid 1 \) (since 1 is not divisible by 2), so neither \( a \mid b \) nor \( a \mid c \) holds.

Therefore, the statement is false.

**Lean Statement:**
```lean
example : ¬ (∀ (a b c : ℤ), a ∣ (b + c) → (a ∣ b ∨ a ∣ c)) := by
  refine ⟨2, 1, 1, ?_, ?_⟩
  · simp [show (2 : ℤ) ∣ (1 + 1) by norm_num]
  · intro h
    cases' h with hb hc
    · have : ¬(2 : ℤ) ∣ 1 := by norm_num
      contradiction
    · have : ¬(2 : ℤ) ∣ 1 := by norm_num
      contradiction
```

**Output in Normal Language:**
The statement is false. A counterexample is when \( a = 2 \), \( b = 1 \), and \( c = 1 \). Here, \( 2 \) divides \( 1 + 1 = 2 \), so \( a \mid (b + c) \). However, \( 2 \) does not divide \( 1 \) (so \( a \nmid b \)) and \( 2 \) does not divide \( 1 \) (so \( a \nmid c \)). Therefore, the implication does not hold in general.