### Step-by-Step Proof and Verification

---

#### (a) Prove that if \( d \mid n \), then \( 2^d - 1 \mid 2^n - 1 \).

**Proof:**

Assume \( d \mid n \), so \( n = d \cdot k \) for some integer \( k \geq 1 \).

We use the identity:
\[
x^k - 1 = (x - 1)(x^{k-1} + x^{k-2} + \cdots + x + 1).
\]

Let \( x = 2^d \). Then:
\[
2^n - 1 = (2^d)^k - 1 = (2^d - 1)\left((2^d)^{k-1} + (2^d)^{k-2} + \cdots + 2^d + 1\right).
\]

Thus, \( 2^d - 1 \) divides \( 2^n - 1 \), i.e.,
\[
2^d - 1 \mid 2^n - 1.
\]

---

#### (b) Verify that \( 2^{35} - 1 \) is divisible by 31 and 127.

We note:
- \( 31 = 2^5 - 1 \)
- \( 127 = 2^7 - 1 \)

Since \( 5 \mid 35 \) and \( 7 \mid 35 \), by part (a):
- \( 2^5 - 1 \mid 2^{35} - 1 \)
- \( 2^7 - 1 \mid 2^{35} - 1 \)

Therefore, \( 2^{35} - 1 \) is divisible by both 31 and 127.

---

### Lean 4 Statement

```lean
theorem part_a (d n : ℕ) (h : d ∣ n) : (2^d - 1) ∣ (2^n - 1) := by
  rcases h with ⟨k, rfl⟩
  have h1 : (2^d : ℤ)^k - 1 = (2^d - 1) * (∑ i in Finset.range k, (2^d)^i) := by
    exact sub_one_mul_sum_pow (2^d) k
  simp [h1, pow_mul]

theorem part_b : 31 ∣ (2^35 - 1) ∧ 127 ∣ (2^35 - 1) := by
  have h1 : 5 ∣ 35 := by decide
  have h2 : 7 ∣ 35 := by decide
  exact ⟨part_a 5 35 h1, part_a 7 35 h2⟩
```

---

### Output in Normal Language

**(a)** If \( d \) divides \( n \), then \( 2^d - 1 \) divides \( 2^n - 1 \). This is proven by writing \( n = d \cdot k \) and factoring \( 2^n - 1 = (2^d)^k - 1 \) as \( (2^d - 1) \) multiplied by a polynomial in \( 2^d \).

**(b)** Since \( 5 \mid 35 \) and \( 7 \mid 35 \), it follows that \( 2^5 - 1 = 31 \mid 2^{35} - 1 \) and \( 2^7 - 1 = 127 \mid 2^{35} - 1 \). Thus, \( 2^{35} - 1 \) is divisible by both 31 and 127.

The Lean code formalizes these proofs, using the fact that \( n = d \cdot k \) and the geometric sum identity to establish divisibility. For part (b), it directly applies part (a) with \( d = 5 \) and \( d = 7 \).