### ‚úÖ Lean 4 Proof

```lean
theorem part_a (a : ‚Ñ§) : 6 ‚à£ a * (a ^ 2 + 11) := by
  have h2 : 2 ‚à£ a * (a ^ 2 + 11) := by
    rcases em (Even a) with (‚ü®k, hk‚ü© | h_odd)
    ¬∑ rw [hk]
      simp [show (2:‚Ñ§) ‚à£ 2 * k * ((2 * k) ^ 2 + 11) by use k * ((2 * k) ^ 2 + 11); ring]
    ¬∑ have : Odd a := by
        rw [Odd, ‚Üê Even.not_odd, not_not] at h_odd
        exact h_odd
      rcases this with ‚ü®k, hk‚ü©
      rw [hk]
      simp [show (2:‚Ñ§) ‚à£ (2 * k + 1) * ((2 * k + 1) ^ 2 + 11) by 
        have : (2 * k + 1) ^ 2 + 11 = 4 * (k^2 + k + 3) := by ring
        rw [this]
        use (2 * k + 1) * (k^2 + k + 3); ring]
  have h3 : 3 ‚à£ a * (a ^ 2 + 11) := by
    have : a ^ 3 + 11 * a = a * (a ^ 2 + 11) := by ring
    rw [‚Üê this]
    exact show 3 ‚à£ a ^ 3 + 11 * a from by
      have : a ^ 3 + 11 * a = a ^ 3 - a + 12 * a := by ring
      rw [this]
      have h : 3 ‚à£ a ^ 3 - a := by
        induction' a using Int.induction_mod3 with a ha
        all_goals { simp [ha] }
      exact ‚ü®h, by simp‚ü©
  exact Nat.Coprime.dvd_of_dvd_mul_left (by decide : Nat.Coprime 2 3) h2 h3
```

### üìù Explanation in Normal Language

**Assertion**: For any integer \( a \), \( 6 \) divides \( a(a^2 + 11) \).

**Proof**:

To prove \( 6 \mid a(a^2 + 11) \), we show that both \( 2 \) and \( 3 \) divide \( a(a^2 + 11) \), and since \( 2 \) and \( 3 \) are coprime, their product \( 6 \) must also divide it.

1. **Divisibility by 2**:
   - Consider two cases based on whether \( a \) is even or odd.
   - If \( a \) is even (\( a = 2k \)), then:
     \[
     a(a^2 + 11) = 2k \cdot ((2k)^2 + 11) = 2k \cdot (4k^2 + 11)
     \]
     which is clearly divisible by 2.
   - If \( a \) is odd (\( a = 2k + 1 \)), then:
     \[
     a^2 + 11 = (2k + 1)^2 + 11 = 4k^2 + 4k + 1 + 11 = 4k^2 + 4k + 12 = 4(k^2 + k + 3)
     \]
     So,
     \[
     a(a^2 + 11) = (2k + 1) \cdot 4(k^2 + k + 3) = 4(2k + 1)(k^2 + k + 3)
     \]
     which is divisible by 2 (in fact, by 4).

2. **Divisibility by 3**:
   - Note that \( a(a^2 + 11) = a^3 + 11a \).
   - We can rewrite:
     \[
     a^3 + 11a = (a^3 - a) + 12a
     \]
   - Observe that \( a^3 - a = a(a - 1)(a + 1) \) is the product of three consecutive integers. Among any three consecutive integers, one is divisible by 3. Hence, \( 3 \mid a^3 - a \).
   - Also, \( 3 \mid 12a \) obviously.
   - Therefore, \( 3 \) divides their sum \( (a^3 - a) + 12a = a^3 + 11a \).

Since \( 2 \) and \( 3 \) are coprime and both divide \( a(a^2 + 11) \), it follows that \( 6 \) divides \( a(a^2 + 11) \). This holds for all integers \( a \).

**Conclusion**: The assertion is true. For any integer \( a \), \( 6 \mid a(a^2 + 11) \).