Let \( t_n = \frac{n(n+1)}{2} \) denote the \(n\)th triangular number. We are asked for which values of \(n\) does \(t_n\) divide the sum \(S_n = t_1 + t_2 + \ldots + t_n\).

First, recall that the sum of the first \(n\) triangular numbers is:
\[
S_n = \sum_{k=1}^n t_k = \sum_{k=1}^n \frac{k(k+1)}{2} = \frac{1}{2} \left( \sum_{k=1}^n k^2 + \sum_{k=1}^n k \right).
\]
Using the formulas:
\[
\sum_{k=1}^n k = \frac{n(n+1)}{2}, \quad \sum_{k=1}^n k^2 = \frac{n(n+1)(2n+1)}{6},
\]
we get:
\[
S_n = \frac{1}{2} \left( \frac{n(n+1)(2n+1)}{6} + \frac{n(n+1)}{2} \right) = \frac{1}{2} \cdot \frac{n(n+1)}{2} \left( \frac{2n+1}{3} + 1 \right) = \frac{n(n+1)}{4} \left( \frac{2n+1 + 3}{3} \right) = \frac{n(n+1)}{4} \cdot \frac{2n+4}{3} = \frac{n(n+1)(2n+4)}{12}.
\]
Simplify \(2n+4 = 2(n+2)\):
\[
S_n = \frac{n(n+1) \cdot 2(n+2)}{12} = \frac{n(n+1)(n+2)}{6}.
\]

So, \(S_n = \frac{n(n+1)(n+2)}{6}\).

We want \(t_n \mid S_n\), i.e.,
\[
\frac{n(n+1)}{2} \mid \frac{n(n+1)(n+2)}{6}.
\]
This is equivalent to:
\[
\frac{\frac{n(n+1)(n+2)}{6}}{\frac{n(n+1)}{2}} = \frac{n(n+1)(n+2)}{6} \cdot \frac{2}{n(n+1)} = \frac{n+2}{3} \in \mathbb{Z}.
\]
So, \(t_n \mid S_n\) if and only if \(\frac{n+2}{3}\) is an integer, i.e., \(n+2\) is divisible by 3. Therefore, \(n \equiv 1 \pmod{3}\).

Thus, \(t_n\) divides \(S_n\) if and only if \(n = 3k + 1\) for some integer \(k \geq 0\).

**Verification with small values:**
- \(n=1\): \(t_1 = 1\), \(S_1 = 1\), \(1 \mid 1\) (holds, and \(n=1 \equiv 1 \pmod{3}\)).
- \(n=2\): \(t_2 = 3\), \(S_2 = 1+3=4\), \(3 \nmid 4\) (fails, \(n=2 \equiv 2 \pmod{3}\)).
- \(n=3\): \(t_3 = 6\), \(S_3 = 1+3+6=10\), \(6 \nmid 10\) (fails, \(n=3 \equiv 0 \pmod{3}\)).
- \(n=4\): \(t_4 = 10\), \(S_4 = 1+3+6+10=20\), \(10 \mid 20\) (holds, \(n=4 \equiv 1 \pmod{3}\)).

This confirms the pattern.

**Final Answer:**
\[
\boxed{n \equiv 1 \pmod{3}}
\]
That is, \(t_n\) divides \(t_1 + t_2 + \cdots + t_n\) if and only if \(n\) is of the form \(n = 3k + 1\) for some nonnegative integer \(k\).

In Lean, we can state this as:
```lean
theorem triangular_div_sum (n : ℕ) : (nth_triangular n) ∣ (sum_triangular n) ↔ n % 3 = 1 :=
by
  -- Define t_n and S_n, then show the divisibility condition holds iff n ≡ 1 mod 3.
  sorry  -- Proof details omitted, but the reasoning above provides the structure.
```

**Normal language output:**
The \(n\)th triangular number \(t_n\) divides the sum \(t_1 + t_2 + \cdots + t_n\) if and only if \(n\) leaves a remainder of 1 when divided by 3. In other words, \(n\) must be one more than a multiple of 3, i.e., \(n = 1, 4, 7, 10, \ldots\).