### Step 1: Understand the Problem

We want to prove that for a positive integer \( n \) and any integer \( a \), \( \gcd(a, a + n) \) divides \( n \). Then, as a special case when \( n = 1 \), we conclude that \( \gcd(a, a + 1) = 1 \).

---

### Step 2: Prove that \( \gcd(a, a + n) \) divides \( n \)

Let \( d = \gcd(a, a + n) \). By definition, \( d \) divides both \( a \) and \( a + n \). Therefore:

- \( d \mid a \)
- \( d \mid (a + n) \)

Since \( d \) divides both \( a \) and \( a + n \), it must also divide their difference:
\[
d \mid (a + n - a) = n
\]
So, \( d \mid n \). This means \( \gcd(a, a + n) \) divides \( n \).

---

### Step 3: Special Case: \( n = 1 \)

Now, let \( n = 1 \). Then:
\[
\gcd(a, a + 1) \mid 1
\]
The only positive divisors of 1 are 1 itself. Therefore:
\[
\gcd(a, a + 1) = 1
\]

---

### ‚úÖ Final Proof in Lean

```lean
theorem gcd_divides_n (n : ‚Ñï) (a : ‚Ñ§) (hn : n > 0) : (Int.gcd a (a + n)) ‚à£ n := by
  let d := Int.gcd a (a + n)
  have h1 : d ‚à£ a := Int.gcd_dvd_left a (a + n)
  have h2 : d ‚à£ (a + n) := Int.gcd_dvd_right a (a + n)
  have h3 : d ‚à£ (a + n - a) := by
    exact Int.dvd_sub h2 h1
  simp at h3
  exact h3

theorem gcd_a_a_plus_one (a : ‚Ñ§) : Int.gcd a (a + 1) = 1 := by
  have h : (Int.gcd a (a + 1)) ‚à£ (1 : ‚Ñï) := by
    exact gcd_divides_n 1 a (by decide)
  rcases h with ‚ü®k, hk‚ü©
  have : Int.gcd a (a + 1) = 1 := by
    apply Nat.eq_one_of_dvd_one h
  exact this
```

---

### üìù Output in Normal Language

We have shown that for any positive integer \( n \) and any integer \( a \), the greatest common divisor \( \gcd(a, a + n) \) divides \( n \). This is because \( \gcd(a, a + n) \) divides both \( a \) and \( a + n \), so it must also divide their difference \( n \).

In particular, when \( n = 1 \), \( \gcd(a, a + 1) \) divides 1. Since the only positive divisor of 1 is 1, it follows that \( \gcd(a, a + 1) = 1 \). This means that \( a \) and \( a + 1 \) are always coprime.

---

### üîç Explanation

- The key step uses the property that if \( d \) divides both \( x \) and \( y \), then \( d \) divides any linear combination of \( x \) and \( y \), in particular \( y - x \).
- For \( n = 1 \), since \( \gcd(a, a+1) \) must be a positive divisor of 1, it must be 1.
- The Lean code formalizes this reasoning using the standard library facts about divisibility and gcd.

This completes the proof.