Let \( a \) and \( b \) be odd integers. We want to prove that \( 16 \mid (a^4 + b^4 - 2) \).

Since \( a \) and \( b \) are odd, we can write them as:
\[
a = 2k + 1, \quad b = 2m + 1
\]
for some integers \( k \) and \( m \).

First, compute \( a^4 \):
\[
a^2 = (2k + 1)^2 = 4k^2 + 4k + 1 = 4k(k + 1) + 1.
\]
Note that \( k(k+1) \) is always even (since one of \( k \) or \( k+1 \) is even), so let \( k(k+1) = 2r \) for some integer \( r \). Then:
\[
a^2 = 4 \cdot 2r + 1 = 8r + 1.
\]
Now,
\[
a^4 = (a^2)^2 = (8r + 1)^2 = 64r^2 + 16r + 1 = 16(4r^2 + r) + 1.
\]
Similarly, for \( b \), we have \( b = 2m + 1 \), and by the same reasoning:
\[
b^2 = 4m(m+1) + 1 = 8s + 1 \quad (\text{where } m(m+1) = 2s),
\]
\[
b^4 = (8s + 1)^2 = 64s^2 + 16s + 1 = 16(4s^2 + s) + 1.
\]

Therefore,
\[
a^4 + b^4 - 2 = [16(4r^2 + r) + 1] + [16(4s^2 + s) + 1] - 2 = 16(4r^2 + r + 4s^2 + s).
\]
This is clearly divisible by 16.

Hence, \( 16 \mid (a^4 + b^4 - 2) \).

**Lean Statement:**
```lean
theorem odd_pow4_sum_minus_two_divisible_by_16 (a b : ℤ) (ha : a % 2 = 1) (hb : b % 2 = 1) :
    16 ∣ a^4 + b^4 - 2 :=
by
  -- Since a and b are odd, we can write them as 2k+1 and 2m+1
  have ⟨k, hk⟩ := Int.even_add_one.mp ha
  have ⟨m, hm⟩ := Int.even_add_one.mp hb
  rw [hk, hm] at *
  -- Compute a^4 and b^4
  have h1 : (2*k+1)^2 = 4*k*(k+1) + 1 := by ring
  have h2 : k*(k+1) = 2*(k*(k+1)/2) := by
    have : Even (k*(k+1)) := even_mul_succ_self k
    rcases this with ⟨t, ht⟩
    exact ht
  have h3 : (2*k+1)^2 = 8*t + 1 := by rw [h1, h2]; ring
  have h4 : ((2*k+1)^2)^2 = (8*t+1)^2 := by rw [h3]
  have h5 : (8*t+1)^2 = 64*t^2 + 16*t + 1 := by ring
  have h6 : (2*k+1)^4 = 16*(4*t^2 + t) + 1 := by rw [h4, h5]; ring
  -- Similarly for b
  have h7 : (2*m+1)^2 = 4*m*(m+1) + 1 := by ring
  have h8 : m*(m+1) = 2*(m*(m+1)/2) := by
    have : Even (m*(m+1)) := even_mul_succ_self m
    rcases this with ⟨u, hu⟩
    exact hu
  have h9 : (2*m+1)^2 = 8*u + 1 := by rw [h7, h8]; ring
  have h10 : ((2*m+1)^2)^2 = (8*u+1)^2 := by rw [h9]
  have h11 : (8*u+1)^2 = 64*u^2 + 16*u + 1 := by ring
  have h12 : (2*m+1)^4 = 16*(4*u^2 + u) + 1 := by rw [h10, h11]; ring
  -- Now combine
  rw [h6, h12]
  ring
  exact ⟨4*t^2 + t + 4*u^2 + u, by ring⟩
```

**Note:** The Lean proof uses the fact that \( k(k+1) \) is even, which is provided by a lemma `even_mul_succ_self` (which should be defined elsewhere). Alternatively, we can avoid introducing `t` and `u` by directly showing that \( a^4 = 16n + 1 \) for some \( n \), and similarly for \( b \), so \( a^4 + b^4 - 2 = 16(n + m) \), which is divisible by 16.

**Output in normal language:**
If \( a \) and \( b \) are both odd integers, then \( a^4 + b^4 - 2 \) is divisible by 16. This is because any odd integer raised to the fourth power is of the form \( 16n + 1 \) for some integer \( n \). Therefore, \( a^4 = 16n + 1 \) and \( b^4 = 16m + 1 \), so \( a^4 + b^4 - 2 = 16n + 1 + 16m + 1 - 2 = 16(n + m) \), which is clearly divisible by 16.