### Step 1: Notation and Definitions

Let \( a, b, c \) be integers, not all zero. Let \( d = \gcd(a, b, c) \). We aim to show:
\[
d = \gcd(\gcd(a, b), c) = \gcd(a, \gcd(b, c)) = \gcd(\gcd(a, c), b).
\]

Let:
- \( d_1 = \gcd(a, b) \)
- \( d_2 = \gcd(d_1, c) = \gcd(\gcd(a, b), c) \)
- \( d_3 = \gcd(a, \gcd(b, c)) \)
- \( d_4 = \gcd(\gcd(a, c), b) \)

We will show \( d = d_2 = d_3 = d_4 \).

---

### Step 2: Show \( d = \gcd(\gcd(a, b), c) \)

Since \( d = \gcd(a, b, c) \), it divides \( a, b, c \). In particular, \( d \mid a \) and \( d \mid b \), so \( d \mid \gcd(a, b) = d_1 \). Also \( d \mid c \). Therefore, \( d \) is a common divisor of \( d_1 \) and \( c \), so \( d \mid d_2 \).

Now, \( d_2 = \gcd(d_1, c) \). Since \( d_1 \mid a \) and \( d_1 \mid b \), and \( d_2 \mid d_1 \) and \( d_2 \mid c \), we have \( d_2 \mid a \), \( d_2 \mid b \), and \( d_2 \mid c \). Thus \( d_2 \) is a common divisor of \( a, b, c \), so \( d_2 \mid d \).

Since \( d \mid d_2 \) and \( d_2 \mid d \), we conclude \( d = d_2 \).

---

### Step 3: Show \( d = \gcd(a, \gcd(b, c)) \)

Let \( d_5 = \gcd(b, c) \). Then \( d_3 = \gcd(a, d_5) \).

Since \( d = \gcd(a, b, c) \), we have \( d \mid a \), \( d \mid b \), \( d \mid c \). So \( d \mid \gcd(b, c) = d_5 \). Also \( d \mid a \), so \( d \) is a common divisor of \( a \) and \( d_5 \), hence \( d \mid d_3 \).

Now, \( d_3 = \gcd(a, d_5) \). Since \( d_5 \mid b \) and \( d_5 \mid c \), and \( d_3 \mid a \) and \( d_3 \mid d_5 \), we have \( d_3 \mid a \), \( d_3 \mid b \), \( d_3 \mid c \). So \( d_3 \) is a common divisor of \( a, b, c \), hence \( d_3 \mid d \).

Therefore \( d = d_3 \).

---

### Step 4: Show \( d = \gcd(\gcd(a, c), b) \)

Let \( d_6 = \gcd(a, c) \). Then \( d_4 = \gcd(d_6, b) \).

Since \( d = \gcd(a, b, c) \), we have \( d \mid a \), \( d \mid b \), \( d \mid c \). So \( d \mid \gcd(a, c) = d_6 \). Also \( d \mid b \), so \( d \) is a common divisor of \( d_6 \) and \( b \), hence \( d \mid d_4 \).

Now, \( d_4 = \gcd(d_6, b) \). Since \( d_6 \mid a \) and \( d_6 \mid c \), and \( d_4 \mid d_6 \) and \( d_4 \mid b \), we have \( d_4 \mid a \), \( d_4 \mid b \), \( d_4 \mid c \). So \( d_4 \) is a common divisor of \( a, b, c \), hence \( d_4 \mid d \).

Therefore \( d = d_4 \).

---

### ✅ Final Conclusion

We have shown:
\[
d = \gcd(\gcd(a, b), c) = \gcd(a, \gcd(b, c)) = \gcd(\gcd(a, c), b).
\]

---

### Lean 4 Statement

```lean
theorem gcd_triple_equality (a b c : ℤ) (h : ¬(a = 0 ∧ b = 0 ∧ c = 0)) :
    gcd (gcd a b) c = gcd a (gcd b c) ∧ gcd (gcd a b) c = gcd (gcd a c) b := by
  have h1 : gcd (gcd a b) c = gcd a b c := by
    apply gcd_gcd_eq_gcd
  have h2 : gcd a (gcd b c) = gcd a b c := by
    rw [gcd_assoc]
  have h3 : gcd (gcd a c) b = gcd a b c := by
    rw [gcd_comm b, gcd_assoc, gcd_comm c, gcd_comm (gcd a c) b]
  rw [h1, h2, h3]
  constructor <;> rfl
```

**Note:** The actual Lean proof might require more detailed steps depending on the library used. The above is a sketch assuming certain lemmas (`gcd_gcd_eq_gcd`, `gcd_assoc`, etc.) are available.

---

### Output in Normal Language

Let \( a, b, c \) be integers, not all zero, and let \( d = \gcd(a, b, c) \). Then:
\[
d = \gcd(\gcd(a, b), c) = \gcd(a, \gcd(b, c)) = \gcd(\gcd(a, c), b).
\]
This means the greatest common divisor of three numbers can be computed by first taking the gcd of any two and then taking the gcd of that result with the third number, in any order. The result is independent of the grouping.