I will prove that for any two positive integers \(a\) and \(b\), \(\gcd(a, b)\) divides \(\text{lcm}(a, b)\).

**Proof:**

Let \(d = \gcd(a, b)\) and \(m = \text{lcm}(a, b)\).

By the fundamental property of gcd and lcm, we have:
\[
a \cdot b = \gcd(a, b) \cdot \text{lcm}(a, b) = d \cdot m
\]
Therefore,
\[
m = \frac{a \cdot b}{d}
\]
Since \(d\) divides both \(a\) and \(b\), it follows that \(d\) divides \(a \cdot b\). Hence, \(m = \frac{a \cdot b}{d}\) is an integer (which we know since \(m\) is the lcm).

Now, we want to show that \(d\) divides \(m\). From the above:
\[
m = \frac{a \cdot b}{d}
\]
Multiply both sides by \(d\):
\[
d \cdot m = a \cdot b
\]
This shows that \(d\) divides \(a \cdot b\). However, we need to show that \(d\) divides \(m\).

Alternatively, since \(d \mid a\) and \(d \mid b\), we can write \(a = d \cdot a'\) and \(b = d \cdot b'\) with \(\gcd(a', b') = 1\).

Then,
\[
m = \text{lcm}(a, b) = \text{lcm}(d a', d b') = d \cdot \text{lcm}(a', b')
\]
But since \(\gcd(a', b') = 1\), we have \(\text{lcm}(a', b') = a' b'\). So,
\[
m = d \cdot a' b'
\]
Therefore, \(d\) divides \(m\).

Thus, \(\gcd(a, b)\) divides \(\text{lcm}(a, b)\).

**Conclusion:** For any positive integers \(a\) and \(b\), the greatest common divisor \(\gcd(a, b)\) always divides their least common multiple \(\text{lcm}(a, b)\).

**Output in normal language:**
The greatest common divisor of two positive integers always divides their least common multiple. This is because the product of the two numbers equals the product of their gcd and lcm, and the gcd can be factored out from both numbers when expressing the lcm. Therefore, the gcd is a divisor of the lcm.