I'll prove each part step by step.

### (a) gcd(a + b, a - b) = 1 or 2

**Proof:**
Let d = gcd(a + b, a - b). Then d divides both (a + b) and (a - b), so:
- d divides their sum: (a + b) + (a - b) = 2a
- d divides their difference: (a + b) - (a - b) = 2b

Thus d divides gcd(2a, 2b) = 2·gcd(a, b) = 2·1 = 2.

Since d divides 2, and d > 0, we must have d = 1 or d = 2.

**Lean statement:**
```lean
theorem gcd_sum_diff (a b : ℤ) (h : gcd a b = 1) : gcd (a + b) (a - b) = 1 ∨ gcd (a + b) (a - b) = 2 := by
  have h1 : gcd (a + b) (a - b) ∣ gcd (2 * a) (2 * b) :=
    gcd_dvd_gcd (by rw [show (a + b) + (a - b) = 2 * a by ring, show (a + b) - (a - b) = 2 * b by ring])
  rw [gcd_mul_right 2, h, mul_one] at h1
  exact eq_one_or_eq_two_of_dvd_two h1
```

### (b) gcd(2a + b, a + 2b) = 1 or 3

**Proof:**
Let d = gcd(2a + b, a + 2b). Then:
- d divides: 2(2a + b) - (a + 2b) = 4a + 2b - a - 2b = 3a
- d divides: 2(a + 2b) - (2a + b) = 2a + 4b - 2a - b = 3b

Thus d divides gcd(3a, 3b) = 3·gcd(a, b) = 3·1 = 3.

Since d divides 3, and d > 0, we must have d = 1 or d = 3.

**Lean statement:**
```lean
theorem gcd_linear_comb (a b : ℤ) (h : gcd a b = 1) : gcd (2*a + b) (a + 2*b) = 1 ∨ gcd (2*a + b) (a + 2*b) = 3 := by
  have h1 : gcd (2*a + b) (a + 2*b) ∣ gcd (3*a) (3*b) :=
    gcd_dvd_gcd (by
      have h2 : 2*(2*a + b) - (a + 2*b) = 3*a := by ring
      have h3 : 2*(a + 2*b) - (2*a + b) = 3*b := by ring
      rw [h2, h3])
  rw [gcd_mul_right 3, h, mul_one] at h1
  exact eq_one_or_eq_three_of_dvd_three h1
```

### (c) gcd(a + b, a² + b²) = 1 or 2

**Proof:**
Let d = gcd(a + b, a² + b²). Then:
- d divides: (a² + b²) - (a + b)(a - b) = a² + b² - (a² - b²) = 2b²
- d divides: (a² + b²) - (a + b)(a - b) + 2ab = 2b² + 2ab = 2b(a + b)

But d also divides a + b, so d divides 2b(a + b), thus d divides gcd(2b², 2b(a + b)) = 2b·gcd(b, a + b)

Since gcd(a, b) = 1, we have gcd(b, a + b) = gcd(b, a) = 1, so d divides 2b.

Similarly, we can show d divides 2a, so d divides gcd(2a, 2b) = 2.

Thus d divides 2, so d = 1 or d = 2.

**Lean statement:**
```lean
theorem gcd_sum_sq_sum (a b : ℤ) (h : gcd a b = 1) : gcd (a + b) (a^2 + b^2) = 1 ∨ gcd (a + b) (a^2 + b^2) = 2 := by
  have h1 : gcd (a + b) (a^2 + b^2) ∣ 2 := by
    have : a^2 + b^2 - (a + b)*(a - b) = 2*b^2 := by ring
    have : gcd (a + b) (a^2 + b^2) ∣ 2*b^2 := by
      rw [← this]
      exact gcd_dvd_right (a + b) (a^2 + b^2)
    have : gcd (a + b) (a^2 + b^2) ∣ 2 :=
      by apply gcd_dvd_gcd_of_dvd_mul_right (gcd_eq_one_of_gcd_eq_one_right h) this
    exact this
  exact eq_one_or_eq_two_of_dvd_two h1
```

### (d) gcd(a + b, a² - ab + b²) = 1 or 3

**Proof:**
Let d = gcd(a + b, a² - ab + b²). Then:
- d divides: (a² - ab + b²) + (a + b)(a - 2b) = a² - ab + b² + a² - 2ab + ab - 2b² = 2a² - 2ab - b²
- d divides: (a² - ab + b²) + (a + b)(-a + 2b) = a² - ab + b² - a² + 2ab - ab + 2b² = b²

Actually, a simpler approach:
Note that a² - ab + b² = (a + b)² - 3ab

So d divides (a + b)² - 3ab, and since d divides (a + b), d divides 3ab.

But gcd(a, b) = 1, and d divides a + b, so gcd(d, b) = gcd(a + b, b) = gcd(a, b) = 1.

Thus d divides 3a, and similarly d divides 3b, so d divides gcd(3a, 3b) = 3.

Therefore d divides 3, so d = 1 or d = 3.

**Lean statement:**
```lean
theorem gcd_sum_sq_diff (a b : ℤ) (h : gcd a b = 1) : gcd (a + b) (a^2 - a*b + b^2) = 1 ∨ gcd (a + b) (a^2 - a*b + b^2) = 3 := by
  have h1 : gcd (a + b) (a^2 - a*b + b^2) ∣ 3 := by
    have : a^2 - a*b + b^2 = (a + b)^2 - 3*a*b := by ring
    rw [this]
    have : gcd (a + b) ((a + b)^2 - 3*a*b) ∣ 3*a*b := by
      exact gcd_dvd_of_dvd_sub (dvd_mul_right (a + b) (a + b))
    have : gcd (a + b) (a^2 - a*b + b^2) ∣ 3 :=
      by apply gcd_dvd_gcd_of_dvd_mul_right (gcd_eq_one_of_gcd_eq_one_right h) this
    exact this
  exact eq_one_or_eq_three_of_dvd_three h1
```

**Output in normal language:**
For all four parts, we've shown that when gcd(a, b) = 1:
- gcd(a + b, a - b) must be 1 or 2
- gcd(2a + b, a + 2b) must be 1 or 3  
- gcd(a + b, a² + b²) must be 1 or 2
- gcd(a + b, a² - ab + b²) must be 1 or 3

The proofs work by showing that each gcd divides a small number (2 or 3), and since gcds are positive integers, they must equal one of the divisors of that number.