### Step-by-Step Proof:

We are to prove:  
If \(\gcd(a, b) = 1\), then \(\gcd(a + b, ab) = 1\).

---

**Proof:**

Let \(d = \gcd(a + b, ab)\).  
We aim to show \(d = 1\).

Since \(d \mid (a + b)\) and \(d \mid ab\), we can write:
\[
a + b = d \cdot k \quad \text{and} \quad ab = d \cdot \ell \quad \text{for some integers } k, \ell.
\]

Now, consider that \(d\) must also divide any integer linear combination of \(a + b\) and \(ab\). In particular, we can relate \(a\) and \(b\):

Note that \(a(a + b) = a^2 + ab\).  
So,
\[
a^2 = a(a + b) - ab = d(k a - \ell).
\]
Thus, \(d \mid a^2\). Similarly,
\[
b^2 = b(a + b) - ab = d(k b - \ell),
\]
so \(d \mid b^2\).

Therefore, \(d\) is a common divisor of \(a^2\) and \(b^2\).  
But since \(\gcd(a, b) = 1\), we also have \(\gcd(a^2, b^2) = 1\).  
Hence, \(d\) must divide \(1\), i.e., \(d = 1\).

Alternatively, we can argue by contradiction:  
Suppose a prime \(p\) divides \(d\). Then \(p \mid (a + b)\) and \(p \mid ab\).  
Since \(p \mid ab\), we have \(p \mid a\) or \(p \mid b\).  
If \(p \mid a\), then from \(p \mid (a + b)\) we get \(p \mid b\).  
Similarly, if \(p \mid b\), then \(p \mid a\).  
So \(p\) divides both \(a\) and \(b\), contradicting \(\gcd(a, b) = 1\).  
Thus, no prime divides \(d\), so \(d = 1\).

Therefore, \(\gcd(a + b, ab) = 1\).  
∎

---

### Lean 4 Statement & Proof:

```lean
theorem gcd_sum_prod (a b : ℕ) (h : gcd a b = 1) : gcd (a + b) (a * b) = 1 := by
  -- Assume d divides both (a+b) and (a*b)
  intro d hd
  have h1 : d ∣ a + b := hd.left
  have h2 : d ∣ a * b := hd.right
  -- Show d divides a^2 and b^2
  have h3 : d ∣ a ^ 2 := by
    calc
      a ^ 2 = a * (a + b) - a * b := by ring
      _ = a * (a + b) - (a * b) := rfl
      _ ≡ 0 - 0 [MOD d] := by exact ?_  -- using `h1` and `h2`
      _ ≡ 0 [MOD d] := by simp
  -- Similarly for b^2
  have h4 : d ∣ b ^ 2 := by
    calc
      b ^ 2 = b * (a + b) - a * b := by ring
      _ ≡ 0 - 0 [MOD d] := ?_
      _ ≡ 0 [MOD d] := by simp
  -- Since gcd(a,b)=1, we have gcd(a^2, b^2)=1, so d must be 1.
  have h5 : gcd (a ^ 2) (b ^ 2) = 1 := by
    rw [gcd_eq_gcd_image, pow_succ, pow_succ]  -- or use `Nat.gcd_eq_left`?
    exact h
  exact Nat.eq_one_of_dvd_copr h5 (gcd_dvd_gcd_mul_right _ _) h3 h4
```

**Note:** The above Lean proof is a sketch. A complete formal proof would require filling in the details (e.g., using `Nat.dvd_sub` for the modulo steps, and ensuring the correct theorems are applied). Alternatively, we can use:

```lean
theorem gcd_sum_prod (a b : ℕ) (h : gcd a b = 1) : gcd (a + b) (a * b) = 1 := by
  by_contra! H
  obtain ⟨p, hp, hpd⟩ := exists_prime_and_dvd H
  have h1 : p ∣ a + b := (gcd_dvd_left _ _).trans hpd
  have h2 : p ∣ a * b := (gcd_dvd_right _ _).trans hpd
  rcases (hp.dvd_mul.mp h2) with (h3 | h3)
  · have h4 : p ∣ b := by
      rw [← Nat.dvd_add_iff_right h3] at h1
      exact h1
    have := hp.not_dvd_one (h ▸ dvd_gcd h3 h4)
    contradiction
  · have h4 : p ∣ a := by
      rw [← Nat.dvd_add_iff_left h3] at h1
      exact h1
    have := hp.not_dvd_one (h ▸ dvd_gcd h4 h3)
    contradiction
```

This uses the contradiction approach with a prime divisor.

---

### Output in Normal Language:

If the greatest common divisor of \(a\) and \(b\) is 1, then the greatest common divisor of \(a + b\) and \(ab\) is also 1. This is because any common divisor of \(a + b\) and \(ab\) must also divide \(a^2\) and \(b^2\), and since \(\gcd(a, b) = 1\) implies \(\gcd(a^2, b^2) = 1\), the only positive common divisor is 1. Alternatively, assuming a prime divides both \(a + b\) and \(ab\) leads to a contradiction with \(\gcd(a, b) = 1\). Therefore, the result holds.