 We know that $p$ is an odd prime, so it can be written in the form $p = 2k + 1$ for some integer $k$.

Now, let's consider the expression $p^2 - 1$. We can rewrite it as $(2k + 1)^2 - 1 = 4k^2 + 4k + 1 - 1 = 4k(k + 1)$.

Since $k$ and $k + 1$ are consecutive integers, one of them must be even. Therefore, the product $k(k + 1)$ is even.

Now, let's consider the expression $p^2 + 1$. We can rewrite it as $(2k + 1)^2 + 1 = 4k^2 + 4k + 1 + 1 = 4k(k + 1) + 2$.

Since $k(k + 1)$ is even, $4k(k + 1)$ is also even. Therefore, $4k(k + 1) + 2$ is even.

So, we have shown that both $p^2 - 1$ and $p^2 + 1$ are divisible by 2. Now, we need to show that one of them is also divisible by 5.

We know that $p$ is an odd prime, so it cannot be divisible by 5. Therefore, $p$ must be in the form $p = 5k \pm 1$ for some integer $k$.

If $p = 5k + 1$, then $p^2 - 1 = (5k + 1)^2 - 1 = 25k^2 + 10k = 5(5k^2 + 2k)$, which is divisible by 5.

If $p = 5k - 1$, then $p^2 + 1 = (5k - 1)^2 + 1 = 25k^2 - 10k + 2 = 5(5k^2 - 2k + 1)$, which is also divisible by 5.

Therefore, we have shown that either $p^2 - 1$ or $p^2 + 1$ is divisible by 10.