 To verify this, we can use the principle of mathematical induction.

Base case: For n = 1, we can express it as $1 = 2^0 \cdot 1$, where k = 0 and m = 1. So, the base case holds.

Inductive step: Assume that the statement is true for some integer n = i, i.e., $i = 2^k m$, where k $\geq{0}$ and m is an odd integer.

Now, we need to show that the statement is true for n = i + 1.

Case 1: If i is odd, then m = i and k = 0. So, $i + 1 = 2^0 \cdot (i + 1)$, where k = 0 and m = i + 1, which is odd.

Case 2: If i is even, then i can be written as $i = 2^k m'$, where m' is an odd integer. So, $i + 1 = 2^k m' + 1$. Now, we can factor out a 2 from the expression: $i + 1 = 2(2^{k-1}m') + 1$. Since m' is odd, $2^{k-1}m'$ is also an integer. Let $m'' = 2^{k-1}m'$, which is an odd integer. Then, $i + 1 = 2m'' + 1$.

In both cases, we have expressed $i + 1$ in the form $2^k m$, where k $\geq{0}$ and m is an odd integer.

Therefore, by the principle of mathematical induction, any integer n can be expressed as $n = 2^km$, where k $\geq{0}$ and m is an odd integer.