Let's analyze the given congruence:

For \( n \geq 1 \), show that
\[
(-13)^{n+1} \equiv (-13)^n + (-13)^{n-1} \pmod{181}.
\]

We can rewrite the congruence as:
\[
(-13)^{n+1} - (-13)^n - (-13)^{n-1} \equiv 0 \pmod{181}.
\]

Factor out \( (-13)^{n-1} \):
\[
(-13)^{n-1} \left[ (-13)^2 - (-13) - 1 \right] \equiv 0 \pmod{181}.
\]

Now compute the expression inside the brackets:
\[
(-13)^2 = 169, \quad -(-13) = 13, \quad \text{so} \quad 169 + 13 - 1 = 181.
\]

Thus,
\[
(-13)^{n-1} \cdot 181 \equiv 0 \pmod{181}.
\]

Since \( 181 \equiv 0 \pmod{181} \), we have:
\[
(-13)^{n-1} \cdot 0 \equiv 0 \pmod{181},
\]
which is always true.

Therefore, the original congruence holds for all \( n \geq 1 \).

**Lean Statement:**
```lean
theorem congruence_property (n : ℕ) (hn : n ≥ 1) : (-13 : ℤ)^(n+1) ≡ (-13)^n + (-13)^(n-1) [ZMOD 181] := by
  have h : (-13 : ℤ)^2 - (-13) - 1 = 181 := by norm_num
  calc
    (-13 : ℤ)^(n+1) = (-13)^(n-1) * (-13)^2 : by ring
    _ = (-13)^(n-1) * ((-13)^2) : rfl
    _ = (-13)^(n-1) * ((-13) + 1 + (-13)^2 - (-13) - 1) : by ring
    _ = (-13)^(n-1) * ((-13) + 1) + (-13)^(n-1) * ((-13)^2 - (-13) - 1) : by ring
    _ = (-13)^n + (-13)^(n-1) * 181 : by ring
    _ ≡ (-13)^n + (-13)^(n-1) * 0 [ZMOD 181] : by
        rw [Int.mul_emod_right, Int.zero_emod]
    _ ≡ (-13)^n + 0 [ZMOD 181] : by simp
    _ ≡ (-13)^n [ZMOD 181] : by simp
    _ ≡ (-13)^n + (-13)^(n-1) ?_ : ?_  -- Wait, this is not exactly the same.

-- Actually, we need to show it is equivalent to the sum.
-- Alternatively, we can do:

  have key : (-13 : ℤ)^(n+1) - (-13)^n - (-13)^(n-1) = (-13)^(n-1) * 181 := by
    calc
      (-13)^(n+1) - (-13)^n - (-13)^(n-1) = (-13)^(n-1) * ((-13)^2 - (-13) - 1) : by ring
      _ = (-13)^(n-1) * 181 : by norm_num

  rw [Int.sub_eq_add_neg, Int.sub_eq_add_neg]
  rw [← Int.add_assoc]
  have : (-13 : ℤ)^(n+1) + -(-13)^n + -(-13)^(n-1) = (-13)^(n+1) - (-13)^n - (-13)^(n-1) := by ring
  rw [this]
  rw [key]
  exact Int.dvd_triv_left (181 : ℤ) |>.modEq_zero_int.right.add (by simp)
```

But note: The above Lean proof is a bit messy. Actually, we can simplify:

Since we have \( (-13)^{n+1} - (-13)^n - (-13)^{n-1} = (-13)^{n-1} \cdot 181 \), and 181 is divisible by 181, so this is 0 mod 181.

So in Lean:

```lean
theorem congruence_property (n : ℕ) (hn : n ≥ 1) : (-13 : ℤ)^(n+1) ≡ (-13)^n + (-13)^(n-1) [ZMOD 181] := by
  have h : (-13 : ℤ)^(n+1) - (-13)^n - (-13)^(n-1) = (-13)^(n-1) * 181 := by
    calc
      (-13)^(n+1) - (-13)^n - (-13)^(n-1) = (-13)^(n-1) * ((-13)^2 - (-13) - 1) : by ring
      _ = (-13)^(n-1) * 181 : by norm_num

  have h2 : (181 : ℤ) ∣ (-13)^(n+1) - (-13)^n - (-13)^(n-1) := by
    rw [h]
    exact ⟨(-13)^(n-1), by ring⟩

  exact Int.modEq_zero_iff_dvd.mpr h2 |>.symm.of_add_right |>.of_add_right
```

This should work.

**Output in normal language:**
The congruence \((-13)^{n+1} \equiv (-13)^n + (-13)^{n-1} \pmod{181}\) holds for all \(n \geq 1\) because the expression \((-13)^{n+1} - (-13)^n - (-13)^{n-1}\) simplifies to \((-13)^{n-1} \cdot 181\), which is clearly divisible by 181. Therefore, the difference is congruent to 0 modulo 181, proving the original statement.