### Lean4 Proof

```lean4
theorem sum_of_powers (a : ℕ) (n : ℕ) (h : a ≥ 2) : a^n - 1 = (a - 1) * (∑ i in Finset.range n, a^i) := by
  have h₁ : ∀ n : ℕ, a^n - 1 = (a - 1) * (∑ i in Finset.range n, a^i) := by
    intro n
    induction n with
    | zero =>
      -- Base case: n = 0
      simp
    | succ n ih =>
      -- Inductive step: assume the statement holds for n, prove for n+1
      cases n with
      | zero =>
        -- Base case: n = 1
        simp [Finset.sum_range_succ, pow_one]
        <;> ring
      | succ n =>
        -- Inductive step: n > 0
        simp_all [Finset.sum_range_succ, pow_succ, Nat.mul_sub_left_distrib, Nat.mul_sub_right_distrib]
        <;> ring_nf at *
        <;> omega
  apply h₁
```

### Explanation

1. **Base Case (`n = 0`)**:
   - For `n = 0`, the sum `∑ i in Finset.range 0, a^i` is empty, so it equals 0.
   - The left-hand side (LHS) becomes `a^0 - 1 = 1 - 1 = 0`.
   - The right-hand side (RHS) becomes `(a - 1) * 0 = 0`.
   - Thus, LHS = RHS.

2. **Inductive Step (`n → n + 1`)**:
   - Assume the statement holds for `n`, i.e., `a^n - 1 = (a - 1) * ∑ i in Finset.range n, a^i`.
   - For `n + 1`, the LHS is `a^(n + 1) - 1 = a * a^n - 1`.
   - The RHS is `(a - 1) * ∑ i in Finset.range (n + 1), a^i = (a - 1) * (∑ i in Finset.range n, a^i + a^n)`.
   - Using the inductive hypothesis, substitute `a^n - 1 = (a - 1) * ∑ i in Finset.range n, a^i` into the LHS:
     \[
     a * a^n - 1 = a * (a^n - 1) + (a - 1) = a * (a - 1) * ∑ i in Finset.range n, a^i + (a - 1) = (a - 1) * (a * ∑ i in Finset.range n, a^i + 1) = (a - 1) * (∑ i in Finset.range n, a^i + a^n).
     \]
   - This matches the RHS, completing the inductive step.

### Normal Language Explanation

The proof uses the Second Principle of Finite Induction, which is a generalization of mathematical induction. The key steps are:

1. **Base Case**: Verify the statement for the smallest value of `n` (here, `n = 0`).
2. **Inductive Step**: Assume the statement holds for `n` and prove it for `n + 1` using the inductive hypothesis.

The Lean4 proof uses `have` to state the general form of the identity and then applies induction to prove it for all `n ≥ 0`. The `simp` and `ring` tactics handle the algebraic manipulations, and `omega` is used to ensure all arithmetic holds.