### Lean4 Proof
```lean4
theorem cube_as_difference_of_squares (n : ℤ) : ∃ a b : ℤ, a^2 - b^2 = n^3 := by
  use (n^2 + n)
  use (n^2 - n)
  ring_nf
  <;> simp [sq, mul_add, mul_comm, mul_left_comm]
  <;> ring
  <;> omega
```

### Explanation
1. **Choose \( a \) and \( b \)**: We choose \( a = n^2 + n \) and \( b = n^2 - n \).
2. **Compute \( a^2 - b^2 \)**:
   \[
   a^2 - b^2 = (n^2 + n)^2 - (n^2 - n)^2
   \]
3. **Expand and simplify**:
   \[
   (n^2 + n)^2 = n^4 + 2n^3 + n^2
   \]
   \[
   (n^2 - n)^2 = n^4 - 2n^3 + n^2
   \]
   \[
   a^2 - b^2 = (n^4 + 2n^3 + n^2) - (n^4 - 2n^3 + n^2) = 4n^3
   \]
   Wait, this seems incorrect. Let's re-evaluate:
   \[
   a^2 - b^2 = (n^2 + n)^2 - (n^2 - n)^2 = (n^4 + 2n^3 + n^2) - (n^4 - 2n^3 + n^2) = 4n^3
   \]
   This is incorrect because \( 4n^3 \neq n^3 \). The mistake is in the initial choice of \( a \) and \( b \). Let's try another approach.

### Correct Approach
We need \( a^2 - b^2 = n^3 \). Notice that:
\[
a^2 - b^2 = (a - b)(a + b)
\]
We can set \( a - b = n \) and \( a + b = n^2 \), then solve for \( a \) and \( b \):
\[
a = \frac{(a - b) + (a + b)}{2} = \frac{n + n^2}{2} = \frac{n^2 + n}{2}
\]
\[
b = \frac{(a + b) - (a - b)}{2} = \frac{n^2 - n}{2}
\]
But this gives \( a \) and \( b \) in terms of \( n \), not integers unless \( n \) is even. To ensure \( a \) and \( b \) are integers, we can instead choose:
\[
a = n^2 + \frac{n}{2}, \quad b = n^2 - \frac{n}{2}
\]
But this requires \( n \) to be even. Alternatively, we can use:
\[
a = \frac{n^2 + n}{2}, \quad b = \frac{n^2 - n}{2}
\]
This works if \( n \) is odd or even. Let's verify:
\[
a^2 - b^2 = \left(\frac{n^2 + n}{2}\right)^2 - \left(\frac{n^2 - n}{2}\right)^2 = \frac{(n^2 + n)^2 - (n^2 - n)^2}{4}
\]
Expanding:
\[
(n^2 + n)^2 = n^4 + 2n^3 + n^2
\]
\[
(n^2 - n)^2 = n^4 - 2n^3 + n^2
\]
Subtracting:
\[
(n^4 + 2n^3 + n^2) - (n^4 - 2n^3 + n^2) = 4n^3
\]
Thus:
\[
a^2 - b^2 = \frac{4n^3}{4} = n^3
\]
This is correct. Therefore, the choice \( a = \frac{n^2 + n}{2} \) and \( b = \frac{n^2 - n}{2} \) works for all integers \( n \).

### Lean4 Proof with Correct Choices
```lean4
theorem cube_as_difference_of_squares (n : ℤ) : ∃ a b : ℤ, a^2 - b^2 = n^3 := by
  use (n^2 + n) / 2
  use (n^2 - n) / 2
  have h₁ : (n^2 + n) % 2 = 0 ∨ (n^2 - n) % 2 = 0 := by
    have : n % 2 = 0 ∨ n % 2 = 1 := by omega
    rcases this with (h | h) <;>
    (try omega) <;>
    (try
      {
        have h₂ : n^2 % 2 = n % 2 := by
          have : n % 2 = 0 ∨ n % 2 = 1 := by omega
          rcases this with (h | h) <;> simp [h, pow_two, Int.mul_emod, Int.add_emod]
        omega
      }) <;>
    omega
  cases h₁ with
  | inl h₁ =>
    have h₂ : (n^2 + n) % 2 = 0 := h₁
    have h₃ : (n^2 - n) % 2 = 0 := by
      have : n % 2 = 0 ∨ n % 2 = 1 := by omega
      rcases this with (h | h) <;>
      (try omega) <;>
      (try
        {
          have h₄ : n^2 % 2 = n % 2 := by
            have : n % 2 = 0 ∨ n % 2 = 1 := by omega
            rcases this with (h | h) <;> simp [h, pow_two, Int.mul_emod, Int.add_emod]
          omega
        }) <;>
      omega
    have h₄ : (n^2 + n) / 2 * 2 = n^2 + n := by omega
    have h₅ : (n^2 - n) / 2 * 2 = n^2 - n := by omega
    nlinarith
  | inr h₁ =>
    have h₂ : (n^2 - n) % 2 = 0 := h₁
    have h₃ : (n^2 + n) % 2 = 0 := by
      have : n % 2 = 0 ∨ n % 2 = 1 := by omega
      rcases this with (h | h) <;>
      (try omega) <;>
      (try
        {
          have h₄ : n^2 % 2 = n % 2 := by
            have : n % 2 = 0 ∨ n % 2 = 1 := by omega
            rcases this with (h | h) <;> simp [h, pow_two, Int.mul_emod, Int.add_emod]
          omega
        }) <;>
      omega
    have h₄ : (n^2 + n) / 2 * 2 = n^2 + n := by omega
    have h₅ : (n^2 - n) / 2 * 2 = n^2 - n := by omega
    nlinarith
```

### Normal Language Explanation
1. **Choose \( a \) and \( b \)**:
   - Let \( a = \frac{n^2 + n}{2} \) and \( b = \frac{n^2 - n}{2} \).
2. **Verify divisibility**:
   - For \( a \) and \( b \) to be integers, \( n^2 + n \) and \( n^2 - n \) must be even. This happens when \( n \) is even or odd.
3. **Compute \( a^2 - b^2 \)**:
   - Expand \( a^2 - b^2 \) and simplify to show it equals \( n^3 \).
4. **Conclusion**:
   - The difference of squares \( a^2 - b^2 \) equals \( n^3 \), proving the theorem.