### Part (a)

**Base Case (n = 1):**
\[
\frac{1}{1^2} = 1 \leq 2 - \frac{1}{1} = 1
\]
This holds with equality.

**Inductive Step:**
Assume the statement holds for some \( n = k \geq 1 \), i.e.,
\[
\sum_{i=1}^k \frac{1}{i^2} \leq 2 - \frac{1}{k}
\]
We need to show it holds for \( n = k + 1 \):
\[
\sum_{i=1}^{k+1} \frac{1}{i^2} = \sum_{i=1}^k \frac{1}{i^2} + \frac{1}{(k+1)^2} \leq 2 - \frac{1}{k} + \frac{1}{(k+1)^2}
\]
We need to show:
\[
2 - \frac{1}{k} + \frac{1}{(k+1)^2} \leq 2 - \frac{1}{k+1}
\]
Simplify the inequality:
\[
\frac{1}{k} - \frac{1}{k+1} \geq \frac{1}{(k+1)^2}
\]
\[
\frac{1}{k(k+1)} \geq \frac{1}{(k+1)^2}
\]
\[
1 \geq \frac{k}{k+1}
\]
\[
k + 1 \geq k
\]
Which is true. Thus, the inductive step holds, and the statement is proved by induction.

### Part (b)

**Base Case (n = 1):**
\[
\frac{1}{2} = 2 - \frac{1 + 2}{2^1} = 2 - \frac{3}{2} = \frac{1}{2}
\]
This holds.

**Inductive Step:**
Assume the statement holds for some \( n = k \geq 1 \), i.e.,
\[
\sum_{i=1}^k \frac{i}{2^i} = 2 - \frac{k + 2}{2^k}
\]
We need to show it holds for \( n = k + 1 \):
\[
\sum_{i=1}^{k+1} \frac{i}{2^i} = \sum_{i=1}^k \frac{i}{2^i} + \frac{k+1}{2^{k+1}} = 2 - \frac{k + 2}{2^k} + \frac{k+1}{2^{k+1}}
\]
We need to show:
\[
2 - \frac{k + 2}{2^k} + \frac{k+1}{2^{k+1}} = 2 - \frac{(k+1) + 2}{2^{k+1}}
\]
Simplify the right-hand side:
\[
2 - \frac{k + 3}{2^{k+1}}
\]
Now, simplify the left-hand side:
\[
2 - \frac{k + 2}{2^k} + \frac{k+1}{2^{k+1}} = 2 - \frac{2(k + 2) + (k + 1)}{2^{k+1}} = 2 - \frac{3k + 5}{2^{k+1}}
\]
Thus, we need:
\[
2 - \frac{3k + 5}{2^{k+1}} = 2 - \frac{k + 3}{2^{k+1}}
\]
Which simplifies to:
\[
\frac{3k + 5}{2^{k+1}} = \frac{k + 3}{2^{k+1}}
\]
\[
3k + 5 = k + 3
\]
\[
2k = -2
\]
\[
k = -1
\]
This is false for \( k \geq 1 \). **This indicates a mistake in the inductive step.**

**Correct Inductive Step:**
The error arises from the incorrect assumption of the inductive hypothesis. The correct inductive hypothesis should be:
\[
\sum_{i=1}^k \frac{i}{2^i} = 2 - \frac{k + 2}{2^k} - \frac{k}{2^k}
\]
But this seems overly complicated. Instead, let's re-express the original statement for \( n = k + 1 \):
\[
\sum_{i=1}^{k+1} \frac{i}{2^i} = 2 - \frac{(k+1) + 2}{2^{k+1}}
\]
This is correct. The error was in the initial assumption. The correct inductive step is:
\[
2 - \frac{k + 2}{2^k} + \frac{k+1}{2^{k+1}} = 2 - \frac{(k+1) + 2}{2^{k+1}}
\]
Which simplifies to:
\[
- \frac{k + 2}{2^k} + \frac{k+1}{2^{k+1}} = - \frac{(k+1) + 2}{2^{k+1}}
\]
Multiply through by \( 2^{k+1} \):
\[
- (k + 2) \cdot 2 + (k + 1) = - (k + 3)
\]
\[
-2k - 4 + k + 1 = -k - 3
\]
\[
-k - 3 = -k - 3
\]
Which holds true. Thus, the inductive step is correct, and the statement is proved by induction.

### Lean4 Proof Sketch

```lean4
theorem part_a (n : ℕ) (hn : n ≥ 1) : ∑ i in Finset.range n, 1 / (i + 1)^2 ≤ 2 - 1 / n := by
  induction' hn with n hn IH
  -- Base case n = 1
  norm_num
  -- Inductive step
  cases n with
  | zero => contradiction  -- n ≥ 1, so n cannot be zero
  | succ n =>
    cases n with
    | zero => norm_num  -- n = 1
    | succ n =>
      simp_all [Finset.sum_range_succ, Nat.div_eq_of_lt, Nat.lt_succ_iff]
      <;> norm_num
      <;> linarith
```

### Lean4 Proof for Part (b)

```lean4
theorem part_b (n : ℕ) : ∑ i in Finset.range n, (i + 1) / 2^(i + 1) = 2 - (n + 2) / 2^n := by
  induction' n with n IH
  -- Base case n = 0
  norm_num
  -- Inductive step
  cases n with
  | zero => norm_num  -- n = 0
  | succ n =>
    simp_all [Finset.sum_range_succ, Nat.div_eq_of_lt, Nat.lt_succ_iff, Nat.succ_div]
    <;> ring_nf at *
    <;> omega
```