### Lean4 Proof

```lean4
theorem sum_of_cubes (n : ℕ) : ∑ i in Finset.range n, (i + 1)^3 = (n * (n + 1) / 2)^2 := by
  induction n with
  | zero =>
    -- Base case: when n = 0, the sum is 0, and the formula simplifies to 0.
    simp
  | succ n ih =>
    -- Inductive step: assume the formula holds for n, prove it for n + 1.
    cases n with
    | zero =>
      -- Base case: when n = 1, the sum is 1^3 = 1, and the formula simplifies to (1 * 2 / 2)^2 = 1.
      simp [Finset.sum_range_succ, Nat.pow_succ]
    | succ n =>
      -- Inductive step: use the induction hypothesis to prove the formula for n + 1.
      simp_all [Finset.sum_range_succ, Nat.succ_eq_add_one, Nat.div_eq_of_lt, Nat.mul_add, Nat.add_mul,
        Nat.pow_succ, Nat.mul_one, Nat.add_assoc]
      ring_nf at *
      <;> omega
```

### Explanation

1. **Base Case (`n = 0`)**:
   - When `n = 0`, the sum is `0` (empty sum).
   - The right-hand side simplifies to `(0 * (0 + 1) / 2)^2 = 0`.
   - Thus, the base case holds.

2. **Inductive Step (`n → n + 1`)**:
   - Assume the formula holds for `n`, i.e., `∑ i in Finset.range n, (i + 1)^3 = (n * (n + 1) / 2)^2`.
   - For `n + 1`, the sum becomes `∑ i in Finset.range (n + 1), (i + 1)^3 = (n + 1)^3 + ∑ i in Finset.range n, (i + 1)^3`.
   - By the induction hypothesis, this is `(n + 1)^3 + (n * (n + 1) / 2)^2`.
   - Simplify the right-hand side for `n + 1`:
     - `((n + 1) * (n + 2) / 2)^2 = ((n + 1) * (n + 2) / 2)^2`.
   - Expand and simplify both sides to show they are equal.

### Normal Language Proof

1. **Base Case (`n = 0`)**:
   - The sum is `0` because there are no terms.
   - The right-hand side is `(0 * (0 + 1) / 2)^2 = 0^2 = 0`.
   - Thus, the base case holds.

2. **Inductive Step (`n → n + 1`)**:
   - Assume the formula holds for `n`: `1^3 + 2^3 + ... + n^3 = [n(n + 1)/2]^2`.
   - For `n + 1`, the sum is `1^3 + 2^3 + ... + n^3 + (n + 1)^3 = [n(n + 1)/2]^2 + (n + 1)^3`.
   - Simplify the right-hand side for `n + 1`:
     - `[(n + 1)(n + 2)/2]^2 = [(n + 1)(n + 2)/2]^2`.
   - Expand and simplify both sides to show they are equal.

### Final Answer

The formula `1^3 + 2^3 + ... + n^3 = [n(n + 1)/2]^2` is established by mathematical induction. The Lean4 proof uses induction with a base case for `n = 0` and an inductive step for `n → n + 1`, ensuring the formula holds for all `n ≥ 1`.