### Lean4 Proof
```lean4
theorem a_n_lt_2_pow_n : ∀ n : ℕ, n ≥ 1 → a n < 2 ^ n := by
  intro n hn
  induction n using Nat.strong_induction_on with
  | h n ih =>
    match n with
    | 0 => contradiction -- n ≥ 1, so n = 0 is impossible
    | 1 => norm_num [a] -- Base case: a_1 = 1 < 2^1 = 2
    | 2 => norm_num [a] -- Base case: a_2 = 2 < 2^2 = 4
    | 3 => norm_num [a] -- Base case: a_3 = 3 < 2^3 = 8
    | n + 4 =>
      have h₁ := ih (n + 3) (by omega) -- Inductive hypothesis for n + 3
      have h₂ := ih (n + 2) (by omega) -- Inductive hypothesis for n + 2
      have h₃ := ih (n + 1) (by omega) -- Inductive hypothesis for n + 1
      have h₄ := ih n (by omega) -- Inductive hypothesis for n
      simp_all [a, pow_succ, Nat.mul_add, Nat.add_mul, Nat.add_assoc]
      -- Use the recurrence relation and inductive hypotheses to prove the inequality
      <;> omega
```
### Explanation
1. **Base Cases**:
   - For \( n = 1 \), \( a_1 = 1 < 2^1 = 2 \).
   - For \( n = 2 \), \( a_2 = 2 < 2^2 = 4 \).
   - For \( n = 3 \), \( a_3 = 3 < 2^3 = 8 \).
2. **Inductive Step**:
   - Assume \( a_k < 2^k \) for all \( k < n + 4 \).
   - We need to show \( a_{n + 4} < 2^{n + 4} \).
   - By the recurrence relation, \( a_{n + 4} = a_{n + 3} + a_{n + 2} + a_{n + 1} \).
   - Using the inductive hypotheses:
     - \( a_{n + 3} < 2^{n + 3} \),
     - \( a_{n + 2} < 2^{n + 2} \),
     - \( a_{n + 1} < 2^{n + 1} \).
   - Summing these inequalities:
     \[
     a_{n + 4} < 2^{n + 3} + 2^{n + 2} + 2^{n + 1} = 2^{n + 1} (2^2 + 2 + 1) = 7 \cdot 2^{n + 1}
     \]
   - We need to show \( 7 \cdot 2^{n + 1} < 2^{n + 4} \), which simplifies to \( 7 < 16 \), which is true.
   - Thus, \( a_{n + 4} < 2^{n + 4} \).
3. **Conclusion**:
   - By the Second Principle of Finite Induction, \( a_n < 2^n \) for all \( n \geq 1 \).

### Normal Language Explanation
1. **Base Cases**:
   - For \( n = 1 \), \( a_1 = 1 < 2 \).
   - For \( n = 2 \), \( a_2 = 2 < 4 \).
   - For \( n = 3 \), \( a_3 = 3 < 8 \).
2. **Inductive Step**:
   - Assume \( a_k < 2^k \) for all \( k < n + 4 \).
   - By the recurrence relation, \( a_{n + 4} = a_{n + 3} + a_{n + 2} + a_{n + 1} \).
   - Using the inductive hypotheses:
     - \( a_{n + 3} < 2^{n + 3} \),
     - \( a_{n + 2} < 2^{n + 2} \),
     - \( a_{n + 1} < 2^{n + 1} \).
   - Summing these inequalities:
     \[
     a_{n + 4} < 2^{n + 3} + 2^{n + 2} + 2^{n + 1} = 7 \cdot 2^{n + 1}
     \]
   - We need to show \( 7 \cdot 2^{n + 1} < 2^{n + 4} \), which simplifies to \( 7 < 16 \), which is true.
   - Thus, \( a_{n + 4} < 2^{n + 4} \).
3. **Conclusion**:
   - By the Second Principle of Finite Induction, \( a_n < 2^n \) for all \( n \geq 1 \).