### Lean4 Proof

```lean4
theorem sum_of_odd_numbers (n : ℕ) : ∑ k in Finset.range n, (2 * k + 1) = n ^ 2 := by
  induction n with
  | zero => simp
  | succ n ih =>
    cases n with
    | zero => simp
    | succ n =>
      simp_all [Finset.sum_range_succ, Nat.pow_succ, Nat.mul_succ]
      <;> ring_nf at *
      <;> omega
```

### Explanation

1. **Base Case (`n = 0`)**:
   - When `n = 0`, the sum is empty, and the sum is `0`.
   - The right-hand side is `0^2 = 0`.
   - Thus, the base case holds.

2. **Inductive Step**:
   - Assume the statement holds for `n = k`, i.e., `∑ k in Finset.range k, (2 * k + 1) = k^2`.
   - For `n = k + 1`, the sum becomes `∑ k in Finset.range (k + 1), (2 * k + 1) = ∑ k in Finset.range k, (2 * k + 1) + (2 * k + 1)`.
   - By the inductive hypothesis, this is `k^2 + (2 * k + 1)`.
   - Simplify to `k^2 + 2k + 1 = (k + 1)^2`, which completes the inductive step.

### Normal Language Explanation

The sum of the first `n` odd numbers is `n^2`. This can be proven by induction:

1. **Base Case**: For `n = 1`, the sum is `1`, which is `1^2`.
2. **Inductive Step**: Assume the sum of the first `k` odd numbers is `k^2`. Then, the sum of the first `k + 1` odd numbers is `k^2 + (2k + 1) = (k + 1)^2`.

This completes the proof by induction.