### Lean4 Proof

```lean4
theorem sum_formula (n : ℕ) : ∑ i in Finset.range n, (i + 1) = n * (n + 1) / 2 := by
  induction n with
  | zero => simp
  | succ n ih =>
    cases n with
    | zero => simp
    | succ n =>
      simp_all [Finset.sum_range_succ, Nat.succ_eq_add_one, Nat.div_eq_of_lt, Nat.mul_add, Nat.add_mul]
      ring_nf at *
      <;> omega
```

### Explanation

1. **Base Case (`n = 0`)**:
   - When `n = 0`, the sum is `0`, and the formula gives `0 * (0 + 1) / 2 = 0`. This matches, so the base case holds.

2. **Inductive Step (`n → n + 1`)**:
   - Assume the formula holds for `n`, i.e., `∑ i in Finset.range n, (i + 1) = n * (n + 1) / 2`.
   - For `n + 1`, the sum becomes `∑ i in Finset.range (n + 1), (i + 1) = ∑ i in Finset.range n, (i + 1) + (n + 1)`.
   - By the inductive hypothesis, this is `n * (n + 1) / 2 + (n + 1)`.
   - Simplify the expression to `(n * (n + 1) + 2 * (n + 1)) / 2 = ((n + 1) * (n + 2)) / 2`, which matches the formula for `n + 1`.

### Normal Language Proof

1. **Base Case (`n = 1`)**:
   - The sum is `1`, and the formula gives `1 * (1 + 1) / 2 = 1`. This matches.

2. **Inductive Step (`n → n + 1`)**:
   - Assume the formula holds for `n`, i.e., `1 + 2 + ... + n = n(n + 1)/2`.
   - For `n + 1`, the sum is `1 + 2 + ... + n + (n + 1) = n(n + 1)/2 + (n + 1)`.
   - Factor out `(n + 1)`: `(n + 1)(n/2 + 1) = (n + 1)(n + 2)/2`, which is the formula for `n + 1`.

This completes the proof by induction.