### Lean4 Proof

```lean4
theorem a_n_formula : ∀ n : ℕ, a n = 5 * 2 ^ n + 1 := by
  intro n
  induction n using Nat.strong_induction_on with
  | h n ih =>
    match n with
    | 0 =>
      -- Base case: n = 0
      simp_all [a]
      <;> norm_num
    | 1 =>
      -- Base case: n = 1
      simp_all [a]
      <;> norm_num
    | 2 =>
      -- Base case: n = 2
      simp_all [a]
      <;> norm_num
    | n + 3 =>
      -- Inductive step: assume the formula holds for n and n+1, prove for n+2
      have h1 := ih (n + 2) (by linarith)
      have h2 := ih (n + 1) (by linarith)
      have h3 := ih n (by linarith)
      simp_all [a, pow_succ, mul_add, mul_one, mul_assoc, mul_comm, mul_left_comm]
      <;> ring_nf at *
      <;> omega
```

### Explanation

1. **Base Cases**:
   - For `n = 0`, we directly compute `a 0` and verify the formula.
   - For `n = 1`, we compute `a 1` and verify the formula.
   - For `n = 2`, we compute `a 2` and verify the formula.

2. **Inductive Step**:
   - Assume the formula holds for `n`, `n+1`, and `n+2` (this is the strong induction hypothesis).
   - Use the recurrence relation to express `a (n+3)` in terms of `a (n+2)`, `a (n+1)`, and `a n`.
   - Substitute the inductive hypothesis into the recurrence relation and simplify to show that the formula holds for `n+3`.

3. **Simplification**:
   - The `ring_nf` tactic is used to simplify the algebraic expressions.
   - The `omega` tactic is used to solve the resulting linear arithmetic problem.

This completes the proof by induction.