### Lean4 Proof

```lean4
theorem sum_formula_c : ∀ n : ℕ, 1 * 2 + 2 * 3 + 3 * 4 + ⋯ + n * (n + 1) = n * (n + 1) * (n + 2) / 3 := by
  intro n
  induction n with
  | zero => simp
  | succ n ih =>
    cases n with
    | zero => simp
    | succ n =>
      simp_all [Nat.mul_succ, Nat.succ_eq_add_one, Nat.add_assoc]
      ring_nf
      <;> omega
```

### Explanation

1. **Base Case (`n = 0`)**:
   - The sum is `0`, and the right-hand side is `0 * (0 + 1) * (0 + 2) / 3 = 0`.
   - This holds trivially.

2. **Inductive Step (`n → n + 1`)**:
   - Assume the formula holds for `n`, i.e., `1 * 2 + 2 * 3 + ... + n * (n + 1) = n * (n + 1) * (n + 2) / 3`.
   - For `n + 1`, the sum becomes `1 * 2 + 2 * 3 + ... + n * (n + 1) + (n + 1) * (n + 2)`.
   - By the inductive hypothesis, this equals `n * (n + 1) * (n + 2) / 3 + (n + 1) * (n + 2)`.
   - Simplify the right-hand side:
     \[
     \frac{n(n + 1)(n + 2)}{3} + (n + 1)(n + 2) = \frac{n(n + 1)(n + 2) + 3(n + 1)(n + 2)}{3}
     \]
     \[
     = \frac{(n + 1)(n + 2)(n + 3)}{3}
     \]
   - This matches the formula for `n + 1`.

### Normal Language Proof

1. **Base Case (`n = 0`)**:
   - The sum is `0`, and the right-hand side is `0 * 1 * 2 / 3 = 0`.
   - The formula holds for `n = 0`.

2. **Inductive Step (`n → n + 1`)**:
   - Assume the formula holds for `n`, i.e., the sum up to `n` is `n(n + 1)(n + 2)/3`.
   - For `n + 1`, the sum is the sum up to `n` plus `(n + 1)(n + 2)`.
   - Substitute the inductive hypothesis:
     \[
     \frac{n(n + 1)(n + 2)}{3} + (n + 1)(n + 2)
     \]
   - Factor out `(n + 1)(n + 2)`:
     \[
     (n + 1)(n + 2)\left(\frac{n}{3} + 1\right) = \frac{(n + 1)(n + 2)(n + 3)}{3}
     \]
   - This is the formula for `n + 1`, completing the induction.