### Lean4 Proof

```lean4
theorem sum_of_geometric_series (a r : ℝ) (n : ℕ) (h : r ≠ 1) : 
  a + ar + ar^2 + ... + ar^n = a * (r^(n+1) - 1) / (r - 1) := by
  have h₁ : a + ar + ar^2 + ... + ar^n = a * (r^(n+1) - 1) / (r - 1) := by
    induction n with
    | zero =>
      -- Base case: n = 0
      simp [mul_comm]
      <;> field_simp [sub_ne_zero.mpr h, sub_ne_zero.mpr h.symm]
      <;> ring
    | succ n ih =>
      -- Inductive step: assume the formula holds for n, prove for n+1
      simp_all [Finset.sum_range_succ, pow_succ, mul_add, mul_comm, mul_left_comm]
      <;> field_simp [sub_ne_zero.mpr h, sub_ne_zero.mpr h.symm] at *
      <;> ring_nf at *
      <;> linarith
  exact h₁
```

### Explanation

1. **Base Case (n = 0)**:
   - For `n = 0`, the sum is simply `a`.
   - The right-hand side simplifies to `a * (r^1 - 1) / (r - 1) = a * (r - 1) / (r - 1) = a` (since `r ≠ 1`).

2. **Inductive Step**:
   - Assume the formula holds for `n`, i.e., `a + ar + ... + ar^n = a * (r^(n+1) - 1) / (r - 1)`.
   - For `n + 1`, the sum becomes `a + ar + ... + ar^n + ar^(n+1)`.
   - Using the inductive hypothesis, this becomes `a * (r^(n+1) - 1) / (r - 1) + ar^(n+1)`.
   - Combine the terms over a common denominator:
     ```
     a * (r^(n+1) - 1) / (r - 1) + ar^(n+1) = [a * (r^(n+1) - 1) + ar^(n+1) * (r - 1)] / (r - 1)
     = [a * r^(n+1) - a + a * r^(n+2) - a * r^(n+1)] / (r - 1)
     = [a * r^(n+2) - a] / (r - 1)
     = a * (r^(n+2) - 1) / (r - 1)
     ```
   - This matches the formula for `n + 1`.

### Normal Language Proof

1. **Base Case (n = 0)**:
   - The sum is `a`.
   - The right-hand side is `a * (r^1 - 1) / (r - 1) = a * (r - 1) / (r - 1) = a` (since `r ≠ 1`).

2. **Inductive Step**:
   - Assume the formula holds for `n`, i.e., `S_n = a * (r^(n+1) - 1) / (r - 1)`.
   - For `n + 1`, the sum is `S_{n+1} = S_n + ar^(n+1)`.
   - Substitute the inductive hypothesis:
     ```
     S_{n+1} = a * (r^(n+1) - 1) / (r - 1) + ar^(n+1)
     = [a * (r^(n+1) - 1) + ar^(n+1) * (r - 1)] / (r - 1)
     = [a * r^(n+1) - a + a * r^(n+2) - a * r^(n+1)] / (r - 1)
     = [a * r^(n+2) - a] / (r - 1)
     = a * (r^(n+2) - 1) / (r - 1)
     ```
   - This matches the formula for `n + 1`.

Thus, the formula is proven by induction.