### Part (a): Verification of the Identity

We need to verify that for all \( n \geq 1 \),
\[ 2 \cdot 6 \cdot 10 \cdot \ldots \cdot (4n - 2) = \frac{(2n)!}{n!} \]

**Proof:**

1. **Base Case (\( n = 1 \)):**
   - Left-hand side (LHS): \( 2 \cdot 6 \cdot 10 \cdot \ldots \cdot (4 \cdot 1 - 2) = 2 \).
   - Right-hand side (RHS): \( \frac{(2 \cdot 1)!}{1!} = \frac{2!}{1!} = \frac{2}{1} = 2 \).
   - Thus, LHS = RHS.

2. **Inductive Step:**
   - Assume the identity holds for some \( n = k \geq 1 \), i.e.,
     \[ 2 \cdot 6 \cdot 10 \cdot \ldots \cdot (4k - 2) = \frac{(2k)!}{k!} \]
   - We need to show it holds for \( n = k + 1 \), i.e.,
     \[ 2 \cdot 6 \cdot 10 \cdot \ldots \cdot (4(k + 1) - 2) = \frac{(2(k + 1))!}{(k + 1)!} \]
   - The LHS for \( n = k + 1 \) is:
     \[ 2 \cdot 6 \cdot 10 \cdot \ldots \cdot (4k - 2) \cdot (4(k + 1) - 2) = \frac{(2k)!}{k!} \cdot (4k + 2) \]
   - The RHS for \( n = k + 1 \) is:
     \[ \frac{(2(k + 1))!}{(k + 1)!} = \frac{(2k + 2)!}{(k + 1)!} \]
   - We need to show:
     \[ \frac{(2k)!}{k!} \cdot (4k + 2) = \frac{(2k + 2)!}{(k + 1)!} \]
   - Simplify the RHS:
     \[ \frac{(2k + 2)!}{(k + 1)!} = \frac{(2k + 2)(2k + 1)(2k)!}{(k + 1)k!} = \frac{(2k + 2)(2k + 1)}{(k + 1)} \cdot \frac{(2k)!}{k!} \]
   - Thus, the RHS becomes:
     \[ \frac{(2k + 2)(2k + 1)}{(k + 1)} \cdot \frac{(2k)!}{k!} \]
   - The LHS is:
     \[ \frac{(2k)!}{k!} \cdot (4k + 2) = \frac{(2k)!}{k!} \cdot 2(2k + 1) \]
   - Equate the two:
     \[ \frac{(2k)!}{k!} \cdot 2(2k + 1) = \frac{(2k + 2)(2k + 1)}{(k + 1)} \cdot \frac{(2k)!}{k!} \]
     \[ 2(2k + 1) = \frac{(2k + 2)(2k + 1)}{(k + 1)} \]
     \[ 2(2k + 1) = \frac{2(k + 1)(2k + 1)}{(k + 1)} \]
     \[ 2(2k + 1) = 2(2k + 1) \]
   - This holds true, completing the inductive step.

**Conclusion:** By the principle of mathematical induction, the identity holds for all \( n \geq 1 \).

### Part (b): Inequality \( 2^n (n!)^2 \leq (2n)! \)

Using the identity from part (a), we can derive the inequality.

1. From part (a), we have:
   \[ 2 \cdot 6 \cdot 10 \cdot \ldots \cdot (4n - 2) = \frac{(2n)!}{n!} \]
2. The product \( 2 \cdot 6 \cdot 10 \cdot \ldots \cdot (4n - 2) \) has \( n \) terms, each of which is at least 2. Thus:
   \[ 2 \cdot 6 \cdot 10 \cdot \ldots \cdot (4n - 2) \geq 2^n \]
3. Therefore:
   \[ \frac{(2n)!}{n!} \geq 2^n \]
   \[ (2n)! \geq 2^n \cdot n! \]
   \[ (2n)! \geq 2^n \cdot (n!)^2 \]
   \[ 2^n (n!)^2 \leq (2n)! \]

**Conclusion:** The inequality \( 2^n (n!)^2 \leq (2n)! \) holds for all \( n \geq 1 \).

### Lean4 Proof Sketch

```lean4
theorem part_a : ∀ n : ℕ, n ≥ 1 → 2 * 6 * 10 * ... * (4 * n - 2) = (2 * n)! / n! := by
  have base_case : 2 * 6 * 10 * ... * (4 * 1 - 2) = (2 * 1)! / 1! := by sorry
  have inductive_step : ∀ k : ℕ, k ≥ 1 → 2 * 6 * 10 * ... * (4 * k - 2) = (2 * k)! / k! → 2 * 6 * 10 * ... * (4 * (k + 1) - 2) = (2 * (k + 1))! / (k + 1)! := by sorry
  sorry
```

### Lean4 Proof of Part (b)

```lean4
theorem part_b : ∀ n : ℕ, n ≥ 1 → 2^n * (n!)^2 ≤ (2 * n)! := by
  have h_part_a : ∀ n : ℕ, n ≥ 1 → 2 * 6 * 10 * ... * (4 * n - 2) = (2 * n)! / n! := by sorry
  have h_product_bound : ∀ n : ℕ, n ≥ 1 → 2 * 6 * 10 * ... * (4 * n - 2) ≥ 2^n := by sorry
  have h_final_bound : ∀ n : ℕ, n ≥ 1 → 2^n * (n!)^2 ≤ (2 * n)! := by sorry
  sorry
```