### Lean4 Proof

```lean4
theorem sum_of_odd_squares (n : ℕ) : ∑ k in Finset.range n, (2 * k + 1) ^ 2 = n * (2 * n - 1) * (2 * n + 1) / 3 := by
  induction n with
  | zero =>
    -- Base case: n = 0
    simp
  | succ n ih =>
    -- Inductive step: assume the statement holds for n, prove for n+1
    cases n with
    | zero =>
      -- Base case: n = 1
      simp [Finset.sum_range_succ, Nat.mul_div_cancel_left]
    | succ n =>
      -- Inductive step: n = k + 1
      simp_all [Finset.sum_range_succ, Nat.mul_div_cancel_left, Nat.mul_sub_left_distrib,
        Nat.mul_add, Nat.add_mul, Nat.mul_one, Nat.mul_assoc]
      ring_nf at *
      omega
```

### Explanation

1. **Base Case (`n = 0`)**:
   - The sum is empty, so the sum is 0.
   - The right-hand side simplifies to `0 * (2 * 0 - 1) * (2 * 0 + 1) / 3 = 0`.
   - Thus, the base case holds.

2. **Inductive Step**:
   - Assume the statement holds for `n = k`, i.e., `∑ k in Finset.range k, (2 * k + 1) ^ 2 = k * (2 * k - 1) * (2 * k + 1) / 3`.
   - For `n = k + 1`, the sum becomes `∑ k in Finset.range (k + 1), (2 * k + 1) ^ 2 = (∑ k in Finset.range k, (2 * k + 1) ^ 2) + (2 * k + 1) ^ 2`.
   - By the inductive hypothesis, this is `k * (2 * k - 1) * (2 * k + 1) / 3 + (2 * k + 1) ^ 2`.
   - Simplify the expression to match the right-hand side for `n = k + 1`.

### Normal Language Explanation

The proof uses mathematical induction:

1. **Base Case**: Verify the formula for `n = 0` and `n = 1` to ensure it holds.
2. **Inductive Step**: Assume the formula holds for `n = k` and prove it for `n = k + 1` by adding the next odd square and simplifying the expression.

The Lean4 code uses `simp` and `ring_nf` to simplify the expressions and `omega` to solve the resulting linear arithmetic problem. The `Finset.sum_range_succ` lemma is used to express the sum for `n + 1` in terms of the sum for `n`.