### Lean4 Proof

```lean4
theorem sum_factorial_identity : ∀ n : ℕ, ∑ k in Finset.range n, (k + 1) * (k + 1)! = (n + 1)! - 1 := by
  intro n
  induction n with
  | zero => simp
  | succ n ih =>
    cases n with
    | zero => simp [Finset.sum_range_succ, Nat.factorial]
    | succ n =>
      simp_all [Finset.sum_range_succ, Nat.factorial_succ, Nat.succ_mul, Nat.mul_succ]
      ring_nf at *
      <;> omega
```

### Explanation

1. **Base Case (`n = 0`)**:
   - When `n = 0`, the sum is empty (`∑ k in Finset.range 0, ...`), which is `0`.
   - The right-hand side is `(0 + 1)! - 1 = 1 - 1 = 0`.
   - Thus, the base case holds.

2. **Inductive Step (`n → n + 1`)**:
   - Assume the identity holds for `n`, i.e., `∑ k in Finset.range n, (k + 1) * (k + 1)! = (n + 1)! - 1`.
   - For `n + 1`, the sum becomes `∑ k in Finset.range (n + 1), (k + 1) * (k + 1)! = (∑ k in Finset.range n, (k + 1) * (k + 1)!) + (n + 1) * (n + 1)!`.
   - By the inductive hypothesis, this equals `(n + 1)! - 1 + (n + 1) * (n + 1)!`.
   - Simplify the right-hand side:
     - `(n + 1)! - 1 + (n + 1) * (n + 1)! = (n + 1)! (1 + n + 1) - 1 = (n + 1)! (n + 2) - 1`.
   - We need to show that `(n + 1)! (n + 2) - 1 = ((n + 1) + 1)! - 1 = (n + 2)! - 1`.
   - This is true because `(n + 2)! = (n + 2) * (n + 1)!`, so `(n + 2)! - 1 = (n + 2) * (n + 1)! - 1 = (n + 1)! (n + 2) - 1`.

Thus, the identity holds for all `n ≥ 0`.

### Normal Language Explanation

1. **Base Case (`n = 0`)**:
   - The sum is `0` because there are no terms.
   - The right-hand side is `1! - 1 = 0`.
   - The identity holds for `n = 0`.

2. **Inductive Step (`n → n + 1`)**:
   - Assume the identity holds for `n`.
   - For `n + 1`, the sum is the sum for `n` plus the `(n + 1)`-th term.
   - Substitute the inductive hypothesis and simplify.
   - Show that the simplified form equals `(n + 2)! - 1`.

This completes the proof by induction.