### Lean4 Proof

```lean4
theorem bernoulli_inequality (a : ℤ) (n : ℕ) (h : 1 + a > 0) : (1 + a)^n ≥ 1 + n * a := by
  induction' n with n ih
  · simp -- Base case: when n = 0, the inequality simplifies to 1 ≥ 1, which is true.
  · cases n with
    | zero =>
      simp -- Base case: when n = 1, the inequality simplifies to 1 + a ≥ 1 + a, which is true.
    | succ n =>
      simp_all [pow_succ, mul_add, mul_one, mul_comm, mul_left_comm]
      -- Inductive step: Assume the inequality holds for n, prove it for n + 1.
      -- Use the fact that (1 + a)^(n + 1) = (1 + a) * (1 + a)^n and the inductive hypothesis.
      nlinarith [sq_nonneg a, sq_nonneg (a + 1), sq_nonneg (a - 1), h, sq_nonneg (a * n)]
```

### Explanation

1. **Base Case (`n = 0`)**:
   - When `n = 0`, the inequality simplifies to `1 ≥ 1`, which is trivially true.

2. **Base Case (`n = 1`)**:
   - When `n = 1`, the inequality simplifies to `1 + a ≥ 1 + a`, which is also trivially true.

3. **Inductive Step**:
   - Assume the inequality holds for `n`, i.e., `(1 + a)^n ≥ 1 + n * a`.
   - We need to prove it for `n + 1`, i.e., `(1 + a)^(n + 1) ≥ 1 + (n + 1) * a`.
   - Expand `(1 + a)^(n + 1) = (1 + a) * (1 + a)^n`.
   - Using the inductive hypothesis, `(1 + a)^n ≥ 1 + n * a`, we get:
     ```
     (1 + a)^(n + 1) = (1 + a) * (1 + a)^n ≥ (1 + a) * (1 + n * a)
     = 1 + n * a + a + n * a^2
     = 1 + (n + 1) * a + n * a^2
     ```
   - Since `n * a^2 ≥ 0` (as `a^2 ≥ 0` and `n ≥ 0`), we have:
     ```
     1 + (n + 1) * a + n * a^2 ≥ 1 + (n + 1) * a
     ```
   - Thus, `(1 + a)^(n + 1) ≥ 1 + (n + 1) * a`.

### Normal Language Explanation

The Bernoulli inequality is a classic result in algebra and number theory. It states that for any real number `a` such that `1 + a > 0` and any non-negative integer `n`, the following inequality holds:

$$(1 + a)^n \geq 1 + n a$$

The proof proceeds by induction on `n`.

1. **Base Case (`n = 0`)**:
   - The inequality simplifies to `1 ≥ 1`, which is trivially true.

2. **Base Case (`n = 1`)**:
   - The inequality simplifies to `1 + a ≥ 1 + a`, which is also trivially true.

3. **Inductive Step**:
   - Assume the inequality holds for `n`, i.e., `(1 + a)^n ≥ 1 + n a`.
   - We need to prove it for `n + 1`, i.e., `(1 + a)^(n + 1) ≥ 1 + (n + 1) a`.
   - Expand `(1 + a)^(n + 1) = (1 + a) * (1 + a)^n` and use the inductive hypothesis.
   - Multiply both sides of the inductive hypothesis by `(1 + a)`:
     ```
     (1 + a) * (1 + a)^n ≥ (1 + a) * (1 + n a)
     ```
   - Simplify the right-hand side:
     ```
     (1 + a) * (1 + n a) = 1 + n a + a + n a^2 = 1 + (n + 1) a + n a^2
     ```
   - Since `n a^2 ≥ 0`, we have:
     ```
     1 + (n + 1) a + n a^2 ≥ 1 + (n + 1) a
     ```
   - Thus, `(1 + a)^(n + 1) ≥ 1 + (n + 1) a`, completing the inductive step.

The Lean4 proof uses `nlinarith` to handle the algebraic manipulations and inequalities, leveraging the fact that `a^2 ≥ 0` and the given condition `1 + a > 0`.