### Part (a): Prove that $\binom{n}{r} < \binom{n}{r+1}$ if and only if $0 \leq r < \frac{1}{2}(n - 1)$

**Lean4 Proof Sketch:**
```lean4
theorem part_a (n : ℕ) (r : ℕ) (hn : n ≥ 1) : 
  (Nat.choose n r < Nat.choose n (r + 1)) ↔ (0 ≤ r ∧ r < (n - 1) / 2) := by
  have h₁ : Nat.choose n r < Nat.choose n (r + 1) ↔ 0 ≤ r ∧ r < (n - 1) / 2 := by
    constructor
    · intro h
      have h₁ : r < n - 1 := by
        by_contra h₂
        have h₃ : r ≥ n - 1 := by omega
        have h₄ : Nat.choose n r ≥ Nat.choose n (r + 1) := by
          -- Use the fact that binomial coefficients are decreasing after the peak
          have h₅ : r ≥ n - 1 := by omega
          have h₆ : Nat.choose n r ≥ Nat.choose n (r + 1) := by
            cases n with
            | zero => contradiction -- n ≥ 1
            | succ n =>
              cases r with
              | zero => simp_all [Nat.choose_succ_succ, Nat.choose_zero_right]
              | succ r =>
                simp_all [Nat.choose_succ_succ, Nat.choose_zero_right]
                <;> omega
          exact h₆
        omega
      have h₂ : 0 ≤ r := by omega
      have h₃ : r < (n - 1) / 2 := by
        by_contra h₄
        have h₅ : r ≥ (n - 1) / 2 := by omega
        have h₆ : Nat.choose n r ≥ Nat.choose n (r + 1) := by
          -- Use the fact that binomial coefficients are decreasing after the peak
          have h₇ : r ≥ (n - 1) / 2 := by omega
          have h₈ : Nat.choose n r ≥ Nat.choose n (r + 1) := by
            cases n with
            | zero => contradiction -- n ≥ 1
            | succ n =>
              cases r with
              | zero => simp_all [Nat.choose_succ_succ, Nat.choose_zero_right]
              | succ r =>
                simp_all [Nat.choose_succ_succ, Nat.choose_zero_right]
                <;> omega
          exact h₈
        omega
      exact ⟨h₂, h₃⟩
    · intro h
      have h₁ : 0 ≤ r := h.1
      have h₂ : r < (n - 1) / 2 := h.2
      have h₃ : r < n - 1 := by
        omega
      have h₄ : Nat.choose n r < Nat.choose n (r + 1) := by
        -- Use the fact that binomial coefficients are increasing before the peak
        cases n with
        | zero => contradiction -- n ≥ 1
        | succ n =>
          cases r with
          | zero => simp_all [Nat.choose_succ_succ, Nat.choose_zero_right]
          | succ r =>
            simp_all [Nat.choose_succ_succ, Nat.choose_zero_right]
            <;> omega
      exact h₄
  exact h₁
```

### Part (b): Prove that $\binom{n}{r} > \binom{n}{r+1}$ if and only if $n - 1 \geq r > \frac{1}{2}(n - 1)$

**Lean4 Proof Sketch:**
```lean4
theorem part_b (n : ℕ) (r : ℕ) (hn : n ≥ 1) : 
  (Nat.choose n r > Nat.choose n (r + 1)) ↔ (n - 1 ≥ r ∧ r > (n - 1) / 2) := by
  have h₁ : Nat.choose n r > Nat.choose n (r + 1) ↔ n - 1 ≥ r ∧ r > (n - 1) / 2 := by
    constructor
    · intro h
      have h₁ : r < n - 1 := by
        by_contra h₂
        have h₃ : r ≥ n - 1 := by omega
        have h₄ : Nat.choose n r ≤ Nat.choose n (r + 1) := by
          -- Use the fact that binomial coefficients are decreasing after the peak
          have h₅ : r ≥ n - 1 := by omega
          have h₆ : Nat.choose n r ≤ Nat.choose n (r + 1) := by
            cases n with
            | zero => contradiction -- n ≥ 1
            | succ n =>
              cases r with
              | zero => simp_all [Nat.choose_succ_succ, Nat.choose_zero_right]
              | succ r =>
                simp_all [Nat.choose_succ_succ, Nat.choose_zero_right]
                <;> omega
          exact h₆
        omega
      have h₂ : n - 1 ≥ r := by omega
      have h₃ : r > (n - 1) / 2 := by
        by_contra h₄
        have h₅ : r ≤ (n - 1) / 2 := by omega
        have h₆ : Nat.choose n r ≥ Nat.choose n (r + 1) := by
          -- Use the fact that binomial coefficients are decreasing after the peak
          have h₇ : r ≤ (n - 1) / 2 := by omega
          have h₈ : Nat.choose n r ≥ Nat.choose n (r + 1) := by
            cases n with
            | zero => contradiction -- n ≥ 1
            | succ n =>
              cases r with
              | zero => simp_all [Nat.choose_succ_succ, Nat.choose_zero_right]
              | succ r =>
                simp_all [Nat.choose_succ_succ, Nat.choose_zero_right]
                <;> omega
          exact h₈
        omega
      exact ⟨h₂, h₃⟩
    · intro h
      have h₁ : n - 1 ≥ r := h.1
      have h₂ : r > (n - 1) / 2 := h.2
      have h₃ : r < n - 1 := by
        omega
      have h₄ : Nat.choose n r > Nat.choose n (r + 1) := by
        -- Use the fact that binomial coefficients are increasing before the peak
        cases n with
        | zero => contradiction -- n ≥ 1
        | succ n =>
          cases r with
          | zero => simp_all [Nat.choose_succ_succ, Nat.choose_zero_right]
          | succ r =>
            simp_all [Nat.choose_succ_succ, Nat.choose_zero_right]
            <;> omega
      exact h₄
  exact h₁
```

### Part (c): Prove that $\binom{n}{r} = \binom{n}{r+1}$ if and only if $n$ is an odd integer, and $r = \frac{1}{2}(n -1)$

**Lean4 Proof Sketch:**
```lean4
theorem part_c (n : ℕ) (r : ℕ) (hn : n ≥ 1) : 
  (Nat.choose n r = Nat.choose n (r + 1)) ↔ (n % 2 = 1 ∧ r = (n - 1) / 2) := by
  have h₁ : Nat.choose n r = Nat.choose n (r + 1) ↔ n % 2 = 1 ∧ r = (n - 1) / 2 := by
    constructor
    · intro h
      have h₁ : r < n := by
        by_contra h₂
        have h₃ : r ≥ n := by omega
        have h₄ : Nat.choose n r = 0 := by
          apply Nat.choose_eq_zero_of_lt
          omega
        have h₅ : Nat.choose n (r + 1) = 0 := by
          apply Nat.choose_eq_zero_of_lt
          omega
        simp_all
      have h₂ : r ≤ n - 1 := by omega
      have h₃ : n % 2 = 1 ∧ r = (