### Lean4 Proof

```lean4
theorem sum_of_odd_squares (n : ℕ) (hn : n ≥ 1) : 
    ∑ k in Finset.range n, (2 * k + 1)^2 = (2 * n + 1).choose 3 := by
  have h : ∀ n : ℕ, n ≥ 1 → ∑ k in Finset.range n, (2 * k + 1)^2 = (2 * n + 1).choose 3 := by
    intro n hn
    induction' hn with n hn
    · norm_num [Nat.choose_succ_succ]
    · cases n with
      | zero =>
        norm_num [Nat.choose_succ_succ]
      | succ n =>
        simp_all [Finset.sum_range_succ, Nat.choose_succ_succ, Nat.mul_add, Nat.add_mul, Nat.pow_succ]
        all_goals ring_nf at *
        <;> omega
  apply h
  exact hn
```

### Explanation

1. **Base Case (`n = 1`)**:
   - For `n = 1`, the sum is `1^2 = 1`.
   - The binomial coefficient is `(2*1 + 1) choose 3 = 3 choose 3 = 1`.
   - Thus, the base case holds.

2. **Inductive Step**:
   - Assume the statement holds for some `n ≥ 1`, i.e., `∑ k in Finset.range n, (2 * k + 1)^2 = (2 * n + 1).choose 3`.
   - For `n + 1`, the sum becomes `∑ k in Finset.range (n + 1), (2 * k + 1)^2 = ∑ k in Finset.range n, (2 * k + 1)^2 + (2 * n + 1)^2`.
   - By the induction hypothesis, this equals `(2 * n + 1).choose 3 + (2 * n + 1)^2`.
   - We need to show that this equals `(2 * (n + 1) + 1).choose 3 = (2 * n + 3).choose 3`.
   - Using the recursive definition of binomial coefficients and algebraic manipulation, we can verify this equality.

### Normal Language Explanation

The proof involves verifying the identity for the sum of squares of odd numbers up to `(2n - 1)^2` and showing it equals the binomial coefficient `(2n + 1 choose 3)`.

1. **Base Case**:
   - For `n = 1`, the sum is `1^2 = 1` and the binomial coefficient is `3 choose 3 = 1`, so they match.

2. **Inductive Step**:
   - Assume the identity holds for `n`.
   - For `n + 1`, the sum becomes the previous sum plus the next odd square `(2n + 1)^2`.
   - Use the recursive definition of binomial coefficients and algebraic identities to show the new sum equals the new binomial coefficient.

This completes the proof by induction.