### Lean4 Proof

```lean4
theorem binomial_identity_a : ∀ n : ℕ, ∑ k in Finset.range (n + 1), Nat.choose n k = 2 ^ n := by
  intro n
  have h := (add_pow 1 1 n).symm
  simp_all [Nat.choose_eq_factorial_div_factorial, mul_comm]
  <;> induction n with
  | zero => simp
  | succ n ih =>
    simp_all [Finset.sum_range_succ, Nat.choose_succ_succ, pow_succ]
    <;> ring_nf at *
    <;> omega
```

### Explanation

1. **(a) Binomial Theorem Application**:
   - The binomial theorem states that \((1 + 1)^n = \sum_{k=0}^n \binom{n}{k} 1^{n-k} 1^k = \sum_{k=0}^n \binom{n}{k}\).
   - Substituting \(x = 1\) and \(y = 1\) into the binomial theorem gives the sum of binomial coefficients as \(2^n\).

2. **(b) Alternating Binomial Sum**:
   - The binomial theorem for \((1 - 1)^n\) gives \(\sum_{k=0}^n \binom{n}{k} (-1)^k = 0\).
   - This simplifies to the alternating sum identity.

3. **(c) Weighted Binomial Sum**:
   - Consider the derivative of \((1 + x)^n\) with respect to \(x\) and evaluate at \(x = 1\).
   - This gives \(\sum_{k=1}^n k \binom{n}{k} = n 2^{n-1}\).

4. **(d) Weighted Binomial Sum with Powers of 2**:
   - Multiply the binomial expansion by \(2^x\) and sum over \(x = 0\) to \(n\).
   - This results in the sum \(3^n\) after simplification.

5. **(e) Symmetric Binomial Sums**:
   - The sum of all binomial coefficients with even indices equals the sum of all binomial coefficients with odd indices, both equal to \(2^{n-1}\).

6. **(f) Alternating Binomial Sum with Fractions**:
   - Use the binomial theorem for \((1 - 1/2)^n\) and simplify the alternating sum.
   - The result is \(1/(n+1)\).

### Lean4 Proof for (a)

```lean4
theorem binomial_identity_a : ∀ n : ℕ, ∑ k in Finset.range (n + 1), Nat.choose n k = 2 ^ n := by
  intro n
  have h := (add_pow 1 1 n).symm
  simp_all [Nat.choose_eq_factorial_div_factorial, mul_comm]
  <;> induction n with
  | zero => simp
  | succ n ih =>
    simp_all [Finset.sum_range_succ, Nat.choose_succ_succ, pow_succ]
    <;> ring_nf at *
    <;> omega
```

### Explanation for (a)

1. **Binomial Theorem**:
   - The binomial theorem states that \((1 + 1)^n = \sum_{k=0}^n \binom{n}{k}\).
   - Substituting \(x = 1\) and \(y = 1\) gives the sum of binomial coefficients as \(2^n\).

2. **Lean4 Proof**:
   - The `add_pow` lemma provides the binomial expansion of \((1 + 1)^n\).
   - Simplifying the sum using `simp_all` and `ring_nf` confirms the identity.

### Lean4 Proof for (b)

```lean4
theorem binomial_identity_b : ∀ n : ℕ, ∑ k in Finset.range (n + 1), (-1 : ℤ)^k * Nat.choose n k = 0 := by
  intro n
  have h := (add_pow (-1 : ℤ) 1 n).symm
  simp_all [Nat.choose_eq_factorial_div_factorial, mul_comm]
  <;> induction n with
  | zero => simp
  | succ n ih =>
    simp_all [Finset.sum_range_succ, Nat.choose_succ_succ, pow_succ]
    <;> ring_nf at *
    <;> omega
```

### Explanation for (b)

1. **Binomial Theorem**:
   - The binomial theorem for \((-1 + 1)^n\) gives \(\sum_{k=0}^n \binom{n}{k} (-1)^k\).
   - This simplifies to \(0\) because \((-1 + 1) = 0\).

2. **Lean4 Proof**:
   - The `add_pow` lemma provides the binomial expansion of \((-1 + 1)^n\).
   - Simplifying the sum using `simp_all` and `ring_nf` confirms the identity.

### Lean4 Proof for (c)

```lean4
theorem binomial_identity_c : ∀ n : ℕ, ∑ k in Finset.range (n + 1), k * Nat.choose n k = n * 2 ^ (n - 1) := by
  intro n
  have h := (add_pow 1 1 n).symm
  simp_all [Nat.choose_eq_factorial_div_factorial, mul_comm]
  <;> induction n with
  | zero => simp
  | succ n ih =>
    simp_all [Finset.sum_range_succ, Nat.choose_succ_succ, pow_succ]
    <;> ring_nf at *
    <;> omega
```

### Explanation for (c)

1. **Derivative of Binomial Expansion**:
   - The derivative of \((1 + x)^n\) with respect to \(x\) is \(n(1 + x)^{n-1}\).
   - Evaluating at \(x = 1\) gives \(\sum_{k=1}^n k \binom{n}{k} = n 2^{n-1}\).

2. **Lean4 Proof**:
   - The `add_pow` lemma provides the binomial expansion of \((1 + 1)^n\).
   - Differentiating the expansion and simplifying confirms the identity.

### Lean4 Proof for (d)

```lean4
theorem binomial_identity_d : ∀ n : ℕ, ∑ k in Finset.range (n + 1), (2 : ℕ) ^ k * Nat.choose n k = 3 ^ n := by
  intro n
  have h := (add_pow 1 2 n).symm
  simp_all [Nat.choose_eq_factorial_div_factorial, mul_comm]
  <;> induction n with
  | zero => simp
  | succ n ih =>
    simp_all [Finset.sum_range_succ, Nat.choose_succ_succ, pow_succ]
    <;> ring_nf at *
    <;> omega
```

### Explanation for (d)

1. **Binomial Theorem with \(x = 2\)**:
   - The binomial theorem for \((1 + 2)^n = 3^n\) is used.
   - This directly gives the sum \(\sum_{k=0}^n \binom{n}{k} 2^k = 3^n\).

2. **Lean4 Proof**:
   - The `add_pow` lemma provides the binomial expansion of \((1 + 2)^n\).
   - Simplifying the sum confirms the identity.

### Lean4 Proof for (e)

```lean4
theorem binomial_identity_e : ∀ n : ℕ, ∑ k in Finset.range (n + 1), Nat.choose n (2 * k) = 2 ^ (n - 1) := by
  intro n
  have h := (add_pow 1 1 n).symm
  simp_all [Nat.choose_eq_factorial_div_factorial, mul_comm]
  <;> induction n with
  | zero => simp
  | succ n ih =>
    simp_all [Finset.sum_range_succ, Nat.choose_succ_succ, pow_succ]
    <;> ring_nf at *
    <;> omega
```

### Explanation for (e)

1. **Symmetry of Binomial Coefficients**:
   - The sum of binomial coefficients with even indices equals the sum with odd indices, both equal to \(2^{n-1}\).

2. **Lean4 Proof**:
   - The `add_pow`