<think>
Okay, so I need to figure out how to represent the primes 23, 29, 31, and 37 using these formulas given. Let me start by understanding the problem again.

The sequence of primes with 1 adjoined is p₀=1, p₁=2, p₂=3, p₃=5, etc. For each n ≥ 1, there's a way to write p_{2n} and p_{2n+1} as combinations of previous primes with coefficients ±1. The examples given are:

For p₄ = 13, it's written as 1 + 2 - 3 - 5 + 7 + 11. Let me check that: 1 + 2 is 3, minus 3 is 0, minus 5 is -5, plus 7 is 2, plus 11 is 13. Yep, that works.

Similarly, p₅ = 17 is 1 + 2 - 3 - 5 + 7 - 11 + 2*13. Let's compute that: 1+2=3, -3=0, -5=-5, +7=2, -11=-9, +2*13=26. So total is -9 +26=17. Correct.

So the pattern seems to be that for even indices (2n), we have p_{2n} = p_{2n-1} + sum_{k=0}^{2n-2} ε_k p_k. Wait, no, the problem says:

For each n ≥ 1, there exists coefficients ε_k = ±1 such that:

p_{2n} = p_{2n - l} + sum_{k=0}^{2n - 2} ε_k p_k

Wait, but in the example for p₄ (which is 13, n=2?), maybe I need to check the indices.

Wait, the problem says for each n ≥ 1, so for p_{2n} and p_{2n+1}. Let me check the example:

For p_4 = 13, which is p_{2n} where n=2? Then p_{2n} = p_{2n - l} + ...? Wait, the original problem says:

"For each n ≥ 1, it is known that there exists a suitable choice of coefficients ε_k = ±1 such that p_{2n} = p_{2n - l} + sum_{k=0}^{2n - 2} ε_k p_k and p_{2n + 1} = 2p_{2n} + sum_{k=0}^{2n - 1} ε_k p_k"

Wait, but in the example for p_4 = 13, which is p_{2n} where n=2? Then the formula would be p_{2n} = p_{2n - l} + sum... but the example shows p_4 = 1 + 2 - 3 - 5 + 7 + 11. Let me check the indices here. The primes up to p_4 (which is 13) are p0=1, p1=2, p2=3, p3=5, p4=7, p5=11, p6=13? Wait no, p0=1, p1=2, p2=3, p3=5, p4=7, p5=11, p6=13. Wait, but in the example, they have 1 + 2 - 3 - 5 + 7 + 11. That's p0 + p1 - p2 - p3 + p4 + p5. So that's sum_{k=0}^5 ε_k p_k? But the formula says for p_{2n} = p_{2n - l} + sum_{k=0}^{2n - 2} ε_k p_k. Wait, maybe there's a typo in my understanding? Let me check again.

The problem says:

For each n ≥ 1, there exists coefficients ε_k = ±1 such that

p_{2n} = p_{2n - l} + sum_{k=0}^{2n - 2} ε_k p_k

and

p_{2n + 1} = 2p_{2n} + sum_{k=0}^{2n - 1} ε_k p_k

Wait, but in the example for p_4 = 13, which is p_{2n} where n=2? Then 2n=4, so the formula would be p_4 = p_{4 - l} + sum_{k=0}^{4 - 2} ε_k p_k. Wait, 4 - 2 is 2, so sum from k=0 to 2? But in the example, the sum goes up to p5 (which is k=5). So maybe there's a misunderstanding here.

Alternatively, maybe the formula is written with a typo, or maybe l is a typo? Wait, the original problem says:

"For each n ≥ 1, it is known that there exists a suitable choice of coefficients ε_k = ±1 such that p_{2n} = p_{2n - l} + sum_{k=0}^{2n - 2} ε_k p_k and p_{2n + 1} = 2p_{2n} + sum_{k=0}^{2n - 1} ε_k p_k"

But in the example for p_4 = 13, the formula is written as p_4 = 1 + 2 - 3 - 5 + 7 + 11. Let's check the indices here. The primes used are p0=1, p1=2, p2=3, p3=5, p4=7, p5=11. So the sum is from k=0 to 5, which is 2n - 2? If 2n is 4, then 2n - 2 = 2. But the sum goes up to k=5. That doesn't match. Alternatively, maybe the formula is different. Wait, maybe the original problem had a different index? Maybe the formula is p_{2n} = p_{something} + sum...?

Alternatively, maybe the formula is p_{2n} = p_{2n - 1} + sum_{k=0}^{2n - 2} ε_k p_k? Let me check with the example.

For p_4 = 13, if n=2, then p_{2n} = p_{2n - 1} + sum... So p_4 = p_3 + sum... p_3 is 5. Then 5 + sum... Let's see, the example is 1 + 2 - 3 - 5 + 7 + 11. If we subtract p_3 (which is 5) from that, we get 1 + 2 - 3 - 5 + 7 + 11 - 5 = 1 + 2 -3 -5 +7 +11 -5 = 1 + 2 -3 is 0, -5 is -5, +7 is 2, +11 is 13, -5 is 8. That's not 13. So that doesn't work.

Alternatively, maybe the formula is p_{2n} = p_{something else} + sum... Maybe the example is p_4 = p_1 + sum...? Let me check. If p_1 is 2, then 2 + sum... The example is 1 + 2 - 3 - 5 + 7 + 11. If that sum is 1 + 2 - 3 - 5 + 7 + 11, then that equals 13. But according to the formula, p_4 should be equal to p_{something} plus that sum. Wait, but in the example, they just have the sum. Maybe the formula is p_{2n} = sum_{k=0}^{2n - 2} ε_k p_k + p_{something}? Maybe the original problem had a different index. Alternatively, maybe the formula is p_{2n} = p_{2n - 1} + sum_{k=0}^{2n - 2} ε_k p_k? Let me check with the example.

For p_4, which is 13. If p_{2n - 1} is p_3 = 5. Then 5 + sum_{k=0}^{2n - 2} ε_k p_k. Here, 2n - 2 is 2, so sum from k=0 to 2. But in the example, the sum is up to p5. So that doesn't match. Maybe the formula is different. Alternatively, maybe there's a typo in the problem statement, and the formula is supposed to be p_{2n} = sum_{k=0}^{2n - 1} ε_k p_k + something? Wait, the example for p_4 is written as 1 + 2 - 3 - 5 + 7 + 11. Let me count the number of terms. From p0 to p5, that's 6 terms. So maybe for p_{2n}, the sum is up to p_{2n - 1}? For p_4, which is 2n=4, then 2n - 1 = 3. But the example goes up to p5. Hmm, not sure.

Wait, maybe the formula is p_{2n} = p_{2n - 1} + sum_{k=0}^{2n - 2} ε_k p_k. Then, for p_4, which is 13, p_{2n - 1} is p_3 = 5. Then the sum from k=0 to 2n - 2 = 2, so sum from k=0 to 2: ε0 p0 + ε1 p1 + ε2 p2. Then 5 + (ε0*1 + ε1*2 + ε2*3) = 13. So that would mean ε0*1 + ε1*2 + ε2*3 = 8. Let's see if that's possible. Let me try ε0=1, ε1=1, ε2=1: 1 + 2 + 3 = 6. Not enough. ε0=1, ε1=1, ε2=-1: 1 + 2 -3 = 0. No. ε0=1, ε1=-1, ε2=1: 1 -2 +3 = 2. No. ε0=-1, ε1=1, ε2=1: -1 +2 +3=4. No. ε0=1, ε1=-1, ε2=-1: 1 -2 -3 = -4. No. ε0=-1, ε1=-1, ε2=1: -1 -2 +3=0. Not helpful. Hmm, maybe this is not the correct formula.

Alternatively, maybe the formula is p_{2n} = sum_{k=0}^{2n - 1} ε_k p_k. But in the example, the sum is 1 + 2 -3 -5 +7 +11 = 13, which is p_4. But p_4 is 7, not 13. Wait, no, p_4 is 7? Wait, no, the primes are p0=1, p1=2, p2=3, p3=5, p4=7, p5=11, p6=13. So p_4 is 7, but the example is for p_4=13? Wait, no. Wait, the example says 13 = 1 + 2 - 3 - 5 + 7 + 11. Let me check which prime is 13. p6=13. So maybe the formula is for p_{2n} where 2n=6? Then n=3. Then p_{2n} = p_{something} + sum... So maybe the formula is p_{2n} = p_{2n - l} + sum...? But in the example, p_6=13 is expressed as 1 + 2 -3 -5 +7 +11. So that's sum_{k=0}^5 ε_k p_k. So maybe the formula is p_{2n} = sum_{k=0}^{2n - 1} ε_k p_k? But then for p_6, which is 13, that would be sum from k=0 to 5. But in the example, that sum is 1 + 2 -3 -5 +7 +11 = 13. So that works. Then for p_5=17, which is p_{2n +1} where n=2? Because 2n +1=5. So p_5=17=2p_4 + sum_{k=0}^{2n -1} ε_k p_k. For n=2, 2n -1=3. So sum from k=0 to 3. But in the example, the sum is 1 + 2 -3 -5 +7 -11 + 2*13. Wait, the example for p_5 is 1 + 2 -3 -5 +7 -11 + 2*13. So that's 2p_4 + sum_{k=0}^5 ε_k p_k? Wait, maybe the formula is p_{2n +1} = 2p_{2n} + sum_{k=0}^{2n} ε_k p_k. Then for p_5=17, which is 2p_4 + sum_{k=0}^4 ε_k p_k. But in the example, they have 2*13 + sum... Let me check: 2*13 is 26. The example is 1 + 2 -3 -5 +7 -11 + 2*13. So that sum is 1 + 2 -3 -5 +7 -11 = (1+2) -3 -5 +7 -11 = 3 -3 -5 +7 -11 = 0 -5 +7 -11 = 2 -11 = -9. Then -9 + 26 = 17. So that works. But according to the formula, p_{2n +1} = 2p_{2n} + sum_{k=0}^{2n} ε_k p_k. For n=2, 2n=4, so sum from k=0 to 4. But in the example, the sum is up to k=5? Wait, in the example, the sum is 1 + 2 -3 -5 +7 -11. That is up to p5? Wait, p0 to p5? Wait, p0=1, p1=2, p2=3, p3=5, p4=7, p5=11. So sum from k=0 to 5 would be 1 + 2 -3 -5 +7 +11 = 13. But in the example, the sum is up to p5? But the formula says for p_{2n +1} = 2p_{2n} + sum_{k=0}^{2n} ε_k p_k. For n=2, 2n=4, so sum from k=0 to 4. Which would be up to p4=7. But the example has sum up to p5=11. So that seems conflicting.

Wait, maybe there's a misunderstanding in the problem statement. Let me recheck the problem statement:

"For each n ≥ 1, it is known that there exists a suitable choice of coefficients ε_k = ±1 such that p_{2n} = p_{2n - l} + sum_{k=0}^{2n - 2} ε_k p_k and p_{2n + 1} = 2p_{2n} + sum_{k=0}^{2n - 1} ε_k p_k"

But in the example, for p_4 = 13, which is p_{2n} where n=2, then according to the formula, it should be p_{2n} = p_{2n - l} + sum_{k=0}^{2n - 2} ε_k p_k. So for n=2, 2n=4, so p_4 = p_{4 - l} + sum_{k=0}^{2} ε_k p_k. But in the example, the sum is up to p5. So maybe there's a typo in the problem statement? Alternatively, maybe "l" is a misprint, and it's supposed to be "something else". Alternatively, maybe the formula is p_{2n} = p_{2n - 1} + sum_{k=0}^{2n - 2} ε_k p_k? Let me check with the example.

For p_4 = 13, which is p_{2n} where n=2. Then p_{2n -1} is p_3 = 5. Then sum from k=0 to 2n -2 = 2. So sum from k=0 to 2. So 5 + (ε0*1 + ε1*2 + ε2*3) = 13. Then ε0*1 + ε1*2 + ε2*3 = 8. Let me see if that's possible. Let me try different combinations:

If ε0=1, ε1=1, ε2=1: 1 + 2 + 3 = 6. Not enough.

If ε0=1, ε1=1, ε2= -1: 1 + 2 -3 = 0.

ε0=1, ε1=-1, ε2=1: 1 -2 +3=2.

ε0=1, ε1=-1, ε2=-1: 1 -2 -3= -4.

ε0=-1, ε1=1, ε2=1: -1 +2 +3=4.

ε0=-1, ε1=1, ε2=-1: -1 +2 -3= -2.

ε0=-1, ε1=-1, ε2=1: -1 -2 +3=0.

ε0=-1, ε1=-1, ε2=-1: -1 -2 -3=-6.

Hmm, none of these give 8. So that can't be right. Therefore, maybe the formula is different. Alternatively, maybe the formula is p_{2n} = sum_{k=0}^{2n - 1} ε_k p_k. For p_4=7, that would be sum up to p3=5. But in the example, it's for p_6=13. So maybe the formula is for p_{2n} where 2n is the index? For example, in the example, p_6=13 is written as sum_{k=0}^5 ε_k p_k. So maybe the formula is p_{2n} = sum_{k=0}^{2n - 1} ε_k p_k. Then for p_6, 2n=6, so sum from k=0 to 5. That works. Then for p_5=17, which is p_{2n +1} where n=2, so 2n +1=5. Then according to the other formula, p_{2n +1} = 2p_{2n} + sum_{k=0}^{2n -1} ε_k p_k. For n=2, 2n=4, so sum from k=0 to 3. Let me check the example: p_5=17=2p_4 + sum_{k=0}^3 ε_k p_k. p_4=7, so 2*7=14. Then sum_{k=0}^3 ε_k p_k = 17 -14=3. So we need to find ε0, ε1, ε2, ε3 such that ε0*1 + ε1*2 + ε2*3 + ε3*5 = 3. Let me try:

Possible combinations. For example, ε0=1, ε1=1, ε2=1, ε3=-1: 1 +2 +3 -5=1. No. ε0=1, ε1=1, ε2=-1, ε3=1: 1+2-3+5=5. No. ε0=1, ε1=-1, ε2=1, ε3=1: 1 -2 +3 +5=7. No. ε0=-1, ε1=1, ε2=1, ε3=1: -1 +2 +3 +5=9. No. ε0=1, ε1=1, ε2=1, ε3=0? Wait, but ε_k must be ±1. Maybe ε0=1, ε1=1, ε2=-1, ε3=1: 1 +2 -3 +5=5. Not 3. ε0=1, ε1=1, ε2= -1, ε3= -1: 1 +2 -3 -5 = -5. No. ε0=1, ε1=-1, ε2=1, ε3=-1: 1 -2 +3 -5 = -3. Close. ε0=1, ε1=-1, ε2=-1, ε3=1: 1 -2 -3 +5=1. Hmm. Maybe ε0=1, ε1=1, ε2= -1, ε3= -1: 1 +2 -3 -5 = -5. Not helpful. Wait, maybe there's a mistake here. Alternatively, maybe the formula is different. The example for p_5 is 1 + 2 - 3 - 5 + 7 - 11 + 2*13. Wait, that seems like 2*13 is 2p_6, but p_6 is 13. But according to the formula, p_{2n +1} = 2p_{2n} + sum... So for p_5=17, which is 2p_4 + sum... So 2*7 + sum... which is 14 + sum... = 17, so sum is 3. But in the example, they have 1 + 2 -3 -5 +7 -11 + 2*13. Wait, that seems like they are using p_0 to p_5 and then 2*p_6. So maybe the formula is p_{2n +1} = 2p_{2n} + sum_{k=0}^{2n} ε_k p_k. Then for n=2, 2n=4, so sum from k=0 to 4. So sum_{k=0}^4 ε_k p_k. Let me check:

In the example, the sum is 1 + 2 -3 -5 +7 -11. Wait, that's up to p5? Wait, p0 to p5 is 1,2,3,5,7,11. But if the formula is sum_{k=0}^4 ε_k p_k, that would be up to p4=7. So the example has an extra term -11. That seems inconsistent. Maybe the example is wrong? Or maybe the formula is different.

Alternatively, maybe the formula is p_{2n} = p_{2n - 1} + sum_{k=0}^{2n - 2} ε_k p_k. Then for p_4=13, p_{2n -1}=p_3=5. Then sum from k=0 to 2n-2=2. So 5 + (ε0*1 + ε1*2 + ε2*3) = 13. So the sum is 8. As before, but we couldn't find such coefficients. Maybe there's another way? Let me try again.

Let me think of possible combinations for 8. Since the primes are 1, 2, 3. The coefficients are ±1. So possible values:

Let me think of equations:

Let me denote x = ε0*1 + ε1*2 + ε2*3 = 8.

Possible values for ε0, ε1, ε2 are ±1.

So possible combinations:

Let me try all possibilities. There are 2^3 = 8 possibilities.

Case 1: ε0=1, ε1=1, ε2=1: 1 + 2 + 3 = 6

Case 2: ε0=1, ε1=1, ε2=-1: 1 + 2 - 3 = 0

Case 3: ε0=1, ε1=-1, ε2=1: 1 - 2 + 3 = 2

Case 4: ε0=1, ε1=-1, ε2=-1: 1 - 2 - 3 = -4

Case 5: ε0=-1, ε1=1, ε2=1: -1 + 2 + 3 = 4

Case 6: ε0=-1, ε1=1, ε2=-1: -1 + 2 - 3 = -2

Case 7: ε0=-1, ε1=-1, ε2=1: -1 - 2 + 3 = 0

Case 8: ε0=-1, ε1=-1, ε2=-1: -1 - 2 - 3 = -6

None of these give 8. So that can't be right. Therefore, the formula must be different.

Alternatively, maybe the formula is p_{2n} = sum_{k=0}^{2n - 1} ε_k p_k. Then for p_4=7, which is p_4, the sum would be up to k=3 (p3=5). Let me check if that's possible. For example, sum_{k=0}^3 ε_k p_k = 7. So 1 + 2 + 3 + 5 = 11, but with ±1 coefficients. Let's try:

Looking for ε0*1 + ε1*2 + ε2*3 + ε3*5 = 7.

Let me think. Let's try ε0=1, ε1=1, ε2=1, ε3=1: 1 + 2 + 3 + 5 = 11. Too big.

If I flip one sign: ε0=1, ε1=1, ε2=1, ε3=-1: 1 + 2 + 3 -5 = 1. No.

ε0=1, ε1=1, ε2=-1, ε3=1: 1 + 2 -3 +5 = 5.

ε0=1, ε1=-1, ε2=1, ε3=1: 1 -2 +3 +5 = 7. Oh! That works! So ε0=1, ε1=-1, ε2=1, ε3=1. So sum is 1 -2 +3 +5 = 7. So p_4=7 can be written as 1 -2 +3 +5. But in the example, p_4 is 13, which is p_6. So maybe the formula is for p_{2n} where n is such that 2n is the index. For example, p_6=13 is written as sum_{k=0}^5 ε_k p_k. So maybe the formula is p_{2n} = sum_{k=0}^{2n -1} ε_k p_k. Then for p_6=13, sum from k=0 to 5: 1 + 2 -3 -5 +7 +11 = 13. Which works. Then for p_5=17, which is p_{2n +1} where n=2, the formula is p_{2n +1} = 2p_{2n} + sum_{k=0}^{2n} ε_k p_k. For n=2, 2n=4, so p_5 = 2p_4 + sum_{k=0}^4 ε_k p_k. p_4=7, so 2*7=14. Then sum_{k=0}^4 ε_k p_k = 17 -14=3. Let me check if that's possible.

So find ε0*1 + ε1*2 + ε2*3 + ε3*5 + ε4*7 = 3.

Let me try different combinations. Let me think of possible values.

Let me try ε0=1, ε1=1, ε2=1, ε3=1, ε4=-1: 1 + 2 + 3 + 5 -7 = 4. Close.

ε0=1, ε1=1, ε2=1, ε3=-1, ε4=1: 1 + 2 + 3 -5 +7 = 8.

ε0=1, ε1=1, ε2=-1, ε3=1, ε4=1: 1 + 2 -3 +5 +7 = 12.

ε0=1, ε1=-1, ε2=1, ε3=1, ε4=1: 1 -2 +3 +5 +7 = 14.

ε0=-1, ε1=1, ε2=1, ε3=1, ε4=1: -1 +2 +3 +5 +7 = 16.

Hmm, not getting 3. Maybe ε0=1, ε1=1, ε2=-1, ε3=-1, ε4=1: 1 + 2 -3 -5 +7 = 2.

Close. ε0=1, ε1=-1, ε2=-1, ε3=-1, ε4=1: 1 -2 -3 -5 +7 = -2.

ε0=1, ε1=1, ε2=-1, ε3=-1, ε4=0? No, ε_k must be ±1.

Wait, maybe ε0=1, ε1=1, ε2=1, ε3=-1, ε4=-1: 1 + 2 + 3 -5 -7 = -6.

No. Hmm. Maybe another approach. Let me think of the equation:

Let me denote S = ε0*1 + ε1*2 + ε2*3 + ε3*5 + ε4*7 = 3.

Let me try to find such coefficients. Let's think of possible combinations. Let me try ε4=1. Then the remaining sum is 3 -7 = -4. So need ε0*1 + ε1*2 + ε2*3 + ε3*5 = -4.

Let me try ε3=-1: then ε0*1 + ε1*2 + ε2*3 = -4 - (-5) = 1. So need 1 + 2ε1 + 3ε2 = 1. So 2ε1 + 3ε2 = 0. Since ε1 and ε2 are ±1.

Possible:

If ε1=1, then 2*1 + 3ε2 = 0 ⇒ 3ε2 = -2 ⇒ no solution.

If ε1=-1, then 2*(-1) + 3ε2 = -2 + 3ε2 = 0 ⇒ 3ε2=2 ⇒ no solution.

So no solution with ε3=-1.

Try ε3=1: then the remaining sum is -4 -5 = -9. So need ε0*1 + ε1*2 + ε2*3 = -9. But the maximum possible is 1 + 2 + 3 = 6, minimum is -6. So impossible.

If ε4=-1: then S = -7 + ... = 3 ⇒ ... = 10. Need ε0*1 + ε1*2 + ε2*3 + ε3*5 = 10. Let's see. The maximum is 1 + 2 + 3 + 5 = 11. So possible.

Let me try ε0=1, ε1=1, ε2=1, ε3=1: 1 + 2 + 3 + 5 = 11. Too big. Need 10. So subtract 1. So maybe flip one sign. For example, ε0=1, ε1=1, ε2=1, ε3=-1: 1 + 2 + 3 -5 = 1. No. ε0=1, ε1=1, ε2=-1, ε3=1: 1 + 2 -3 +5 = 5. Still not. ε0=1, ε1=-1, ε2=1, ε3=1: 1 -2 +3 +5 = 7. ε0=-1, ε1=1, ε2=1, ε3=1: -1 + 2 + 3 + 5 = 9. Close. ε0=-1, ε1=1, ε2=1, ε3=-1: -1 + 2 + 3 -5 = -1. No. ε0=1, ε1=1, ε2=1, ε3=1: 11. If I flip ε3 to -1, it's 1 + 2 + 3 -5 = 1. If I flip ε2 to -1: 1 + 2 -3 +5 = 5. If I flip ε1 to -1: 1 -2 +3 +5 = 7. If I flip ε0 to -1: -1 + 2 + 3 +5 = 9. Not 10. Hmm. What if I flip two signs? For example, ε0=-1, ε1=-1, ε2=1, ε3=1: -1 -2 +3 +5 = 5. Still not. Maybe this isn't working. Maybe there is no solution? But the example says that p_5=17 is expressed as 1 + 2 -3 -5 +7 -11 + 2*13. Wait, that is 2*13 + (sum). Let me check: 2*13 is 26. The sum is 1 + 2 -3 -5 +7 -11 = (1 + 2) -3 -5 +7 -11 = 3 -3 -5 +7 -11 = 0 -5 +7 -11 = 2 -11 = -9. So 26 -9 = 17. But according to the formula, it should be 2p_4 + sum_{k=0}^{2n -1} ε_k p_k. For n=2, 2n -1 = 3. So sum from k=0 to 3. But in the example, the sum goes up to k=5. So there's inconsistency.

Alternatively, maybe the formula is p_{2n +1} = 2p_{2n} + sum_{k=0}^{2n} ε_k p_k. Then for n=2, sum from k=0 to 4. Let's check:

p_5 = 2p_4 + sum_{k=0}^4 ε_k p_k. p_4=7, so 2*7=14. Then sum_{k=0}^4 ε_k p_k = 3. So need ε0*1 + ε1*2 + ε2*3 + ε3*5 + ε4*7 = 3. Which is the same as before. But I couldn't find such coefficients. However, in the example, they have sum up to k=5 (p5=11) with ε5=-1. So maybe the formula is different. Maybe the formula is p_{2n +1} = 2p_{2n} + sum_{k=0}^{2n +1} ε_k p_k? For n=2, that would be sum up to k=5. Then p_5=2*7 + sum_{k=0}^5 ε_k p_k. So 14 + sum = 17 ⇒ sum = 3. But in the example, the sum is 1 + 2 -3 -5 +7 -11 = -9. So 14 + (-9) = 5, not 17. Wait, no, the example says it's 1 + 2 -3 -5 +7 -11 + 2*13. So that is 2*13 + sum... So maybe the formula is p_{2n +1} = 2p_{2n} + sum_{k=0}^{2n} ε_k p_k? For n=2, that would be 2p_4 + sum_{k=0}^4 ε_k p_k. But in the example, they have 2*13 + sum... which is 2p_6. So maybe the formula is for p_{2n +1} = 2p_{2n + something}... This is getting too confusing.

Alternatively, maybe the original problem has a typo, and the formula is p_{2n} = sum_{k=0}^{2n -1} ε_k p_k and p_{2n +1} = 2p_{2n} + sum_{k=0}^{2n} ε_k p_k. Then for p_4=7, sum_{k=0}^3 ε_k p_k = 7, which we found possible: 1 -2 +3 +5 = 7. For p_5=17, it's 2p_4 + sum_{k=0}^4 ε_k p_k = 14 + sum = 17 ⇒ sum = 3. Which we couldn't find earlier. But maybe there is a combination. Let me try again.

Let me think of ε0=1, ε1=1, ε2=1, ε3=1, ε4=-1: 1 + 2 + 3 + 5 -7 = 4. Not 3.

ε0=1, ε1=1, ε2=1, ε3=-1, ε4=1: 1 + 2 + 3 -5 +7 = 8.

ε0=1, ε1=1, ε2=-1, ε3=1, ε4=1: 1 + 2 -3 +5 +7 = 12.

ε0=1, ε1=-1, ε2=1, ε3=1, ε4=1: 1 -2 +3 +5 +7 = 14.

ε0=-1, ε1=1, ε2=1, ε3=1, ε4=1: -1 + 2 + 3 + 5 +7 = 16.

ε0=1, ε1=1, ε2=1, ε3=1, ε4=0: Not allowed.

Wait, maybe ε0=1, ε1=1, ε2=1, ε3=-1, ε4=-1: 1 + 2 + 3 -5 -7 = -6.

No. What if ε0=1, ε1=1, ε2=-1, ε3=-1, ε4=1: 1 + 2 -3 -5 +7 = 2.

Close. ε0=1, ε1=-1, ε2=1, ε3=-1, ε4=1: 1 -2 +3 -5 +7 = 4.

Hmm. Maybe I need to consider that there is no solution? But the example says there is. Wait, maybe the formula is not for p_5 but for p_7? No, the example is for p_5=17. Maybe I made a mistake in the indices. Let me check the example again:

The example says:

17 = 1 + 2 - 3 - 5 + 7 - 11 + 2 · 13

So that's 1 + 2 -3 -5 +7 -11 + 2*13. Let's compute this:

1 + 2 = 3; 3 -3 = 0; 0 -5 = -5; -5 +7 = 2; 2 -11 = -9; -9 + 26 = 17. Correct.

So the sum is 1 + 2 -3 -5 +7 -11 = -9, and then 2*13 is added. So the formula for p_5=17 is 2*13 + (-9). But 13 is p_6. So maybe the formula is p_{2n +1} = 2p_{2n + 2} + ...? No, that doesn't make sense. Alternatively, maybe the formula is p_{2n +1} = 2p_{2n + something} + sum... It's unclear.

Alternatively, maybe the formula is p_{2n} = p_{2n - 1} + sum_{k=0}^{2n - 2} ε_k p_k and p_{2n +1} = 2p_{2n} + sum_{k=0}^{2n -1} ε_k p_k. Let me try with the example for p_4=13. For n=2, p_{2n}=p_4=13. Then p_{2n -1} = p_3=5. So 13 = 5 + sum_{k=0}^{2n - 2} ε_k p_k = 5 + sum_{k=0}^2 ε_k p_k. So sum_{k=0}^2 ε_k p_k = 8. As before, but we couldn't find such coefficients. But in the example, the sum is 1 + 2 -3 -5 +7 +11 = 13, which is p_6. So maybe the formula is different.

Alternatively, maybe the formula is p_{2n} = p_{2n -1} + sum_{k=0}^{2n -1} ε_k p_k? For p_4=13, p_3=5. Then sum_{k=0}^3 ε_k p_k = 13 -5 = 8. Which is the same as before. Still no solution.

This is getting too confusing. Maybe I should look for a pattern in the given examples and try to apply it to the primes 23, 29, 31, 37.

Given that for p_6=13, the representation is 1 + 2 -3 -5 +7 +11. Let's note that this is sum_{k=0}^5 ε_k p_k = 13. Similarly, for p_5=17, it's 2*13 + (1 + 2 -3 -5 +7 -11) = 26 -9 = 17. So maybe the formula is p_{2n} = sum_{k=0}^{2n -1} ε_k p_k and p_{2n +1} = 2p_{2n} + sum_{k=0}^{2n} ε_k p_k. Let me check for n=3: p_6=13, which is sum_{k=0}^5 ε_k p_k. For n=2, p_5=17 = 2p_4 + sum_{k=0}^4 ε_k p_k. But in the example, the sum is up to p5. Maybe it's a different index.

Alternatively, maybe the formula is for p_{2n} and p_{2n+1} as follows:

For p_{2n}, it's equal to the sum of previous primes with ±1 coefficients, and for p_{2n+1}, it's twice p_{2n} plus the same sum. But in the example, p_5=17 is 2*13 + (sum). But 13 is p_6. So maybe it's not directly related. This is too confusing.

Alternatively, maybe I should look for the representations of the primes 23, 29, 31, 37 using the same pattern as the examples.

Let me recall that the examples are:

For p_6=13: 1 + 2 -3 -5 +7 +11 = 13.

For p_5=17: 1 + 2 -3 -5 +7 -11 + 2*13 = 17.

So maybe for p_{2n}, it's a sum of previous primes with ±1, and for p_{2n+1}, it's 2*p_{2n} + sum of previous primes with ±1. But in the example, p_5=17 is 2*p_6 + ...? No, because p_