 Let the two consecutive triangular numbers be $T_n = \frac{n(n+1)}{2}$ and $T_{n+1} = \frac{(n+1)(n+2)}{2}$.

The difference between the squares of these two numbers is:

$(T_{n+1})^2 - (T_n)^2 = \left(\frac{(n+1)(n+2)}{2}\right)^2 - \left(\frac{n(n+1)}{2}\right)^2$

Expanding the squares, we get:

$(T_{n+1})^2 - (T_n)^2 = \frac{(n+1)^2(n+2)^2}{4} - \frac{n^2(n+1)^2}{4}$

Factoring out a common factor of $\frac{(n+1)^2}{4}$, we get:

$(T_{n+1})^2 - (T_n)^2 = \frac{(n+1)^2}{4}[(n+2)^2 - n^2]$

Simplifying the expression inside the brackets, we get:

$(T_{n+1})^2 - (T_n)^2 = \frac{(n+1)^2}{4}[n^2 + 4n + 4 - n^2]$

Simplifying further, we get:

$(T_{n+1})^2 - (T_n)^2 = \frac{(n+1)^2}{4}[4n + 4]$

Factoring out a common factor of 4, we get:

$(T_{n+1})^2 - (T_n)^2 = (n+1)^2(n+1)$

Since $(n+1)^3 = (n+1)^2(n+1)$, we can see that the difference between the squares of two consecutive triangular numbers is always a cube.

Therefore, the difference between the squares of two consecutive triangular numbers is always a cube.