 (a) To establish the identity $t_x = t_y + t_z$, we need to show that the sum of the triangular numbers $t_y$ and $t_z$ is equal to the triangular number $t_x$.

The formula for the nth triangular number is $t_n = \frac{n(n+1)}{2}$.

Let's substitute the given expressions for $x$, $y$, and $z$ into the formula for $t_n$:

$t_x = t_{\frac{n(n+3)}{2}+1} = \frac{(\frac{n(n+3)}{2}+1)(\frac{n(n+3)}{2}+2)}{2}$

$t_y = t_{n+1} = \frac{(n+1)(n+2)}{2}$

$t_z = t_{\frac{n(n+3)}{2}} = \frac{\frac{n(n+3)}{2}(\frac{n(n+3)}{2}+1)}{2}$

Now, let's simplify the expressions for $t_x$, $t_y$, and $t_z$:

$t_x = \frac{(\frac{n(n+3)}{2}+1)(\frac{n(n+3)}{2}+2)}{2} = \frac{n(n+3)+2}{2} \cdot \frac{n(n+3)+4}{2} = \frac{(n^2+3n+2)(n^2+3n+4)}{8}$

$t_y = \frac{(n+1)(n+2)}{2} = \frac{n^2+3n+2}{2}$

$t_z = \frac{\frac{n(n+3)}{2}(\frac{n(n+3)}{2}+1)}{2} = \frac{n(n+3)}{4} \cdot \frac{n(n+3)+2}{2} = \frac{n(n+3)(n^2+3n+2)}{8}$

Now, let's add $t_y$ and $t_z$:

$t_y + t_z = \frac{n^2+3n+2}{2} + \frac{n(n+3)(n^2+3n+2)}{8}$

Factor out $\frac{n^2+3n+2}{2}$:

$t_y + t_z = \frac{n^2+3n+2}{2} \cdot (1 + \frac{n(n+3)}{4})$

Simplify the expression:

$t_y + t_z = \frac{n^2+3n+2}{2} \cdot \frac{4+n(n+3)}{4}$

$t_y + t_z = \frac{n^2+3n+2}{2} \cdot \frac{n^2+3n+4}{4}$

Now, compare this expression with the expression for $t_x$:

$t_x = \frac{(n^2+3n+2)(n^2+3n+4)}{8}$

$t_y + t_z = \frac{n^2+3n+2}{2} \cdot \frac{n^2+3n+4}{4}$

We can see that $t_x$ and $t_y + t_z$ are equal, so the identity $t_x = t_y + t_z$ is established.

(b) To find three examples of triangular numbers that are sums of two other triangular numbers, we can substitute different values of $n$ into the expressions for $t_x$, $t_y$, and $t_z$:

For $n=1$:

$t_x = t_{2} = \frac{2(2+1)}{2} = 3$

$t_y = t_{2} = \frac{2(2+1)}{2} = 3$

$t_z = t_{1} = \frac{1(1+3)}{2} = 2$

$3 = 3 + 2$

For $n=2$:

$t_x = t_{4} = \frac{4(4+1)}{2} = 10$

$t_y = t_{3} = \frac{3(3+1)}{2} = 6$

$t_z = t_{2} = \frac{2(2+1)}{2} = 3$

$10 = 6 + 3$

For $n=3$:

$t_x = t_{6} = \frac{6(6+1)}{2} = 21$

$t_y = t_{4} = \frac{4(4+1)}{2} = 10$

$t_z = t_{3} = \frac{3(3+1)}{2} = 6$

$21 = 10 + 6$

So, three examples of triangular numbers that are sums of two other triangular numbers are 3, 10, and 21.