 To verify these relations, we first need to define the pentagonal, square, and triangular numbers.

A pentagonal number is a figurate number that represents a pentagon. The nth pentagonal number is given by the formula: $p_n = \frac{n(3n - 1)}{2}$.

A square number is a number that is the square of an integer. The nth square number is given by the formula: $s_n = n^2$.

A triangular number is a number that can be represented as a regular triangle. The nth triangular number is given by the formula: $t_n = \frac{n(n + 1)}{2}$.

Now, let's verify the given relations:

(a) $p_n = t_{n-l} + n^2$

We know that $p_n = \frac{n(3n - 1)}{2}$ and $t_{n-l} = \frac{(n-1)n}{2}$. So, we can substitute these expressions into the given relation:

$\frac{n(3n - 1)}{2} = \frac{(n-1)n}{2} + n^2$

Simplify the equation:

$3n^2 - n = n^2 - n + 2n^2$

$3n^2 - n = 3n^2 - n$

Since both sides of the equation are equal, the relation is verified.

(b) $p_n = 3t_{n-l} + n = 2t_{n-l} + t_n$

We already know that $p_n = \frac{n(3n - 1)}{2}$, $t_{n-l} = \frac{(n-1)n}{2}$, and $t_n = \frac{n(n + 1)}{2}$. So, we can substitute these expressions into the given relation:

$\frac{n(3n - 1)}{2} = 3\left(\frac{(n-1)n}{2}\right) + n = 2\left(\frac{(n-1)n}{2}\right) + \frac{n(n + 1)}{2}$

Simplify the equation:

$3n^2 - n = \frac{3n^2 - 3n}{2} + n = n^2 - n + \frac{n^2 + n}{2}$

$3n^2 - n = \frac{3n^2 - 3n + 2n}{2} = \frac{2n^2 - 2n + n^2 + n}{2}$

$3n^2 - n = \frac{5n^2 - 2n}{2} = \frac{3n^2 - n}{2}$

Since both sides of the equation are equal, the relation is verified.

Therefore, the given relations between the pentagonal, square, and triangular numbers are verified.