<think>
Okay, so I need to prove that the square of any odd multiple of 3 can be expressed as the difference of two triangular numbers. The specific equation given is:

$$9(2n + 1)^2 = t_{9n+4} - t_{3n+l}$$

Wait, hold on. The problem mentions "specifically, that 9(2n + 1)^2 = t_{9n+4} - t_{3n+l}". But there's a variable "l" here. Maybe that's a typo? Because the original problem says "the difference of two triangular numbers specifically, that 9(2n + 1)^2 = t_{9n+4} - t_{3n+l}". Maybe "l" is supposed to be another expression? Maybe it's a typo for "something else"? Let me check again.

Wait, the original problem says: "Prove that the square of any odd multiple of 3 is the difference of two triangular numbers specifically, that 9(2n + 1)^2 = t_{9n+4} - t_{3n+l}". Hmm. Maybe "l" is a typo for another variable? Or maybe it's supposed to be "3n + something". Let me think.

Alternatively, maybe the problem is written correctly, and "l" is a specific number? Wait, but the problem says "the square of any odd multiple of 3", so 9(2n + 1)^2 is the square of an odd multiple of 3, since 2n + 1 is odd, so 3*(2n + 1) is an odd multiple of 3. So 9*(2n + 1)^2 is [3*(2n + 1)]^2. So the square of an odd multiple of 3.

But the problem says that this equals t_{9n+4} - t_{3n + l}. So maybe there's a typo in the exponent of the second triangular number? Maybe "l" is supposed to be "something else". Let me check if maybe it's supposed to be "3n + 1" or "3n + something else". Alternatively, maybe "l" is a variable, but then the problem would need to specify what l is. Wait, the problem is stated as:

"Prove that the square of any odd multiple of 3 is the difference of two triangular numbers specifically, that

$$9( 2 n + 1)^2 = t_{9n+4} - t_{3n+l}$$"

So maybe "l" is a typo for "something else", or perhaps it's supposed to be "3n + something". Alternatively, maybe the original problem had a specific value for l? Wait, perhaps in the original problem, maybe "l" is supposed to be "something" that can be determined? Let me try to figure it out.

Alternatively, maybe the user made a typo and "l" is supposed to be "something else". Let me check the problem again. Wait, maybe the original problem is from somewhere, and maybe "l" is a typo for "n" or another number. Alternatively, maybe the problem is correct, and I need to find what l is? Wait, but the problem says "specifically, that 9(2n + 1)^2 = t_{9n+4} - t_{3n+l}". So maybe l is supposed to be a specific value depending on n? Let me try to work through it.

First, let me recall that triangular numbers are given by t_k = k(k + 1)/2. So if I can express 9(2n + 1)^2 as t_{9n+4} - t_{something}, then I can solve for that something.

So let me write down:

t_{9n + 4} - t_{m} = 9(2n + 1)^2, where m is some expression in terms of n. Let me compute t_{9n + 4} first.

t_{9n + 4} = (9n + 4)(9n + 5)/2.

Similarly, t_m = m(m + 1)/2.

So the difference between them is:

[(9n + 4)(9n + 5)/2] - [m(m + 1)/2] = 9(2n + 1)^2.

Multiply both sides by 2:

(9n + 4)(9n + 5) - m(m + 1) = 18(2n + 1)^2.

Let me compute the left-hand side:

First, expand (9n + 4)(9n + 5):

= (9n)^2 + 9n*5 + 4*9n + 4*5

= 81n² + 45n + 36n + 20

= 81n² + 81n + 20.

So left-hand side is 81n² + 81n + 20 - m(m + 1).

Set equal to 18*(4n² + 4n + 1) = 18*(4n² + 4n + 1) = 72n² + 72n + 18.

Therefore:

81n² + 81n + 20 - m(m + 1) = 72n² + 72n + 18.

Subtract 72n² + 72n + 18 from both sides:

(81n² - 72n²) + (81n - 72n) + (20 - 18) - m(m + 1) = 0

Which simplifies to:

9n² + 9n + 2 - m(m + 1) = 0

Therefore:

m(m + 1) = 9n² + 9n + 2.

So, m(m + 1) = 9n² + 9n + 2.

So we need to find m such that m(m + 1) equals 9n² + 9n + 2. Let me try to solve for m.

Let me write m² + m - (9n² + 9n + 2) = 0.

Using quadratic formula:

m = [-1 ± sqrt(1 + 4*(9n² + 9n + 2))]/2

Compute discriminant:

sqrt(1 + 36n² + 36n + 8) = sqrt(36n² + 36n + 9) = sqrt( (6n + 3)^2 )

Because (6n + 3)^2 = 36n² + 36n + 9. Yes!

Therefore, sqrt( (6n + 3)^2 ) = 6n + 3.

Therefore, m = [ -1 ± (6n + 3) ] / 2.

Since m must be positive, take the positive root:

m = [ -1 + 6n + 3 ] / 2 = (6n + 2)/2 = 3n + 1.

So m = 3n + 1.

Therefore, the second triangular number is t_{3n + 1}.

Wait, but in the original problem, it was written as t_{3n + l}. So if m = 3n + 1, then l is 1? So maybe the original problem had a typo, and it's supposed to be t_{3n + 1}? Let me check.

If that's the case, then the equation would be:

9(2n + 1)^2 = t_{9n + 4} - t_{3n + 1}

But let me verify this with an example. Let me take n = 0. Then:

Left-hand side: 9*(2*0 + 1)^2 = 9*1 = 9.

Right-hand side: t_{9*0 + 4} - t_{3*0 + 1} = t_4 - t_1.

t_4 = 4*5/2 = 10, t_1 = 1*2/2 = 1. So 10 - 1 = 9. Correct.

Another example: n = 1.

Left-hand side: 9*(2*1 + 1)^2 = 9*(3)^2 = 81.

Right-hand side: t_{9*1 + 4} - t_{3*1 + 1} = t_{13} - t_4.

t_13 = 13*14/2 = 91, t_4 = 10. 91 - 10 = 81. Correct.

Another example: n = 2.

Left-hand side: 9*(5)^2 = 9*25 = 225.

Right-hand side: t_{9*2 + 4} - t_{3*2 + 1} = t_{22} - t_7.

t_22 = 22*23/2 = 253, t_7 = 7*8/2 = 28. 253 - 28 = 225. Correct.

So seems like the correct expression is t_{9n + 4} - t_{3n + 1} = 9(2n + 1)^2. Therefore, the original problem probably had a typo where "l" was supposed to be "1". So maybe in the original problem, the exponent was written as 3n + l, and l