 To prove this, we need to show that the nth triangular number $t_n$ is equal to the binomial coefficient $\binom{n+1}{2}$ for all $n \geq 1$.

The nth triangular number $t_n$ is defined as the sum of the first $n$ natural numbers. We can express this as:

$$t_n = 1 + 2 + 3 + \cdots + n$$

We can also express this sum using the formula for the sum of an arithmetic series:

$$t_n = \frac{n(n+1)}{2}$$

Now, let's compare this with the binomial coefficient $\binom{n+1}{2}$:

$$\binom{n+1}{2} = \frac{(n+1)!}{2!(n-1)!} = \frac{(n+1)n}{2}$$

We can see that the formula for the nth triangular number $t_n$ is the same as the binomial coefficient $\binom{n+1}{2}$:

$$t_n = \frac{n(n+1)}{2} = \binom{n+1}{2}$$

Therefore, we have proved that the nth triangular number $t_n$ is equal to the binomial coefficient $\binom{n+1}{2}$ for all $n \geq 1$.