 To prove this, we will use mathematical induction.

Base case (n = 1):
The first triangular number is 1, so the sum of the reciprocals of the first triangular number is $\frac{1}{1} = 1$, which is less than 2.

Inductive step:
Assume that the statement is true for n = k, i.e.,
$$\frac{1}{1} + \frac{1}{3} + \frac{1}{6} + \frac{1}{10} + \ldots + \frac{1}{t_k} < 2$$

Now, we need to prove that the statement is true for n = k + 1, i.e.,
$$\frac{1}{1} + \frac{1}{3} + \frac{1}{6} + \frac{1}{10} + \ldots + \frac{1}{t_k} + \frac{1}{t_{k+1}} < 2$$

We know that the (k + 1)th triangular number is given by $t_{k+1} = \frac{(k+1)(k+2)}{2}$.

Now, let's add the reciprocal of the (k + 1)th triangular number to both sides of the inequality:

$$\frac{1}{1} + \frac{1}{3} + \frac{1}{6} + \frac{1}{10} + \ldots + \frac{1}{t_k} + \frac{1}{t_{k+1}} < 2 + \frac{1}{t_{k+1}}$$

We need to show that $2 + \frac{1}{t_{k+1}} < 2$.

Since $t_{k+1} = \frac{(k+1)(k+2)}{2}$, we have $\frac{1}{t_{k+1}} = \frac{2}{(k+1)(k+2)}$.

Now, let's consider the expression $2 + \frac{1}{t_{k+1}} = 2 + \frac{2}{(k+1)(k+2)}$.

We know that $2 = \frac{2(k+1)(k+2)}{(k+1)(k+2)}$, so we can rewrite the expression as:

$$2 + \frac{2}{(k+1)(k+2)} = \frac{2(k+1)(k+2)}{(k+1)(k+2)} + \frac{2}{(k+1)(k+2)} = \frac{2(k+1)(k+2) + 2}{(k+1)(k+2)}$$

Simplifying the numerator, we get:

$$2(k+1)(k+2) + 2 = 2k^2 + 6k + 4$$

Now, let's divide both the numerator and the denominator by 2:

$$\frac{2k^2 + 6k + 4}{(k+1)(k+2)} = \frac{k^2 + 3k + 2}{k^2 + 3k + 2} = 1$$

Since $1 < 2$, we have proven that the sum of the reciprocals of the first (k + 1) triangular numbers is less than 2.

Therefore, by mathematical induction, the statement is true for all positive integers n.