 To prove this, we first need to understand what triangular numbers are. A triangular number is a number that can be represented as the sum of consecutive positive integers. The nth triangular number, denoted as T(n), can be calculated using the formula:

T(n) = n * (n + 1) / 2

Now, let's consider the square of any odd multiple of 3, which can be represented as 9(2n + 1)^2. We can expand this expression:

9(2n + 1)^2 = 9 * (4n^2 + 4n + 1) = 36n^2 + 36n + 9

Now, let's try to express this in the form of two triangular numbers:

36n^2 + 36n + 9 = T(9n + 4) - T(3n + 1)

We can calculate T(9n + 4) and T(3n + 1) using the formula for triangular numbers:

T(9n + 4) = (9n + 4) * (9n + 5) / 2
T(3n + 1) = (3n + 1) * (3n + 2) / 2

Now, let's subtract T(3n + 1) from T(9n + 4):

T(9n + 4) - T(3n + 1) = [(9n + 4) * (9n + 5) / 2] - [(3n + 1) * (3n + 2) / 2]

We can simplify this expression by multiplying both sides by 2:

2 * [T(9n + 4) - T(3n + 1)] = (9n + 4) * (9n + 5) - (3n + 1) * (3n + 2)

Now, let's expand the products:

(9n + 4) * (9n + 5) = 81n^2 + 81n + 20
(3n + 1) * (3n + 2) = 9n^2 + 9n + 2

Subtracting the second expression from the first:

81n^2 + 81n + 20 - (9n^2 + 9n + 2) = 72n^2 + 72n + 18

Now, we can factor out a 9 from this expression:

9 * (8n^2 + 8n + 2)

We can see that this expression is equal to the original expression 36n^2 + 36n + 9:

9 * (8n^2 + 8n + 2) = 36n^2 + 36n + 9

Therefore, we have proven that the square of any odd multiple of 3 is the difference of two triangular numbers specifically, that

$$9( 2 n + 1)^2 = t_{9n+4} - t_{3n+l}$$