 We will prove this by induction.

Base case: For $n=1$, we have $p_1 = 1$ and $\frac{1(3(1)-1)}{2} = \frac{1(2)}{2} = 1$. So, the formula holds for $n=1$.

Inductive step: Assume that the formula holds for $n=k$, i.e., $p_k = \frac{k(3k-1)}{2}$. We will show that the formula also holds for $n=k+1$.

Using the recursive formula, we have $p_{k+1} = p_k + (3(k+1) - 2)$. Substituting the formula for $p_k$, we get

\begin{align*}
p_{k+1} &= \frac{k(3k-1)}{2} + (3(k+1) - 2) \\
&= \frac{3k^2 - k}{2} + 3k + 1 \\
&= \frac{3k^2 + 2k + 1}{2} \\
&= \frac{(k+1)(3(k+1)-1)}{2}.
\end{align*}

Thus, the formula holds for $n=k+1$.

By induction, the formula $p_n = \frac{n(3n-1)}{2}$ holds for all $n \geq 1$.