 (a) If $n(n + 1)/2$ is a triangular number, then $n(n + 1)/2 = k(k + 1)/2$ for some $k \leq n$.
      Solving for $k$, we find $k = n$.
      Conversely, if $n$ is a triangular number, then $n = k(k + 1)/2$ for some $k$.
      Then $n(n + 1)/2 = k(k + 1)(k + 2)/4$, which is a triangular number.

(b) If $n$ is a triangular number, then $8n + 1 = 4k(k + 1) + 1 = (2k + 1)^2$.
      Conversely, if $8n + 1$ is a perfect square, then $8n + 1 = (2k + 1)^2$ for some $k$.
      Then $n = k(k + 1)/2$, which is a triangular number.

(c) If $n$ and $m$ are consecutive triangular numbers, then $n = k(k + 1)/2$ and $m = (k + 1)(k + 2)/2$ for some $k$.
      Then $n + m = k(k + 1) + (k + 1)(k + 2)/2 = (k + 1)^2$, which is a perfect square.

(d) If $n$ is a triangular number, then $9n + 1 = 9k(k + 1)/2 + 1 = (3k + 1)^2$.
      Similarly, $25n + 3 = (5k + 2)^2$ and $49n + 6 = (7k + 3)^2$.
      Therefore, $9n + 1$, $25n + 3$, and $49n + 6$ are all triangular numbers.

(a) If $n(n + 1)/2$ is a triangular number, then $n(n + 1)/2 = k(k + 1)/2$ for some $k \leq n$.
      Solving for $k$, we find $k = n$.
      Conversely, if $n$ is a triangular number, then $n = k(k + 1)/2$ for some $k$.
      Then $n(n + 1)/2 = k(k + 1)(k + 2)/4$, which is a triangular number.

(b) If $n$ is a triangular number, then $8n + 1 = 4k(k + 1) + 1 = (2k + 1)^2$.
      Conversely, if $8n + 1$ is a perfect square, then $8n + 1 = (2k + 1)^2$ for some $k$.
      Then $n = k(k + 1)/2$, which is a triangular number.

(c) If $n$ and $m$ are consecutive triangular numbers, then $n = k(k + 1)/2$ and $m = (k + 1)(k + 2)/2$ for some $k$.
      Then $n + m = k(k + 1) + (k + 1)(k + 2)/2 = (k + 1)^2$, which is a perfect square.

(d) If $n$ is a triangular number, then $9n + 1 = 9k(k + 1)/2 + 1 = (3k + 1)^2$.
      Similarly, $25n + 3 = (5k + 2)^2$ and $49n + 6 = (7k + 3)^2$.
      Therefore, $9n + 1$, $25n + 3$, and $49n + 6$ are all triangular numbers.