<think>
Okay, so I need to show that if n is an odd integer, then the expression n⁴ + 4n² + 11 is divisible by 16, meaning it can be written as 16k for some integer k. Let me think about how to approach this. 

First, since n is odd, maybe I can express n as 2m + 1, where m is an integer. That way, I can substitute this into the expression and see if it simplifies to something that's clearly divisible by 16. Let me try that.

Let n = 2m + 1. Then, let's compute each term step by step.

First, compute n²:
n² = (2m + 1)² = 4m² + 4m + 1.

Then n⁴ would be (n²)², so:
n⁴ = (4m² + 4m + 1)². Hmm, that seems a bit complicated. Maybe expanding it will help?

Let me expand (4m² + 4m + 1)². Let me recall that (a + b + c)² = a² + b² + c² + 2ab + 2ac + 2bc. Applying that here:

(4m²)² + (4m)² + (1)² + 2*(4m²*4m) + 2*(4m²*1) + 2*(4m*1)

Calculating each term:

(16m⁴) + (16m²) + (1) + 2*(16m³) + 2*(4m²) + 2*(4m)

Simplify each term:

16m⁴ + 16m² + 1 + 32m³ + 8m² + 8m

Combine like terms:

16m⁴ + 32m³ + (16m² + 8m²) + 8m + 1

Which is:

16m⁴ + 32m³ + 24m² + 8m + 1

Okay, so n⁴ = 16m⁴ + 32m³ + 24m² + 8m + 1.

Now, let's compute 4n². Earlier, we found n² = 4m² + 4m + 1, so multiplying by 4:

4n² = 4*(4m² + 4m + 1) = 16m² + 16m + 4.

So now, let's add n⁴ + 4n² + 11:

n⁴ + 4n² + 11 = [16m⁴ + 32m³ + 24m² + 8m + 1] + [16m² + 16m + 4] + 11.

Let me combine these terms:

First, the 16m⁴ term stays as is.

Then the 32m³ term stays.

For the m² terms: 24m² + 16m² = 40m².

For the m terms: 8m + 16m = 24m.

Constants: 1 + 4 + 11 = 16.

So altogether:

16m⁴ + 32m³ + 40m² + 24m + 16.

Hmm, so the entire expression simplifies to 16m⁴ + 32m³ + 40m² + 24m + 16.

Now, I need to check if this is divisible by 16. Let me factor out 16 from each term if possible.

Looking at each term:

- 16m⁴ is obviously divisible by 16.
- 32m³ is 16*2m³, so divisible by 16.
- 40m² is 16*2.5m²? Wait, 40 divided by 16 is 2.5? Wait, but 40 is 16*2 + 8, so not divisible by 16. Hmm, so maybe factoring 16 isn't straightforward here. Maybe I made a mistake in calculation?

Wait, let me check my steps again. Let me verify the expansion of n⁴ and the addition.

First, n = 2m + 1.

n² = (2m + 1)^2 = 4m² + 4m + 1. That's correct.

n⁴ = (n²)^2 = (4m² + 4m + 1)^2. Let me recompute this expansion:

First, (a + b + c)^2 where a = 4m², b = 4m, c = 1.

So, a² = 16m^4, b² = 16m², c² = 1.

Then cross terms: 2ab = 2*(4m²)*(4m) = 32m³, 2ac = 2*(4m²)*(1) = 8m², 2bc = 2*(4m)*(1) = 8m. So adding all together:

16m^4 + 16m² + 1 + 32m³ + 8m² + 8m. Then combining like terms:

16m^4 + 32m³ + (16m² + 8m²) + 8m + 1 = 16m^4 + 32m³ + 24m² + 8m + 1. That's correct.

Then 4n² = 4*(4m² + 4m + 1) = 16m² + 16m + 4. Correct.

Adding n⁴ + 4n² + 11:

[16m^4 + 32m³ + 24m² + 8m + 1] + [16m² + 16m + 4] + 11.

Adding term by term:

16m^4 + 32m³ + (24m² + 16m²) + (8m + 16m) + (1 + 4 + 11)

Which is 16m^4 + 32m³ + 40m² + 24m + 16. That's correct.

So now, the expression is 16m⁴ + 32m³ + 40m² + 24m + 16.

Now, factor 16 out of each term? Let me see:

But 40m² is 16*(2.5m²) which isn't an integer coefficient. Wait, but maybe I can factor 8 from all terms?

Wait, let me check if the entire expression is divisible by 16. Let me check each term modulo 16.

Alternatively, maybe factor 8? Let me see:

16m⁴ + 32m³ + 40m² + 24m + 16.

Let me factor 8 out:

8*(2m⁴ + 4m³ + 5m² + 3m + 2). Hmm, but then 8*(something). But we need to show that the original expression is divisible by 16, so this would require that 2m⁴ + 4m³ + 5m² + 3m + 2 is even. Let me check if that is the case.

So, if I can show that 2m⁴ + 4m³ + 5m² + 3m + 2 is even, then multiplying by 8 would give a multiple of 16. So let's check that.

Let me consider the expression 2m⁴ + 4m³ + 5m² + 3m + 2. Let me check if it's even for any integer m.

Note that m can be any integer. Let me check parity. Let me consider m even and m odd.

Case 1: m is even. Let m = 2k.

Then:

2*(2k)^4 + 4*(2k)^3 + 5*(2k)^2 + 3*(2k) + 2

Compute each term:

2*(16k^4) = 32k^4

4*(8k^3) = 32k^3

5*(4k^2) = 20k^2

3*(2k) = 6k

+2

Total: 32k^4 + 32k^3 + 20k^2 + 6k + 2. All terms are even, so the sum is even.

Case 2: m is odd. Let m = 2k + 1.

Compute each term:

2*(2k + 1)^4 + 4*(2k + 1)^3 + 5*(2k + 1)^2 + 3*(2k + 1) + 2.

This might get complicated, but let's compute modulo 2. Since we only care about parity.

Note that any even number is 0 mod 2, odd is 1 mod 2.

But since m is odd, m ≡ 1 mod 2.

Let me compute each term modulo 2:

First term: 2*(m^4) ≡ 0 mod 2.

Second term: 4*(m^3) ≡ 0 mod 2.

Third term: 5*(m^2) ≡ 1*(m^2) ≡ 1*1 = 1 mod 2.

Fourth term: 3*(m) ≡ 1*(m) ≡ 1*1 = 1 mod 2.

Fifth term: 2 ≡ 0 mod 2.

Adding all together: 0 + 0 + 1 + 1 + 0 = 2 ≡ 0 mod 2. Therefore, the entire expression is even.

Therefore, regardless of whether m is even or odd, the expression 2m⁴ + 4m³ + 5m² + 3m + 2 is even. Therefore, 8*(even) = 16*(integer). Therefore, the original expression is divisible by 16. Therefore, n⁴ + 4n² + 11 is of the form 16k. 

Wait, so that seems to work. But let me check with specific numbers to make sure.

Let me take n = 1 (which is odd). Then compute n⁴ + 4n² + 11:

1 + 4 + 11 = 16. Which is 16*1. So yes, 16k where k=1.

Another example, n=3:

n⁴ = 81, 4n² = 4*9=36, so total is 81 + 36 + 11 = 128. 128 is 16*8, so yes.

Another example, n=5:

n⁴ = 625, 4n² = 4*25=100, so total is 625 + 100 + 11 = 736. 736 divided by 16 is 46. So 16*46 = 736. Correct.

Another example, n= -1 (odd):

(-1)^4 + 4*(-1)^2 + 11 = 1 + 4 + 11 = 16. Same as n=1. Correct.

n= -3:

(-3)^4 + 4*(-3)^2 + 11 = 81 + 36 + 11 = 128. Same as n=3. Correct.

So seems like the examples check out. Therefore, the algebra seems correct. Therefore, the conclusion is that for any odd integer n, n⁴ + 4n² + 11 is divisible by 16.

But let me think again if there's another way to approach this problem, maybe using modular arithmetic directly. Maybe considering n mod 16 or something. But since n is odd, n can be 1, 3, 5, ..., 15 mod 16. Maybe compute n⁴ + 4n² + 11 mod 16 for each possible n mod 16. Since there are only 8 possibilities for odd n mod 16 (since odd numbers are 1, 3, 5, 7, 9, 11, 13, 15 mod 16). Let me check that.

Let me compute n⁴ + 4n² + 11 mod 16 for n odd.

Let me compute for each odd n from 1 to 15:

Case 1: n=1:

1⁴ + 4*1² + 11 = 1 + 4 + 11 = 16 ≡ 0 mod 16.

Case 2: n=3:

3⁴ + 4*3² + 11 = 81 + 36 + 11 = 128. 128 mod 16 is 0.

Case 3: n=5:

5⁴ + 4*5² + 11 = 625 + 100 + 11 = 736. 736 / 16 = 46, so 0 mod 16.

Case 4: n=7:

7⁴ = 2401; 4*7² = 4*49 = 196; total is 2401 + 196 + 11 = 2608. 2608 divided by 16 is 163, so 0 mod 16.

Case 5: n=9:

9⁴ = 6561; 4*9² = 4*81 = 324; total is 6561 + 324 + 11 = 6896. 6896 / 16 = 431, so 0 mod 16.

Case 6: n=11:

11⁴ = 14641; 4*11² = 4*121 = 484; total is 14641 + 484 + 11 = 15136. 15136 / 16 = 946, so 0 mod 16.

Case 7: n=13:

13⁴ = 28561; 4*13² = 4*169 = 676; total is 28561 + 676 + 11 = 29248. 29248 / 16 = 1828, so 0 mod 16.

Case 8: n=15:

15⁴ = 50625; 4*15² = 4*225 = 900; total is 50625 + 900 + 11 = 51536. 51536 / 16 = 3221, so 0 mod 16.

So all cases give 0 mod 16. Therefore, regardless of which odd integer n we take, the expression is divisible by 16. Therefore, the original statement is proven.

Alternatively, maybe there's a more algebraic way. Let me think again. Since n is odd, n ≡ 1 or 3 mod 4. Wait, but perhaps using modulo 16. But since we already saw that for all odd residues mod 16, the expression is 0 mod 16, that's sufficient. But maybe there is another way. 

Alternatively, since n is odd, n can be written as 2m + 1, and we did the substitution earlier, which led us to the expression being 16*(something). So that's another way. 

But maybe there's a smarter way. For example, note that n is odd, so n² ≡ 1 mod 8. Let me check that. Since n is odd, n = 2m + 1, so n² = 4m² + 4m + 1 = 4m(m + 1) + 1. Since m and m + 1 are consecutive integers, one of them is even, so 4m(m + 1) is divisible by 8. Therefore, n² ≡ 1 mod 8. Therefore, n² = 8k + 1 for some integer k. 

Then n⁴ = (n²)² = (8k + 1)² = 64k² + 16k + 1. Therefore, n⁴ ≡ 1 mod 16? Wait, let's compute that:

(8k + 1)^2 = 64k² + 16k + 1. So mod 16, 64k² is 0 mod 16, 16k is 0 mod 16, so n⁴ ≡ 1 mod 16. 

Therefore, n⁴ ≡ 1 mod 16. Also, n² ≡ 1 mod 8, but mod 16?

Wait, n² mod 16. Let me check. If n is odd, then n can be 1, 3, 5, 7, 9, 11, 13, 15 mod 16. Let me compute n² mod 16:

1² = 1 mod 16.

3² = 9 mod 16.

5² = 25 ≡ 9 mod 16.

7² = 49 ≡ 1 mod 16.

9² = 81 ≡ 1 mod 16.

11² = 121 ≡ 9 mod 16.

13² = 169 ≡ 9 mod 16.

15² = 225 ≡ 1 mod 16.

So, n² mod 16 is either 1 or 9