 (a) We want to show that $8 | 5^{2n} + 7$ for all $n \geq 1$.

Base case: For $n = 1$, we have $5^{2(1)} + 7 = 25 + 7 = 32$, which is divisible by 8. So the statement holds for $n = 1$.

Inductive step: Assume the statement is true for $n = k$, i.e., $8 | 5^{2k} + 7$. We want to show that the statement is also true for $n = k + 1$.

Using the hint, we have:

$5^{2(k+1)} + 7 = 5^2(5^{2k} + 7) + (7 - 5^2 \cdot 7)$

Since $8 | 5^{2k} + 7$ by the inductive hypothesis, we can write $5^{2k} + 7 = 8m$ for some integer $m$. Substituting this into the equation, we get:

$5^{2(k+1)} + 7 = 5^2(8m) + (7 - 5^2 \cdot 7) = 8(5^2m) + (7 - 5^2 \cdot 7)$

The term $7 - 5^2 \cdot 7$ is divisible by 8 because $5^2 \cdot 7$ is divisible by 8. Therefore, the entire expression is divisible by 8.

Thus, the statement is true for $n = k + 1$.

By mathematical induction, the statement $8 | 5^{2n} + 7$ is true for all $n \geq 1$.

(b) We want to show that $15 | 2^{4n} - 1$ for all $n \geq 1$.

Base case: For $n = 1$, we have $2^{4(1)} - 1 = 16 - 1 = 15$, which is divisible by 15. So the statement holds for $n = 1$.

Inductive step: Assume the statement is true for $n = k$, i.e., $15 | 2^{4k} - 1$. We want to show that the statement is also true for $n = k + 1$.

Using the hint, we have:

$2^{4(k+1)} - 1 = 2^4(2^{4k} - 1) + (16 - 1)$

Since $15 | 2^{4k} - 1$ by the inductive hypothesis, we can write $2^{4k} - 1 = 15m$ for some integer $m$. Substituting this into the equation, we get:

$2^{4(k+1)} - 1 = 2^4(15m) + (16 - 1) = 15(16m) + 15$

The term $15(16m)$ is divisible by 15, so the entire expression is divisible by 15.

Thus, the statement is true for $n = k + 1$.

By mathematical induction, the statement $15 | 2^{4n} - 1$ is true for all $n \geq 1$.

(c) We want to show that $5 | 3^{3n+1} + 2^{n+1}$ for all $n \geq 1$.

Base case: For $n = 1$, we have $3^{3(1)+1} + 2^{1+1} = 27 + 4 = 31$, which is not divisible by 5. So the statement does not hold for $n = 1$.

Therefore, the statement $5 | 3^{3n+1} + 2^{n+1}$ is not true for all $n \geq 1$.

(d) We want to show that $21 | 4^{n+1}+ 5^{2n-1}$ for all $n \geq 1$.

Base case: For $n = 1$, we have $4^{1+1}+ 5^{2(1)-1} = 16 + 25 = 41$, which is not divisible by 21. So the statement does not hold for $n = 1$.

Therefore, the statement $21 | 4^{n+1}+ 5^{2n-1}$ is not true for all $n \geq 1$.

(e) We want to show that $24 | 2 \cdot 7^n + 3 \cdot 5^n - 5$ for all $n \geq 1$.

Base case: For $n = 1$, we have $2 \cdot 7^1 + 3 \cdot 5^1 - 5 = 14 + 15 - 5 = 24$, which is divisible by 24. So the statement holds for $n = 1$.

Inductive step: Assume the statement is true for $n = k$, i.e., $24 | 2 \cdot 7^k + 3 \cdot 5^k - 5$. We want to show that the statement is also true for $n = k + 1$.

Using the hint, we have:

$2 \cdot 7^{k+1} + 3 \cdot 5^{k+1} - 5 = 7(2 \cdot 7^k + 3 \cdot 5^k - 5) + 5(3 \cdot 5^k - 2)$

Since $24 | 2 \cdot 7^k + 3 \cdot 5^k - 5$ by the inductive hypothesis, we can write $2 \cdot 7^k + 3 \cdot 5^k - 5 = 24m$ for some integer $m$. Substituting this into the equation, we get:

$2 \cdot 7^{k+1} + 3 \cdot 5^{k+1} - 5 = 7(24m) + 5(3 \cdot 5^k - 2)$

The term $5(3 \cdot 5^k - 2)$ is divisible by 24 because $3 \cdot 5^k - 2$ is an integer. Therefore, the entire expression is divisible by 24.

Thus, the statement is true for $n = k + 1$.

By mathematical induction, the statement $24 | 2 \cdot 7^n + 3 \cdot 5^n - 5$ is true for all $n \geq 1$.