 We will prove this by induction.

Base case: For n = 0, we have $(3*0)!/(3!)^0 = 1/1 = 1$, which is an integer. So, the base case holds.

Inductive step: Assume that the expression is an integer for n = k, i.e., $(3k)!/(3!)^k$ is an integer. We need to prove that the expression is also an integer for n = k + 1, i.e., $(3(k+1))!/(3!)^{k+1}$ is an integer.

Consider the expression $(3(k+1))!/(3!)^{k+1}$. We can rewrite this as:

$(3k+3)!/(3!)^{k+1} = (3k+3)(3k+2)(3k+1)(3k)!/(3!)^{k+1}$

Now, we can factor out $(3k)!/(3!)^k$ from the numerator:

= $(3k+3)(3k+2)(3k+1)(3k)!/(3!)^k * (3!)^k/(3!)^{k+1}$

The first term, $(3k)!/(3!)^k$, is an integer by our assumption. The second term, $(3!)^k/(3!)^{k+1}$, simplifies to $1/(3!)$, which is also an integer. Therefore, the product of these two terms is an integer.

Thus, we have proved that if the expression is an integer for n = k, it is also an integer for n = k + 1. By the principle of mathematical induction, the expression $(3n)!/(3!)^n$ is an integer for all n $\geq{0}$.