 (a) First, we prove that if there exist integers x and y for which c = ax + by, then gcd(a, b) | c.

Let d = gcd(a, b). Since d | a and d | b, we have d | (ax + by) by the properties of divisibility. Therefore, gcd(a, b) | c.

Now, we prove that if gcd(a, b) | c, then there exist integers x and y for which c = ax + by.

Since gcd(a, b) | c, there exist integers x' and y' such that c = d * x' = (a * x' + b * y'). We can rewrite this as c = a * (x' - y') + b * y'. Let x = x' - y' and y = y', then c = ax + by.

(b) We are given that ax + by = gcd(a, b). We want to prove that gcd(x, y) = 1.

Since gcd(a, b) = ax + by, we have gcd(a, b) | (ax + by). By the properties of divisibility, gcd(a, b) | ax and gcd(a, b) | by. 

Now, let d = gcd(x, y). Since d | x and d | y, we have d | (ax + by) by the properties of divisibility. Therefore, d | gcd(a, b).

Since gcd(a, b) | gcd(a, b), we have d ≤ gcd(a, b). But gcd(a, b) = ax + by, and since d | (ax + by), we have d ≤ ax + by. 

Now, we know that gcd(a, b) = ax + by and d ≤ ax + by, so d = gcd(a, b). But gcd(a, b) = 1, so d = 1.

Therefore, gcd(x, y) = 1.