<think>
Okay, so I need to show that for any odd integer a, the expression a² + (a + 2)² + (a + 4)² + 1 is divisible by 12. Hmm, let me think about how to approach this. 

First, since a is odd, maybe I can represent it in terms of some variable that makes it easier to handle. Like, maybe express a as 2k + 1, where k is an integer. That way, I can substitute this into the expression and simplify it. Let me try that.

Let’s let a = 2k + 1. Then, substituting into each term:

First term: a² = (2k + 1)² = 4k² + 4k + 1.

Second term: (a + 2)² = (2k + 1 + 2)² = (2k + 3)². Let me expand that: (2k + 3)² = 4k² + 12k + 9.

Third term: (a + 4)² = (2k + 1 + 4)² = (2k + 5)². Expanding that: 4k² + 20k + 25.

Fourth term is just 1.

So adding all these together:

First term: 4k² + 4k + 1

Second term: 4k² + 12k + 9

Third term: 4k² + 20k + 25

Fourth term: 1

Adding them up:

Let me add the coefficients step by step.

For the k² terms: 4k² + 4k² + 4k² = 12k².

For the k terms: 4k + 12k + 20k = 36k.

For the constants: 1 + 9 + 25 + 1 = 36.

So overall, the entire expression becomes 12k² + 36k + 36.

Hmm, so that simplifies to 12k² + 36k + 36. Now, can I factor out a 12 from this expression?

Let me see: 12k² + 36k + 36. Let's factor 12 out of each term:

First term: 12k² is 12 times k².

Second term: 36k is 12 times 3k.

Third term: 36 is 12 times 3.

So altogether, that would be 12(k² + 3k + 3). Therefore, the entire expression is 12 times (k² + 3k + 3). Since 12 is a factor, that means the original expression is divisible by 12. 

Wait, so does that mean that regardless of the value of k, this expression is divisible by 12? Because we factored out 12, so yes, it's 12 multiplied by some integer (since k is an integer). Therefore, the expression is divisible by 12. 

But let me check if I did the algebra correctly. Let me re-add the terms:

Original terms:

First term: 4k² + 4k + 1

Second term: 4k² + 12k + 9

Third term: 4k² + 20k + 25

Fourth term: 1

Adding them up:

k² terms: 4 + 4 + 4 = 12, so 12k². Correct.

k terms: 4k + 12k + 20k = 36k. Correct.

Constants: 1 + 9 + 25 + 1 = 36. Correct. So 12k² + 36k + 36. Then factoring 12, we get 12(k² + 3k + 3). So that seems right. 

Therefore, since 12 divides this expression, the original expression is divisible by 12. Therefore, the statement is proven. 

But maybe I should check with specific examples to make sure. Let me pick some odd integers for a and compute the expression to see if it's divisible by 12.

First example: Let a = 1.

Compute 1² + (1 + 2)² + (1 + 4)² + 1 = 1 + 9 + 25 + 1 = 36. 36 divided by 12 is 3, so yes, divisible by 12.

Another example: a = 3.

Compute 3² + 5² + 7² + 1 = 9 + 25 + 49 + 1 = 84. 84 divided by 12 is 7. So that works.

Another example: a = 5.

5² + 7² + 9² + 1 = 25 + 49 + 81 + 1 = 156. 156 divided by 12 is 13. Correct.

Another example: a = -1 (since a can be negative as well, as long as it's odd).

Compute (-1)^2 + (-1 + 2)^2 + (-1 + 4)^2 + 1 = 1 + 1^2 + 3^2 + 1 = 1 + 1 + 9 + 1 = 12. 12 divided by 12 is 1. So that works too.

Another example: a = 7.

7² + 9² + 11² + 1 = 49 + 81 + 121 + 1 = 252. 252 divided by 12 is 21. Correct.

So all these examples check out. Therefore, my algebra seems correct. 

Alternatively, maybe there's another way to approach this problem, perhaps by considering modulo 12 or breaking it into modulo 3 and modulo 4, since 12 is 3*4 and they are coprime. Maybe that's another method?

Let me try that approach as well, just to confirm.

We need to show that the expression is divisible by both 3 and 4, since 3 and 4 are coprime, so if it's divisible by both, then it's divisible by 12.

First, check divisibility by 3.

Let me compute the expression modulo 3.

Given that a is odd. Let me note that odd integers modulo 3 can be 0, 1, or 2. Wait, but since a is odd, maybe there's some restriction? Wait, no, oddness is separate from modulo 3. For example, 3 is odd, 1 is odd, 5 is odd, etc. So a can be congruent to 0, 1, or 2 modulo 3, but with the constraint that a is odd. Wait, but if a is odd, then a mod 2 is 1, but mod 3 can be anything. So maybe I need to consider different cases. However, perhaps it's easier to compute the expression modulo 3.

But maybe first, let me compute the expression a² + (a + 2)² + (a + 4)² + 1 modulo 3.

But since a is odd, let me note that a ≡ 1 or 2 mod 3? Wait, no, actually, a can be any integer, odd, so modulo 3, a can be 0, 1, or 2. For example, a = 3 is odd and 0 mod 3, a = 1 is 1 mod 3, a = 5 is 2 mod 3, etc. So maybe we need to check all possibilities? But perhaps there's a better way.

Alternatively, maybe I can use that since a is odd, then a ≡ 1 mod 2. However, modulo 3, it's not restricted. But maybe I can compute the expression modulo 3 and 4 separately.

Let me try modulo 3 first.

Let me compute each term modulo 3.

Let me denote the expression as E = a² + (a + 2)² + (a + 4)² + 1.

Note that modulo 3, 4 ≡ 1, so (a + 4) ≡ (a + 1) mod 3. Similarly, 2 mod 3 is 2.

So:

E ≡ a² + (a + 2)² + (a + 1)² + 1 mod 3.

Let me expand each term:

First term: a²

Second term: (a + 2)² = a² + 4a + 4 ≡ a² + a + 1 mod 3 (since 4 ≡ 1 mod 3, and 4a ≡ a mod 3)

Third term: (a + 1)² = a² + 2a + 1 mod 3.

Fourth term: 1.

So adding all together:

First term: a²

Second term: a² + a + 1

Third term: a² + 2a + 1

Fourth term: 1

Total:

a² + (a² + a + 1) + (a² + 2a + 1) + 1

Combine like terms:

a² + a² + a² = 3a² ≡ 0 mod 3

a terms: a + 2a = 3a ≡ 0 mod 3

Constants: 1 + 1 + 1 = 3 ≡ 0 mod 3

So total E ≡ 0 + 0 + 0 = 0 mod 3. Therefore, E is divisible by 3.

Now check divisibility by 4. Let me compute E modulo 4.

Again, since a is odd, let me note that odd numbers are congruent to 1 or 3 mod 4.

So let me consider two cases: a ≡ 1 mod 4 and a ≡ 3 mod 4.

Case 1: a ≡ 1 mod 4.

Then, compute each term:

a = 1 mod 4.

a + 2 = 1 + 2 = 3 mod 4.

a + 4 = 1 + 4 = 5 ≡ 1 mod 4.

So:

a² ≡ 1² = 1 mod 4.

(a + 2)² ≡ 3² = 9 ≡ 1 mod 4.

(a + 4)² ≡ 1² = 1 mod 4.

Adding these: 1 + 1 + 1 = 3 mod 4. Then add the last term, which is 1: 3 + 1 = 4 ≡ 0 mod 4. So E ≡ 0 mod 4.

Case 2: a ≡ 3 mod 4.

Then, compute each term:

a = 3 mod 4.

a + 2 = 3 + 2 = 5 ≡ 1 mod 4.

a + 4 = 3 + 4 = 7 ≡ 3 mod 4.

So:

a² ≡ 3² = 9 ≡ 1 mod 4.

(a + 2)² ≡ 1² = 1 mod 4.

(a + 4)² ≡ 3² = 9 ≡ 1 mod 4.

Adding these: 1 + 1 + 1 = 3 mod 4. Then add the last term, 1: 3 + 1 = 4 ≡ 0 mod 4. Therefore, E ≡ 0 mod 4.

Therefore, regardless of whether a is 1 or 3 mod 4, E is divisible by 4. Hence, since E is divisible by both 3 and 4, it is divisible by 12. Therefore, this confirms the result.

Alternatively, maybe there's another way to approach this, by expanding the original expression and simplifying.

Let me try that again. Let me compute the original expression:

a² + (a + 2)² + (a + 4)² + 1.

Expanding each term:

First term: a².

Second term: a² + 4a + 4.

Third term: a² + 8a + 16.

Fourth term: 1.

Adding them up:

a² + (a² + 4a + 4) + (a² + 8a + 16) + 1.

Combine like terms:

Total a² terms: 1 + 1 + 1 = 3a².

Total a terms: 4a + 8a = 12a.

Constants: 4 + 16 + 1 = 21.

So the entire expression is 3a² + 12a + 21. Wait, but earlier when I substituted a = 2k + 1, I got 12k² + 36k + 36. Wait, but here, if I do this expansion, I get 3a² + 12a + 21. Wait, but that seems different. Which one is correct? Let me check with a specific value. Let me take a = 1. Then according to the first method, substituting a = 1 gives 1 + 9 + 25 + 1 = 36. According to this second expansion, 3(1)^2 + 12(1) + 21 = 3 + 12 + 21 = 36. Correct. So both expressions are equivalent. So 3a² + 12a + 21. Let me factor this expression. 

Factor 3 out: 3(a² + 4a + 7). Wait, but earlier I had 12(k² + 3k + 3). How are these related?

Wait, if a is odd, then a = 2k + 1. Let me substitute that into 3a² + 12a + 21:

First compute a²: (2k + 1)^2 = 4k² + 4k + 1.

Then 3a² = 3*(4k² + 4k + 1) = 12k² + 12k + 3.

Then 12a = 12*(2k + 1) = 24k + 12.

Adding those to 21:

Total expression: 12k² + 12k + 3 + 24k + 12 + 21 = 12k² + (12k + 24k) + (3 + 12 + 21) = 12k² + 36k + 36. Which is the same as before, which factors into 12(k² + 3k + 3). So that's consistent. Therefore, the expression is 3a² + 12a + 21, which can be written as 3(a² + 4a + 7). However, since we have shown that this is equal to 12(k² + 3k + 3), which is divisible by 12, then this shows that 3(a² + 4a + 7) is divisible by 12, which implies that (a² + 4a + 7) is divisible by 4. 

Alternatively, maybe we can analyze 3a² + 12a + 21. Let me factor 3: 3(a² + 4a + 7). For this to be divisible by 12, since 3 divides 12, we need a² + 4a + 7 to be divisible by 4. Let me check that.

So, if I can show that a² + 4a + 7 ≡ 0 mod 4, then 3*(something divisible by 4) is divisible by 12. Let me check that.

Since a is odd, let me write a as 2k + 1 again. Then:

a² + 4a + 7 = (2k + 1)^2 + 4*(2k + 1) + 7 = 4k² + 4k + 1 + 8k + 4 + 7 = 4k² + 12k + 12. Which is 4(k² + 3k + 3). Therefore, this is divisible by 4, so 3*(4(...)) is divisible by 12. So that works. 

Alternatively, since a is odd, let me compute a² + 4a + 7 modulo 4. Since a is odd, a ≡ 1 or 3 mod 4.

Case 1: a ≡ 1 mod 4.

Then a² ≡ 1² = 1 mod 4.

4a ≡ 0 mod 4.

7 ≡ 3 mod 4.

Therefore, total: 1 + 0 + 3 = 4 ≡ 0 mod 4.

Case 2: a ≡ 3 mod 4.

a² ≡ 9 ≡ 1 mod 4.

4a ≡ 0 mod 4.

7 ≡ 3 mod 4.

Total: 1 + 0 + 3 = 4 ≡ 0 mod 4.

Therefore, regardless of a being 1 or 3 mod 4, a² + 4a + 7 ≡ 0 mod 4. Therefore, the expression 3(a² + 4a + 7) is divisible by 3*4 = 12. Therefore, the original expression is divisible by 12. 

So this gives another way to look at it. 

Alternatively, maybe there's a way to do this without substitution, by considering the expression modulo 12 directly. But that might be more complicated. 

Alternatively, note that since a is odd, then a ≡ 1, 3, 5, 7, 9, 11 mod 12. Wait, but maybe considering modulo 12 is overkill. But let me try.

Let me compute the expression for a ≡ 1, 3, 5, 7, 9, 11 mod 12. Since if it works for all residues, then it's divisible by 12. But since a is odd, we can check for these residues.

But that might take longer, but let me try.

Case 1: a ≡ 1