 To show that (-a) | b, we need to show that there exists an integer k such that b = (-a) * k.
Since a | b, we know that there exists an integer k' such that b = a * k'.
Now, let's multiply both sides of the equation b = a * k' by -1:
-b = -a * k'
Rearranging the equation, we get:
b = (-a) * (-k')
Since -k' is an integer, we have shown that (-a) | b.

To show that a | (-b), we need to show that there exists an integer k'' such that -b = a * k''.
Since a | b, we know that there exists an integer k' such that b = a * k'.
Now, let's multiply both sides of the equation b = a * k' by -1:
-b = a * (-k')
Rearranging the equation, we get:
-b = a * k'' (where k'' = -k')
Since k'' is an integer, we have shown that a | (-b).

To show that (-a) | (-b), we need to show that there exists an integer k''' such that -b = (-a) * k'''.
Since a | b, we know that there exists an integer k' such that b = a * k'.
Now, let's multiply both sides of the equation b = a * k' by -1:
-b = (-a) * k'
Since k' is an integer, we have shown that (-a) | (-b).

Therefore, we have shown that (-a) | b, a | (-b), and (-a) | (-b) given that a | b.