 (a) To show that gcd(2a + 1, 9a + 4) = 1, we need to show that 2a + 1 and 9a + 4 have no common divisors other than 1.

Let d be a common divisor of 2a + 1 and 9a + 4. Then, d divides both 2a + 1 and 9a + 4.

Now, consider the equation 2(9a + 4) - 9(2a + 1) = 2(9a + 4) - 18a - 9 = 8.

Since d divides both 2a + 1 and 9a + 4, it also divides 8.

However, 8 has only two divisors: 1 and 8. If d = 1, then gcd(2a + 1, 9a + 4) = 1. If d = 8, then gcd(2a + 1, 9a + 4) = 8.

But, we know that gcd(2a + 1, 9a + 4) cannot be 8, because 8 does not divide 2a + 1.

Therefore, gcd(2a + 1, 9a + 4) = 1.

(b) To show that gcd(5a + 2, 7a + 3) = 1, we need to show that 5a + 2 and 7a + 3 have no common divisors other than 1.

Let d be a common divisor of 5a + 2 and 7a + 3. Then, d divides both 5a + 2 and 7a + 3.

Now, consider the equation 5(7a + 3) - 7(5a + 2) = 35a + 15 - 35a - 14 = 1.

Since d divides both 5a + 2 and 7a + 3, it also divides 1.

However, 1 has only one divisor: 1. If d = 1, then gcd(5a + 2, 7a + 3) = 1.

Therefore, gcd(5a + 2, 7a + 3) = 1.

(c) To show that if a is odd, then gcd(3a, 3a + 2) = 1, we need to show that 3a and 3a + 2 have no common divisors other than 1 when a is odd.

Let d be a common divisor of 3a and 3a + 2. Then, d divides both 3a and 3a + 2.

Now, consider the equation 3a + 2 - 3a = 2.

Since d divides both 3a and 3a + 2, it also divides 2.

However, 2 has only two divisors: 1 and 2. If d = 1, then gcd(3a, 3a + 2) = 1. If d = 2, then gcd(3a, 3a + 2) = 2.

But, we know that gcd(3a, 3a + 2) cannot be 2, because 2 does not divide 3a when a is odd.

Therefore, gcd(3a, 3a + 2) = 1 when a is odd.