 To establish the assertion, we need to show that $a^2 + 23$ is divisible by 24 when a is an integer not divisible by 2 or 3.

Let's consider the possible remainders when a is divided by 24. Since a is not divisible by 2 or 3, it cannot be divisible by 24. Therefore, the possible remainders when a is divided by 24 are 1, 5, 7, 11, 13, 17, 19, and 23.

Now, let's consider the values of $a^2 + 23$ for each of these remainders:

1. If the remainder is 1, then $a = 24k + 1$ for some integer k. So, $a^2 + 23 = (24k + 1)^2 + 23 = 576k^2 + 48k + 1 + 23 = 24(24k^2 + 2k) + 24$. Since 24 is a factor of $24(24k^2 + 2k) + 24$, we have $24 | ( a^2 + 23)$.

2. If the remainder is 5, then $a = 24k + 5$ for some integer k. So, $a^2 + 23 = (24k + 5)^2 + 23 = 576k^2 + 240k + 25 + 23 = 24(24k^2 + 10k + 1) + 24$. Since 24 is a factor of $24(24k^2 + 10k + 1) + 24$, we have $24 | ( a^2 + 23)$.

3. If the remainder is 7, then $a = 24k + 7$ for some integer k. So, $a^2 + 23 = (24k + 7)^2 + 23 = 576k^2 + 336k + 49 + 23 = 24(24k^2 + 14k + 2) + 24$. Since 24 is a factor of $24(24k^2 + 14k + 2) + 24$, we have $24 | ( a^2 + 23)$.

4. If the remainder is 11, then $a = 24k + 11$ for some integer k. So, $a^2 + 23 = (24k + 11)^2 + 23 = 576k^2 + 528k + 121 + 23 = 24(24k^2 + 22k + 5) + 24$. Since 24 is a factor of $24(24k^2 + 22k + 5) + 24$, we have $24 | ( a^2 + 23)$.

5. If the remainder is 13, then $a = 24k + 13$ for some integer k. So, $a^2 + 23 = (24k + 13)^2 + 23 = 576k^2 + 624k + 169 + 23 = 24(24k^2 + 26k + 7) + 24$. Since 24 is a factor of $24(24k^2 + 26k + 7) + 24$, we have $24 | ( a^2 + 23)$.

6. If the remainder is 17, then $a = 24k + 17$ for some integer k. So, $a^2 + 23 = (24k + 17)^2 + 23 = 576k^2 + 752k + 289 + 23 = 24(24k^2 + 31k + 11) + 24$. Since 24 is a factor of $24(24k^2 + 31k + 11) + 24$, we have $24 | ( a^2 + 23)$.

7. If the remainder is 19, then $a = 24k + 19$ for some integer k. So, $a^2 + 23 = (24k + 19)^2 + 23 = 576k^2 + 864k + 361 + 23 = 24(24k^2 + 36k + 15) + 24$. Since 24 is a factor of $24(24k^2 + 36k + 15) + 24$, we have $24 | ( a^2 + 23)$.

8. If the remainder is 23, then $a = 24k + 23$ for some integer k. So, $a^2 + 23 = (24k + 23)^2 + 23 = 576k^2 + 1008k + 529 + 23 = 24(24k^2 + 42k + 21) + 24$. Since 24 is a factor of $24(24k^2 + 42k + 21) + 24$, we have $24 | ( a^2 + 23)$.

In all cases, we have shown that $24 | ( a^2 + 23)$ when a is an integer not divisible by 2 or 3. Therefore, the assertion is established.