 To prove this, we will use the properties of the greatest common divisor (gcd) and the fact that the gcd of a set of integers is the same as the gcd of any subset of those integers.

First, let's denote $d_1 = gcd(a, b)$, $d_2 = gcd(b, c)$, and $d_3 = gcd(a, c)$. We want to show that $d = d_1 = d_2 = d_3$.

Since $d = gcd(a, b, c)$, by definition, $d$ divides $a$, $b$, and $c$. 

Now, let's consider $d_1 = gcd(a, b)$. Since $d$ divides both $a$ and $b$, and $d_1$ is the greatest common divisor of $a$ and $b$, we have $d_1 \leq d$.

Similarly, since $d$ divides both $b$ and $c$, and $d_2$ is the greatest common divisor of $b$ and $c$, we have $d_2 \leq d$.

Finally, since $d$ divides both $a$ and $c$, and $d_3$ is the greatest common divisor of $a$ and $c$, we have $d_3 \leq d$.

Now, let's show that $d$ divides $d_1$, $d_2$, and $d_3$. 

Since $d_1 = gcd(a, b)$, $d_1$ divides both $a$ and $b$. But $d$ divides both $a$ and $b$ as well, so $d$ divides $d_1$.

Similarly, since $d_2 = gcd(b, c)$, $d_2$ divides both $b$ and $c$. But $d$ divides both $b$ and $c$ as well, so $d$ divides $d_2$.

Finally, since $d_3 = gcd(a, c)$, $d_3$ divides both $a$ and $c$. But $d$ divides both $a$ and $c$ as well, so $d$ divides $d_3$.

Therefore, we have $d \leq d_1$, $d \leq d_2$, and $d \leq d_3$. Combining with the previous inequalities, we have $d = d_1 = d_2 = d_3$.

This completes the proof that $d = gcd(gcd(a, b), c ) = gcd(a, gcd(b, c )) = gcd(gcd(a, c ), b)$.