 (a) If a = ±b, then gcd(a, b) = |a| = |b|, and lcm(a, b) = |ab|/gcd(a, b) = |a| = |b|, so gcd(a, b) = lcm(a, b). Conversely, if gcd(a, b) = lcm(a, b), then |ab|/gcd(a, b) = gcd(a, b), so |ab| = gcd(a, b)^2. Since gcd(a, b) divides both a and b, it must divide their product, so |ab| = gcd(a, b)^2 implies that gcd(a, b) = |a| or gcd(a, b) = |b|. Without loss of generality, assume that gcd(a, b) = |a|. Then |b| = gcd(a, b) divides a, so |b| = ±a, which means a = ±b.

(b) Let d = gcd(a, b) and let m = lcm(a, b). Then m = ab/d, and kd = gcd(ka, kb) and km = lcm(ka, kb). We have km = kab/d = k(ab/d) = k(ab/gcd(a, b)) = k lcm(a, b).

(c) Let m be a common multiple of a and b. Then m = ra and m = sb for some integers r and s. Then lcm(a, b) = ab/gcd(a, b) divides m = ra = (ab/gcd(a, b)) * (r/b), so lcm(a, b) | m.