<think>
Okay, so I need to prove that the square of any odd multiple of 3 is equal to the difference between two triangular numbers. The specific equation given is 9(2n + 1)^2 = t_{9n+4} - t_{3n + l}, where l is some number. Wait, actually, looking back, the problem says "specifically, that 9(2n + 1)^2 = t_{9n+4} - t_{3n + l}". But the problem statement might have a typo? Because the original problem says "the difference of two triangular numbers specifically, that 9(2n + 1)^2 = t_{9n+4} - t_{3n + l}". But maybe l is supposed to be a specific number? Let me check again.

Wait, the original problem is written as:

"Prove that the square of any odd multiple of 3 is the difference of two triangular numbers specifically, that

$$9( 2 n + 1)^2 = t_{9n+4} - t_{3n+l}$$"

Hmm, so the problem is to prove that 9(2n + 1)^2 equals t_{9n + 4} minus t_{3n + l}. But the problem says "specifically", so maybe l is supposed to be a particular number? Wait, maybe there's a typo in the problem? Maybe it's supposed to be t_{3n + 1} or something else? Or maybe l is a variable? Wait, but the problem is written as "t_{3n + l}", which is strange because l is not defined. Maybe it's supposed to be t_{3n + something}? Let me check the original problem again.

Wait, the original problem says "the difference of two triangular numbers specifically, that 9(2n + 1)^2 = t_{9n+4} - t_{3n + l}". Maybe the user made a typo, and l is supposed to be a specific number? For example, maybe it's supposed to be t_{3n + 1} or t_{3n + 2} or something else? Alternatively, maybe l is a function of n? But the problem says "specifically", which suggests that there is a specific expression for the second triangular number. Maybe the original problem had a specific value for l, but it was mistyped?

Alternatively, maybe the problem is from a source where l is defined earlier, but since it's not here, perhaps there's an error. Alternatively, maybe l is supposed to be 4? Wait, but then 3n + 4 would be the second triangular number. Let me check if that works. Let me try plugging in some numbers.

Alternatively, maybe there's a mistake in the problem. Let me think. The square of an odd multiple of 3 is 9*(2n + 1)^2. So, for example, if n = 0, then 9*(1)^2 = 9. Then t_{9*0 + 4} - t_{3*0 + l} = t_4 - t_l. The triangular numbers are t_k = k(k + 1)/2. So t_4 is 4*5/2 = 10. Then 10 - t_l = 9 implies t_l = 1. So t_l = 1 implies l = 1, since t_1 = 1. So in that case, l would be 1. If n = 1, then 9*(2*1 + 1)^2 = 9*9 = 81. Then t_{9*1 + 4} = t_{13} = 13*14/2 = 91. Then 91 - t_{3*1 + l} = 81 implies t_{3 + l} = 10. t_{3 + l} = 10. Let's solve for k: k(k + 1)/2 = 10. So k^2 + k - 20 = 0. Solutions: [-1 ± sqrt(1 + 80)] / 2 = [-1 ± 9]/2. Positive solution is (8)/2 = 4. So k = 4. Therefore, 3 + l = 4 => l = 1. So again, l = 1. So maybe l is 1? Then the equation is t_{9n + 4} - t_{3n + 1} = 9(2n + 1)^2.

Let me check for n = 2. Then 9*(5)^2 = 225. t_{9*2 + 4} = t_{22} = 22*23/2 = 253. Then t_{3*2 + 1} = t_7 = 7*8/2 = 28. Then 253 - 28 = 225. Correct! So that works. So maybe the original problem had a typo, and l is supposed to be 1. Therefore, the equation is 9(2n + 1)^2 = t_{9n + 4} - t_{3n + 1}. Therefore, the problem statement might have a typo, with l being 1. So assuming that, we need to prove that t_{9n + 4} - t_{3n + 1} equals 9(2n + 1)^2.

So, let's proceed with that. Let me write down the formula for triangular numbers: t_k = k(k + 1)/2. Therefore, t_{9n + 4} - t_{3n + 1} = [ (9n + 4)(9n + 5)/2 ] - [ (3n + 1)(3n + 2)/2 ].

Let me compute this expression:

First term: (9n + 4)(9n + 5)/2. Let's expand that:

(9n + 4)(9n + 5) = 81n² + 45n + 36n + 20 = 81n² + 81n + 20.

Second term: (3n + 1)(3n + 2) = 9n² + 6n + 3n + 2 = 9n² + 9n + 2.

Therefore, subtracting the second term from the first term:

[81n² + 81n + 20]/2 - [9n² + 9n + 2]/2 = [ (81n² + 81n + 20) - (9n² + 9n + 2) ] / 2

Compute numerator:

81n² - 9n² = 72n²

81n - 9n = 72n

20 - 2 = 18

So numerator is 72n² + 72n + 18.

Divide by 2: (72n² + 72n + 18)/2 = 36n² + 36n + 9.

Factor this expression: 36n² + 36n + 9 = 9*(4n² + 4n + 1) = 9*(2n + 1)^2.

Which is exactly the left-hand side of the equation. Therefore, the equation holds.

Therefore, the original problem likely had a typo, with l being 1 instead of some other variable. Therefore, the correct equation is t_{9n + 4} - t_{3n + 1} = 9(2n + 1)^2.

But since the problem statement says "t_{3n + l}", maybe the user intended l = 1? Therefore, the answer is that the equation holds with l = 1. Therefore, the proof is as above.

Alternatively, maybe the problem is correct as stated, and l is a function of n? But in the examples above, l was 1. Let me check for another n. Let me take n = 3. Then 9*(2*3 + 1)^2 = 9*(7)^2 = 9*49 = 441. t_{9*3 + 4} = t_{31} = 31*32/2 = 496. t_{3*3 + 1} = t_{10} = 10*11/2 = 55. Then 496 - 55 = 441. Correct. So again, l = 1. Therefore, the equation is correct with l = 1.

Therefore, the problem statement probably had a typo, and l is supposed to be 1. Therefore, the answer is that the equation holds with l = 1. Therefore, the proof is as above.

But since the problem says "specifically, that 9(2n + 1)^2 = t_{9n+4} - t_{3n + l}", maybe the original problem had l = 1. Therefore, the answer is that l = 1. However, since the problem didn't specify l, but in the equation, maybe l is supposed to be 1. Therefore, the proof is correct as above.

Alternatively, maybe the problem is correct, and the user made a typo in the problem statement. But given that in the problem statement, the user wrote "t_{3n + l}" but in the examples, l is 1, so maybe that's the case.

Alternatively, maybe l is a function of n? But in the problem statement, it's written as "t_{3n + l}", which is a bit strange. Maybe the original problem was in Chinese or another language, and the translation had an error. Alternatively, maybe the problem is correct, and l is supposed to be a specific expression. But given the examples, it seems that l is 1.

Therefore, I think the correct equation is t_{9n + 4} - t_{3n + 1} = 9(2n + 1)^2, so l = 1.

Therefore, the proof is as follows: compute the difference of the two triangular numbers, expand both terms, subtract, simplify, and show that it equals 9(2n + 1)^2. Which we did.

Therefore, the answer is that the equation holds with l = 1, and the proof is as shown above.

But since the problem says "prove that...", maybe I need to present the proof step by step.

So, step by step:

First, recall that the nth triangular number is t_n = n(n + 1)/2.

We need to show that t_{9n + 4} - t_{3n + 1} = 9(2n + 1)^2.

Compute t_{9n + 4}:

t_{9n + 4} = (9n + 4)(9n + 5)/2.

Compute t_{3n + 1}:

t_{3n + 1} = (3n + 1)(3n + 2)/2.

Subtracting the two:

[(9n + 4)(9n + 5) - (3n + 1)(3n + 2)] / 2.

Expand the numerator:

First, expand (9n + 4)(9n + 5):

= 81n² + 45n + 36n + 20

= 81n² + 81n + 20.

Then expand (3n + 1)(3n + 2):

= 9n² + 6n + 3n + 2

= 9n² + 9n + 2.

Subtracting the second expansion from the first:

(81n² + 81n + 20) - (9n² + 9n + 2) = 72n² + 72n + 18.

Divide by 2:

(72n² + 72n + 18)/2 = 36n² + 36n + 9.

Factor:

36n² + 36n + 9 = 9(4n² + 4n + 1) = 9(2n + 1)^2.

Therefore, the equation holds.

Therefore, the original problem had a typo, and the correct expression is with l = 1. Hence, the proof is complete.

**Final Answer**
\boxed{9(2n + 1)^2}
</think>

To prove that the square of any odd multiple of 3 is the difference of two triangular numbers, we begin by analyzing the given expression:

$$
9(2n + 1)^2 = t_{9n+4} - t_{3n+1}
$$

---

### Step 1: Recall the formula for triangular numbers

The $ k $-th triangular number is given by:

$$
t_k = \frac{k(k+1)}{2}
$$

---

### Step 2: Compute the two triangular numbers

Let’s compute $ t_{9n+4} $ and $ t_{3n+1} $:

$$
t_{9n+4} = \frac{(9n+4)(9n+5)}{2}
$$
$$
t_{3n+1} = \frac{(3n+1)(3n+2)}{2}
$$

Now compute the difference:

$$
t_{9n+4} - t_{3n+1} = \frac{(9n+4)(9n+5) - (3n+1)(3n+2)}{2}
$$

---

### Step 3: Expand the numerator

First, expand the product $ (9n+4)(9n+5) $:

$$
(9n+4)(9n+5) = 81n^2 + 45n + 36n + 20 = 81n^2 + 81n + 20
$$

Now expand $ (3n+1)(3n+2) $:

$$
(3n+1)(3n+2) = 9n^2 + 6n + 3n + 2 = 9n^2 + 9n + 2
$$

Now subtract the two:

$$
(81n^2 + 81n + 20) - (9n^2 + 9n + 2) = 72n^2 + 72n + 18
$$

Divide by 2:

$$
\frac{72n^2 + 72n + 18}{2} = 36n^2 + 36n + 9
$$

---

### Step 4: Factor the result

$$
36n^2 + 36n + 9 = 9(4n^2 + 4n + 1) = 9(2n+1)^2
$$

---

### Final Conclusion

We have shown that:

$$
t_{9n+4} - t_{3n+1} = 9(2n+1)^2
$$

Thus, the square of any odd multiple of 3 is indeed the difference of the triangular numbers $ t_{9n+4} $ and $ t_{3n+1} $.

---

### Final Answer

$$
\boxed{9(2n + 1)^2}
$$