<think>
Okay, so I need to show that if n is an odd integer, then the expression n⁴ + 4n² + 11 is divisible by 16. In other words, it should be equal to 16 times some integer k. Let me try to figure this out step by step.

First, since n is odd, I can represent it as n = 2m + 1, where m is an integer. Maybe substituting this into the expression will help me see the pattern or simplify the equation. Let me try that.

So, substituting n = 2m + 1 into the expression:

n⁴ + 4n² + 11 = (2m + 1)⁴ + 4*(2m + 1)² + 11.

Now, I need to expand each term. Let me start with (2m + 1)⁴. I remember that (a + b)⁴ can be expanded using the binomial theorem:

(a + b)⁴ = a⁴ + 4a³b + 6a²b² + 4ab³ + b⁴.

Applying this to (2m + 1)⁴:

= (2m)⁴ + 4*(2m)³*1 + 6*(2m)²*1² + 4*(2m)*1³ + 1⁴
= 16m⁴ + 4*8m³ + 6*4m² + 4*2m + 1
= 16m⁴ + 32m³ + 24m² + 8m + 1.

Okay, that's the expansion of (2m + 1)⁴. Now let me expand 4*(2m + 1)². First, compute (2m + 1)²:

(2m + 1)² = 4m² + 4m + 1.

Multiply by 4:

4*(4m² + 4m + 1) = 16m² + 16m + 4.

Now, adding all the terms together:

Original expression is (2m + 1)⁴ + 4*(2m + 1)² + 11.

So substituting the expansions:

[16m⁴ + 32m³ + 24m² + 8m + 1] + [16m² + 16m + 4] + 11.

Let me combine like terms:

First, the m⁴ term: 16m⁴.

Then the m³ term: 32m³.

Next, the m² terms: 24m² + 16m² = 40m².

Then the m terms: 8m + 16m = 24m.

Constant terms: 1 + 4 + 11 = 16.

So putting it all together:

16m⁴ + 32m³ + 40m² + 24m + 16.

Now, the problem says this should be of the form 16k. Let me factor out 16 from each term:

16*(m⁴ + 2m³ + 2.5m² + 1.5m + 1). Wait, that doesn't seem right. Because 40m² divided by 16 is 2.5, which is not an integer. Hmm, that suggests I made a mistake in my calculation. Wait, no, actually, maybe I need to check my expansion again.

Wait, let me check the expansion again step by step.

First, expanding (2m + 1)^4:

First term: (2m)^4 = 16m^4. Correct.

Second term: 4*(2m)^3*1 = 4*(8m^3) = 32m^3. Correct.

Third term: 6*(2m)^2*1^2 = 6*(4m^2) = 24m^2. Correct.

Fourth term: 4*(2m)*1^3 = 4*(2m) = 8m. Correct.

Fifth term: 1^4 = 1. Correct.

So that part is correct. Then 4*(2m + 1)^2:

(2m + 1)^2 = 4m² + 4m + 1. Multiply by 4: 16m² + 16m + 4. Correct.

Then adding all terms:

Original expression:

(16m⁴ + 32m³ + 24m² + 8m + 1) + (16m² + 16m + 4) + 11.

So combining:

16m⁴ + 32m³ + (24m² + 16m²) + (8m + 16m) + (1 + 4 + 11).

So:

16m⁴ + 32m³ + 40m² + 24m + 16. Yes, that's correct.

So factoring 16 out:

16*(m⁴ + 2m³ + (40/16)m² + (24/16)m + 1). Wait, but 40/16 is 2.5 and 24/16 is 1.5. That's not helpful because we need the entire expression to be 16 times an integer. But here, the coefficients inside the parentheses are not integers. That suggests that maybe my approach is wrong?

Wait, but the original expression is supposed to be divisible by 16. However, when I expanded it, I get 16*(something), but the something is not an integer? That can't be. Therefore, I must have made a mistake in my expansion. Wait, but how?

Wait, maybe I need to check if the entire expression is indeed divisible by 16. Let me compute the expression for a specific odd integer and see if it is divisible by 16. Let's take n = 1.

n = 1: 1^4 + 4*(1)^2 + 11 = 1 + 4 + 11 = 16. 16 is 16*1, so that works.

n = 3: 3^4 + 4*(3)^2 + 11 = 81 + 36 + 11 = 128. 128 divided by 16 is 8. So that works.

n = 5: 625 + 4*25 + 11 = 625 + 100 + 11 = 736. 736 divided by 16 is 46. So that's 16*46. Okay, that works too.

So maybe my expansion is correct, but the problem is that when I factor out 16, the remaining terms are not integers? But that can't be, because the original expression is an integer, so when I factor out 16, the remaining part must be an integer. Therefore, I must have made an error in my algebra.

Wait, let me check again:

Original expression after expansion:

16m⁴ + 32m³ + 40m² + 24m + 16.

Let me factor 16 out:

16*(m⁴ + 2m³ + (40/16)m² + (24/16)m + 1). Wait, but that's not correct. Wait, no, actually, the entire expression is 16m⁴ + 32m³ + 40m² + 24m + 16. So if I factor 16 from each term:

16*(m⁴ + 2m³ + (40/16)m² + (24/16)m + 1). But that's not correct. Wait, actually, no. Wait, 16m⁴ is 16*(m⁴), 32m³ is 16*(2m³), 40m² is 16*(2.5m²), 24m is 16*(1.5m), and 16 is 16*1. So that's correct. But how can that be? Because the entire expression is 16 times something, but that something is not an integer? But that's impossible because the original expression is an integer. Therefore, there must be a mistake here. Wait, but when I tested with n=1, m=(1-1)/2=0. Let's plug m=0 into the expression:

16*(0 + 0 + 0 + 0 + 1) = 16*1=16. Which is correct. For m=0, that works. For m=1 (n=3):

Original expression: 16*(1 + 2 + 2.5 + 1.5 + 1) = 16*(1 + 2 + 2.5 + 1.5 + 1) = 16*(8) = 128. Which is correct. Wait, but 1 + 2 + 2.5 + 1.5 + 1 = 8? Let me check:

1 + 2 is 3, plus 2.5 is 5.5, plus 1.5 is 7, plus 1 is 8. Yes, that's correct. So even though the coefficients inside the parentheses are fractions, when you add them up, they result in an integer. Therefore, the entire expression is 16 times an integer. So maybe my initial thought was wrong. The problem is that when I factor out 16, the remaining terms are not integers individually, but their sum is. Therefore, the expression is indeed divisible by 16. Therefore, the conclusion is that n⁴ + 4n² + 11 is 16k for some integer k. Therefore, the problem is solved? But maybe I need to show it more formally.

Alternatively, maybe there's another approach. Let me think.

Since n is odd, n can be written as 2m + 1. But maybe instead of expanding everything, I can consider modulo 16. Let me try that approach.

If I can show that n⁴ + 4n² + 11 ≡ 0 mod 16 for any odd integer n, then that would suffice.

So let me consider n is odd. Let me note that any odd integer can be congruent to 1, 3, 5, 7, 9, 11, 13, 15 mod 16. But since n is odd, it's equivalent to 1, 3, 5, 7, 9, 11, 13, 15 mod 16. However, since we are working mod 16, maybe we can check for n ≡ 1, 3, 5, 7 mod 16? Wait, but maybe there's a pattern.

Alternatively, since n is odd, n ≡ 1 or 3 mod 4. Wait, but mod 16 is more detailed. Alternatively, perhaps we can note that for odd integers, n² ≡ 1 mod 8. Wait, let me check.

For any odd integer n, n = 2k + 1. Then n² = 4k(k + 1) + 1. Since either k or k + 1 is even, so 4k(k + 1) is divisible by 8. Therefore, n² ≡ 1 mod 8. Therefore, n² ≡ 1 mod 8. Therefore, n² = 8m + 1 for some integer m.

Similarly, n⁴ = (n²)² = (8m + 1)² = 64m² + 16m + 1. Therefore, n⁴ ≡ 1 mod 16? Wait, let's check.

Wait, if n² ≡ 1 mod 8, then n² can be 1 or 9 mod 16? Wait, let me check. Let me take n odd:

If n ≡ 1 mod 16: n² ≡ 1 mod 16.

If n ≡ 3 mod 16: 3² = 9 mod 16.

n ≡ 5 mod 16: 25 ≡ 9 mod 16.

n ≡ 7 mod 16: 49 ≡ 1 mod 16.

n ≡ 9 mod 16: 81 ≡ 1 mod 16.

n ≡ 11 mod 16: 121 ≡ 9 mod 16.

n ≡ 13 mod 16: 169 ≡ 9 mod 16.

n ≡ 15 mod 16: 225 ≡ 1 mod 16.

So, in fact, for odd n, n² ≡ 1 or 9 mod 16. Therefore, n² ≡ 1 mod 8, but mod 16, it's either 1 or 9.

Therefore, n⁴ = (n²)². If n² ≡ 1 mod 16, then n⁴ ≡ 1² = 1 mod 16. If n² ≡ 9 mod 16, then n⁴ ≡ 9² = 81 ≡ 1 mod 16. Therefore, in either case, n⁴ ≡ 1 mod 16. Therefore, n⁴ ≡ 1 mod 16.

Therefore, n⁴ + 4n² + 11 ≡ 1 + 4n² + 11 mod 16.

So that's 12 + 4n² mod 16.

But since n² ≡ 1 or 9 mod 16, let's compute 4n²:

If n² ≡ 1 mod 16, then 4n² ≡ 4*1 = 4 mod 16.

If n² ≡ 9 mod 16, then 4n² ≡ 4*9 = 36 ≡ 4 mod 16 (since 36 - 2*16 = 4).

Therefore, in both cases, 4n² ≡ 4 mod 16. Therefore, the entire expression is 12 + 4 = 16 ≡ 0 mod 16. Therefore, n⁴ + 4n² + 11 ≡ 0 mod 16. Therefore, it is divisible by 16. Therefore, the expression is of the form 16k.

So this approach works. Therefore, the answer is proven by considering modulo 16.

But let me check with the earlier expansion. Earlier, when I expanded, I had 16m⁴ + 32m³ + 40m² + 24m + 16. Let me check if this is divisible by 16. Well, 16m⁴ is divisible by 16, 32m³ is divisible by 16, 40m² is 16*2.5m², but 24m is 16*1.5m, and 16 is 16*1. However, when I tested with specific values, like m=0 (n=1), it worked. For m=1 (n=3), it worked. So even though the coefficients inside the parentheses are fractions, when combined, they result in an integer. Therefore, the entire expression is divisible by 16.

But maybe there's another way to see this. Let me try another approach. Since n is odd, let me write n = 2k + 1. Then compute n²:

n² = (2k + 1)^2 = 4k² + 4k + 1 = 4k(k + 1) + 1. Since k and k + 1 are consecutive integers, one of them is even, so 4k(k + 1) is divisible by 8. Therefore, n² = 8m + 1 for some integer m. Therefore, n² ≡ 1 mod 8. Therefore, n² = 8m + 1. Then n⁴ = (n²)^2 = (8m + 1)^2 = 64m² + 16m + 1. Therefore, n⁴ = 16*(4m² + m) + 1. Therefore, n⁴ ≡ 1 mod 16. Therefore, n⁴ + 4n² + 11 ≡ 1 + 4*(8m + 1) + 11 mod 16. Let me compute that:

1 + 4*(8m + 1) + 11 = 1 + 32m + 4 + 11 = 32m + 16. 32m is divisible by 16, and 16 is 16*1. Therefore, 32m + 16 ≡ 0 mod 16. Therefore, the expression is divisible by 16. Therefore, that's another way to see it.

So this seems to confirm the result. Therefore, regardless of the approach, the expression is divisible by 16. Therefore, the original statement is proven.

Alternatively, maybe I can use induction? Although for induction, I need to check the base case and then assume it's true for n and show for n + 2 or something. But since n is odd, maybe induction is possible, but perhaps more complicated.

Alternatively, maybe I can look at the expression n⁴ + 4n² + 11 and try to factor it or rewrite it. Let me see.

n⁴ + 4n² + 11. Hmm. Maybe complete the square or something. Let me try:

n⁴ + 4n² + 4 + 7 = (n² + 2)^2 + 7. Not sure if that helps. Alternatively, n⁴ + 4n² + 11. Maybe not helpful.

Alternatively, think about n⁴ + 4n² + 11 = n⁴ + 4n² + 4 + 7 = (n² + 2)^2 + 7. But again, not sure.

Alternatively, since we know that n is odd, maybe write n = 2k + 1 and substitute into the expression:

(2k + 1)^4 + 4*(2k + 1)^2 + 11. Which is what I did earlier, and then expanded to 16m⁴ + 32m³ + 40m² + 24m + 16. Which is 16*(m⁴ + 2m³ + 2.5m² + 1.5m + 1). But since m is integer, maybe the fractional parts cancel out?

Wait, let me check for m integer:

Let me write 40m² + 24m as 16*(2.5m² + 1.5m). But 2.5m² + 1.5m = (5m² + 3m)/2. Therefore, the entire expression is 16*(m⁴ + 2m³ + (5m² + 3m)/2 + 1). Therefore, to have this be an integer, (5m² + 3m)/2 must be integer. Let me check if that is the case.

Since m is integer, 5m² + 3m = m(5m + 3). Let me check if this is even. Let me consider m even or odd.

If m is even: m = 2p. Then 5m + 3 = 10p + 3, which is odd. Therefore, m(5m + 3) = 2p*(odd) which is even. Therefore, (5m² + 3m)/2 is integer.

If m is odd: m = 2p + 1. Then 5m + 3 = 5*(2p + 1) + 3 = 10p + 5 + 3 = 10p + 8 = 2*(5p + 4), which is even. Therefore, m(5m + 3) = (2p + 1)*even, which is even. Therefore, again, (5m² + 3m)/2 is integer.

Therefore, regardless of m being even or odd, (5m² + 3m)/2 is integer. Therefore, the entire expression is 16 times an integer. Therefore, the original expression is divisible by 16. Therefore, that's another way to see it.

So, in conclusion, whether I use modular arithmetic, substitution and expansion, or check divisibility by 16 through the expression's components, I arrive at the conclusion that n⁴ + 4n² + 11 is divisible by 16 when n is odd.

Therefore, the problem is solved.

**Final Answer**
\boxed{16k}
</think>

To show that $ n^4 + 4n^2 + 11 $ is of the form $ 16k $ when $ n $ is an odd integer, we proceed by analyzing the structure of the expression and leveraging modular arithmetic.

---

### Step 1: Understand the Nature of $ n $

Let $ n $ be an odd integer. Then we can write $ n = 2m + 1 $, where $ m \in \mathbb{Z} $. This representation helps us analyze the expression in terms of even and odd components.

---

### Step 2: Use Modular Arithmetic

We aim to show that $ n^4 + 4n^2 + 11 \equiv 0 \mod 16 $ for all odd $ n $. This is equivalent to showing that the expression is divisible by 16.

First, recall that for any odd integer $ n $, we have:

$$
n^2 \equiv 1 \mod 8
$$

But more precisely, when considering modulo 16, we find that:

- If $ n \equiv 1, 7, 9, 15 \mod 16 $, then $ n^2 \equiv 1 \mod 16 $
- If $ n \equiv 3, 5, 11, 13 \mod 16 $, then $ n^2 \equiv 9 \mod 16 $

In both cases, $ n^2 \equiv 1 \text{ or } 9 \mod 16 $, and hence:

$$
n^4 = (n^2)^2 \equiv 1^2 = 1 \mod 16 \quad \text{or} \quad 9^2 = 81 \equiv 1 \mod 16
$$

Thus, in all cases, $ n^4 \equiv 1 \mod 16 $.

---

### Step 3: Compute the Expression Modulo 16

Now we compute:

$$
n^4 + 4n^2 + 11 \equiv 1 + 4n^2 + 11 \mod 16
$$

We know $ n^2 \equiv 1 \text{ or } 9 \mod 16 $, so:

- If $ n^2 \equiv 1 \mod 16 $, then $ 4n^2 \equiv 4 \mod 16 $
- If $ n^2 \equiv 9 \mod 16 $, then $ 4n^2 \equiv 36 \equiv 4 \mod 16 $

So in both cases:

$$
n^4 + 4n^2 + 11 \equiv 1 + 4 + 11 = 16 \equiv 0 \mod 16
$$

---

### Step 4: Conclusion

Since the expression is congruent to 0 modulo 16 for all odd integers $ n $, it follows that:

$$
n^4 + 4n^2 + 11 = 16k \quad \text{for some integer } k
$$

---

### Final Answer

$$
\boxed{16k}
$$