<think>
Okay, so I need to prove that if a and b are integers, not both zero, then the greatest common divisor of 2a - 3b and 4a - 5b divides b. Then, using that result, I have to show that gcd(2a + 3, 4a + 5) is 1. Hmm, let me start by recalling some number theory concepts. 

First, the problem is about gcds and divisibility. I remember that if d divides two numbers, then it divides any linear combination of those numbers. So maybe I can use the Euclidean algorithm here? The Euclidean algorithm says that gcd(m, n) = gcd(n, m - kn) for any integer k. Maybe I can apply that here.

Let me denote the two numbers as m = 2a - 3b and n = 4a - 5b. I need to find gcd(m, n) and show that it divides b. Let me try to express m and n in terms that can help me find their gcd.

Alternatively, maybe I can find a linear combination of m and n that gives me something involving b. Let me try to compute n - 2m. Let's see:

n - 2m = (4a - 5b) - 2*(2a - 3b) = 4a - 5b - 4a + 6b = (4a - 4a) + (-5b + 6b) = 0 + b = b. 

Oh! So n - 2m equals b. That means that the difference between n and 2m is b. Therefore, any common divisor of m and n must also divide b. Because if d divides both m and n, then d divides their difference, which is b. Therefore, gcd(m, n) divides b. So that's the first part of the problem. 

So that's the first part. Therefore, gcd(2a - 3b, 4a - 5b) divides b. 

Now, the second part is to show that gcd(2a + 3, 4a + 5) = 1. Wait, but how does this relate to the first part? Maybe I need to adjust the variables to fit into the first part's structure. Let me think.

Let me consider the second part. Let me denote x = 2a + 3 and y = 4a + 5. I need to show that gcd(x, y) = 1. Let me try to apply the same method as before. Let me compute y - 2x. 

y - 2x = (4a + 5) - 2*(2a + 3) = 4a + 5 - 4a - 6 = (4a - 4a) + (5 - 6) = 0 - 1 = -1. 

So, y - 2x = -1. Therefore, gcd(x, y) divides -1, which is 1. Therefore, gcd(x, y) must be 1. 

Wait, so that's straightforward? Because if the difference between y and 2x is -1, then the gcd of x and y divides 1, hence it must be 1. Therefore, gcd(2a + 3, 4a + 5) = 1. 

But wait, the problem says "hence, gcd(2a + 3, 4a + 5) = 1". So maybe they want me to use the first part's result? Let me check if there's a connection.

Alternatively, maybe I can relate 2a + 3 and 4a + 5 to the first part. Let me think. If I set up variables similar to the first problem. Let me see. In the first problem, we had 2a - 3b and 4a - 5b. In the second problem, it's 2a + 3 and 4a + 5. Maybe I can think of b as some value here. Wait, but in the second problem, there is no b. Maybe I need to adjust variables.

Alternatively, maybe I can think of the second problem as a special case of the first problem. Let me try. Suppose I set b = 1? Wait, but in the first problem, we have variables a and b. Maybe I need to adjust the coefficients. Let me think.

Alternatively, perhaps the second problem is similar to the first problem but with different coefficients. Let me try to use the same approach as in the first part. Let me denote m = 2a + 3 and n = 4a + 5. Then, as before, n - 2m = -1, so gcd(m, n) divides -1, hence 1. Therefore, the gcd is 1. 

But why does the problem say "hence"? Maybe there is a way to use the first part's result? Let me check. The first part says that gcd(2a - 3b, 4a - 5b) divides b. So if I can somehow relate 2a + 3 and 4a + 5 to that structure. 

Wait, maybe if I set b to some value. Let me think. Suppose I set 2a - 3b = 2a + 3 and 4a - 5b = 4a + 5. Then, solving for b. Let me see:

From 2a - 3b = 2a + 3, subtract 2a: -3b = 3 => b = -1.

Then check if 4a - 5b = 4a + 5. Substitute b = -1: 4a -5*(-1) = 4a + 5. Which is correct. So if I set b = -1, then 2a - 3b = 2a + 3 and 4a - 5b = 4a + 5. Therefore, according to the first part, gcd(2a + 3, 4a + 5) divides b, which is -1. Therefore, gcd divides -1, hence gcd is 1. 

Therefore, that's another way to see it. So since in this case, the gcd divides b, which is -1, so it must be 1. Therefore, that's the "hence" part. 

So, putting it all together: first part is proved by showing that the gcd divides b, and then for the second part, by setting b = -1, we can apply the first part's result to show that the gcd divides -1, hence is 1. 

But let me check if that is correct. Let me verify with an example. Let me take a = 1. Then 2a + 3 = 5, 4a + 5 = 9. gcd(5, 9) is 1. If a = 2, then 2a + 3 = 7, 4a + 5 = 13, gcd(7, 13) is 1. If a = 0, then 2a + 3 = 3, 4a + 5 = 5, gcd(3, 5) is 1. If a = -1, then 2*(-1) + 3 = 1, 4*(-1) + 5 = 1, gcd(1, 1) is 1. So that works. 

Alternatively, if I take a = 1, b = -1, then 2a - 3b = 2*1 - 3*(-1) = 2 + 3 = 5, and 4a - 5b = 4*1 - 5*(-1) = 4 + 5 = 9, which is the same as before. So indeed, gcd(5, 9) divides b = -1, so it must be 1. 

Therefore, the reasoning is correct. 

But let me think again about the first part. The problem says "prove that gcd(2a - 3b, 4a - 5b) divides b". So I need to make sure that my first part is correct. 

Let me recall that if d divides both m and n, then d divides any linear combination of m and n. So if I have m = 2a - 3b and n = 4a - 5b, then n - 2m = b. Therefore, if d divides m and n, then d divides b. Therefore, d divides b. Therefore, gcd(m, n) divides b. 

Yes, that's correct. Therefore, the first part is proved. 

Therefore, the second part is a special case where we set b = -1, so that 2a - 3b = 2a + 3 and 4a - 5b = 4a + 5. Then, since gcd(2a - 3b, 4a - 5b) divides b = -1, so the gcd must be 1. 

Therefore, the conclusion is that gcd(2a + 3, 4a + 5) = 1. 

Alternatively, maybe there's another way to think about it. Let me try using the Euclidean algorithm directly on 2a + 3 and 4a + 5. 

Let me denote x = 2a + 3 and y = 4a + 5. Then, compute gcd(x, y). 

First, divide y by x. Let me see: y = 2x + (4a + 5 - 2*(2a + 3)) = 2x + (4a + 5 - 4a - 6) = 2x - 1. Therefore, y = 2x - 1. Therefore, gcd(x, y) = gcd(x, 2x - 1). 

Then, gcd(x, 2x - 1) = gcd(x, -1) = 1, since gcd(x, -1) is 1 for any integer x. Therefore, the gcd is 1. 

So that's another way to see it. Therefore, regardless of the value of a, the gcd is 1. 

But in this case, the problem says "hence", so maybe they want us to use the first part's result. But both methods are valid. 

But since the problem says "hence", maybe the first part is supposed to be used. So if we use the first part, then by setting b = -1, we can apply the first part's result. 

Therefore, the answer is that the gcd is 1. 

So, in summary:

First part: Let d = gcd(2a - 3b, 4a - 5b). Then, since 4a - 5b - 2*(2a - 3b) = b, so d divides b. Therefore, d divides b.

Second part: Letâ€™s set b = -1. Then, gcd(2a - 3*(-1), 4a - 5*(-1)) = gcd(2a + 3, 4a + 5). From the first part, this gcd divides b = -1, so it must be 1. Therefore, gcd(2a + 3, 4a + 5) = 1.

Therefore, the conclusion is correct.

I think that's thorough. Let me check if there are any edge cases. For example, if a = 0, then 2a + 3 = 3, 4a + 5 = 5, gcd(3,5)=1. If a = -1, 2*(-1) + 3 = 1, 4*(-1) + 5 = 1, gcd(1,1)=1. If a = 1, 5 and 9, gcd is 1. So all these cases work. 

Another way: suppose that there is a common divisor d > 1 of 2a + 3 and 4a + 5. Then, d divides 2a + 3 and 4a + 5. Then, d divides 4a + 5 - 2*(2a + 3) = 4a + 5 - 4a - 6 = -1. Therefore, d divides -1, so d = 1. Therefore, gcd is 1. 

So that's another way. Therefore, regardless of the method, the conclusion is 1. 

Therefore, the answer is \boxed{1}.

**Final Answer**
\boxed{1}
</think>

To prove the given statements, we analyze the structure of the greatest common divisors (gcds) of two expressions involving integers $ a $ and $ b $, and apply number-theoretic reasoning.

---

### **Part 1: Prove that $ \gcd(2a - 3b, 4a - 5b) $ divides $ b $**

Let:
- $ m = 2a - 3b $
- $ n = 4a - 5b $

We compute the difference $ n - 2m $:
$$
n - 2m = (4a - 5b) - 2(2a - 3b) = 4a - 5b - 4a + 6b = b
$$

This shows that $ n - 2m = b $, which means that **any common divisor of $ m $ and $ n $ must also divide $ b $**. Therefore, the gcd of $ m $ and $ n $ divides $ b $.

Thus, we conclude:
$$
\gcd(2a - 3b, 4a - 5b) \mid b
$$

---

### **Part 2: Show that $ \gcd(2a + 3, 4a + 5) = 1 $**

We now consider the expressions:
- $ x = 2a + 3 $
- $ y = 4a + 5 $

We compute the difference $ y - 2x $:
$$
y - 2x = (4a + 5) - 2(2a + 3) = 4a + 5 - 4a - 6 = -1
$$

This means that $ y - 2x = -1 $, so the gcd of $ x $ and $ y $ divides $ -1 $, which implies:
$$
\gcd(x, y) = 1
$$

Therefore:
$$
\gcd(2a + 3, 4a + 5) = 1
$$

Alternatively, we can also use the result from Part 1. If we set $ b = -1 $, then:
- $ 2a - 3b = 2a + 3 $
- $ 4a - 5b = 4a + 5 $

So, by Part 1, we know that:
$$
\gcd(2a + 3, 4a + 5) \mid b = -1
$$
Thus, the gcd must be 1, since the only divisor of $ -1 $ is 1.

---

### **Conclusion**

From the above, we have shown that:
- $ \gcd(2a - 3b, 4a - 5b) $ divides $ b $
- Therefore, $ \gcd(2a + 3, 4a + 5) = 1 $

$$
\boxed{1}
$$