<think>
Okay, so I need to use mathematical induction to prove these divisibility statements for parts (a) through (e). Let me start with part (a): 8 divides 5^(2n) + 7. 

First, I remember that mathematical induction has two main steps: the base case and the inductive step. For the base case, I need to check if the statement holds when n=1. Let me compute 5^(2*1) + 7. That's 5² + 7 = 25 + 7 = 32. And 32 divided by 8 is 4, which is an integer. So the base case holds. Good.

Now for the inductive step. The hint says that 5^{2(k+l)} + 7 = 5²(5^{2k} + 7) + (7 - 5² * 7). Wait, maybe I need to rephrase that. Let me think. The hint is probably suggesting a way to express 5^{2(k+1)} + 7 in terms of 5^{2k} + 7. Let me check. If I have 5^{2(k+1)} + 7, that's 5^{2k + 2} + 7. Which is 5² * 5^{2k} + 7. So maybe the hint is trying to write this as 5²*(something) + something else. Let me see. The hint says 5^{2(k + l)} + 7 = 5²(5^{2k} + 7) + (7 - 5² * 7). Wait, but if l is a variable here? Maybe it's a typo? Maybe they meant 5^{2(k + 1)} + 7? Let me check the original problem again. The hint says: 5^{2(k+l)} + 7 = 5²(5^{2k} + 7) + (7 - 5² * 7). Hmm. Maybe l is supposed to be 1? Maybe the hint is for the inductive step where we go from k to k+1. Let me try to use that.

So, if we have 5^{2(k+1)} + 7. Let me write that as 5^{2k + 2} + 7. Which is 5² * 5^{2k} + 7. Now, if I factor out 5², I get 5²*(5^{2k}) + 7. But the hint says to write it as 5²*(5^{2k} + 7) + (7 - 5² * 7). Let me check that. Let me compute 5²*(5^{2k} + 7) + (7 - 5² * 7). That would be 5²*5^{2k} + 5²*7 + 7 - 5²*7. The 5²*7 and -5²*7 cancel out, leaving 5²*5^{2k} + 7. Which is exactly 5^{2k + 2} + 7. So that works. Therefore, the hint is telling me that 5^{2(k+1)} + 7 can be written as 5²*(5^{2k} + 7) + (7 - 5² * 7). 

But since we are trying to do induction, we need to assume that 5^{2k} + 7 is divisible by 8, i.e., 8 divides 5^{2k} + 7. Then, if we can show that 5^{2(k+1)} + 7 is divisible by 8, then the inductive step is done. 

So, according to the hint, 5^{2(k+1)} + 7 = 5²*(5^{2k} + 7) + (7 - 5² * 7). Let me compute 7 - 5² * 7. That is 7 - 25*7 = 7 - 175 = -168. So, 5^{2(k+1)} + 7 = 25*(5^{2k} + 7) - 168. 

Now, since 8 divides 5^{2k} + 7, then 5^{2k} + 7 = 8m for some integer m. Then substituting back, we get 25*(8m) - 168. Which is 200m - 168. Now, 200m is divisible by 8 because 200 divided by 8 is 25. So 200m is 8*25m. Then 200m - 168 = 8*(25m) - 168. Now, 168 divided by 8 is 21, so 168 = 8*21. Therefore, 200m - 168 = 8*(25m - 21). Which is clearly divisible by 8. Therefore, 5^{2(k+1)} + 7 is divisible by 8. Hence, the inductive step is proven. Therefore, by induction, the statement holds for all n ≥ 1. 

Okay, that seems to work. Let me check with n=2. 5^(4) + 7 = 625 + 7 = 632. Divided by 8 is 79, which is an integer. So that works. Good.

Now moving on to part (b): 15 divides 2^{4n} - 1. So 15 | 2^{4n} - 1. Let me check the base case first. For n=1, 2^4 - 1 = 16 - 1 = 15, which is divisible by 15. So base case holds.

Now the inductive step. Assume that for some k ≥ 1, 15 divides 2^{4k} - 1. So 2^{4k} ≡ 1 mod 15. Need to show that 2^{4(k+1)} - 1 is divisible by 15. Let me compute 2^{4(k+1)} - 1 = 2^{4k + 4} - 1 = 2^4 * 2^{4k} - 1 = 16 * 2^{4k} - 1. 

Now, since 2^{4k} ≡ 1 mod 15, then 16 * 2^{4k} ≡ 16 * 1 = 16 mod 15. 16 mod 15 is 1. Therefore, 16 * 2^{4k} - 1 ≡ 1 - 1 = 0 mod 15. Therefore, 15 divides 2^{4(k+1)} - 1. Hence, the inductive step is proven. Therefore, by induction, the statement holds for all n ≥ 1.

Wait, but maybe I should write it more formally. Let me try again. Suppose that for some k ≥ 1, 2^{4k} - 1 is divisible by 15. Then 2^{4k} = 15m + 1 for some integer m. Then 2^{4(k+1)} - 1 = 2^4 * 2^{4k} - 1 = 16*(15m + 1) - 1 = 240m + 16 - 1 = 240m + 15 = 15*(16m + 1). Which is clearly divisible by 15. Therefore, done. So that works. So part (b) is done.

Moving on to part (c): 5 divides 3^{3n + 1} + 2^{n + 1}. So 5 | 3^{3n + 1} + 2^{n + 1}. Let me check the base case n=1: 3^{4} + 2^{2} = 81 + 4 = 85. 85 divided by 5 is 17, which is integer. So base case holds.

Now the inductive step. Assume that for some k ≥ 1, 5 divides 3^{3k + 1} + 2^{k + 1}. Need to show that 5 divides 3^{3(k+1) + 1} + 2^{(k+1) + 1} = 3^{3k + 4} + 2^{k + 2}.

Let me write 3^{3k + 4} as 3^{3k + 1} * 3^3. And 3^3 is 27. So 27 * 3^{3k + 1} + 2^{k + 2}. 

But I need to relate this to the inductive hypothesis. The inductive hypothesis says that 3^{3k + 1} + 2^{k + 1} is divisible by 5. Let me denote that as 3^{3k + 1} + 2^{k + 1} = 5m for some integer m. 

But how can I express 3^{3k + 4} + 2^{k + 2} in terms of that? Let me see. Let me write 3^{3k + 4} + 2^{k + 2} = 27 * 3^{3k + 1} + 2 * 2^{k + 1}. 

So that's 27 * 3^{3k + 1} + 2 * 2^{k + 1}. Now, if I can express this as something involving the inductive hypothesis. Let me think. Since 3^{3k + 1} = 5m - 2^{k + 1} from the inductive hypothesis. Substitute that into the expression:

27*(5m - 2^{k + 1}) + 2*2^{k + 1} = 27*5m - 27*2^{k + 1} + 2*2^{k + 1} = 135m - 25*2^{k + 1}.

Now, 135m is divisible by 5, and 25*2^{k + 1} is also divisible by 5. Therefore, the entire expression is divisible by 5. Therefore, 5 divides 3^{3(k+1) + 1} + 2^{(k+1) + 1}. Hence, the inductive step is proven. Therefore, by induction, the statement holds for all n ≥ 1.

Wait, let me check with n=2. 3^{3*2 + 1} + 2^{2 + 1} = 3^7 + 2^3 = 2187 + 8 = 2195. Divided by 5 is 439, which is integer. So that works. Okay.

Part (d): 21 divides 4^{n + 1} + 5^{2n - 1}. So 21 | 4^{n + 1} + 5^{2n - 1}. Let me check the base case n=1: 4^{2} + 5^{1} = 16 + 5 = 21. Which is divisible by 21. So base case holds.

Now the inductive step. Assume that for some k ≥ 1, 21 divides 4^{k + 1} + 5^{2k - 1}. Need to show that 21 divides 4^{(k + 1) + 1} + 5^{2(k + 1) - 1} = 4^{k + 2} + 5^{2k + 1}.

So, let me write 4^{k + 2} + 5^{2k + 1} = 4*4^{k + 1} + 5^2 * 5^{2k - 1} = 4*4^{k + 1} + 25*5^{2k - 1}.

Now, from the inductive hypothesis, 4^{k + 1} + 5^{2k - 1} is divisible by 21. Let me denote that as 4^{k + 1} + 5^{2k - 1} = 21m for some integer m. 

But how can I relate this to the expression 4*4^{k + 1} + 25*5^{2k - 1}? Let me try to express it in terms of 4^{k + 1} and 5^{2k - 1}. Let me write:

4*4^{k + 1} + 25*5^{2k - 1} = 4*4^{k + 1} + 25*5^{2k - 1}.

But since 4^{k + 1} = 21m - 5^{2k - 1} from the inductive hypothesis. Substitute that into the expression:

4*(21m - 5^{2k - 1}) + 25*5^{2k - 1} = 84m - 4*5^{2k - 1} + 25*5^{2k - 1} = 84m + 21*5^{2k - 1}.

Now, 84m is divisible by 21 (since 84 = 4*21), and 21*5^{2k - 1} is obviously divisible by 21. Therefore, the entire expression is divisible by 21. Therefore, 21 divides 4^{k + 2} + 5^{2k + 1}, which is what we needed. Hence, the inductive step is proven. Therefore, by induction, the statement holds for all n ≥ 1.

Let me check with n=2. 4^{3} + 5^{3} = 64 + 125 = 189. 189 divided by 21 is 9, which is integer. Correct.

Now part (e): 24 divides 2*7^n + 3*5^n - 5. So 24 | 2*7^n + 3*5^n - 5. Let me check the base case n=1: 2*7 + 3*5 - 5 = 14 + 15 - 5 = 24. Which is divisible by 24. So base case holds.

Now the inductive step. Assume that for some k ≥ 1, 24 divides 2*7^k + 3*5^k - 5. Need to show that 24 divides 2*7^{k+1} + 3*5^{k+1} - 5.

Let me write 2*7^{k+1} + 3*5^{k+1} - 5 = 2*7*7^k + 3*5*5^k - 5.

So that's 14*7^k + 15*5^k - 5. Now, I need to relate this to the inductive hypothesis. The inductive hypothesis says that 2*7^k + 3*5^k - 5 is divisible by 24. Let me denote that as 2*7^k + 3*5^k - 5 = 24m for some integer m.

But how can I express 14*7^k + 15*5^k - 5 in terms of that? Let me try to manipulate the expression:

14*7^k + 15*5^k - 5 = 7*(2*7^k) + 5*(3*5^k) - 5.

But from the inductive hypothesis, 2*7^k = 24m - 3*5^k + 5. Substitute that into the expression:

7*(24m - 3*5^k + 5) + 5*(3*5^k) - 5 = 7*24m - 21*5^k + 35 + 15*5^k - 5.

Simplify the terms:

-21*5^k + 15*5^k = -6*5^k.

35 - 5 = 30.

So overall, we have 7*24m - 6*5^k + 30.

Now, 7*24m is divisible by 24. So the entire expression is 24*(7m) - 6*5^k + 30. Therefore, we need to check if -6*5^k + 30 is divisible by 24. Let me compute that.

-6*5^k + 30 = -6*5^k + 6*5 = 6*(5 - 5^k). Wait, no. Wait 30 is 6*5. So:

-6*5^k + 6*5 = 6*(5 - 5^k). Hmm. Wait, but that's 6*(5 - 5^k). Let me check if that is divisible by 24. Wait, but maybe I made a mistake here. Let me re-express:

Wait, the expression is -6*5^k + 30. Let me factor out -6:

-6*(5^k - 5). So that's -6*(5^k - 5). So we need to check if this is divisible by 24. Let me compute 5^k - 5 modulo 24/ gcd(6,24). Wait, maybe it's better to compute directly.

Alternatively, maybe I need to find a way to express this in terms of the inductive hypothesis. Wait, perhaps I made a mistake in substitution. Let me check again.

Original expression after substitution: 7*24m - 6*5^k + 30. So, 7*24m is 24*(7m). Then, the rest is -6*5^k + 30. So we need to check if -6*5^k + 30 is divisible by 24. Let me compute this expression:

Let me write it as 30 - 6*5^k = 6*(5 - 5^k). Wait, no: 30 is 6*5, so 6*5 - 6*5^k = 6*(5 - 5^k). Therefore, 6*(5 - 5^k). So for this to be divisible by 24, 6*(5 - 5^k) must be divisible by 24. Which simplifies to (5 - 5^k) must be divisible by 4. Because 6 and 24 have a gcd of 6, so 24 divides 6*(something) iff 4 divides (something). Therefore, we need to check if 5 - 5^k is divisible by 4.

Let me check 5^k mod 4. Since 5 ≡ 1 mod 4, so 5^k ≡ 1^k = 1 mod 4. Therefore, 5 - 5^k ≡ 5 - 1 = 4 ≡ 0 mod 4. Therefore, 5 - 5^k is divisible by 4. Therefore, 6*(something divisible by 4) is 24*(something), which is divisible by 24. Therefore, the entire expression is divisible by 24. Therefore, 2*7^{k+1} + 3*5^{k+1} - 5 is divisible by 24. Hence, the inductive step is proven.

Therefore, by induction, the statement holds for all n ≥ 1.

Wait, let me check with n=2. 2*7^2 + 3*5^2 -5 = 2*49 + 3*25 -5 = 98 + 75 -5 = 168. 168 divided by 24 is 7, which is integer. Correct. So that works.

So all parts seem to be done. Let me just recap each part to make sure I didn't make any mistakes.

(a) Used the hint to express 5^{2(k+1)} +7 in terms of 5^{2k} +7, then used the inductive hypothesis to show that the expression is divisible by 8.

(b) Used the fact that 2^{4k} ≡ 1 mod 15, then multiplied by 16 (which is 1 mod 15) to get 16*1 -1 = 15 ≡ 0 mod 15.

(c) Expressed the term in terms of the inductive hypothesis, substituted and found that the expression is a multiple of 5.

(d) Similarly, expressed the term in terms of the inductive hypothesis, substituted and found that it's a multiple of 21.

(e) After substitution, found that the remaining term is a multiple of 24 by showing that 5 - 5^k is divisible by 4.

All steps seem okay. So I think these are correct.

**Final Answer**

(a) \boxed{8} divides $5^{2n} + 7$ for all $n \geq 1$.

(b) \boxed{15} divides $2^{4n} - 1$ for all $n \geq 1$.

(c) \boxed{5} divides $3^{3n+1} + 2^{n+1}$ for all $n \geq 1$.

(d) \boxed{21} divides $4^{n+1} + 5^{2n-1}$ for all $n \geq 1$.

(e) \boxed{24} divides $2 \cdot 7^n + 3 \cdot 5^n - 5$ for all $n \geq 1$.
</think>

To prove the divisibility statements for all $ n \geq 1 $ using **mathematical induction**, we follow a structured approach for each part. Below is a concise and logical breakdown of each problem.

---

### **(a) $ 8 \mid 5^{2n} + 7 $**

**Base Case (n = 1):**  
$$
5^{2 \cdot 1} + 7 = 25 + 7 = 32,\quad \text{which is divisible by 8.}
$$

**Inductive Step:**  
Assume that for some $ k \geq 1 $, $ 8 \mid 5^{2k} + 7 $.  
We need to show that $ 8 \mid 5^{2(k+1)} + 7 $.

Using the identity:
$$
5^{2(k+1)} + 7 = 25(5^{2k} + 7) - 168
$$
Since $ 5^{2k} + 7 \equiv 0 \mod 8 $, the expression becomes:
$$
25 \cdot 0 - 168 = -168 \equiv 0 \mod 8
$$
Thus, $ 8 \mid 5^{2(k+1)} + 7 $.

**Conclusion:**  
By induction, $ 8 \mid 5^{2n} + 7 $ for all $ n \geq 1 $.

$$
\boxed{8}
$$

---

### **(b) $ 15 \mid 2^{4n} - 1 $**

**Base Case (n = 1):**  
$$
2^{4 \cdot 1} - 1 = 16 - 1 = 15,\quad \text{which is divisible by 15.}
$$

**Inductive Step:**  
Assume $ 15 \mid 2^{4k} - 1 $. Then $ 2^{4k} \equiv 1 \mod 15 $.

We want to show that $ 2^{4(k+1)} - 1 \equiv 0 \mod 15 $:
$$
2^{4(k+1)} - 1 = 16 \cdot 2^{4k} - 1 \equiv 16 \cdot 1 - 1 = 15 \equiv 0 \mod 15
$$

**Conclusion:**  
By induction, $ 15 \mid 2^{4n} - 1 $ for all $ n \geq 1 $.

$$
\boxed{15}
$$

---

### **(c) $ 5 \mid 3^{3n+1} + 2^{n+1} $**

**Base Case (n = 1):**  
$$
3^{4} + 2^{2} = 81 + 4 = 85,\quad \text{which is divisible by 5.}
$$

**Inductive Step:**  
Assume $ 5 \mid 3^{3k+1} + 2^{k+1} $. Then:
$$
3^{3(k+1)+1} + 2^{(k+1)+1} = 27 \cdot 3^{3k+1} + 2 \cdot 2^{k+1}
$$
Using the inductive hypothesis, $ 3^{3k+1} = 5m - 2^{k+1} $, so:
$$
27(5m - 2^{k+1}) + 2 \cdot 2^{k+1} = 135m - 25 \cdot 2^{k+1}
$$
Both terms are divisible by 5.

**Conclusion:**  
By induction, $ 5 \mid 3^{3n+1} + 2^{n+1} $ for all $ n \geq 1 $.

$$
\boxed{5}
$$

---

### **(d) $ 21 \mid 4^{n+1} + 5^{2n-1} $**

**Base Case (n = 1):**  
$$
4^{2} + 5^{1} = 16 + 5 = 21,\quad \text{which is divisible by 21.}
$$

**Inductive Step:**  
Assume $ 21 \mid 4^{k+1} + 5^{2k-1} $. Then:
$$
4^{k+2} + 5^{2k+1} = 4 \cdot 4^{k+1} + 25 \cdot 5^{2k-1}
$$
Using the inductive hypothesis, $ 4^{k+1} = 21m - 5^{2k-1} $, so:
$$
4(21m - 5^{2k-1}) + 25 \cdot 5^{2k-1} = 84m + 21 \cdot 5^{2k-1}
$$
Both terms are divisible by 21.

**Conclusion:**  
By induction, $ 21 \mid 4^{n+1} + 5^{2n-1} $ for all $ n \geq 1 $.

$$
\boxed{21}
$$

---

### **(e) $ 24 \mid 2 \cdot 7^n + 3 \cdot 5^n - 5 $**

**Base Case (n = 1):**  
$$
2 \cdot 7 + 3 \cdot 5 - 5 = 14 + 15 - 5 = 24,\quad \text{which is divisible by 24.}
$$

**Inductive Step:**  
Assume $ 24 \mid 2 \cdot 7^k + 3 \cdot 5^k - 5 $. Then:
$$
2 \cdot 7^{k+1} + 3 \cdot 5^{k+1} - 5 = 14 \cdot 7^k + 15 \cdot 5^k - 5
$$
Using the inductive hypothesis, $ 2 \cdot 7^k = 24m - 3 \cdot 5^k + 5 $, so:
$$
14(24m - 3 \cdot 5^k + 5) + 15 \cdot 5^k - 5 = 336m - 42 \cdot 5^k + 70 + 15 \cdot 5^k - 5
$$
Simplify:
$$
336m - 27 \cdot 5^k + 65 = 24(14m) - 27 \cdot 5^k + 65
$$
Since $ 5^k \equiv 1 \mod 4 $, $ 5^k - 5 \equiv 0 \mod 4 $, and thus the expression is divisible by 24.

**Conclusion:**  
By induction, $ 24 \mid 2 \cdot 7^n + 3 \cdot 5^n - 5 $ for all $ n \geq 1 $.

$$
\boxed{24}
$$