<think>
Okay, so I need to prove that if a and b are both odd integers, then 16 divides a⁴ + b⁴ - 2. That is, 16 | (a⁴ + b⁴ - 2). Let me think about how to approach this. 

First, since a and b are both odd, maybe I can express them in terms of some other integers. For example, any odd integer can be written as 2k + 1, where k is an integer. So let me let a = 2k + 1 and b = 2m + 1, where k and m are integers. Then I can substitute these into the expression a⁴ + b⁴ - 2 and see what happens.

But before I dive into substitution, maybe there's a better way. Since we're dealing with divisibility by 16, perhaps I can look at the expression modulo 16. If I can show that a⁴ + b⁴ - 2 ≡ 0 mod 16, then that would prove the statement. So maybe working modulo 16 is the way to go.

Let me recall that for any integer x, x mod 16 can be between 0 and 15. Since a and b are odd, their possible residues mod 16 are 1, 3, 5, 7, 9, 11, 13, 15. Maybe I can compute a⁴ mod 16 and b⁴ mod 16 for these residues and see what they are.

Alternatively, since a is odd, maybe I can find a pattern for odd numbers raised to the fourth power modulo 16. Let me try that.

Let me compute n⁴ mod 16 for n odd. Let's take n = 1: 1⁴ = 1 mod 16. n = 3: 3⁴ = 81. 81 divided by 16 is 5*16=80, so 81 ≡ 1 mod 16. Wait, 3⁴ is 81, which is 1 mod 16. Hmm. Let me check n = 5: 5⁴ = 625. 625 divided by 16: 16*39 = 624, so 625 ≡ 1 mod 16. Interesting. Similarly, n = 7: 7² = 49 ≡ 1 mod 16, so 7⁴ = (7²)² ≡ 1² = 1 mod 16. Wait, so is this true for all odd numbers?

Wait, let me check n = 9: 9² = 81 ≡ 1 mod 16, so 9⁴ = (9²)² ≡ 1² = 1 mod 16. Similarly, n = 11: 11² = 121. 121 - 7*16 = 121 - 112 = 9. So 11² ≡ 9 mod 16. Then 11⁴ = (11²)² ≡ 9² = 81 ≡ 1 mod 16. Wait, so 11⁴ ≡ 1 mod 16? That's interesting. Similarly, n = 13: 13² = 169. 169 - 10*16 = 169 - 160 = 9. So 13² ≡ 9 mod 16, then 13⁴ ≡ 9² = 81 ≡ 1 mod 16. Similarly, n = 15: 15² = 225. 225 - 14*16 = 225 - 224 = 1. So 15² ≡ 1 mod 16, so 15⁴ ≡ 1² = 1 mod 16. 

So, seems like for any odd integer n, n⁴ ≡ 1 mod 16. Is that true? Let me check n = 1, 3, 5, 7, 9, 11, 13, 15. All of them squared are either 1 or 9 mod 16, and then squaring again gives 1. So yes, n⁴ ≡ 1 mod 16 for any odd integer n. Therefore, if a and b are odd, then a⁴ ≡ 1 mod 16 and b⁴ ≡ 1 mod 16. Therefore, a⁴ + b⁴ ≡ 1 + 1 = 2 mod 16. Therefore, a⁴ + b⁴ - 2 ≡ 2 - 2 = 0 mod 16. Therefore, 16 divides a⁴ + b⁴ - 2. 

Wait, so that seems straightforward. But let me check with some examples to make sure. Let's take a = 1, b = 1. Then a⁴ + b⁴ - 2 = 1 + 1 - 2 = 0, which is divisible by 16. Okay. Take a = 1, b = 3. Then 1⁴ + 3⁴ - 2 = 1 + 81 - 2 = 80. 80 divided by 16 is 5, so yes, 16 divides 80. Another example: a = 3, b = 3. 81 + 81 - 2 = 160. 160 / 16 = 10. Okay. How about a = 1, b = 5? 1 + 625 - 2 = 624. 624 / 16 = 39. Yep, that works. 

But wait, let me check a case where maybe the result is not obvious. Let me take a = 7, b = 9. 7⁴ is 2401, 9⁴ is 6561. 2401 + 6561 = 8962. 8962 - 2 = 8960. Divided by 16: 8960 / 16 = 560. Yep, that works. 

So seems like the conclusion is correct. Therefore, if a and b are odd, then a⁴ + b⁴ - 2 is divisible by 16. Therefore, the statement is proven. 

But let me think again if there's any possible mistake here. For example, is it really true that for any odd integer n, n⁴ ≡ 1 mod 16? Let me check n = 1, 3, 5, 7, 9, 11, 13, 15. As before, all of them squared are 1 or 9 mod 16. Then squaring again gives 1. So yes, n⁴ ≡ 1 mod 16. 

Alternatively, maybe we can prove this algebraically. Let me try that. Let me take an odd integer n. Then n can be written as 2k + 1. Let me compute n² first. 

n² = (2k + 1)² = 4k² + 4k + 1 = 4k(k + 1) + 1. Now, since either k or k + 1 is even, so 4k(k + 1) is divisible by 8. Therefore, n² ≡ 1 mod 8. Therefore, n² ≡ 1 mod 8. Therefore, n⁴ = (n²)² ≡ 1² = 1 mod 8. But we need mod 16. So maybe we can do better. 

Let me compute n² mod 16. For n odd, n = 2k + 1. Let me compute n²:

n² = 4k² + 4k + 1 = 4k(k + 1) + 1. Now, k and k + 1 are consecutive integers, so one of them is even, so k(k + 1) is even. Therefore, 4k(k + 1) is divisible by 8. Therefore, n² ≡ 1 mod 8. But to compute mod 16, let's see. Let me write k(k + 1) as 2m, so 4*2m = 8m. Therefore, n² = 8m + 1. Therefore, n² ≡ 1 + 8m mod 16. So depending on m, which is k(k + 1)/2. 

But m can be either even or odd? Let me think. For example, if k is even, say k = 2t, then k + 1 = 2t + 1. Then k(k + 1) = 2t*(2t + 1) = 2t*(odd). Therefore, m = t*(2t + 1). So m can be even or odd depending on t. Similarly, if k is odd, k = 2t + 1, then k + 1 = 2t + 2 = 2(t + 1). Then k(k + 1) = (2t + 1)*2(t + 1) = 2*(2t + 1)(t + 1). Therefore, m = (2t + 1)(t + 1). Again, m can be even or odd. 

Therefore, m can be either even or odd. Therefore, 8m mod 16 can be 0 or 8. Therefore, n² ≡ 1 + 0 = 1 mod 16 or 1 + 8 = 9 mod 16. Therefore, n² ≡ 1 or 9 mod 16. Therefore, when we square n² again to get n⁴, we have:

If n² ≡ 1 mod 16, then n⁴ ≡ 1² = 1 mod 16.

If n² ≡ 9 mod 16, then n⁴ ≡ 9² = 81 ≡ 1 mod 16.

Therefore, regardless of whether n² is 1 or 9 mod 16, n⁴ ≡ 1 mod 16. Therefore, indeed, for any odd integer n, n⁴ ≡ 1 mod 16. 

Therefore, this confirms that if a and b are odd, then a⁴ ≡ 1 mod 16 and b⁴ ≡ 1 mod 16. Therefore, a⁴ + b⁴ ≡ 1 + 1 = 2 mod 16, so a⁴ + b⁴ - 2 ≡ 0 mod 16. Hence, 16 divides a⁴ + b⁴ - 2. 

Therefore, the statement is proven. 

But let me check another approach. Maybe using mathematical induction or some other method. However, since we already have a solid proof using modular arithmetic and verified with examples, maybe that's sufficient. 

Alternatively, maybe we can think in terms of expanding (a^4 + b^4). But since we already have the modular approach, perhaps that's the most straightforward. 

Alternatively, let me think about the original problem again. Maybe there's another way to see this. For example, since a is odd, write a = 2k + 1, then compute a^4. Let me try expanding (2k + 1)^4.

(2k + 1)^4 = 16k^4 + 32k^3 + 24k^2 + 8k + 1. 

Similarly for b^4. Then a^4 + b^4 - 2 would be 16k^4 + 32k^3 + 24k^2 + 8k + 1 + 16m^4 + 32m^3 + 24m^2 + 8m + 1 - 2. 

Simplify that: 16(k^4 + m^4) + 32(k^3 + m^3) + 24(k^2 + m^2) + 8(k + m) + (1 + 1 - 2) = 16(...) + 32(...) + 24(...) + 8(...) + 0. 

Therefore, the entire expression is a multiple of 8. But we need to show it's a multiple of 16. So perhaps we need to check if the coefficients are multiples of 16? Wait, no, because the coefficients are 16, 32, 24, 8. So 16 is divisible by 16, 32 is divisible by 16, 24 is 16*1 + 8, and 8 is 8. Therefore, the entire expression is 16*(...) + 32*(...) + 24*(...) + 8*(...). 

But maybe we can factor out 8: 8*(2*(k^4 + m^4) + 4*(k^3 + m^3) + 3*(k^2 + m^2) + (k + m)). 

So the entire expression is 8 times something. Therefore, to show that it's divisible by 16, we need to show that the something is even. 

So let me check if 2*(k^4 + m^4) + 4*(k^3 + m^3) + 3*(k^2 + m^2) + (k + m) is even. 

Let me denote this expression as E. So E = 2(k^4 + m^4) + 4(k^3 + m^3) + 3(k^2 + m^2) + (k + m). 

Let me check if E is even. Let's consider parity of each term. Since a and b are odd, then a = 2k + 1, so k can be any integer. Similarly for m. However, k and m can be even or odd. Wait, but maybe we can analyze E modulo 2. 

Let me compute E mod 2. 

First, note that 2(k^4 + m^4) ≡ 0 mod 2. Similarly, 4(k^3 + m^3) ≡ 0 mod 2. 3(k^2 + m^2) ≡ (k^2 + m^2) mod 2, since 3 ≡ 1 mod 2. And (k + m) is as is. Therefore, E ≡ (k^2 + m^2) + (k + m) mod 2. 

Now, since a = 2k + 1 is odd, then k can be any integer. But let's think about k mod 2. Let me note that k can be even or odd. However, since a is odd, 2k + 1 is odd regardless of k. So k can be any integer. But to compute k^2 + m^2 + k + m mod 2, let me note that:

For any integer x, x² ≡ x mod 2. Because if x is even, x² is even; if x is odd, x² is odd. Therefore, x² ≡ x mod 2. Therefore, k² ≡ k mod 2 and m² ≡ m mod 2. Therefore, k² + m² ≡ k + m mod 2. Therefore, E ≡ (k + m) + (k + m) = 2(k + m) ≡ 0 mod 2. Therefore, E is even. Therefore, the entire expression is 8 * even = 16 * something, hence divisible by 16. 

Therefore, this approach also shows that a⁴ + b⁴ - 2 is divisible by 16. 

So this confirms the result again. Therefore, regardless of whether we use modular arithmetic directly on the fourth powers or expand the expression and analyze the parity, we get the same conclusion. 

Alternatively, maybe there is a more straightforward way. Since we know that for any odd integer n, n ≡ 1 or 3 or 5 or ... mod 16, but we saw that n⁴ ≡ 1 mod 16. Therefore, regardless of the specific odd integer, the fourth power is congruent to 1 mod 16. Therefore, adding two such terms gives 2 mod 16, subtracting 2 gives 0. 

Therefore, the conclusion is solid. 

I think this is sufficient. The key insight is recognizing that any odd number to the fourth power is congruent to 1 modulo 16. This can be shown by squaring twice, as we did earlier, or by expanding the expression. 

Therefore, the proof is complete.

**Final Answer**
\boxed{16}
</think>

To prove that if $ a $ and $ b $ are both odd integers, then $ 16 \mid a^4 + b^4 - 2 $, we proceed by analyzing the expression modulo 16.

---

### Step 1: Express $ a $ and $ b $ as odd integers

Let $ a = 2k + 1 $ and $ b = 2m + 1 $, where $ k, m \in \mathbb{Z} $. These expressions represent any odd integer in terms of an integer parameter.

We are interested in the expression:

$$
a^4 + b^4 - 2
$$

Our goal is to show that this expression is divisible by 16, i.e.,

$$
a^4 + b^4 - 2 \equiv 0 \pmod{16}
$$

---

### Step 2: Analyze $ n^4 \mod 16 $ for odd $ n $

Let’s compute $ n^4 \mod 16 $ for any odd integer $ n $. Since $ n $ is odd, it can be written as $ n = 2k + 1 $, and we can compute:

$$
n^2 = (2k + 1)^2 = 4k^2 + 4k + 1 = 4k(k + 1) + 1
$$

Now, since $ k $ and $ k + 1 $ are consecutive integers, one of them is even. Therefore, $ k(k + 1) $ is even, and so $ 4k(k + 1) $ is divisible by 8. Hence:

$$
n^2 \equiv 1 \pmod{8}
$$

Now square $ n^2 $ to get $ n^4 $:

$$
n^4 = (n^2)^2 \equiv 1^2 = 1 \pmod{16}
$$

This is true regardless of whether $ n^2 \equiv 1 $ or $ 9 \pmod{16} $, because $ 1^2 = 1 \mod 16 $ and $ 9^2 = 81 \equiv 1 \mod 16 $.

Thus, for any odd integer $ n $, we have:

$$
n^4 \equiv 1 \pmod{16}
$$

---

### Step 3: Apply to $ a $ and $ b $

Since $ a $ and $ b $ are both odd, we have:

$$
a^4 \equiv 1 \pmod{16}, \quad b^4 \equiv 1 \pmod{16}
$$

Therefore:

$$
a^4 + b^4 \equiv 1 + 1 = 2 \pmod{16}
$$

Subtracting 2 from both sides:

$$
a^4 + b^4 - 2 \equiv 2 - 2 = 0 \pmod{16}
$$

---

### Conclusion

We have shown that for any odd integers $ a $ and $ b $, the expression $ a^4 + b^4 - 2 $ is congruent to 0 modulo 16. Therefore, it is divisible by 16.

$$
\boxed{16}
$$