<think>
Okay, so I need to show that for any odd integer a, the expression a² + (a+2)² + (a+4)² + 1 is divisible by 12. Let me start by understanding the problem step by step.

First, since a is an odd integer, I can represent it as 2k + 1, where k is some integer. Maybe substituting this into the expression will help simplify things. Let me try that.

Let a = 2k + 1. Then:

a² = (2k + 1)² = 4k² + 4k + 1

Next term is (a + 2)². Let's compute that:

a + 2 = 2k + 1 + 2 = 2k + 3

So (a + 2)² = (2k + 3)² = 4k² + 12k + 9

Then (a + 4)²:

a + 4 = 2k + 1 + 4 = 2k + 5

So (a + 4)² = (2k + 5)² = 4k² + 20k + 25

Now, adding all these together with the +1 at the end:

a² + (a+2)² + (a+4)² + 1 = [4k² + 4k + 1] + [4k² + 12k + 9] + [4k² + 20k + 25] + 1

Let me combine like terms:

First, the k² terms: 4k² + 4k² + 4k² = 12k²

Then the k terms: 4k + 12k + 20k = 36k

Then the constants: 1 + 9 + 25 + 1 = 36

So altogether, the expression becomes 12k² + 36k + 36.

Factor out 12: 12(k² + 3k + 3). Wait, but 12 times something. So if this is 12 times (k² + 3k + 3), then it's obviously divisible by 12. So that would mean the original expression is divisible by 12. So that seems straightforward. But maybe I should check with specific numbers to make sure I didn't make a mistake.

Let me test with a = 1 (which is odd):

1² + 3² + 5² + 1 = 1 + 9 + 25 + 1 = 36. 36 divided by 12 is 3, so yes, divisible by 12.

Another test: a = 3.

3² + 5² + 7² + 1 = 9 + 25 + 49 + 1 = 84. 84 / 12 = 7. Also divisible by 12.

Another test: a = -1 (also odd).

(-1)² + 1² + 3² + 1 = 1 + 1 + 9 + 1 = 12. 12 / 12 = 1. Yep.

Another test: a = 5.

5² + 7² + 9² + 1 = 25 + 49 + 81 + 1 = 156. 156 / 12 = 13. Correct.

So seems like the algebraic approach works. But maybe I should try another way, just to verify.

Alternatively, maybe I can consider modulo 12. Since we need the expression to be divisible by 12, we can check if the expression is congruent to 0 modulo 12.

Since a is odd, let's consider possible residues of a modulo 12. Since a is odd, possible residues are 1, 3, 5, 7, 9, 11 modulo 12.

But maybe even better to consider modulo 3 and modulo 4, since 12 = 3*4 and 3 and 4 are coprime. If the expression is divisible by both 3 and 4, then it's divisible by 12.

So maybe check divisibility by 3 and 4 separately.

First, check modulo 3.

Let me compute the expression modulo 3.

Since a is odd, but modulo 3, odd numbers can be 0, 1, 2. Wait, but actually, since a is odd, but modulo 3, the parity isn't directly related. However, maybe I can compute the expression modulo 3 regardless.

But let's see:

Let me compute each term modulo 3.

First, note that a is odd. However, modulo 3, oddness isn't directly relevant. Let me compute the expression:

a² + (a + 2)² + (a + 4)² + 1 mod 3.

Note that 4 ≡ 1 mod 3, so (a + 4) ≡ (a + 1) mod 3.

So the expression becomes:

a² + (a + 2)² + (a + 1)² + 1 mod 3.

Let me compute each term:

First term: a²

Second term: (a + 2)² = a² + 4a + 4 ≡ a² + a + 1 mod 3 (since 4 ≡ 1 mod 3, and 4 ≡ 1 mod 3)

Third term: (a + 1)² = a² + 2a + 1

Fourth term: 1

So adding all together:

a² + (a² + a + 1) + (a² + 2a + 1) + 1

Combine like terms:

a² + a² + a² = 3a² ≡ 0 mod 3

a terms: a + 2a = 3a ≡ 0 mod 3

Constants: 1 + 1 + 1 = 3 ≡ 0 mod 3

So overall, the entire expression is 0 + 0 + 0 = 0 mod 3. Therefore, divisible by 3.

Now check modulo 4.

Since 12 = 3*4, and we need divisibility by 4 as well.

So compute the expression modulo 4.

Again, a is odd. So a ≡ 1 or 3 mod 4.

Let me compute the expression:

a² + (a + 2)² + (a + 4)² + 1 mod 4.

Note that 4 ≡ 0 mod 4, so (a + 4) ≡ a mod 4. Therefore, (a + 4)² ≡ a² mod 4.

So the expression becomes:

a² + (a + 2)² + a² + 1 mod 4.

So that is 2a² + (a + 2)² + 1 mod 4.

Compute (a + 2)²:

Since a is odd, let's take a ≡ 1 or 3 mod 4.

Case 1: a ≡ 1 mod 4.

Then a + 2 ≡ 1 + 2 = 3 mod 4. Then (a + 2)² ≡ 9 ≡ 1 mod 4.

So expression becomes 2*(1) + 1 + 1 = 2 + 1 + 1 = 4 ≡ 0 mod 4.

Case 2: a ≡ 3 mod 4.

Then a + 2 ≡ 3 + 2 = 5 ≡ 1 mod 4. Then (a + 2)² ≡ 1 mod 4.

So expression becomes 2*(3²) + 1 + 1. Wait, but a ≡ 3 mod 4, so a² ≡ 9 ≡ 1 mod 4. Therefore, 2*(1) + 1 + 1 = 2 + 1 + 1 = 4 ≡ 0 mod 4.

So in both cases, the expression is 0 mod 4. Therefore, the entire expression is divisible by 4 and 3, hence by 12. Therefore, the expression is divisible by 12.

So that seems to confirm it.

Alternatively, maybe I can check for the original expression modulo 12 directly.

But since we already have two different methods (algebraic substitution and modular arithmetic) that both lead to the conclusion that the expression is divisible by 12, and the test cases also confirm it, I think that's sufficient.

But just to make sure, let me try another approach.

Another way is to note that for any odd integer a, the numbers a, a+2, a+4 are three consecutive odd numbers. So, for example, if a is odd, then a, a+2, a+4 are three consecutive odd integers. The sum of their squares plus 1. Maybe there's a pattern here.

But maybe not necessary. Alternatively, since we have three consecutive odd numbers, their squares... Hmm.

Alternatively, think about the expression as follows:

Let me expand the original expression:

a² + (a + 2)² + (a + 4)² + 1

Expanding each term:

a² + (a² + 4a + 4) + (a² + 8a + 16) + 1

Combine like terms:

a² + a² + a² = 3a²

4a + 8a = 12a

4 + 16 + 1 = 21

So total expression is 3a² + 12a + 21.

Wait, but earlier when I substituted a = 2k + 1, I got 12k² + 36k + 36, which is 12(k² + 3k + 3). However, here, expanding directly, I get 3a² + 12a + 21. Wait, there's a discrepancy here. Which one is correct?

Wait, let me check the expansion again.

Original expression:

a² + (a + 2)^2 + (a + 4)^2 + 1.

Expanding:

a² + [a² + 4a + 4] + [a² + 8a + 16] + 1.

So adding them up:

a² + a² + a² = 3a².

4a + 8a = 12a.

4 + 16 + 1 = 21. So total is 3a² + 12a + 21. But earlier, when I substituted a = 2k + 1, I got 12k² + 36k + 36. Let me check if these are equivalent.

Let me compute 3a² + 12a + 21 with a = 2k + 1.

First, compute 3a²:

3*(2k + 1)^2 = 3*(4k² + 4k + 1) = 12k² + 12k + 3.

Then 12a = 12*(2k + 1) = 24k + 12.

Adding 21:

Total expression: 12k² + 12k + 3 + 24k + 12 + 21 = 12k² + (12k + 24k) + (3 + 12 + 21) = 12k² + 36k + 36. Which matches the previous result. So both methods are consistent.

So, 3a² + 12a + 21. Let me see if this can be simplified or factored.

Factor 3: 3(a² + 4a + 7). Wait, but 3(a² + 4a + 7). However, earlier we had 12(k² + 3k + 3). But maybe this isn't helpful. However, since we need to show that this is divisible by 12, let's check.

So 3(a² + 4a + 7). For this to be divisible by 12, since 3 divides 12, then (a² + 4a + 7) must be divisible by 4. Let's check if that's the case.

So, check if a² + 4a + 7 ≡ 0 mod 4.

Since a is odd, let me write a = 2k + 1. Then:

a² + 4a + 7 = (4k² + 4k + 1) + 4*(2k + 1) + 7 = 4k² + 4k + 1 + 8k + 4 + 7 = 4k² + 12k + 12 = 4(k² + 3k + 3). Which is clearly divisible by 4. Therefore, 3*(4*(...)) = 12*(...). Therefore, the entire expression is divisible by 12. So that's another way to see it.

So, this seems to confirm again.

Alternatively, since we have a² + 4a + 7 ≡ 0 mod 4. Let me check directly for a odd.

If a is odd, then a ≡ 1 or 3 mod 4.

Case 1: a ≡ 1 mod 4.

Then a² ≡ 1, 4a ≡ 4*1 = 4 ≡ 0 mod 4. Then a² + 4a + 7 ≡ 1 + 0 + 7 = 8 ≡ 0 mod 4. Since 8 is 0 mod 4.

Case 2: a ≡ 3 mod 4.

Then a² ≡ 9 ≡ 1 mod 4. 4a ≡ 4*3 = 12 ≡ 0 mod 4. Then a² + 4a + 7 ≡ 1 + 0 + 7 = 8 ≡ 0 mod 4. Same result. Therefore, yes, divisible by 4. Therefore, 3*(something divisible by 4) is divisible by 12. So that's another way.

Therefore, all approaches lead to the conclusion that the expression is divisible by 12.

Alternatively, maybe think about the original expression:

a² + (a + 2)^2 + (a + 4)^2 + 1.

Since a is odd, let me consider the parity. Wait, but since we need divisibility by 12, which is 4*3, and we already checked modulo 3 and 4, which worked.

Alternatively, think about the expression as follows:

Let me note that for any integer a, a² ≡ 0 or 1 mod 4. Since if a is even, a² ≡ 0 mod 4; if a is odd, a² ≡ 1 mod 4. Since a is odd, each term a², (a + 2)^2, (a + 4)^2 is 1 mod 4. Therefore, adding three 1s: 1 + 1 + 1 = 3 mod 4. Then adding 1 gives 3 + 1 = 4 ≡ 0 mod 4. Therefore, the entire expression is 0 mod 4. Which is consistent with previous results.

Similarly, mod 3: For any integer a, a² ≡ 0 or 1 mod 3. Since a is odd, but mod 3, it can be 0, 1, or 2. However, let's check:

If a ≡ 0 mod 3, then a² ≡ 0 mod 3.

If a ≡ 1 mod 3, then a² ≡ 1 mod 3.

If a ≡ 2 mod 3, then a² ≡ 4 ≡ 1 mod 3.

So regardless of a, a² ≡ 0 or 1 mod 3. Similarly, (a + 2)^2 and (a + 4)^2.

But since a is odd, but mod 3, let's check:

But maybe it's easier to compute the sum:

a² + (a + 2)^2 + (a + 4)^2 + 1 mod 3.

As before, we can compute this as 0 mod 3. But maybe there's a simpler way.

Alternatively, since a is odd, let me check for a ≡ 0, 1, 2 mod 3.

But maybe not necessary. Since we already did that earlier.

But in any case, all methods confirm that the expression is divisible by 12.

Therefore, I think the conclusion is correct.

But just to make sure, let me try another example with a different odd number, say a = 7.

Compute 7² + 9² + 11² + 1 = 49 + 81 + 121 + 1 = 49 + 81 = 130, 130 + 121 = 251, 251 + 1 = 252. 252 divided by 12 is 21. Correct.

Another example: a = -3.

(-3)^2 + (-1)^2 + 1^2 + 1 = 9 + 1 + 1 + 1 = 12. 12 / 12 = 1. Correct.

Another example: a = 5, which we did before, 156 / 12 = 13. Correct.

Therefore, all tests pass.

So, in conclusion, regardless of the method used—whether substitution, modular arithmetic, or direct expansion—the expression is indeed divisible by 12 for any odd integer a.

**Final Answer**
\boxed{12}
</think>

To show that the expression  
$$
a^2 + (a+2)^2 + (a+4)^2 + 1
$$  
is divisible by 12 for any **odd integer** $ a $, we proceed by analyzing the structure of the expression and leveraging modular arithmetic.

---

### Step 1: Express in Terms of a General Odd Integer

Let $ a $ be an **odd integer**, which we can write as:
$$
a = 2k + 1, \quad \text{for some integer } k.
$$

Now substitute this into the expression:

- $ a^2 = (2k + 1)^2 = 4k^2 + 4k + 1 $
- $ (a+2)^2 = (2k + 3)^2 = 4k^2 + 12k + 9 $
- $ (a+4)^2 = (2k + 5)^2 = 4k^2 + 20k + 25 $

Adding them together and including the final $ +1 $:

$$
a^2 + (a+2)^2 + (a+4)^2 + 1 = (4k^2 + 4k + 1) + (4k^2 + 12k + 9) + (4k^2 + 20k + 25) + 1
$$

Group like terms:

- $ k^2 $: $ 4k^2 + 4k^2 + 4k^2 = 12k^2 $
- $ k $: $ 4k + 12k + 20k = 36k $
- Constants: $ 1 + 9 + 25 + 1 = 36 $

So the expression becomes:
$$
12k^2 + 36k + 36 = 12(k^2 + 3k + 3)
$$

This is clearly divisible by 12, as it is 12 times an integer.

---

### Step 2: Verify via Modular Arithmetic

We can also verify this using modular arithmetic, by checking that the expression is divisible by both 3 and 4 (since $ 12 = 3 \times 4 $).

#### **Modulo 3:**

Let’s compute the expression modulo 3:

- Since $ a $ is odd, $ a \equiv 0, 1, \text{or } 2 \mod 3 $, but the parity of $ a $ doesn't affect the modulo 3 behavior directly.

Compute:
$$
a^2 + (a+2)^2 + (a+4)^2 + 1 \mod 3
$$

Note that $ 4 \equiv 1 \mod 3 $, so $ (a + 4)^2 \equiv (a + 1)^2 \mod 3 $.

Thus, the expression becomes:
$$
a^2 + (a+2)^2 + (a+1)^2 + 1 \mod 3
$$

Now expand each term:

- $ a^2 $
- $ (a+2)^2 = a^2 + 4a + 4 \equiv a^2 + a + 1 \mod 3 $
- $ (a+1)^2 = a^2 + 2a + 1 $

Add them all:
$$
a^2 + (a^2 + a + 1) + (a^2 + 2a + 1) + 1 = 3a^2 + 3a + 3 \equiv 0 \mod 3
$$

So the expression is divisible by 3.

#### **Modulo 4:**

Since $ a $ is odd, $ a \equiv 1 \text{ or } 3 \mod 4 $.

Compute:
$$
a^2 + (a+2)^2 + (a+4)^2 + 1 \mod 4
$$

Note that $ a + 4 \equiv a \mod 4 $, so $ (a+4)^2 \equiv a^2 \mod 4 $.

Thus, the expression becomes:
$$
a^2 + (a+2)^2 + a^2 + 1 = 2a^2 + (a+2)^2 + 1
$$

Compute $ (a+2)^2 \mod 4 $:
- If $ a \equiv 1 \mod 4 $, then $ a+2 \equiv 3 \mod 4 $, and $ (a+2)^2 \equiv 9 \equiv 1 \mod 4 $
- If $ a \equiv 3 \mod 4 $, then $ a+2 \equiv 1 \mod 4 $, and $ (a+2)^2 \equiv 1 \mod 4 $

So in both cases, $ (a+2)^2 \equiv 1 \mod 4 $, and $ a^2 \equiv 1 \mod 4 $ (since $ a $ is odd).

Thus:
$$
2a^2 + (a+2)^2 + 1 \equiv 2(1) + 1 + 1 = 4 \equiv 0 \mod 4
$$

So the expression is divisible by 4.

---

### Step 3: Conclusion

Since the expression is divisible by both 3 and 4, and since 3 and 4 are coprime, it is divisible by $ 12 $.

Hence, for any **odd integer** $ a $, the expression
$$
a^2 + (a+2)^2 + (a+4)^2 + 1
$$
is divisible by **12**.

---

### Final Answer

$$
\boxed{12}
$$