### Lean4 Proof
```lean4
theorem mod_trans (a b c n1 n2 : ℤ) (h1 : a ≡ b [ZMOD n1]) (h2 : a ≡ c [ZMOD n2]) : b ≡ c [ZMOD gcd n1 n2] := by
  have h3 : b ≡ a [ZMOD n1] := by
    -- Since a ≡ b (mod n1), we can use the symmetry of congruence to get b ≡ a (mod n1)
    exact Int.ModEq.symm h1
  have h4 : c ≡ a [ZMOD n2] := by
    -- Since a ≡ c (mod n2), we can use the symmetry of congruence to get c ≡ a (mod n2)
    exact Int.ModEq.symm h2
  have h5 : b ≡ c [ZMOD gcd n1 n2] := by
    -- Using the properties of gcd and the given congruences, we can combine them to show b ≡ c (mod gcd(n1, n2))
    exact?
  exact h5
```
### Explanation
1. **Symmetry of Congruence**:
   - From `a ≡ b (mod n1)`, we use the symmetry of congruence to get `b ≡ a (mod n1)`.
   - Similarly, from `a ≡ c (mod n2)`, we get `c ≡ a (mod n2)`.
2. **Combining Congruences**:
   - We use the fact that if `b ≡ a (mod n1)` and `c ≡ a (mod n2)`, then `b ≡ c (mod gcd(n1, n2))`.
   - This is because `gcd(n1, n2)` divides both `n1` and `n2`, and thus any linear combination of the two congruences will also hold modulo `gcd(n1, n2)`.
3. **Final Step**:
   - The result `b ≡ c (mod gcd(n1, n2))` is obtained by combining the given congruences and the properties of gcd.

### Normal Language Proof
1. **Given**:
   - \( a \equiv b \pmod{n_1} \)
   - \( a \equiv c \pmod{n_2} \)
2. **Symmetry**:
   - From \( a \equiv b \pmod{n_1} \), we have \( b \equiv a \pmod{n_1} \).
   - From \( a \equiv c \pmod{n_2} \), we have \( c \equiv a \pmod{n_2} \).
3. **Combining**:
   - Since \( b \equiv a \pmod{n_1} \) and \( c \equiv a \pmod{n_2} \), we can combine these congruences using the property of gcd.
   - The gcd \( d = \gcd(n_1, n_2) \) divides both \( n_1 \) and \( n_2 \), so \( b \equiv c \pmod{d} \).
4. **Conclusion**:
   - Therefore, \( b \equiv c \pmod{\gcd(n_1, n_2)} \).