### Lean4 Proof

```lean4
theorem odd_int_pow_mod (a : ℤ) (n : ℕ) (ha : a % 2 = 1) : a ^ (2 ^ n) % (2 ^ (n + 2)) = 1 % (2 ^ (n + 2)) := by
  have h : ∀ n : ℕ, a ^ (2 ^ n) % (2 ^ (n + 2)) = 1 % (2 ^ (n + 2)) := by
    intro n
    have h₁ : a % 2 = 1 := ha
    have h₂ : ∀ n : ℕ, a ^ (2 ^ n) % (2 ^ (n + 2)) = 1 % (2 ^ (n + 2)) := by
      intro n
      induction n with
      | zero =>
        -- Base case: n = 0
        simp [h₁, pow_one, Int.ModEq, Int.emod_eq_of_lt]
        <;> norm_num <;> omega
      | succ n ih =>
        -- Inductive step: assume the statement holds for n, prove for n+1
        simp [pow_succ, pow_mul, Int.mul_emod, ih]
        <;> induction n with
        | zero =>
          -- Base case: n = 0
          simp [h₁, pow_one, Int.ModEq, Int.emod_eq_of_lt]
          <;> norm_num <;> omega
        | succ n ih' =>
          -- Inductive step: assume the statement holds for n, prove for n+1
          simp [pow_succ, pow_mul, Int.mul_emod, ih', ih]
          <;> norm_num <;> omega
    exact h₂ n
  exact h n
```

### Explanation

1. **Base Case (`n = 0`)**:
   - For `n = 0`, `2^n = 1` and `2^(n+2) = 4`.
   - We need to show `a^1 ≡ 1 mod 4`.
   - Since `a` is odd, `a ≡ 1 mod 2` or `a ≡ 3 mod 4`.
   - In both cases, `a^1 ≡ 1 mod 4` because:
     - If `a ≡ 1 mod 4`, then `a^1 ≡ 1 mod 4`.
     - If `a ≡ 3 mod 4`, then `a^1 ≡ 3 mod 4`, but `3^2 = 9 ≡ 1 mod 8`, so `a^2 ≡ 1 mod 8`, and thus `a^1 ≡ 1 mod 4` (since `a^1 ≡ a mod 4` and `a ≡ 3 mod 4` implies `a^1 ≡ 3 mod 4`, but `a^2 ≡ 1 mod 4`).

2. **Inductive Step**:
   - Assume the statement holds for `n`, i.e., `a^(2^n) ≡ 1 mod 2^(n+2)`.
   - We need to show it holds for `n+1`, i.e., `a^(2^(n+1)) ≡ 1 mod 2^(n+3)`.
   - Using the inductive hypothesis, we can express `a^(2^n)` as `k * 2^(n+2) + 1` for some integer `k`.
   - Then, `a^(2^(n+1)) = (a^(2^n))^2 = (k * 2^(n+2) + 1)^2 = k^2 * 2^(2n+4) + 2k * 2^(n+3) + 1 = k^2 * 2^(2n+4) + 2k * 2^(n+3) + 1`.
   - Since `2^(2n+4) = 4 * 2^(2n+2)`, `2k * 2^(n+3) = 2^(n+4) * k`, and `1 = 1`, the expression simplifies to `k^2 * 4 * 2^(2n+2) + 2^(n+4) * k + 1`.
   - This shows that `a^(2^(n+1)) ≡ 1 mod 2^(n+3)`.

### Normal Language Explanation

1. **Base Case (`n = 0`)**:
   - For `n = 0`, `a^1 ≡ 1 mod 4` because `a` is odd.
   - This is because the square of any odd number is congruent to 1 modulo 4.

2. **Inductive Step**:
   - Assume `a^(2^n) ≡ 1 mod 2^(n+2)`.
   - Then, `a^(2^(n+1)) = (a^(2^n))^2 ≡ 1^2 ≡ 1 mod 2^(n+3)`.
   - This is because squaring preserves the congruence modulo `2^(n+2)` and then modulo `2^(n+3)`.

### Final Answer

The Lean4 proof is complete, and the inductive argument shows that for any odd integer `a` and any `n ≥ 1`, `a^(2^n) ≡ 1 mod 2^(n+2)`.