### Lean4 Proof
```lean4
theorem divisible_by_39 : 39 ∣ (53^103 + 103^53) := by
  apply Nat.dvd_of_mod_eq_zero
  rfl
  <;> norm_num
  <;> rfl
  <;> norm_num
  <;> rfl
```

### Explanation
1. **Modular Arithmetic Approach**:
   - We use the fact that \(39 = 3 \times 13\) and check divisibility by both 3 and 13.
   - For \(39 \mid (53^{103} + 103^{53})\), we need to show that \(53^{103} + 103^{53} \equiv 0 \mod 3\) and \(53^{103} + 103^{53} \equiv 0 \mod 13\).

2. **Checking Modulo 3**:
   - \(53 \equiv 2 \mod 3\) and \(103 \equiv 1 \mod 3\).
   - Thus, \(53^{103} + 103^{53} \equiv 2^{103} + 1^{53} \equiv 2 + 1 \equiv 0 \mod 3\).

3. **Checking Modulo 13**:
   - \(53 \equiv 53 - 4 \times 13 = 53 - 52 = 1 \mod 13\).
   - \(103 \equiv 103 - 7 \times 13 = 103 - 91 = 12 \mod 13\).
   - Thus, \(53^{103} + 103^{53} \equiv 1^{103} + 12^{53} \mod 13\).
   - We need to compute \(12^{53} \mod 13\).
   - Using Fermat's Little Theorem, \(12^{12} \equiv 1 \mod 13\), so \(12^{53} = 12^{52} \times 12 \equiv 1 \times 12 \equiv 12 \mod 13\).
   - Therefore, \(1^{103} + 12^{53} \equiv 1 + 12 \equiv 13 \equiv 0 \mod 13\).

4. **Conclusion**:
   - Since \(53^{103} + 103^{53} \equiv 0 \mod 3\) and \(53^{103} + 103^{53} \equiv 0 \mod 13\), it follows that \(39 \mid (53^{103} + 103^{53})\).

### Lean4 Proof for \(111^{333} + 333^{111}\) divisible by 7
```lean4
theorem divisible_by_7 : 7 ∣ (111^333 + 333^111) := by
  apply Nat.dvd_of_mod_eq_zero
  rfl
  <;> norm_num
  <;> rfl
  <;> norm_num
  <;> rfl
```

### Explanation
1. **Modular Arithmetic Approach**:
   - We check divisibility by 7.
   - For \(7 \mid (111^{333} + 333^{111})\), we need to show that \(111^{333} + 333^{111} \equiv 0 \mod 7\).

2. **Checking Modulo 7**:
   - \(111 \mod 7 = 111 - 15 \times 7 = 111 - 105 = 6 \mod 7\).
   - \(333 \mod 7 = 333 - 47 \times 7 = 333 - 329 = 4 \mod 7\).
   - Thus, \(111^{333} + 333^{111} \equiv 6^{333} + 4^{111} \mod 7\).
   - We know that \(6 \equiv -1 \mod 7\), so \(6^{333} \equiv (-1)^{333} \equiv -1 \mod 7\).
   - Similarly, \(4 \equiv 4 \mod 7\), and \(4^3 = 64 \equiv 1 \mod 7\), so \(4^{111} = 4^{3 \times 37} \equiv 1^{37} \equiv 1 \mod 7\).
   - Therefore, \(6^{333} + 4^{111} \equiv -1 + 1 \equiv 0 \mod 7\).

3. **Conclusion**:
   - Since \(111^{333} + 333^{111} \equiv 0 \mod 7\), it follows that \(7 \mid (111^{333} + 333^{111})\).

### Final Answer
Both \(53^{103} + 103^{53}\) and \(111^{333} + 333^{111}\) are divisible by 39 and 7, respectively.