### (a) If $a \equiv b$ (mod n) and m | n, then $a \equiv b$ (mod m).

**Lean4 Proof Sketch:**
```lean4
theorem part_a (a b n m : ℤ) (h₁ : a ≡ b [ZMOD n]) (h₂ : m ∣ n) : a ≡ b [ZMOD m] := by
  have h₃ : a % n = b % n := by
    rw [Int.ModEq] at h₁
    exact h₁
  have h₄ : m ∣ n := h₂
  have h₅ : a % m = b % m := by
    have h₆ : m ∣ n := h₂
    have h₇ : a % m = b % m := by
      -- Use the fact that m divides n to reduce the problem to a simpler form.
      rw [← Int.emod_emod_of_dvd a h₆]
      rw [← Int.emod_emod_of_dvd b h₆]
      simp [h₃]
    exact h₇
  rw [Int.ModEq]
  exact h₅
```

**Normal Language Proof:**
1. By definition, \( a \equiv b \mod n \) means \( a - b = kn \) for some integer \( k \).
2. Since \( m \mid n \), there exists an integer \( t \) such that \( n = mt \).
3. Substitute \( n = mt \) into \( a - b = kn \): \( a - b = k(mt) = (kt)m \).
4. This shows \( a - b \) is a multiple of \( m \), i.e., \( a \equiv b \mod m \).

### (b) If \( a \equiv b \mod n \) and \( c > 0 \), then \( ca \equiv cb \mod cn \).

**Lean4 Proof Sketch:**
```lean4
theorem part_b (a b n c : ℤ) (h₁ : a ≡ b [ZMOD n]) (h₂ : c > 0) : a * c ≡ b * c [ZMOD n * c] := by
  have h₃ : a % n = b % n := by
    rw [Int.ModEq] at h₁
    exact h₁
  have h₄ : a * c % (n * c) = b * c % (n * c) := by
    rw [← Int.emod_add_ediv a n]
    rw [← Int.emod_add_ediv b n]
    simp [h₃, Int.mul_emod, Int.add_emod, Int.emod_emod, h₂.ne']
    <;> ring_nf
    <;> simp_all [Int.mul_emod, Int.add_emod, Int.emod_emod]
  rw [Int.ModEq]
  exact h₄
```

**Normal Language Proof:**
1. By definition, \( a \equiv b \mod n \) implies \( a - b = kn \) for some integer \( k \).
2. Multiply both sides by \( c \): \( ca - cb = c(kn) = (ck)n \).
3. This shows \( ca - cb \) is a multiple of \( cn \), i.e., \( ca \equiv cb \mod cn \).

### (c) If \( a \equiv b \mod n \) and the integers \( a, b, n \) are all divisible by \( d > 0 \), then \( a/d \equiv b/d \mod n/d \).

**Lean4 Proof Sketch:**
```lean4
theorem part_c (a b n d : ℤ) (h₁ : a ≡ b [ZMOD n]) (h₂ : d ∣ a) (h₃ : d ∣ b) (h₄ : d ∣ n) (h₅ : d > 0) : a / d ≡ b / d [ZMOD n / d] := by
  have h₆ : a % n = b % n := by
    rw [Int.ModEq] at h₁
    exact h₁
  have h₇ : (a / d) * d + a % d = a := by
    rw [Int.ediv_add_emod]
  have h₈ : (b / d) * d + b % d = b := by
    rw [Int.ediv_add_emod]
  have h₉ : d ∣ a := h₂
  have h₁₀ : d ∣ b := h₃
  have h₁₁ : d ∣ n := h₄
  have h₁₂ : a % d = 0 := by
    exact Int.emod_eq_zero_of_dvd h₂
  have h₁₃ : b % d = 0 := by
    exact Int.emod_eq_zero_of_dvd h₃
  have h₁₄ : n % d = 0 := by
    exact Int.emod_eq_zero_of_dvd h₄
  have h₁₅ : a / d ≡ b / d [ZMOD n / d] := by
    rw [Int.ModEq]
    have h₁₆ : (a / d) * d = a := by
      rw [← Int.ediv_mul_cancel h₂]
    have h₁₇ : (b / d) * d = b := by
      rw [← Int.ediv_mul_cancel h₃]
    have h₁₈ : n / d * d = n := by
      rw [← Int.ediv_mul_cancel h₄]
    simp_all [Int.ModEq, Int.emod_eq_emod_iff_emod_sub_eq_zero]
    <;> ring_nf
    <;> omega
  exact h₁₅
```

**Normal Language Proof:**
1. Since \( a \equiv b \mod n \), we have \( a - b = kn \) for some integer \( k \).
2. Since \( d \mid a, b, n \), we can write \( a = d a' \), \( b = d b' \), and \( n = d n' \).
3. Substitute into \( a - b = kn \): \( d a' - d b' = k d n' \), which simplifies to \( a' - b' = k n' \).
4. This shows \( a' \equiv b' \mod n' \), i.e., \( a/d \equiv b/d \mod n/d \).