### Lean4 Proof

```lean4
theorem proof_89_divides_2_pow_44_minus_1 : 89 ∣ 2 ^ 44 - 1 := by
  apply Nat.dvd_of_mod_eq_zero
  norm_num [Nat.pow_mod, Nat.mod_eq_of_lt]
  <;> rfl
  <;> norm_num
  <;> rfl
```

### Explanation

1. **Theorem Statement**: We need to prove that \(89\) divides \(2^{44} - 1\).
2. **Approach**: Use the property that \(a \mid b\) if and only if \(b \mod a = 0\).
3. **Proof Steps**:
   - Compute \(2^{44} \mod 89\) and show it equals \(1\).
   - This is done by direct computation using `norm_num` and properties of modular arithmetic.
4. **Lean4 Code**:
   - `apply Nat.dvd_of_mod_eq_zero` converts the problem to showing \(2^{44} - 1 \mod 89 = 0\).
   - `norm_num [Nat.pow_mod, Nat.mod_eq_of_lt]` simplifies the expression \(2^{44} \mod 89\) to \(1\).
   - `rfl` confirms that the simplified form is indeed \(0\), completing the proof.

### Normal Language Explanation

1. **Objective**: Prove that \(89\) divides \(2^{44} - 1\).
2. **Key Idea**: Use the fact that \(a \mid b\) if and only if \(b \mod a = 0\).
3. **Steps**:
   - Compute \(2^{44} \mod 89\) and show it equals \(1\).
   - Since \(2^{44} \mod 89 = 1\), \(2^{44} - 1 \mod 89 = 0\), meaning \(89 \mid 2^{44} - 1\).
4. **Verification**:
   - \(2^4 = 16 \mod 89\)
   - \(2^8 = (2^4)^2 = 256 \mod 89 = 256 - 2 \times 89 = 256 - 178 = 78\)
   - \(2^{16} = (2^8)^2 = 78^2 = 6084 \mod 89 = 6084 - 68 \times 89 = 6084 - 6052 = 32\)
   - \(2^{22} = 2^{16} \times 2^6 = 32 \times 64 = 2048 \mod 89 = 2048 - 23 \times 89 = 2048 - 2047 = 1\)
   - \(2^{44} = 2^{22} \times 2^{22} = 1 \times 1 = 1 \mod 89\)
   - Thus, \(2^{44} - 1 \mod 89 = 0\), so \(89 \mid 2^{44} - 1\).

### Lean4 Proof for \(97 \mid 2^{48} - 1\)

```lean4
theorem proof_97_divides_2_pow_48_minus_1 : 97 ∣ 2 ^ 48 - 1 := by
  apply Nat.dvd_of_mod_eq_zero
  norm_num [Nat.pow_mod, Nat.mod_eq_of_lt]
  <;> rfl
  <;> norm_num
  <;> rfl
```

### Explanation for \(97 \mid 2^{48} - 1\)

1. **Objective**: Prove that \(97\) divides \(2^{48} - 1\).
2. **Approach**: Use the property that \(a \mid b\) if and only if \(b \mod a = 0\).
3. **Steps**:
   - Compute \(2^{48} \mod 97\) and show it equals \(1\).
   - This is done by direct computation using `norm_num` and properties of modular arithmetic.
4. **Lean4 Code**:
   - `apply Nat.dvd_of_mod_eq_zero` converts the problem to showing \(2^{48} - 1 \mod 97 = 0\).
   - `norm_num [Nat.pow_mod, Nat.mod_eq_of_lt]` simplifies the expression \(2^{48} \mod 97\) to \(1\).
   - `rfl` confirms that the simplified form is indeed \(0\), completing the proof.

### Normal Language Explanation for \(97 \mid 2^{48} - 1\)

1. **Objective**: Prove that \(97\) divides \(2^{48} - 1\).
2. **Key Idea**: Use the fact that \(a \mid b\) if and only if \(b \mod a = 0\).
3. **Steps**:
   - Compute \(2^{48} \mod 97\) and show it equals \(1\).
   - Since \(2^{48} \mod 97 = 1\), \(2^{48} - 1 \mod 97 = 0\), meaning \(97 \mid 2^{48} - 1\).
4. **Verification**:
   - \(2^3 = 8 \mod 97\)
   - \(2^6 = 64 \mod 97\)
   - \(2^{12} = 64^2 = 4096 \mod 97 = 4096 - 42 \times 97 = 4096 - 4074 = 22\)
   - \(2^{24} = 2^{12} \times 2^{12} = 22 \times 22 = 484 \mod 97 = 484 - 4 \times 97 = 484 - 388 = 96\)
   - \(2^{48} = 2^{24} \times 2^{24} = 96 \times 96 = 9216 \mod 97 = 9216 - 95 \times 97 = 9216 - 9215 = 1\)
   - Thus, \(2^{48} - 1 \mod 97 = 0\), so \(97 \mid 2^{48} - 1\).