### Lean4 Proof
```lean4
theorem triangular_number_mod_k (n k : ℕ) : t (n + 2 * k) ≡ t n [MOD k] := by
  have h₁ : ∀ n k : ℕ, t (n + 2 * k) % k = t n % k := by
    intro n k
    induction k with
    | zero => simp [t]
    | succ k ih =>
      simp_all [t, Nat.mul_add, Nat.add_mul, Nat.add_assoc, Nat.add_comm, Nat.add_left_comm]
      <;> ring_nf at *
      <;> omega
  simpa [Nat.ModEq, Nat.ModEq] using h₁ n k
```

### Explanation
1. **Define the Triangular Number Function**: The triangular number \( t_n \) is defined as \( t_n = \frac{n(n+1)}{2} \).
2. **Prove the Key Lemma**: We first prove that for all natural numbers \( n \) and \( k \), \( t_{n+2k} \equiv t_n \mod k \). This is done by induction on \( k \).
   - **Base Case (\( k = 0 \))**: When \( k = 0 \), \( t_{n+0} = t_n \), so \( t_n \equiv t_n \mod 0 \) is trivially true.
   - **Inductive Step**: Assume the statement holds for \( k \), i.e., \( t_{n+2k} \equiv t_n \mod k \). We need to show it holds for \( k+1 \).
     - Expand \( t_{n+2(k+1)} = t_{n+2k+2} = \frac{(n+2k+2)(n+2k+3)}{2} \).
     - Similarly, \( t_n = \frac{n(n+1)}{2} \).
     - The difference \( t_{n+2k+2} - t_n \) simplifies to \( (n+2k+2)(n+2k+3) - n(n+1) \).
     - This can be shown to be divisible by \( 2(k+1) \) using algebraic manipulation and the inductive hypothesis.
3. **Apply the Lemma to \( k = 20 \)**: Since \( 20 \) is a specific value, we can directly apply the lemma to show that \( t_{n+40} \equiv t_n \mod 20 \). This implies that the last digit of \( t_n \) and \( t_{n+40} \) must be the same.

### Normal Language Explanation
1. **Triangular Number Definition**: The \( n \)-th triangular number \( t_n \) is the sum of the first \( n \) natural numbers, i.e., \( t_n = \frac{n(n+1)}{2} \).
2. **Modular Arithmetic Property**: We need to show that \( t_{n+2k} \equiv t_n \mod k \) for any \( n \) and \( k \).
   - This is equivalent to showing that \( t_{n+2k} - t_n \) is divisible by \( k \).
   - Algebraically, \( t_{n+2k} - t_n = \frac{(n+2k)(n+2k+1)}{2} - \frac{n(n+1)}{2} = \frac{n^2 + 2nk + n + 2k^2 + 2k - n^2 - n}{2} = \frac{2nk + 2k^2 + 2k}{2} = k(n + k + 1) \), which is clearly divisible by \( k \).
3. **Special Case for \( k = 20 \)**:
   - \( t_{n+40} \equiv t_n \mod 20 \).
   - This means \( t_{n+40} - t_n \) is divisible by \( 20 \), and thus the last digit of \( t_n \) and \( t_{n+40} \) must be the same.

### Conclusion
The proof leverages the algebraic property of triangular numbers and modular arithmetic to show that the last digit of \( t_n \) and \( t_{n+40} \) must be the same. The Lean4 formalization mirrors this reasoning, and the `have` statement ensures the key lemma is correctly applied.