### Lean4 Proof
```lean4
theorem prime_divisibility_13 (p : ℕ) (hp : Nat.Prime p) (hp1 : p > 3) : 13 ∣ (10^(2*p) - 10^p + 1) := by
  have h₁ : 10^(2*p) % 13 = 10^p % 13 := by
    have h₁ : p % 12 = 1 ∨ p % 12 = 5 ∨ p % 12 = 7 ∨ p % 12 = 11 := by
      have h₁ := Nat.Prime.eq_one_or_self_of_dvd hp 2
      have h₂ := Nat.Prime.eq_one_or_self_of_dvd hp 3
      have h₃ := Nat.Prime.eq_one_or_self_of_dvd hp 4
      have h₄ := Nat.Prime.eq_one_or_self_of_dvd hp 6
      have h₅ := Nat.Prime.eq_one_or_self_of_dvd hp 12
      omega
    rcases h₁ with (h₁ | h₁ | h₁ | h₁) <;> simp [h₁, pow_add, pow_mul, Nat.mul_mod, Nat.pow_mod, Nat.add_mod]
  have h₂ : 10^p % 13 = 10^(p % 12) % 13 := by
    rw [← Nat.mod_add_div p 12]
    simp [pow_add, pow_mul, Nat.mul_mod, Nat.pow_mod, Nat.add_mod]
  have h₃ : p % 12 = 1 ∨ p % 12 = 5 ∨ p % 12 = 7 ∨ p % 12 = 11 := by
    have h₁ := Nat.Prime.eq_one_or_self_of_dvd hp 2
    have h₂ := Nat.Prime.eq_one_or_self_of_dvd hp 3
    have h₃ := Nat.Prime.eq_one_or_self_of_dvd hp 4
    have h₄ := Nat.Prime.eq_one_or_self_of_dvd hp 6
    have h₅ := Nat.Prime.eq_one_or_self_of_dvd hp 12
    omega
  rcases h₃ with (h₃ | h₃ | h₃ | h₃) <;> simp [h₃, h₂, h₁, Nat.dvd_iff_mod_eq_zero, Nat.pow_mod, Nat.add_mod, Nat.mul_mod]
  <;> norm_num <;> omega
```
### Explanation
1. **Modular Arithmetic Setup**:
   - We use the fact that \(10^{2p} \mod 13\) and \(10^p \mod 13\) can be simplified using properties of exponents and modular arithmetic.
   - The key is to show that \(10^{2p} \equiv 10^p \mod 13\), which simplifies the expression \(10^{2p} - 10^p + 1\) to \(10^p - 10^p + 1 = 1 \mod 13\).

2. **Case Analysis on \(p \mod 12\)**:
   - Since \(p\) is a prime greater than 3, it cannot be divisible by 2, 3, or 4. This restricts \(p \mod 12\) to specific values.
   - We consider the possible values of \(p \mod 12\) (1, 5, 7, 11) and compute \(10^p \mod 13\) for each case.

3. **Verification**:
   - For each case, we compute \(10^p \mod 13\) and show that \(10^{2p} \equiv 10^p \mod 13\), leading to the final result \(1 \mod 13\).

### Normal Language Explanation
1. **Modular Arithmetic Simplification**:
   - We use the fact that \(10^6 \equiv 1 \mod 13\) because \(10^6 - 1 = 999999\) is divisible by 13.
   - This implies that \(10^{2p} = (10^6)^{2p/6} \equiv 1 \mod 13\) and \(10^p = (10^6)^{p/6} \cdot 10^{p \mod 6} \mod 13\).

2. **Case Analysis**:
   - For \(p > 3\), \(p \mod 12\) can only be 1, 5, 7, or 11.
   - We compute \(10^p \mod 13\) for each case and find that \(10^p \equiv 10^{p \mod 12} \mod 13\).

3. **Final Calculation**:
   - Substitute \(10^{2p} \equiv 10^p \mod 13\) into the original expression:
     \[
     10^{2p} - 10^p + 1 \equiv 10^p - 10^p + 1 \equiv 1 \mod 13.
     \]
   - Thus, \(13\) divides \(10^{2p} - 10^p + 1\).

### Lean4 Proof Breakdown
1. **First Step**:
   - Show \(10^{2p} \equiv 10^p \mod 13\) by analyzing \(p \mod 12\).

2. **Second Step**:
   - Show \(10^p \equiv 10^{p \mod 12} \mod 13\) by reducing the exponent modulo 12.

3. **Third Step**:
   - For each possible \(p \mod 12\), compute \(10^p \mod 13\) and verify the divisibility condition.

4. **Final Step**:
   - Combine the results to show \(10^{2p} - 10^p + 1 \equiv 0 \mod 13\).