### Lean4 Proof
```lean4
theorem mod_2n_cases (x a n : ℕ) (h : x ≡ a [MOD n]) : x ≡ a [MOD 2 * n] ∨ x ≡ a + n [MOD 2 * n] := by
  have h₁ : x % n = a % n := by
    simp_all [Nat.ModEq, Nat.mod_eq_of_lt]
  have h₂ : x % (2 * n) = a % (2 * n) ∨ x % (2 * n) = (a + n) % (2 * n) := by
    have : x % (2 * n) = a % (2 * n) ∨ x % (2 * n) = (a + n) % (2 * n) := by
      have : x % n = a % n := h₁
      have : x % (2 * n) = x % n ∨ x % (2 * n) = (x % n + n) % (2 * n) := by
        have : x % (2 * n) = x % n ∨ x % (2 * n) = (x % n + n) % (2 * n) := by
          omega
        exact this
      cases this with
      | inl h₃ =>
        simp_all [Nat.add_mod, Nat.mul_mod, Nat.mod_mod]
        <;> omega
      | inr h₃ =>
        simp_all [Nat.add_mod, Nat.mul_mod, Nat.mod_mod]
        <;> omega
    exact this
  simp_all [Nat.ModEq, Nat.mod_eq_of_lt]
  <;> omega
```
### Explanation
1. **Understand the Given Information**:
   - We are given that \( x \equiv a \pmod{n} \), which means \( x \mod n = a \mod n \).
   - We need to show that either \( x \equiv a \pmod{2n} \) or \( x \equiv a + n \pmod{2n} \).

2. **Break Down the Problem**:
   - We know that \( x \mod n = a \mod n \).
   - We need to find \( x \mod (2n) \) in terms of \( a \mod (2n) \).

3. **Use the Chinese Remainder Theorem**:
   - Since \( n \) and \( 2 \) are coprime, we can consider the two cases for \( x \mod n \):
     - \( x \mod n = a \mod n \)
     - \( x \mod n = (a \mod n + n) \mod n \) (which simplifies to \( a \mod n \) because \( n \mod n = 0 \))

4. **Case Analysis**:
   - **Case 1**: \( x \mod n = a \mod n \)
     - Then \( x \mod (2n) \) could be either \( x \mod n \) or \( (x \mod n + n) \mod (2n) \).
     - Substituting \( x \mod n = a \mod n \), we get \( x \mod (2n) = a \mod (2n) \) or \( (a \mod n + n) \mod (2n) \).
   - **Case 2**: \( x \mod n = (a \mod n + n) \mod n \)
     - This simplifies to \( x \mod n = a \mod n \), which is the same as Case 1.

5. **Conclusion**:
   - In both cases, \( x \mod (2n) \) is either \( a \mod (2n) \) or \( (a + n) \mod (2n) \).
   - Therefore, either \( x \equiv a \pmod{2n} \) or \( x \equiv a + n \pmod{2n} \).

### Normal Language Explanation
1. **Given**: \( x \equiv a \pmod{n} \) means \( x \mod n = a \mod n \).
2. **Find \( x \mod (2n) \)**:
   - Since \( 2n = 2 \times n \), we can use the Chinese Remainder Theorem.
   - The possible remainders of \( x \) when divided by \( 2n \) are determined by the remainders of \( x \) when divided by \( n \) and \( 2 \).
3. **Case 1**: \( x \mod n = a \mod n \)
   - Then \( x \mod (2n) \) could be \( a \mod (2n) \) or \( (a + n) \mod (2n) \).
4. **Case 2**: \( x \mod n = (a \mod n + n) \mod n \)
   - This simplifies to \( x \mod n = a \mod n \), which is the same as Case 1.
5. **Conclusion**:
   - Either \( x \mod (2n) = a \mod (2n) \) or \( x \mod (2n) = (a + n) \mod (2n) \).
   - Therefore, either \( x \equiv a \pmod{2n} \) or \( x \equiv a + n \pmod{2n} \).