### Part (a)

**Problem Statement:**
Find an integer having the remainders 1, 2, 5, 5 when divided by 2, 3, 6, 12, respectively.

**Solution:**

We need to find an integer \( x \) such that:
1. \( x \equiv 1 \mod 2 \)
2. \( x \equiv 2 \mod 3 \)
3. \( x \equiv 5 \mod 6 \)
4. \( x \equiv 5 \mod 12 \)

**Step 1: Solve the first two congruences.**
We have:
1. \( x \equiv 1 \mod 2 \)
2. \( x \equiv 2 \mod 3 \)

Let \( x = 2k + 1 \) for some integer \( k \). Substitute into the second congruence:
\[ 2k + 1 \equiv 2 \mod 3 \]
\[ 2k \equiv 1 \mod 3 \]
Multiply both sides by the modular inverse of 2 modulo 3, which is 2 (since \( 2 \times 2 = 4 \equiv 1 \mod 3 \)):
\[ k \equiv 2 \mod 3 \]
Thus, \( k = 3m + 2 \) for some integer \( m \). Substitute back:
\[ x = 2(3m + 2) + 1 = 6m + 4 + 1 = 6m + 5 \]
So, \( x \equiv 5 \mod 6 \). This satisfies the third congruence.

**Step 2: Solve the fourth congruence.**
We have:
\[ x \equiv 5 \mod 12 \]
From Step 1, \( x = 6m + 5 \). Substitute into the fourth congruence:
\[ 6m + 5 \equiv 5 \mod 12 \]
\[ 6m \equiv 0 \mod 12 \]
\[ m \equiv 0 \mod 2 \]
Thus, \( m = 2n \) for some integer \( n \). Substitute back:
\[ x = 6(2n) + 5 = 12n + 5 \]
So, \( x \equiv 5 \mod 12 \), which satisfies the fourth congruence.

**Final Solution:**
The general solution is \( x = 12n + 5 \). To find a specific solution, set \( n = 0 \):
\[ x = 5 \]
Verify:
1. \( 5 \div 2 = 2 \) with remainder 1.
2. \( 5 \div 3 = 1 \) with remainder 2.
3. \( 5 \div 6 = 0 \) with remainder 5.
4. \( 5 \div 12 = 0 \) with remainder 5.

Thus, \( x = 5 \) is a solution.

### Part (b)

**Problem Statement:**
Find an integer having the remainders 2, 3, 4, 5 when divided by 3, 4, 5, 6, respectively.

**Solution:**

We need to find an integer \( x \) such that:
1. \( x \equiv 2 \mod 3 \)
2. \( x \equiv 3 \mod 4 \)
3. \( x \equiv 4 \mod 5 \)
4. \( x \equiv 5 \mod 6 \)

**Step 1: Solve the first two congruences.**
We have:
1. \( x \equiv 2 \mod 3 \)
2. \( x \equiv 3 \mod 4 \)

Let \( x = 3k + 2 \) for some integer \( k \). Substitute into the second congruence:
\[ 3k + 2 \equiv 3 \mod 4 \]
\[ 3k \equiv 1 \mod 4 \]
Multiply both sides by the modular inverse of 3 modulo 4, which is 3 (since \( 3 \times 3 = 9 \equiv 1 \mod 4 \)):
\[ k \equiv 3 \mod 4 \]
Thus, \( k = 4m + 3 \) for some integer \( m \). Substitute back:
\[ x = 3(4m + 3) + 2 = 12m + 9 + 2 = 12m + 11 \]
So, \( x \equiv 11 \mod 12 \).

**Step 2: Solve the third congruence.**
We have:
\[ x \equiv 4 \mod 5 \]
From Step 1, \( x = 12m + 11 \). Substitute into the third congruence:
\[ 12m + 11 \equiv 4 \mod 5 \]
\[ 12m \equiv -7 \mod 5 \]
\[ 12 \equiv 2 \mod 5 \]
\[ -7 \equiv 3 \mod 5 \]
\[ 2m \equiv 3 \mod 5 \]
Multiply both sides by the modular inverse of 2 modulo 5, which is 3 (since \( 2 \times 3 = 6 \equiv 1 \mod 5 \)):
\[ m \equiv 9 \mod 5 \]
\[ m \equiv 4 \mod 5 \]
Thus, \( m = 5n + 4 \) for some integer \( n \). Substitute back:
\[ x = 12(5n + 4) + 11 = 60n + 48 + 11 = 60n + 59 \]
So, \( x \equiv 59 \mod 60 \).

**Step 3: Solve the fourth congruence.**
We have:
\[ x \equiv 5 \mod 6 \]
From Step 2, \( x = 60n + 59 \). Substitute into the fourth congruence:
\[ 60n + 59 \equiv 5 \mod 6 \]
\[ 60n \equiv -54 \mod 6 \]
\[ 60 \equiv 0 \mod 6 \]
\[ -54 \equiv 0 \mod 6 \]
Thus:
\[ 0 \equiv 0 \mod 6 \]
This is always true, so no additional constraint is needed.

**Final Solution:**
The general solution is \( x = 60n + 59 \). To find a specific solution, set \( n = 0 \):
\[ x = 59 \]
Verify:
1. \( 59 \div 3 = 19 \) with remainder 2.
2. \( 59 \div 4 = 14 \) with remainder 3.
3. \( 59 \div 5 = 11 \) with remainder 4.
4. \( 59 \div 6 = 9 \) with remainder 5.

Thus, \( x = 59 \) is a solution.

### Part (c)

**Problem Statement:**
Find an integer having the remainders 3, 11, 15 when divided by 10, 13, 17, respectively.

**Solution:**

We need to find an integer \( x \) such that:
1. \( x \equiv 3 \mod 10 \)
2. \( x \equiv 11 \mod 13 \)
3. \( x \equiv 15 \mod 17 \)

**Step 1: Solve the first two congruences.**
We have:
1. \( x \equiv 3 \mod 10 \)
2. \( x \equiv 11 \mod 13 \)

Let \( x = 10k + 3 \) for some integer \( k \). Substitute into the second congruence:
\[ 10k + 3 \equiv 11 \mod 13 \]
\[ 10k \equiv 8 \mod 13 \]
Multiply both sides by the modular inverse of 10 modulo 13, which is 7 (since \( 10 \times 7 = 70 \equiv 1 \mod 13 \)):
\[ k \equiv 56 \mod 13 \]
\[ k \equiv 5 \mod 13 \]
Thus, \( k = 13m + 5 \) for some integer \( m \). Substitute back:
\[ x = 10(13m + 5) + 3 = 130m + 50 + 3 = 130m + 53 \]
So, \( x \equiv 53 \mod 130 \).

**Step 2: Solve the third congruence.**
We have:
\[ x \equiv 15 \mod 17 \]
From Step 1, \( x = 130m + 53 \). Substitute into the third congruence:
\[ 130m + 53 \equiv 15 \mod 17 \]
\[ 130 \equiv 130 - 7 \times 17 = 130 - 11