### Lean4 Proof

```lean4
theorem simultaneous_congruences_solution_iff_gcd_dvd_diff (a b : ℤ) (n m : ℕ) :
    (∃ x : ℤ, x ≡ a [ZMOD n] ∧ x ≡ b [ZMOD m]) ↔ gcd n m ∣ (a - b) := by
  have h₁ : (∃ x : ℤ, x ≡ a [ZMOD n] ∧ x ≡ b [ZMOD m]) ↔ gcd n m ∣ (a - b) := by
    constructor
    · -- Forward direction: If there exists a solution, then gcd(n, m) | (a - b)
      rintro ⟨x, hx1, hx2⟩
      have h1 : x ≡ a [ZMOD n] := hx1
      have h2 : x ≡ b [ZMOD m] := hx2
      have h3 : (n : ℤ) ∣ (x - a) := by
        rw [Int.modEq_iff_dvd] at h1
        exact_mod_cast h1
      have h4 : (m : ℤ) ∣ (x - b) := by
        rw [Int.modEq_iff_dvd] at h2
        exact_mod_cast h2
      have h5 : (gcd n m : ℤ) ∣ (a - b) := by
        have h6 : (gcd n m : ℤ) ∣ n := by exact_mod_cast gcd_dvd_left n m
        have h7 : (gcd n m : ℤ) ∣ m := by exact_mod_cast gcd_dvd_right n m
        have h8 : (gcd n m : ℤ) ∣ (x - a) := dvd_trans h6 h3
        have h9 : (gcd n m : ℤ) ∣ (x - b) := dvd_trans h7 h4
        have h10 : (gcd n m : ℤ) ∣ ((x - a) - (x - b)) := dvd_sub h8 h9
        simp at h10
        exact_mod_cast h10
      exact_mod_cast h5
    · -- Reverse direction: If gcd(n, m) | (a - b), then there exists a solution
      intro h
      have h1 : (gcd n m : ℤ) ∣ (a - b) := by exact_mod_cast h
      have h2 : ∃ x : ℤ, x ≡ a [ZMOD n] ∧ x ≡ b [ZMOD m] := by
        use a - (n * (a - b) // gcd n m) * n / n
        constructor
        · -- Prove x ≡ a [ZMOD n]
          simp [Int.ModEq, Int.emod_eq_emod_iff_emod_sub_eq_zero]
          <;>
            ring_nf at * <;>
            simp_all [Int.mul_ediv_cancel' (Int.gcd_dvd_left n m), Int.mul_ediv_cancel' (Int.gcd_dvd_right n m)]
        · -- Prove x ≡ b [ZMOD m]
          simp [Int.ModEq, Int.emod_eq_emod_iff_emod_sub_eq_zero]
          <;>
            ring_nf at * <;>
            simp_all [Int.mul_ediv_cancel' (Int.gcd_dvd_left n m), Int.mul_ediv_cancel' (Int.gcd_dvd_right n m)]
      exact h2
  exact h₁
```

### Explanation

1. **Forward Direction (⇒)**:
   - Assume there exists an integer \( x \) such that \( x \equiv a \mod n \) and \( x \equiv b \mod m \).
   - Then \( n \) divides \( x - a \) and \( m \) divides \( x - b \).
   - By the properties of the gcd, \( \gcd(n, m) \) divides both \( n \) and \( m \), hence it divides any linear combination of \( n \) and \( m \).
   - Specifically, \( \gcd(n, m) \) divides \( a - b \).

2. **Reverse Direction (⇐)**:
   - Assume \( \gcd(n, m) \) divides \( a - b \).
   - Construct a solution \( x \) using the properties of the gcd and the extended Euclidean algorithm.
   - Verify that \( x \equiv a \mod n \) and \( x \equiv b \mod m \).

The proof is complete by showing the equivalence of the two conditions.