For n $\geq{1}$, derive each of the identities below:
  (a) $\binom{n}{0} + \binom{n}{1} + \binom{n}{2} + \ldots + \binom{n}{n} = 2^n$. 
      [Hint: Let a = b = 1 in the binomial theorem.]
  (b) $\binom{n}{0} - \binom{n}{1} + \binom{n}{2} + \ldots + (-1)^n\binom{n}{n} = 0$. 
  (c) $\binom{n}{1} + 2\binom{n}{2} + 3\binom{n}{3} + \ldots + n\binom{n}{n} = n2^{n-1}$. 
  (d) $\binom{n}{0} + 2\binom{n}{1} + 2^2\binom{n}{2} + \ldots + 2^n\binom{n}{n} = 3^n$. 
  (e) $\binom{n}{0} + \binom{n}{2} + \binom{n}{4} + \binom{n}{6} + \ldots = \binom{n}{1} + \binom{n}{3} + \binom{n}{3} + \ldots = 2^{n-1}$
  (f) $\binom{n}{0} - \frac{1}{2}\binom{n}{1} + \frac{1}{3}\binom{n}{2} - \ldots + \frac{(-1)^n}{n+1}\binom{n}{n} = \frac{1}{n+1}$