### Lean4 Proof

```lean4
theorem proof_13_181 (n : ℕ) (hn : n ≥ 1) : (-13)^(n+1) ≡ (-13)^n + (-13)^(n-1) [ZMOD 181] := by
  induction n with
  | zero => contradiction -- n cannot be zero since hn : n ≥ 1
  | succ n ih =>
    cases n with
    | zero =>
      -- Base case: n = 1
      norm_num [Int.ModEq, Int.ModEq]
    | succ n =>
      -- Inductive step: assume the statement holds for n, prove for n+1
      simp [pow_succ, Int.ModEq] at ih ⊢
      <;> omega
```

### Explanation

1. **Base Case (`n = 1`)**:
   - For `n = 1`, the statement becomes `(-13)^2 ≡ (-13)^1 + (-13)^0 mod 181`.
   - Calculate `(-13)^2 = 169` and `(-13)^1 = -13`, `(-13)^0 = 1`.
   - So, `169 ≡ -13 + 1 = -12 mod 181`.
   - `169 ≡ 169 mod 181` is trivially true.

2. **Inductive Step**:
   - Assume the statement holds for `n`, i.e., `(-13)^(n+1) ≡ (-13)^n + (-13)^(n-1) mod 181`.
   - We need to show it holds for `n+1`, i.e., `(-13)^(n+2) ≡ (-13)^(n+1) + (-13)^n mod 181`.
   - Multiply the inductive hypothesis by `-13` on both sides:
     `(-13) * (-13)^(n+1) ≡ (-13) * ((-13)^n + (-13)^(n-1)) mod 181`.
   - Simplify the left side: `(-13)^(n+2)`.
   - Simplify the right side: `(-13)^(n+1) + (-13)^(n+1 - 1) = (-13)^(n+1) + (-13)^n`.
   - Thus, `(-13)^(n+2) ≡ (-13)^(n+1) + (-13)^n mod 181`, which is the desired result.

### Normal Language Explanation

The proof is by induction on `n`. The base case is `n = 1`, which is verified by direct computation. The inductive step assumes the statement holds for `n` and proves it for `n+1` by multiplying the inductive hypothesis by `-13` and simplifying. The key insight is that the congruence relation is preserved under multiplication by `-13` modulo `181`.