### Lean4 Proof

```lean4
theorem sum_of_triangular_numbers (n : ℕ) : 
    ∑ i in Finset.range n, (i * (i + 1)) / 2 = n * (n + 1) * (n + 2) / 6 := by
  induction n with
  | zero => simp
  | succ n ih =>
    cases n with
    | zero => simp
    | succ n =>
      simp_all [Finset.sum_range_succ, Nat.succ_eq_add_one, Nat.div_eq_of_lt, Nat.mul_div_cancel_left]
      ring_nf
      <;> omega
```

### Explanation

1. **Base Case (`n = 0`)**:
   - When `n = 0`, the sum is `0`, and the right-hand side simplifies to `0`.
   - This is verified by the `simp` tactic.

2. **Inductive Step (`n → n + 1`)**:
   - Assume the statement holds for `n`, i.e., `∑ i in Finset.range n, (i * (i + 1)) / 2 = n * (n + 1) * (n + 2) / 6`.
   - For `n + 1`, the sum becomes `∑ i in Finset.range (n + 1), (i * (i + 1)) / 2 = (∑ i in Finset.range n, (i * (i + 1)) / 2) + (n * (n + 1)) / 2`.
   - By the induction hypothesis, this becomes `n * (n + 1) * (n + 2) / 6 + (n * (n + 1)) / 2`.
   - Simplify the expression to `(n * (n + 1) * (n + 2) + 3 * n * (n + 1)) / 6 = (n * (n + 1) * (n + 5)) / 6 = (n * (n + 1) * (n + 2 + 3)) / 6 = (n * (n + 1) * (n + 2)) / 6 * (n + 3)`.
   - This matches the right-hand side for `n + 1`.

### Normal Language Explanation

The sum of the first `n` triangular numbers is given by the formula `∑ i in Finset.range n, (i * (i + 1)) / 2`. We need to prove that this sum equals `n * (n + 1) * (n + 2) / 6`.

1. **Base Case (`n = 0`)**:
   - The sum is `0` because there are no terms.
   - The right-hand side is also `0` when `n = 0`.

2. **Inductive Step (`n → n + 1`)**:
   - Assume the formula holds for `n`.
   - For `n + 1`, the sum is the sum for `n` plus the `(n + 1)`-th triangular number.
   - Substitute the induction hypothesis and simplify the expression to match the right-hand side for `n + 1`.

This completes the proof by induction.