### Lean4 Proof

```lean4
theorem pentagonal_number_formula : ∀ n : ℕ, n ≥ 1 → 
  (∀ n : ℕ, n ≥ 1 → p n = n * (3 * n - 1) / 2) := by
  intro n hn
  have h : ∀ n : ℕ, n ≥ 1 → p n = n * (3 * n - 1) / 2 := by
    intro n hn
    induction n with
    | zero => contradiction
    | succ n ih =>
      cases n with
      | zero =>
        -- Base case: n = 1
        simp [p]
      | succ n =>
        -- Inductive step
        simp_all [p, Nat.mul_sub_left_distrib, Nat.mul_sub_right_distrib, Nat.mul_add, Nat.add_mul]
        ring_nf
        <;> omega
  exact h n hn
```

### Explanation

1. **Base Case (`n = 1`)**:
   - For `n = 1`, the formula simplifies to `1 * (3 * 1 - 1) / 2 = 1`, which matches the first pentagonal number.

2. **Inductive Step**:
   - Assume the formula holds for `n = k`, i.e., `p_k = k * (3k - 1) / 2`.
   - For `n = k + 1`, the formula becomes `(k + 1) * (3(k + 1) - 1) / 2 = (k + 1) * (3k + 2) / 2`.
   - Using the recursive definition `p_{k+1} = p_k + (3(k + 1) - 2) = p_k + (3k + 1)`, substitute the inductive hypothesis:
     \[
     p_{k+1} = \frac{k(3k - 1)}{2} + 3k + 1 = \frac{3k^2 - k + 6k + 2}{2} = \frac{3k^2 + 5k + 2}{2}
     \]
   - Simplify the expression:
     \[
     \frac{3k^2 + 5k + 2}{2} = \frac{(k + 1)(3k + 2)}{2}
     \]
   - This matches the formula for `n = k + 1`, completing the induction.

### Normal Language Proof

1. **Base Case (`n = 1`)**:
   - The first pentagonal number is `1`.
   - Substitute `n = 1` into the formula: `1 * (3 * 1 - 1) / 2 = 1 * 2 / 2 = 1`.
   - Thus, the formula holds for `n = 1`.

2. **Inductive Step**:
   - Assume the formula holds for `n = k`, i.e., `p_k = k * (3k - 1) / 2`.
   - For `n = k + 1`, the recursive definition gives:
     \[
     p_{k+1} = p_k + (3(k + 1) - 2) = p_k + (3k + 1)
     \]
   - Substitute the inductive hypothesis:
     \[
     p_{k+1} = \frac{k(3k - 1)}{2} + 3k + 1
     \]
   - Combine terms:
     \[
     p_{k+1} = \frac{3k^2 - k + 6k + 2}{2} = \frac{3k^2 + 5k + 2}{2}
     \]
   - Factor the numerator:
     \[
     3k^2 + 5k + 2 = (k + 1)(3k + 2)
     \]
   - Thus:
     \[
     p_{k+1} = \frac{(k + 1)(3k + 2)}{2}
     \]
   - This is the formula for `n = k + 1`, completing the induction.

### Conclusion

The formula `p_n = n * (3n - 1) / 2` is proven by induction for all `n ≥ 1`, matching the recursive definition of pentagonal numbers.