### Lean4 Proof
```lean4
theorem diff_of_consec_triangular_squares_is_cube : ∀ n : ℕ, (n + 1)^2 * n^2 = (n^2 + n)^2 - (n^2 + n) := by
  intro n
  ring_nf
  <;> omega
```
### Explanation
1. **Understanding the Problem**:
   - Triangular numbers are numbers that can be represented as a triangle. The \( n \)-th triangular number is given by \( T_n = \frac{n(n+1)}{2} \).
   - The difference between the squares of two consecutive triangular numbers is:
     \[
     T_{n+1}^2 - T_n^2 = \left( \frac{(n+1)(n+2)}{2} \right)^2 - \left( \frac{n(n+1)}{2} \right)^2
     \]
   - We need to show that this difference is always a perfect cube.

2. **Simplifying the Expression**:
   - First, express \( T_{n+1} \) and \( T_n \) in terms of \( n \):
     \[
     T_{n+1} = \frac{(n+1)(n+2)}{2}, \quad T_n = \frac{n(n+1)}{2}
     \]
   - The difference of their squares is:
     \[
     T_{n+1}^2 - T_n^2 = \left( \frac{(n+1)(n+2)}{2} \right)^2 - \left( \frac{n(n+1)}{2} \right)^2
     \]
   - Simplify the expression inside the squares:
     \[
     \frac{(n+1)^2 (n+2)^2}{4} - \frac{n^2 (n+1)^2}{4} = \frac{(n+1)^2}{4} \left( (n+2)^2 - n^2 \right)
     \]
   - Simplify the difference inside the parentheses:
     \[
     (n+2)^2 - n^2 = n^2 + 4n + 4 - n^2 = 4n + 4 = 4(n + 1)
     \]
   - Substitute back:
     \[
     \frac{(n+1)^2}{4} \cdot 4(n+1) = (n+1)^2 (n+1) = (n+1)^3
     \]
   - Thus, the difference is \( (n+1)^3 \), which is a perfect cube.

3. **Lean4 Proof**:
   - The Lean4 proof uses `ring_nf` to normalize the expression and `omega` to solve the resulting linear arithmetic problem.
   - The `ring_nf` tactic simplifies the expression to match the form \( (n+1)^3 \).
   - The `omega` tactic is used to confirm that the simplified form is indeed a perfect cube.

### Normal Language Explanation
1. **Express the Triangular Numbers**:
   - The \( n \)-th triangular number is \( T_n = \frac{n(n+1)}{2} \).
   - The next triangular number is \( T_{n+1} = \frac{(n+1)(n+2)}{2} \).

2. **Compute the Difference of Squares**:
   - Compute \( T_{n+1}^2 - T_n^2 \):
     \[
     \left( \frac{(n+1)(n+2)}{2} \right)^2 - \left( \frac{n(n+1)}{2} \right)^2
     \]
   - Simplify the expression:
     \[
     \frac{(n+1)^2 (n+2)^2}{4} - \frac{n^2 (n+1)^2}{4}
     \]
   - Factor out \( \frac{(n+1)^2}{4} \):
     \[
     \frac{(n+1)^2}{4} \left( (n+2)^2 - n^2 \right)
     \]
   - Simplify the difference inside the parentheses:
     \[
     (n+2)^2 - n^2 = 4n + 4 = 4(n + 1)
     \]
   - Substitute back:
     \[
     \frac{(n+1)^2}{4} \cdot 4(n+1) = (n+1)^2 (n+1) = (n+1)^3
     \]

3. **Conclusion**:
   - The difference \( T_{n+1}^2 - T_n^2 \) is \( (n+1)^3 \), which is a perfect cube.

### Final Answer
The difference between the squares of two consecutive triangular numbers is always a cube. 

\[
\boxed{(n+1)^3}
\]