### Lean4 Proof

```lean4
theorem triangular_number_binomial (n : ℕ) : t n = Nat.choose (n + 1) 2 := by
  induction n with
  | zero => simp [t]
  | succ n ih =>
    simp_all [t, Nat.choose_succ_succ, Nat.add_comm, Nat.add_assoc, Nat.add_left_comm]
    <;> ring_nf at *
    <;> omega
```

### Explanation

1. **Base Case (`n = 0`)**:
   - For `n = 0`, the first triangular number is `t_0 = 0`.
   - The binomial coefficient is `C(0 + 1, 2) = C(1, 2) = 0` (since `C(n, k) = 0` when `k > n`).
   - Thus, `t_0 = C(1, 2) = 0` holds.

2. **Inductive Step (`n → n + 1`)**:
   - Assume the statement holds for `n`, i.e., `t_n = C(n + 1, 2)`.
   - For `n + 1`, the next triangular number is `t_{n + 1} = t_n + (n + 1)`.
   - By the inductive hypothesis, `t_n = C(n + 1, 2)`.
   - Thus, `t_{n + 1} = C(n + 1, 2) + (n + 1)`.
   - We need to show that `C(n + 1 + 1, 2) = C(n + 2, 2) = C(n + 1, 2) + (n + 1)`.
   - This is a known property of binomial coefficients: `C(n + 2, 2) = C(n + 1, 2) + C(n + 1, 1) = C(n + 1, 2) + (n + 1)`.
   - Therefore, the inductive step holds.

### Normal Language Explanation

The proof is by induction on `n`.

1. **Base Case (`n = 0`)**:
   - `t_0 = 0` and `C(1, 2) = 0` because `C(n, k) = 0` when `k > n`.

2. **Inductive Step (`n → n + 1`)**:
   - Assume `t_n = C(n + 1, 2)`.
   - Then, `t_{n + 1} = t_n + (n + 1) = C(n + 1, 2) + (n + 1)`.
   - We need to show that `C(n + 2, 2) = C(n + 1, 2) + (n + 1)`.
   - This is a known identity for binomial coefficients: `C(n + 2, 2) = C(n + 1, 2) + C(n + 1, 1) = C(n + 1, 2) + (n + 1)`.
   - Thus, the inductive step is complete.

### Final Answer

The proof is complete by induction, and the identity `t_n = C(n + 1, 2)` holds for all `n ≥ 0`.