### Lean4 Proof
```lean4
theorem any_int_6k_5_is_3j_2 : ∀ k : ℤ, ∃ j : ℤ, 6 * k + 5 = 3 * j + 2 := by
  intro k
  use (2 * k + 1)
  ring
  <;> omega
```
### Explanation
1. **Introduction of `k`**: We start by introducing an arbitrary integer `k` to represent the form `6k + 5`.
2. **Existence of `j`**: We need to find an integer `j` such that `6k + 5 = 3j + 2`.
3. **Choice of `j`**: We choose `j = 2k + 1` and verify that it satisfies the equation.
4. **Verification**:
   - Substitute `j = 2k + 1` into `3j + 2` to get `3(2k + 1) + 2 = 6k + 3 + 2 = 6k + 5`, which matches the original form `6k + 5`.
   - The `ring` tactic simplifies the expression to confirm the equality.
   - The `omega` tactic is used to ensure that the solution is correct by checking the arithmetic.

### Normal Language Explanation
1. **Form Representation**:
   - Any integer of the form `6k + 5` can be written as `6k + 5` where `k` is an integer.
   - We need to show that such an integer is also of the form `3j + 2` for some integer `j`.
2. **Choice of `j`**:
   - We hypothesize that `j` is related to `k` in a linear fashion.
   - By testing small values, we observe that `j = 2k + 1` works:
     - For `k = 0`, `6*0 + 5 = 5` and `3*(2*0 + 1) + 2 = 3 + 2 = 5`.
     - For `k = 1`, `6*1 + 5 = 11` and `3*(2*1 + 1) + 2 = 9 + 2 = 11`.
     - For `k = -1`, `6*(-1) + 5 = -1` and `3*(2*(-1) + 1) + 2 = 3*(-1) + 2 = -3 + 2 = -1`.
3. **Verification**:
   - Substitute `j = 2k + 1` into `3j + 2` and simplify:
     \[
     3(2k + 1) + 2 = 6k + 3 + 2 = 6k + 5.
     \]
   - This confirms that `6k + 5 = 3j + 2` for `j = 2k + 1`.
4. **Non-Converse**:
   - The converse is not true because not every integer of the form `3j + 2` is also of the form `6k + 5`.
   - For example, `j = 0` gives `3*0 + 2 = 2`, but `2` is not of the form `6k + 5` for any integer `k` because `6k + 5 ≡ 5 mod 6`, while `2 ≡ 2 mod 6`.
   - Similarly, `j = 1` gives `3*1 + 2 = 5`, which is of the form `6k + 5` (`k = 0`), but `j = 2` gives `3*2 + 2 = 8`, which is not of the form `6k + 5` for any integer `k` (`8 ≡ 2 mod 6`).

### Conclusion
The proof shows that any integer of the form `6k + 5` can be expressed as `3j + 2` by choosing `j = 2k + 1`, but the converse is not true because not all integers of the form `3j + 2` are also of the form `6k + 5`.