### Lean4 Proof

```lean4
theorem square_form_3k_or_3k_plus_1 (n : ℤ) : n^2 % 3 = 0 ∨ n^2 % 3 = 1 := by
  have h : n % 3 = 0 ∨ n % 3 = 1 ∨ n % 3 = 2 := by omega
  rcases h with (h | h | h) <;>
  simp [h, pow_two, Int.mul_emod, Int.add_emod, Int.emod_emod]
  <;>
  omega
  <;>
  omega
  <;>
  omega
```

### Explanation

1. **Division Algorithm Setup**:
   - We use the fact that any integer `n` modulo 3 can only be 0, 1, or 2. This is because 3 is the divisor.

2. **Case Analysis**:
   - For each possible residue of `n` modulo 3, we compute `n^2 % 3`:
     - If `n % 3 = 0`, then `n^2 % 3 = 0`.
     - If `n % 3 = 1`, then `n^2 % 3 = 1`.
     - If `n % 3 = 2`, then `n^2 % 3 = 4 % 3 = 1` (since `2^2 = 4` and `4 % 3 = 1`).

3. **Conclusion**:
   - The possible values of `n^2 % 3` are 0 and 1, which proves the claim.

### Normal Language Proof

1. **Division Algorithm**:
   - Any integer `n` can be written as `n = 3k`, `n = 3k + 1`, or `n = 3k + 2` for some integer `k`.

2. **Case 1: `n = 3k`**:
   - Then `n^2 = (3k)^2 = 9k^2 = 3 * (3k^2)`, which is divisible by 3.

3. **Case 2: `n = 3k + 1`**:
   - Then `n^2 = (3k + 1)^2 = 9k^2 + 6k + 1 = 3(3k^2 + 2k) + 1`, so `n^2 % 3 = 1`.

4. **Case 3: `n = 3k + 2`**:
   - Then `n^2 = (3k + 2)^2 = 9k^2 + 12k + 4 = 9k^2 + 12k + 3 + 1 = 3(3k^2 + 4k + 1) + 1`, so `n^2 % 3 = 1`.

5. **Conclusion**:
   - The square of any integer is either of the form `3k` or `3k + 1`.

### Lean4 Proof for (b)

```lean4
theorem cube_form_9k_or_9k_plus_1_or_9k_plus_8 (n : ℤ) : n^3 % 9 = 0 ∨ n^3 % 9 = 1 ∨ n^3 % 9 = 8 := by
  have h : n % 9 = 0 ∨ n % 9 = 1 ∨ n % 9 = 2 ∨ n % 9 = 3 ∨ n % 9 = 4 ∨ n % 9 = 5 ∨ n % 9 = 6 ∨ n % 9 = 7 ∨ n % 9 = 8 := by omega
  rcases h with (h | h | h | h | h | h | h | h | h) <;>
  simp [h, pow_three, Int.mul_emod, Int.add_emod, Int.emod_emod]
  <;>
  omega
  <;>
  omega
  <;>
  omega
  <;>
  omega
  <;>
  omega
  <;>
  omega
  <;>
  omega
  <;>
  omega
```

### Explanation for (b)

1. **Division Algorithm Setup**:
   - Any integer `n` modulo 9 can be 0, 1, 2, 3, 4, 5, 6, 7, or 8.

2. **Case Analysis**:
   - For each residue, compute `n^3 % 9`:
     - If `n % 9 = 0`, then `n^3 % 9 = 0`.
     - If `n % 9 = 1`, then `n^3 % 9 = 1`.
     - If `n % 9 = 2`, then `n^3 % 9 = 8`.
     - If `n % 9 = 3`, then `n^3 % 9 = 0`.
     - If `n % 9 = 4`, then `n^3 % 9 = 1`.
     - If `n % 9 = 5`, then `n^3 % 9 = 8`.
     - If `n % 9 = 6`, then `n^3 % 9 = 0`.
     - If `n % 9 = 7`, then `n^3 % 9 = 1`.
     - If `n % 9 = 8`, then `n^3 % 9 = 8`.

3. **Conclusion**:
   - The possible values of `n^3 % 9` are 0, 1, and 8.

### Normal Language Proof for (b)

1. **Division Algorithm**:
   - Any integer `n` can be written as `n = 9k`, `n = 9k + 1`, ..., `n = 9k + 8` for some integer `k`.

2. **Case 1: `n = 9k`**:
   - Then `n^3 = (9k)^3 = 729k^3 = 9 * 81k^3`, which is divisible by 9.

3. **Case 2: `n = 9k + 1`**:
   - Then `n^3 = (9k + 1)^3 = 729k^3 + 243k^2 + 27k + 1 = 9(81k^3 + 27k^2 + 3k) + 1`, so `n^3 % 9 = 1`.

4. **Case 3: `n = 9k + 2`**:
   - Then `n^3 = (9k + 2)^3 = 729k^3 + 486k^2 + 108k + 8 = 9(81k^3 + 54k^2 + 12k) + 8`, so `n^3 % 9 = 8`.

5. **Case 4: `n = 9k + 3`**:
   - Then `n^3 = (9k + 3)^3 = 729k^3 + 810k^2 + 243k + 27 = 9(81k^3 + 90k^2 + 27k + 3)`, which is divisible by 9.

6. **Case 5: `n = 9k + 4`**:
   - Then `n^3 = (9k + 4)^3 = 729k^3 + 1080k^2 + 576k + 64 = 9(81k^3 + 120k^2 + 64k + 7) + 1`, so `n^3 % 9 = 1`.

7. **Case 6: `n = 9k + 5`**:
   - Then `n^3 = (9k + 5)^3 = 729k^3 + 1458k^2 + 720k + 125 = 9(81k^3 + 162k^2 + 80k + 13) + 8`, so `n^3 % 9 = 8`.

8. **Case 7: `n = 9k + 6`**:
   - Then `n^3 = (9k + 6)^3 = 729k^3 + 1701k^2 + 972k + 216 = 9(81k^3 + 189k^2 + 108k + 24)`, which is divisible by 9.

9. **Case 8: