### Lean4 Proof

```lean4
theorem part_a (a : ℤ) : 6 ∣ a * (a^2 + 11) := by
  apply Int.dvd_of_emod_eq_zero
  have : a % 6 = 0 ∨ a % 6 = 1 ∨ a % 6 = 2 ∨ a % 6 = 3 ∨ a % 6 = 4 ∨ a % 6 = 5 := by
    omega
  rcases this with (h | h | h | h | h | h) <;>
    simp [h, Int.mul_emod, Int.add_emod, pow_two, Int.emod_emod]
  <;>
  omega
```

### Explanation

1. **Understanding the Problem**: We need to show that for any integer `a`, `6` divides `a * (a^2 + 11)`. This is equivalent to showing that `a * (a^2 + 11) % 6 = 0`.

2. **Approach**: We consider all possible residues of `a` modulo 6, i.e., `a % 6` can be `0, 1, 2, 3, 4,` or `5`, and check that in each case, `a * (a^2 + 11) % 6 = 0`.

3. **Case-by-Case Verification**:
   - If `a % 6 = 0`, then `a` is a multiple of 6, so `a * (a^2 + 11)` is a multiple of 6.
   - If `a % 6 = 1`, then `a^2 + 11 ≡ 1 + 11 ≡ 12 ≡ 0 mod 6`, so the product is `1 * 0 ≡ 0 mod 6`.
   - Similarly, for `a % 6 = 2, 3, 4, 5`, we can compute `a^2 + 11 mod 6` and show that the product is `0 mod 6`.

4. **Lean4 Implementation**:
   - We use `Int.emod_emod` to simplify the expression `a % 6` and then check each case.
   - The `rcases` statement branches on the possible values of `a % 6`, and `simp` simplifies the expression for each case.
   - Finally, `omega` is used to solve the resulting arithmetic in each case.

### Normal Language Proof

1. **Case 1: `a` is a multiple of 6 (`a ≡ 0 mod 6`)**
   - Then `a = 6k` for some integer `k`.
   - `a * (a^2 + 11) = 6k * (36k^2 + 11) = 6 * (6k * (36k^2 + 11))`, which is clearly divisible by 6.

2. **Case 2: `a ≡ 1 mod 6`**
   - Then `a^2 + 11 ≡ 1 + 11 ≡ 12 ≡ 0 mod 6`.
   - So `a * (a^2 + 11) ≡ 1 * 0 ≡ 0 mod 6`.

3. **Case 3: `a ≡ 2 mod 6`**
   - Then `a^2 ≡ 4 mod 6`, so `a^2 + 11 ≡ 4 + 11 ≡ 15 ≡ 3 mod 6`.
   - But `a ≡ 2 mod 6` implies `a * (a^2 + 11) ≡ 2 * 3 ≡ 6 ≡ 0 mod 6`.

4. **Case 4: `a ≡ 3 mod 6`**
   - Then `a^2 ≡ 9 ≡ 3 mod 6`, so `a^2 + 11 ≡ 3 + 11 ≡ 14 ≡ 2 mod 6`.
   - Thus, `a * (a^2 + 11) ≡ 3 * 2 ≡ 6 ≡ 0 mod 6`.

5. **Case 5: `a ≡ 4 mod 6`**
   - Then `a^2 ≡ 16 ≡ 4 mod 6`, so `a^2 + 11 ≡ 4 + 11 ≡ 15 ≡ 3 mod 6`.
   - Thus, `a * (a^2 + 11) ≡ 4 * 3 ≡ 12 ≡ 0 mod 6`.

6. **Case 6: `a ≡ 5 mod 6`**
   - Then `a^2 ≡ 25 ≡ 1 mod 6`, so `a^2 + 11 ≡ 1 + 11 ≡ 12 ≡ 0 mod 6`.
   - Thus, `a * (a^2 + 11) ≡ 5 * 0 ≡ 0 mod 6`.

In all cases, `6` divides `a * (a^2 + 11)`.

### Conclusion

The proof is complete by verifying each possible residue of `a` modulo 6. The Lean4 code automates this verification, and the normal language proof provides the detailed reasoning for each case.