### Part (a): If \( a \mid b \), then \( a \mid bc \).

**Lean4 Proof Sketch:**
```lean4
theorem part_a (a b c : ℤ) (h : a ∣ b) : a ∣ b * c := by
  obtain ⟨k, hk⟩ := h
  use k * c
  rw [hk]
  ring
```

**Explanation:**
1. We start by assuming \( a \mid b \), which means there exists an integer \( k \) such that \( b = a \cdot k \).
2. We need to show \( a \mid bc \). To do this, we express \( bc \) in terms of \( a \):
   \[
   bc = (a \cdot k) \cdot c = a \cdot (k \cdot c).
   \]
3. Since \( k \cdot c \) is an integer, \( a \mid bc \) holds.

### Part (b): If \( a \mid b \) and \( a \mid c \), then \( a^2 \mid bc \).

**Lean4 Proof Sketch:**
```lean4
theorem part_b (a b c : ℤ) (h₁ : a ∣ b) (h₂ : a ∣ c) : a^2 ∣ b * c := by
  obtain ⟨k, hk⟩ := h₁
  obtain ⟨m, hm⟩ := h₂
  use k * m
  rw [hk, hm]
  ring
  <;> simp [mul_assoc, mul_comm, mul_left_comm]
  <;> ring
  <;> simp [mul_assoc, mul_comm, mul_left_comm]
  <;> ring
```

**Explanation:**
1. From \( a \mid b \), we have \( b = a \cdot k \) for some integer \( k \).
2. From \( a \mid c \), we have \( c = a \cdot m \) for some integer \( m \).
3. We need to show \( a^2 \mid bc \). Substitute \( b \) and \( c \):
   \[
   bc = (a \cdot k) \cdot (a \cdot m) = a^2 \cdot (k \cdot m).
   \]
4. Since \( k \cdot m \) is an integer, \( a^2 \mid bc \) holds.

### Part (c): \( a \mid b \) if and only if \( ac \mid bc \), where \( c \neq 0 \).

**Lean4 Proof Sketch:**
```lean4
theorem part_c (a b c : ℤ) (hc : c ≠ 0) : a ∣ b ↔ a * c ∣ b * c := by
  constructor
  · intro h
    obtain ⟨k, hk⟩ := h
    use k
    rw [hk]
    ring
  · intro h
    obtain ⟨k, hk⟩ := h
    use k
    rw [hk]
    ring
```

**Explanation:**
1. **Forward direction (\( a \mid b \implies ac \mid bc \)):**
   - Assume \( a \mid b \), so \( b = a \cdot k \) for some integer \( k \).
   - Then \( bc = a \cdot k \cdot c \), so \( ac \mid bc \) because \( bc = (ac) \cdot k \).

2. **Backward direction (\( ac \mid bc \implies a \mid b \)):**
   - Assume \( ac \mid bc \), so \( bc = (ac) \cdot k \) for some integer \( k \).
   - Since \( c \neq 0 \), we can divide both sides by \( c \) to get \( b = a \cdot k \), so \( a \mid b \).

### Part (d): If \( a \mid b \) and \( c \mid d \), then \( ac \mid bd \).

**Lean4 Proof Sketch:**
```lean4
theorem part_d (a b c d : ℤ) (h₁ : a ∣ b) (h₂ : c ∣ d) : a * c ∣ b * d := by
  obtain ⟨k, hk⟩ := h₁
  obtain ⟨m, hm⟩ := h₂
  use k * m
  rw [hk, hm]
  ring
  <;> simp [mul_assoc, mul_comm, mul_left_comm]
  <;> ring
  <;> simp [mul_assoc, mul_comm, mul_left_comm]
  <;> ring
```

**Explanation:**
1. From \( a \mid b \), we have \( b = a \cdot k \) for some integer \( k \).
2. From \( c \mid d \), we have \( d = c \cdot m \) for some integer \( m \).
3. We need to show \( ac \mid bd \). Substitute \( b \) and \( d \):
   \[
   bd = (a \cdot k) \cdot (c \cdot m) = a \cdot c \cdot (k \cdot m).
   \]
4. Since \( k \cdot m \) is an integer, \( ac \mid bd \) holds.

### Complete Lean4 Proof

```lean4
theorem part_a (a b c : ℤ) (h : a ∣ b) : a ∣ b * c := by
  obtain ⟨k, hk⟩ := h
  use k * c
  rw [hk]
  ring
```

```lean4
theorem part_b (a b c : ℤ) (h₁ : a ∣ b) (h₂ : a ∣ c) : a^2 ∣ b * c := by
  obtain ⟨k, hk⟩ := h₁
  obtain ⟨m, hm⟩ := h₂
  use k * m
  rw [hk, hm]
  ring
  <;> simp [mul_assoc, mul_comm, mul_left_comm]
  <;> ring
```

```lean4
theorem part_c (a b c : ℤ) (hc : c ≠ 0) : a ∣ b ↔ a * c ∣ b * c := by
  constructor
  · intro h
    obtain ⟨k, hk⟩ := h
    use k
    rw [hk]
    ring
  · intro h
    obtain ⟨k, hk⟩ := h
    use k
    rw [hk]
    ring
```

```lean4
theorem part_d (a b c d : ℤ) (h₁ : a ∣ b) (h₂ : c ∣ d) : a * c ∣ b * d := by
  obtain ⟨k, hk⟩ := h₁
  obtain ⟨m, hm⟩ := h₂
  use k * m
  rw [hk, hm]
  ring
  <;> simp [mul_assoc, mul_comm, mul_left_comm]
  <;> ring
```