### Part (a): gcd(2a + 1, 9a + 4) = 1

**Lean4 Proof Sketch:**
```lean4
theorem gcd_2a_plus_1_9a_plus_4 : ∀ a : ℤ, gcd (2 * a + 1) (9 * a + 4) = 1 := by
  intro a
  have h : gcd (2 * a + 1) (9 * a + 4) = 1 := by
    -- Use the Euclidean algorithm to find the gcd
    rw [gcd_comm]
    -- Apply the Euclidean algorithm step: 9a + 4 = 4 * (2a + 1) + (a)
    have h₁ : 9 * a + 4 = 4 * (2 * a + 1) + (a) := by ring
    -- Apply the Euclidean algorithm step: 2a + 1 = 2 * (a) + 1
    have h₂ : 2 * a + 1 = 2 * (a) + 1 := by ring
    -- Continue applying the Euclidean algorithm
    simp_all [gcd_eq_natAbs, Nat.gcd_eq_right]
    <;>
    omega
  exact h
```

**Normal Language Proof:**
1. We need to show that \(\gcd(2a + 1, 9a + 4) = 1\) for any integer \(a\).
2. Using the Euclidean algorithm:
   - \(9a + 4 = 4(2a + 1) + (a)\).
   - \(2a + 1 = 2(a) + 1\).
3. The gcd of \(2a + 1\) and \(9a + 4\) is the same as the gcd of \(2a + 1\) and \(a\) (since \(9a + 4 - 4(2a + 1) = a\)).
4. Now, consider \(\gcd(2a + 1, a)\):
   - \(2a + 1 = 2a + 1\).
   - \(a = 1 \cdot a + 0\).
5. The gcd of \(2a + 1\) and \(a\) is the same as the gcd of \(a\) and \(1\) (since \(2a + 1 - 2a = 1\)).
6. The gcd of \(a\) and \(1\) is \(1\) for any integer \(a\).
7. Thus, \(\gcd(2a + 1, 9a + 4) = 1\).

### Part (b): gcd(5a + 2, 7a + 3) = 1

**Lean4 Proof Sketch:**
```lean4
theorem gcd_5a_plus_2_7a_plus_3 : ∀ a : ℤ, gcd (5 * a + 2) (7 * a + 3) = 1 := by
  intro a
  have h : gcd (5 * a + 2) (7 * a + 3) = 1 := by
    -- Use the Euclidean algorithm to find the gcd
    rw [gcd_comm]
    -- Apply the Euclidean algorithm step: 7a + 3 = 1 * (5a + 2) + (2a + 1)
    have h₁ : 7 * a + 3 = 1 * (5 * a + 2) + (2 * a + 1) := by ring
    -- Apply the Euclidean algorithm step: 5a + 2 = 2 * (2a + 1) + (a)
    have h₂ : 5 * a + 2 = 2 * (2 * a + 1) + (a) := by ring
    -- Continue applying the Euclidean algorithm
    simp_all [gcd_eq_natAbs, Nat.gcd_eq_right]
    <;>
    omega
  exact h
```

**Normal Language Proof:**
1. We need to show that \(\gcd(5a + 2, 7a + 3) = 1\) for any integer \(a\).
2. Using the Euclidean algorithm:
   - \(7a + 3 = 1 \cdot (5a + 2) + (2a + 1)\).
   - \(5a + 2 = 2 \cdot (2a + 1) + (a)\).
3. The gcd of \(5a + 2\) and \(7a + 3\) is the same as the gcd of \(5a + 2\) and \(2a + 1\) (since \(7a + 3 - 1 \cdot (5a + 2) = 2a + 1\)).
4. Now, consider \(\gcd(5a + 2, 2a + 1)\):
   - \(5a + 2 = 2 \cdot (2a + 1) + (a)\).
   - \(2a + 1 = 2 \cdot a + 1\).
5. The gcd of \(5a + 2\) and \(2a + 1\) is the same as the gcd of \(2a + 1\) and \(a\) (since \(5a + 2 - 2 \cdot (2a + 1) = a\)).
6. The gcd of \(2a + 1\) and \(a\) is the same as the gcd of \(a\) and \(1\) (since \(2a + 1 - 2a = 1\)).
7. The gcd of \(a\) and \(1\) is \(1\) for any integer \(a\).
8. Thus, \(\gcd(5a + 2, 7a + 3) = 1\).

### Part (c): If \(a\) is odd, then \(\gcd(3a, 3a + 2) = 1\)

**Lean4 Proof Sketch:**
```lean4
theorem gcd_3a_3a_plus_2_odd_a : ∀ a : ℤ, Odd a → gcd (3 * a) (3 * a + 2) = 1 := by
  intro a ha
  have h : gcd (3 * a) (3 * a + 2) = 1 := by
    -- Use the Euclidean algorithm to find the gcd
    rw [gcd_comm]
    -- Apply the Euclidean algorithm step: 3a + 2 = 1 * (3a) + 2
    have h₁ : 3 * a + 2 = 1 * (3 * a) + 2 := by ring
    -- Continue applying the Euclidean algorithm
    simp_all [gcd_eq_natAbs, Nat.gcd_eq_right]
    <;>
    omega
  exact h
```

**Normal Language Proof:**
1. We need to show that if \(a\) is odd, then \(\gcd(3a, 3a + 2) = 1\).
2. Since \(a\) is odd, let \(a = 2k + 1\) for some integer \(k\).
3. Then \(3a = 6k + 3\) and \(3a + 2 = 6k + 5\).
4. The gcd of \(6k + 3\) and \(6k + 5\) is the same as the gcd of \(6k + 3\) and \(2\) (since \(6k + 5 - (6k + 3) = 2\)).
5. The gcd of \(6k + 3\) and \(2\) is the same as the gcd of \(3\) and \(2\) (since \(6k + 3 = 3(2k + 1) = 3a\)).
6. The gcd of \(3\) and \(2\) is \(1\).
7. Thus, \(\gcd(3a, 3a + 2) = 1\).