### Part (a)

**Lean4 Proof Sketch:**
```lean4
theorem part_a (a : ℤ) : 2 ∣ a * (a + 1) ∧ 3 ∣ a * (a + 1) * (a + 2) := by
  have h1 : 2 ∣ a * (a + 1) := by
    -- Show that a(a + 1) is even by considering the parity of a.
    have h1 : a % 2 = 0 ∨ a % 2 = 1 := by omega
    rcases h1 with (h1 | h1) <;>
    (try omega) <;>
    (try {
      -- If a is even, a = 2k, then a(a + 1) = 2k(2k + 1) is divisible by 2.
      use a / 2 * (a + 1)
      omega
    }) <;>
    (try {
      -- If a is odd, a = 2k + 1, then a(a + 1) = (2k + 1)(2k + 2) = 2(2k + 1)(k + 1) is divisible by 2.
      use (a + 1) / 2 * a
      omega
    })
  have h2 : 3 ∣ a * (a + 1) * (a + 2) := by
    -- Show that a(a + 1)(a + 2) is divisible by 3 by considering the residues modulo 3.
    have h2 : a % 3 = 0 ∨ a % 3 = 1 ∨ a % 3 = 2 := by omega
    rcases h2 with (h2 | h2 | h2) <;>
    (try omega) <;>
    (try {
      -- If a ≡ 0 mod 3, then a(a + 1)(a + 2) is divisible by 3.
      use a / 3 * (a + 1) * (a + 2)
      omega
    }) <;>
    (try {
      -- If a ≡ 1 mod 3, then a + 2 ≡ 0 mod 3, so a(a + 1)(a + 2) is divisible by 3.
      use (a + 1) / 3 * a * (a + 2)
      omega
    }) <;>
    (try {
      -- If a ≡ 2 mod 3, then a + 1 ≡ 0 mod 3, so a(a + 1)(a + 2) is divisible by 3.
      use (a + 2) / 3 * a * (a + 1)
      omega
    })
  exact ⟨h1, h2⟩
```

**Normal Language Proof:**
1. **Part (a)(i):** \(2 \mid a(a + 1)\)
   - Consider the parity of \(a\). If \(a\) is even, \(a = 2k\), then \(a(a + 1) = 2k(2k + 1)\), which is divisible by 2. If \(a\) is odd, \(a = 2k + 1\), then \(a(a + 1) = (2k + 1)(2k + 2) = 2(2k + 1)(k + 1)\), which is divisible by 2. Thus, \(2 \mid a(a + 1)\) in all cases.

2. **Part (a)(ii):** \(3 \mid a(a + 1)(a + 2)\)
   - By the Pigeonhole Principle, among any three consecutive integers, one is divisible by 3. Thus, \(3 \mid a(a + 1)(a + 2)\).

### Part (b)

**Lean4 Proof Sketch:**
```lean4
theorem part_b (a : ℤ) : 3 ∣ a * (2 * a ^ 2 + 7) := by
  have h1 : a % 3 = 0 ∨ a % 3 = 1 ∨ a % 3 = 2 := by omega
  rcases h1 with (h1 | h1 | h1) <;>
  (try omega) <;>
  (try {
    -- If a ≡ 0 mod 3, then a(2a^2 + 7) ≡ 0 mod 3.
    use a / 3 * (2 * a ^ 2 + 7)
    omega
  }) <;>
  (try {
    -- If a ≡ 1 mod 3, then 2a^2 + 7 ≡ 2*1 + 7 ≡ 9 ≡ 0 mod 3.
    use (2 * a ^ 2 + 7) / 3 * a
    omega
  }) <;>
  (try {
    -- If a ≡ 2 mod 3, then 2a^2 + 7 ≡ 2*4 + 7 ≡ 15 ≡ 0 mod 3.
    use (2 * a ^ 2 + 7) / 3 * a
    omega
  })
```

**Normal Language Proof:**
- Consider \(a \mod 3\). If \(a \equiv 0 \mod 3\), then \(3 \mid a(2a^2 + 7)\). If \(a \equiv 1 \mod 3\), then \(2a^2 + 7 \equiv 2*1 + 7 \equiv 9 \equiv 0 \mod 3\), so \(3 \mid a(2a^2 + 7)\). If \(a \equiv 2 \mod 3\), then \(2a^2 + 7 \equiv 2*4 + 7 \equiv 15 \equiv 0 \mod 3\), so \(3 \mid a(2a^2 + 7)\). Thus, \(3 \mid a(2a^2 + 7)\) in all cases.

### Part (c)

**Lean4 Proof Sketch:**
```lean4
theorem part_c (a : ℤ) (h : a % 2 = 1) : 32 ∣ (a ^ 2 + 3) * (a ^ 2 + 7) := by
  have h1 : a ^ 2 % 16 = 1 := by
    have : a % 16 = 1 ∨ a % 16 = 3 ∨ a % 16 = 5 ∨ a % 16 = 7 ∨ a % 16 = 9 ∨ a % 16 = 11 ∨ a % 16 = 13 ∨ a % 16 = 15 := by omega
    rcases this with (h1 | h1 | h1 | h1 | h1 | h1 | h1 | h1) <;>
    simp [h1, pow_two, Int.mul_emod, Int.add_emod]
  have h2 : a ^ 2 % 2 = 1 := by
    have : a % 2 = 1 := h
    have : a ^ 2 % 2 = 1 := by
      have : a % 2 = 1 := h
      simp [this, pow_two, Int.mul_emod]
    exact this
  have h3 : (a ^ 2 + 3) * (a ^ 2 + 7) % 32 = 0 := by
    have : a ^ 2 % 32 = 1 ∨ a ^ 2 % 32 = 9 ∨ a ^ 2 % 32 = 25 := by
      omega
    rcases this with (h1 | h1 | h1) <;>
    simp [h1, Int.mul_emod, Int.add_emod, Int.emod_emod]
    <;>
    omega
  omega
```

**Normal Language Proof:**
- Since \(a\) is odd, \(a^2 \equiv 1 \mod 8\) and \(a^2 \equiv 1 \mod 4\). Thus, \(a^2 + 3 \equiv 0 \mod 4\) and \(a^2 + 7 \equiv 0 \mod 8\). Therefore, \((a^2 + 3)(a^2 + 7) \equiv 0 \mod 32\). Hence, \(32 \mid (a^2 + 3)(a^2 + 7)\).