### Lean4 Proof
```lean4
theorem gcd_dvd_n (n : ℕ) (a : ℤ) : (gcd a (a + n)) ∣ n := by
  have h : gcd a (a + n) ∣ a + n := gcd_dvd_right a (a + n)
  have h' : gcd a (a + n) ∣ a := gcd_dvd_left a (a + n)
  have h'' : gcd a (a + n) ∣ (a + n) - a := dvd_sub h h'
  simp at h''
  simp_all
```
### Explanation
1. **`gcd_dvd_right` and `gcd_dvd_left`**: These lemmas state that the gcd of two numbers divides each of the numbers. Specifically, `gcd a (a + n)` divides `a` and `a + n`.
2. **`dvd_sub`**: This lemma states that if a number divides two other numbers, it divides their difference. Here, `gcd a (a + n)` divides both `a` and `a + n`, so it divides their difference `(a + n) - a = n`.
3. **Simplification**: The final step simplifies the expression to show that `gcd a (a + n)` divides `n`.

### Normal Language Proof
1. Let `d = gcd(a, a + n)`. By definition, `d` divides both `a` and `a + n`.
2. Since `d` divides `a + n` and `a`, it must also divide their difference, which is `(a + n) - a = n`.
3. Therefore, `d` divides `n`, and hence `gcd(a, a + n)` divides `n`.
4. For the specific case `gcd(a, a + 1)`, we set `n = 1` in the above reasoning, so `gcd(a, a + 1)` divides `1`, which implies `gcd(a, a + 1) = 1` because the only positive divisors of `1` are `1` and `-1`, and `gcd` is positive.

### Lean4 Proof for `gcd(a, a + 1) = 1`
```lean4
theorem gcd_a_a_plus_1 : ∀ a : ℤ, gcd a (a + 1) = 1 := by
  intro a
  have h : gcd a (a + 1) ∣ 1 := by
    have h₁ : gcd a (a + 1) ∣ a := gcd_dvd_left a (a + 1)
    have h₂ : gcd a (a + 1) ∣ (a + 1) := gcd_dvd_right a (a + 1)
    have h₃ : gcd a (a + 1) ∣ (a + 1) - a := dvd_sub h₂ h₁
    simp at h₃
    exact h₃
  have h₄ : gcd a (a + 1) = 1 := by
    have h₅ : gcd a (a + 1) ∣ 1 := h
    have h₆ : gcd a (a + 1) ≥ 0 := by apply Int.natCast_nonneg
    have h₇ : gcd a (a + 1) ≤ 1 := by
      apply Int.le_of_dvd
      norm_num
      exact h₅
    have h₈ : gcd a (a + 1) ≥ 0 := by apply Int.natCast_nonneg
    have h₉ : gcd a (a + 1) ≤ 1 := by
      apply Int.le_of_dvd
      norm_num
      exact h₅
    have h₁₀ : gcd a (a + 1) = 1 := by
      omega
    exact h₁₀
  exact h₄
```