### Lean4 Proof
```lean4
theorem divisible_by_3 (a : ℤ) : ∃ k : ℤ, a = 3 * k ∨ a + 2 = 3 * k ∨ a + 4 = 3 * k := by
  have h₁ : a % 3 = 0 ∨ a % 3 = 1 ∨ a % 3 = 2 := by omega
  rcases h₁ with (h₁ | h₁ | h₁) <;>
  (try { use a / 3; omega }) <;>
  (try { use (a + 2) / 3; omega }) <;>
  (try { use (a + 4) / 3; omega })
```

### Explanation
1. **Case Analysis on Remainder Modulo 3**:
   - We know that any integer `a` when divided by 3 can have a remainder of 0, 1, or 2. This is captured by `h₁ : a % 3 = 0 ∨ a % 3 = 1 ∨ a % 3 = 2`.

2. **Handling Each Case**:
   - **Case 1 (`a % 3 = 0`)**:
     - If `a % 3 = 0`, then `a = 3 * (a / 3)`, so we can choose `k = a / 3` and the first disjunct holds.
   - **Case 2 (`a % 3 = 1`)**:
     - If `a % 3 = 1`, then `a + 2 = 3 * (a / 3)`, so we can choose `k = (a + 2) / 3` and the second disjunct holds.
   - **Case 3 (`a % 3 = 2`)**:
     - If `a % 3 = 2`, then `a + 4 = 3 * (a / 3)`, so we can choose `k = (a + 4) / 3` and the third disjunct holds.

3. **Conclusion**:
   - In all cases, we have found an integer `k` such that one of the three conditions holds, proving the theorem.

### Normal Language Explanation
The proof is based on the fact that any integer `a` when divided by 3 can only have a remainder of 0, 1, or 2. We then consider each possible remainder:
1. If `a` is divisible by 3, then `a` is the desired multiple of 3.
2. If `a` leaves a remainder of 1 when divided by 3, then `a + 2` is the desired multiple of 3.
3. If `a` leaves a remainder of 2 when divided by 3, then `a + 4` is the desired multiple of 3.

This covers all possible cases, proving the theorem.