### Lean4 Proof
```lean4
theorem odd_integers_divisible_by_16 (a b : ℤ) (ha : a % 2 = 1) (hb : b % 2 = 1) : 16 ∣ (a^4 + b^4 - 2) := by
  have h₁ : a^4 % 16 = 1 := by
    have : a % 16 = 1 ∨ a % 16 = 3 ∨ a % 16 = 5 ∨ a % 16 = 7 ∨ a % 16 = 9 ∨ a % 16 = 11 ∨ a % 16 = 13 ∨ a % 16 = 15 := by omega
    rcases this with (h | h | h | h | h | h | h | h) <;> simp [h, pow_succ, Int.mul_emod, Int.add_emod]
  have h₂ : b^4 % 16 = 1 := by
    have : b % 16 = 1 ∨ b % 16 = 3 ∨ b % 16 = 5 ∨ b % 16 = 7 ∨ b % 16 = 9 ∨ b % 16 = 11 ∨ b % 16 = 13 ∨ b % 16 = 15 := by omega
    rcases this with (h | h | h | h | h | h | h | h) <;> simp [h, pow_succ, Int.mul_emod, Int.add_emod]
  have h₃ : (a^4 + b^4 - 2) % 16 = 0 := by omega
  exact Int.dvd_of_emod_eq_zero h₃
```
### Explanation
1. **Modulo 16 Analysis for \(a^4\) and \(b^4\)**:
   - Since \(a\) and \(b\) are odd, \(a \equiv 1, 3, 5, 7, 9, 11, 13, 15 \pmod{16}\).
   - For each case, compute \(a^4 \pmod{16}\) and \(b^4 \pmod{16}\).
   - The result is \(a^4 \equiv 1 \pmod{16}\) and \(b^4 \equiv 1 \pmod{16}\).

2. **Sum and Modulo 16**:
   - \(a^4 + b^4 - 2 \equiv 1 + 1 - 2 = 0 \pmod{16}\).
   - Thus, \(16 \mid (a^4 + b^4 - 2)\).

### Normal Language Explanation
- **Odd Integers Modulo 16**:
  - Any odd integer \(a\) can be written as \(a = 2k + 1\) for some integer \(k\).
  - Then \(a^2 = 4k(k + 1) + 1\), so \(a^2 \equiv 1 \pmod{8}\).
  - Similarly, \(a^4 \equiv 1 \pmod{16}\).

- **Sum and Modulo 16**:
  - Since \(a^4 \equiv 1 \pmod{16}\) and \(b^4 \equiv 1 \pmod{16}\), their sum is \(2 \pmod{16}\).
  - Subtracting 2 gives \(0 \pmod{16}\), so \(16\) divides the expression.