### Lean4 Proof
```lean4
theorem neg_dvd_of_dvd {α : Type*} [Ring α] {a b : α} (h : a ∣ b) : (-a) ∣ b := by
  obtain ⟨k, hk⟩ := h
  use -k
  rw [← neg_neg a, ← neg_mul]
  <;> simp [hk]
  <;> ring
  <;> simp_all
  <;> ring
  <;> simp_all
  <;> ring
  <;> simp_all
  <;> ring
  <;> simp_all
```

### Explanation
1. **Given**: `a ∣ b` means there exists a `k` such that `b = a * k`.
2. **To Prove**: `(-a) ∣ b`
3. **Proof**:
   - Since `a ∣ b`, there exists a `k` such that `b = a * k`.
   - We need to find a `m` such that `b = (-a) * m`.
   - Let `m = -k`. Then `b = a * k = a * (-(-k)) = a * (-m)`.
   - But we need `b = (-a) * m`, so `b = (-a) * (-k) = a * k`, which is correct.
   - Thus, `(-a) ∣ b`.

### Normal Language Proof
1. **Given**: `a` divides `b` means there exists an integer `k` such that `b = a * k`.
2. **To Prove**: `-a` divides `b`
3. **Proof**:
   - Since `a` divides `b`, there exists an integer `k` such that `b = a * k`.
   - We need to find an integer `m` such that `b = (-a) * m`.
   - Let `m = -k`. Then `b = a * k = a * (-(-k)) = a * (-m)`.
   - But we need `b = (-a) * m`, so `b = (-a) * (-k) = a * k`, which is correct.
   - Thus, `-a` divides `b`.

### Lean4 Proof for `a ∣ (-b)`
```lean4
theorem dvd_neg_of_dvd {α : Type*} [Ring α] {a b : α} (h : a ∣ b) : a ∣ (-b) := by
  obtain ⟨k, hk⟩ := h
  use -k
  rw [← neg_neg b, ← mul_neg]
  <;> simp [hk]
  <;> ring
  <;> simp_all
  <;> ring
  <;> simp_all
  <;> ring
  <;> simp_all
```

### Normal Language Proof for `a ∣ (-b)`
1. **Given**: `a` divides `b` means there exists an integer `k` such that `b = a * k`.
2. **To Prove**: `a` divides `-b`
3. **Proof**:
   - Since `a` divides `b`, there exists an integer `k` such that `b = a * k`.
   - We need to find an integer `m` such that `-b = a * m`.
   - Let `m = -k`. Then `-b = - (a * k) = a * (-k) = a * m`.
   - Thus, `a` divides `-b`.

### Lean4 Proof for `(-a) ∣ (-b)`
```lean4
theorem neg_dvd_neg_of_dvd {α : Type*} [Ring α] {a b : α} (h : a ∣ b) : (-a) ∣ (-b) := by
  obtain ⟨k, hk⟩ := h
  use k
  rw [← neg_neg b, ← neg_mul]
  <;> simp [hk]
  <;> ring
  <;> simp_all
  <;> ring
  <;> simp_all
  <;> ring
  <;> simp_all
```

### Normal Language Proof for `(-a) ∣ (-b)`
1. **Given**: `a` divides `b` means there exists an integer `k` such that `b = a * k`.
2. **To Prove**: `-a` divides `-b`
3. **Proof**:
   - Since `a` divides `b`, there exists an integer `k` such that `b = a * k`.
   - We need to find an integer `m` such that `-b = (-a) * m`.
   - Let `m = k`. Then `-b = - (a * k) = (-a) * k = (-a) * m`.
   - Thus, `-a` divides `-b`.

### Summary
- `a ∣ b` implies `(-a) ∣ b` by using `m = -k`.
- `a ∣ b` implies `a ∣ (-b)` by using `m = -k`.
- `a ∣ b` implies `(-a) ∣ (-b)` by using `m = k`.