### (a) If gcd(a, b) = 1, and gcd(a, c) = 1, then gcd(a, bc)= 1.

**Lean4 Proof Sketch:**
```lean4
theorem gcd_a : ∀ a b c : ℕ, gcd a b = 1 → gcd a c = 1 → gcd a (b * c) = 1 := by
  intro a b c h₁ h₂
  have h₃ : Nat.gcd a (b * c) = 1 := by
    -- Use the property that gcd(a, bc) = 1 if gcd(a, b) = 1 and gcd(a, c) = 1
    rw [Nat.gcd_comm]
    simp_all [Nat.coprime_mul_iff_left, Nat.coprime_comm]
  exact h₃
```

**Normal Language Proof:**
1. We know that \(\gcd(a, b) = 1\) and \(\gcd(a, c) = 1\).
2. By the property of gcd, if \(\gcd(a, b) = 1\) and \(\gcd(a, c) = 1\), then \(\gcd(a, bc) = 1\).
3. This is because \(a\) and \(b\) are coprime, and \(a\) and \(c\) are coprime, so \(a\) and \(bc\) are also coprime.

### (b) If gcd(a, b) = 1, and c | a, then gcd(b, c) = 1.

**Lean4 Proof Sketch:**
```lean4
theorem gcd_b : ∀ a b c : ℕ, gcd a b = 1 → c ∣ a → gcd b c = 1 := by
  intro a b c h₁ h₂
  have h₃ : Nat.gcd b c = 1 := by
    -- Use the property that if c divides a and gcd(a, b) = 1, then gcd(b, c) = 1
    apply Nat.Coprime.coprime_dvd_left h₂
    simp_all [Nat.coprime_comm]
  exact h₃
```

**Normal Language Proof:**
1. We know that \(\gcd(a, b) = 1\) and \(c \mid a\).
2. Since \(c \mid a\), we can write \(a = k \cdot c\) for some integer \(k\).
3. We need to show that \(\gcd(b, c) = 1\).
4. Suppose for contradiction that \(\gcd(b, c) = d > 1\). Then \(d \mid b\) and \(d \mid c\).
5. But \(d \mid c\) and \(c \mid a\) implies \(d \mid a\).
6. Since \(d \mid a\) and \(d \mid b\), we have \(d \mid \gcd(a, b) = 1\), which is a contradiction.
7. Thus, \(\gcd(b, c) = 1\).

### (c) If gcd(a, b) = 1, then gcd(ac, b) = gcd(c, b).

**Lean4 Proof Sketch:**
```lean4
theorem gcd_c : ∀ a b c : ℕ, gcd a b = 1 → gcd (a * c) b = gcd c b := by
  intro a b c h
  have h₁ : Nat.gcd (a * c) b = Nat.gcd c b := by
    -- Use the property that gcd(ac, b) = gcd(c, b) if gcd(a, b) = 1
    rw [Nat.gcd_comm]
    rw [Nat.gcd_comm]
    simp_all [Nat.coprime_mul_iff_left, Nat.coprime_comm]
  exact h₁
```

**Normal Language Proof:**
1. We know that \(\gcd(a, b) = 1\).
2. We need to show that \(\gcd(ac, b) = \gcd(c, b)\).
3. Since \(\gcd(a, b) = 1\), \(a\) and \(b\) are coprime.
4. The gcd of \(ac\) and \(b\) is the same as the gcd of \(c\) and \(b\) because \(a\) and \(b\) are coprime.
5. This is because \(a\) does not introduce any common factors with \(b\) that would affect the gcd with \(b\).

### (d) If gcd(a, b) = 1, and c | a+ b, then gcd(a, c) = gcd(b, c) = 1.

**Lean4 Proof Sketch:**
```lean4
theorem gcd_d : ∀ a b c : ℕ, gcd a b = 1 → c ∣ a + b → gcd a c = 1 ∧ gcd b c = 1 := by
  intro a b c h₁ h₂
  have h₃ : Nat.gcd a c = 1 := by
    -- Use the property that if c divides a + b and gcd(a, b) = 1, then gcd(a, c) = 1
    have h₃ := Nat.Coprime.symm h₁
    have h₄ := Nat.dvd_sub' h₂ (h₂.trans (Nat.dvd_add_right (Nat.dvd_refl a)))
    simp_all [Nat.coprime_iff_gcd_eq_one, Nat.gcd_comm]
    <;> omega
  have h₄ : Nat.gcd b c = 1 := by
    -- Similarly, gcd(b, c) = 1
    have h₃ := Nat.Coprime.symm h₁
    have h₄ := Nat.dvd_sub' h₂ (h₂.trans (Nat.dvd_add_left (Nat.dvd_refl b)))
    simp_all [Nat.coprime_iff_gcd_eq_one, Nat.gcd_comm]
    <;> omega
  exact ⟨h₃, h₄⟩
```

**Normal Language Proof:**
1. We know that \(\gcd(a, b) = 1\) and \(c \mid a + b\).
2. We need to show that \(\gcd(a, c) = 1\) and \(\gcd(b, c) = 1\).
3. Suppose for contradiction that \(\gcd(a, c) \neq 1\) or \(\gcd(b, c) \neq 1\).
4. Then there exists a prime \(p\) dividing both \(a\) and \(c\) or \(b\) and \(c\), respectively.
5. Since \(c \mid a + b\), \(p\) divides \(a + b\).
6. This implies \(p\) divides both \(a\) and \(b\), contradicting \(\gcd(a, b) = 1\).
7. Thus, \(\gcd(a, c) = 1\) and \(\gcd(b, c) = 1\).

### (e) If gcd(a, b) = 1, d | ac, and d | be, then d | c.

**Lean4 Proof Sketch:**
```lean4
theorem gcd_e : ∀ a b d : ℕ, gcd a b = 1 → d ∣ a * c → d ∣ b * e → d ∣ c := by
  intro a b d h₁ h₂ h₃
  have h₄ : d ∣ c := by
    -- Use the property that if d divides both ac and be, and gcd(a, b) = 1, then d divides c
    have h₄ := Nat.dvd_gcd h₂ h₃
    simp_all [Nat.coprime_mul_iff_left, Nat.coprime_mul_iff_right, Nat.coprime_comm]
    <;> aesop
  exact h₄
```

**Normal Language Proof:**
1. We know that \(\gcd(a, b) = 1\), \(d \mid ac\), and \(d \mid be\).
2. We need to show that \(d \mid c\).
3. Since \(d \mid ac\) and \(d \mid be\), we can write \(ac = k_1 d\) and \(be = k_2 d\) for some integers \(k_1\) and \(k_2\).
4. From \(ac = k_1 d\), we have \(a \cdot c = k_1 d\).
5. From \(be = k_2 d\), we have \(b \cdot e = k_2 d\).
6. Since \(\gcd(a, b) = 1\), \(a\) and \(b\) are coprime.
7. Thus, \(d\) must divide \(c\) because \(d\) cannot introduce any new common factors with \(a\) or \(b\) beyond those already present in \(c\).

### (f) If