### Lean4 Proof

```lean4
theorem odd_square_sum_divisible_by_12 (a : ℤ) (h : a % 2 = 1) : 12 ∣ (a^2 + (a + 2)^2 + (a + 4)^2 + 1) := by
  have h1 : a^2 + (a + 2)^2 + (a + 4)^2 + 1 = 3 * a^2 + 12 * a + 21 := by
    ring
  rw [h1]
  apply Int.dvd_of_emod_eq_zero
  have h2 : (3 * a^2 + 12 * a + 21) % 12 = 0 := by
    have h3 : a % 12 = 1 ∨ a % 12 = 3 ∨ a % 12 = 5 ∨ a % 12 = 7 ∨ a % 12 = 9 ∨ a % 12 = 11 := by
      omega
    rcases h3 with (h3 | h3 | h3 | h3 | h3 | h3) <;>
      simp [h3, pow_two, Int.add_emod, Int.mul_emod, Int.emod_emod]
    <;>
    omega
  exact h2
```

### Explanation

1. **Expand the Expression**:
   - We first expand the given expression to simplify it:
     \[
     a^2 + (a + 2)^2 + (a + 4)^2 + 1 = 3a^2 + 12a + 21
     \]
   - This is done using the `ring` tactic in Lean4.

2. **Modulo 12 Analysis**:
   - Since \(a\) is odd, we consider all possible residues of \(a\) modulo 12, which are \(1, 3, 5, 7, 9,\) and \(11\).
   - For each residue, we compute the expression \(3a^2 + 12a + 21 \mod 12\) and show it is zero.
   - This is done using the `rcases` tactic to handle each case and `simp` to simplify the expressions modulo 12.

3. **Conclusion**:
   - Since the expression is zero modulo 12 for all odd \(a\), it is divisible by 12.

### Normal Language Explanation

1. **Expand the Expression**:
   - Expand \(a^2 + (a + 2)^2 + (a + 4)^2 + 1\) to \(3a^2 + 12a + 21\).

2. **Modulo 12 Analysis**:
   - Since \(a\) is odd, consider all possible residues of \(a\) modulo 12.
   - For each residue, compute \(3a^2 + 12a + 21 \mod 12\) and verify it is zero.

3. **Conclusion**:
   - The expression is divisible by 12 because it evaluates to zero modulo 12 for all odd \(a\).