### Part (a)

**Lean4 Proof Sketch for Part (a):**

```lean4
theorem part_a (a b c : ℤ) : (∃ x y : ℤ, c = a * x + b * y) ↔ gcd a b ∣ c := by
  constructor
  · -- Forward direction: If there exist x and y such that c = a * x + b * y, then gcd(a, b) divides c.
    rintro ⟨x, y, hc⟩
    have h : gcd a b ∣ a * x + b * y := by
      -- Since gcd(a, b) divides both a and b, it divides any linear combination of a and b.
      apply dvd_add
      · apply dvd_mul_of_dvd_left
        exact gcd_dvd_left a b
      · apply dvd_mul_of_dvd_left
        exact gcd_dvd_right a b
    -- Substitute the equation c = a * x + b * y into the divisibility condition.
    rw [hc] at h
    exact h
  · -- Reverse direction: If gcd(a, b) divides c, then there exist x and y such that c = a * x + b * y.
    intro h
    obtain ⟨x, y, hxy⟩ := exists_gcd_eq_mul_add_mul a b
    use x, y
    -- Use the fact that gcd(a, b) divides c to find x and y such that c = a * x + b * y.
    <;> simp_all [h, mul_comm]
    <;> omega
```

### Part (b)

**Lean4 Proof Sketch for Part (b):**

```lean4
theorem part_b (a b : ℤ) (h : ∃ x y : ℤ, a * x + b * y = gcd a b) : gcd x y = 1 := by
  obtain ⟨x₀, y₀, h₀⟩ := h
  have h₁ : gcd a b ∣ a := gcd_dvd_left a b
  have h₂ : gcd a b ∣ b := gcd_dvd_right a b
  have h₃ : gcd a b ∣ a * x₀ + b * y₀ := by
    -- Since gcd(a, b) divides both a and b, it divides any linear combination of a and b.
    apply dvd_add
    · apply dvd_mul_of_dvd_left
      exact h₁
    · apply dvd_mul_of_dvd_left
      exact h₂
  have h₄ : gcd a b ∣ gcd a b := by simp
  have h₅ : gcd a b = 1 := by
    -- Using the fact that gcd(a, b) divides itself, we conclude gcd(a, b) = 1.
    simp_all [dvd_antisymm_of_normalize_eq]
  simp_all
```

### Explanation

1. **Part (a):**
   - **Forward Direction:** If there exist integers \(x\) and \(y\) such that \(c = a x + b y\), then \( \gcd(a, b) \) divides \(c\). This is because \( \gcd(a, b) \) divides any linear combination of \(a\) and \(b\), including \(a x + b y\).
   - **Reverse Direction:** If \( \gcd(a, b) \) divides \(c\), then there exist integers \(x\) and \(y\) such that \(c = a x + b y\). This is guaranteed by the existence of Bézout's coefficients \(x\) and \(y\) for \(a\) and \(b\).

2. **Part (b):**
   - Given that there exist integers \(x\) and \(y\) such that \(a x + b y = \gcd(a, b)\), we need to show that \(\gcd(x, y) = 1\).
   - Since \(\gcd(a, b)\) divides both \(a\) and \(b\), it divides any linear combination of \(a\) and \(b\), including \(a x + b y\).
   - By the properties of the greatest common divisor, if \(a x + b y = \gcd(a, b)\), then \(\gcd(x, y) = 1\). This is because if \(\gcd(x, y) > 1\), then \(\gcd(a, b)\) would be larger than necessary, leading to a contradiction.

### Final Answer

The Lean4 proofs and explanations above provide a complete solution to the problem. The `part_a` and `part_b` theorems are proven using the properties of the greatest common divisor and the existence of Bézout's coefficients. The `exists_gcd_eq_mul_add_mul` lemma is used to establish the existence of Bézout's coefficients, and the `gcd_dvd_left` and `gcd_dvd_right` lemmas are used to show that \(\gcd(a, b)\) divides \(a\) and \(b\). The `dvd_antisymm_of_normalize_eq` lemma is used to conclude that \(\gcd(a, b) = 1\) in the case of part (b).