### Part (a): $8 \mid 5^{2n} + 7$

**Base Case (n = 1):**
- $5^{2 \cdot 1} + 7 = 25 + 7 = 32$
- $32 \div 8 = 4$, so $8 \mid 32$

**Inductive Step:**
Assume $8 \mid 5^{2k} + 7$ for some $k \geq 1$. We need to show $8 \mid 5^{2(k+1)} + 7$.
- $5^{2(k+1)} + 7 = 25 \cdot 5^{2k} + 7 = 25(5^{2k} + 7) - 175 + 7 = 25(5^{2k} + 7) - 168$
- By the inductive hypothesis, $5^{2k} + 7$ is divisible by 8, so $25(5^{2k} + 7)$ is divisible by $25 \cdot 8 = 200$.
- $168 \div 8 = 21$, so $168$ is divisible by 8.
- Thus, $25(5^{2k} + 7) - 168$ is divisible by 8.

### Part (b): $15 \mid 2^{4n} - 1$

**Base Case (n = 1):**
- $2^{4 \cdot 1} - 1 = 16 - 1 = 15$
- $15 \div 15 = 1$, so $15 \mid 15$

**Inductive Step:**
Assume $15 \mid 2^{4k} - 1$ for some $k \geq 1$. We need to show $15 \mid 2^{4(k+1)} - 1$.
- $2^{4(k+1)} - 1 = 16 \cdot 2^{4k} - 1 = 16(2^{4k} - 1) + 15$
- By the inductive hypothesis, $2^{4k} - 1$ is divisible by 15, so $16(2^{4k} - 1)$ is divisible by $16 \cdot 15 = 240$.
- $15$ is divisible by 15, so $16(2^{4k} - 1) + 15$ is divisible by 15.

### Part (c): $5 \mid 3^{3n+1} + 2^{n+1}$

**Base Case (n = 1):**
- $3^{3 \cdot 1 + 1} + 2^{1+1} = 3^4 + 2^2 = 81 + 4 = 85$
- $85 \div 5 = 17$, so $5 \mid 85$

**Inductive Step:**
Assume $5 \mid 3^{3k+1} + 2^{k+1}$ for some $k \geq 1$. We need to show $5 \mid 3^{3(k+1)+1} + 2^{(k+1)+1}$.
- $3^{3(k+1)+1} + 2^{(k+1)+1} = 27 \cdot 3^{3k+1} + 2 \cdot 2^{k+1} = 27(3^{3k+1} + 2^{k+1}) - 27 \cdot 2^{k+1} + 2 \cdot 2^{k+1} = 27(3^{3k+1} + 2^{k+1}) - 51 \cdot 2^{k+1}$
- By the inductive hypothesis, $3^{3k+1} + 2^{k+1}$ is divisible by 5, so $27(3^{3k+1} + 2^{k+1})$ is divisible by $27 \cdot 5 = 135$.
- $51 \cdot 2^{k+1} \equiv 3 \cdot 2^{k+1} \mod 5$ (since $51 \equiv 1 \mod 5$).
- For $k \geq 1$, $2^{k+1} \equiv 2, 4, 3, 1 \mod 5$ cyclically, so $3 \cdot 2^{k+1} \equiv 6, 12, 9, 3 \mod 5 \equiv 1, 2, 4, 3 \mod 5$.
- Thus, $51 \cdot 2^{k+1} \equiv 1, 2, 4, 3 \mod 5$, and $-51 \cdot 2^{k+1} \equiv 4, 3, 1, 2 \mod 5$.
- Adding $27(3^{3k+1} + 2^{k+1}) \equiv 0 \mod 5$ and $-51 \cdot 2^{k+1} \equiv 4, 3, 1, 2 \mod 5$ gives $3^{3(k+1)+1} + 2^{(k+1)+1} \equiv 4, 3, 1, 2 \mod 5$, which is not always 0. This suggests a flaw in the inductive step.

**Revised Approach:**
Instead, directly check the pattern modulo 5:
- For $n=1$: $3^4 + 2^2 = 81 + 4 = 85 \equiv 0 \mod 5$
- For $n=2$: $3^5 + 2^3 = 243 + 8 = 251 \equiv 1 + 3 = 4 \mod 5$ (Wait, this contradicts the earlier result. Let's re-examine.)

**Correct Inductive Step:**
Assume $5 \mid 3^{3k+1} + 2^{k+1}$ for some $k \geq 1$. We need to show $5 \mid 3^{3(k+1)+1} + 2^{(k+1)+1}$.
- $3^{3(k+1)+1} + 2^{(k+1)+1} = 27 \cdot 3^{3k+1} + 2 \cdot 2^{k+1} = 27(3^{3k+1} + 2^{k+1}) - 25 \cdot 2^{k+1} + 2 \cdot 2^{k+1} = 27(3^{3k+1} + 2^{k+1}) - 23 \cdot 2^{k+1}$
- By the inductive hypothesis, $3^{3k+1} + 2^{k+1}$ is divisible by 5, so $27(3^{3k+1} + 2^{k+1})$ is divisible by $27 \cdot 5 = 135$.
- $23 \cdot 2^{k+1} \equiv 3 \cdot 2^{k+1} \mod 5$ (since $23 \equiv 3 \mod 5$).
- For $k \geq 1$, $2^{k+1} \equiv 2, 4, 3, 1 \mod 5$ cyclically, so $3 \cdot 2^{k+1} \equiv 6, 12, 9, 3 \mod 5 \equiv 1, 2, 4, 3 \mod 5$.
- Thus, $23 \cdot 2^{k+1} \equiv 1, 2, 4, 3 \mod 5$, and $-23 \cdot 2^{k+1} \equiv 4, 3, 1, 2 \mod 5$.
- Adding $27(3^{3k+1} + 2^{k+1}) \equiv 0 \mod 5$ and $-23 \cdot 2^{k+1} \equiv 4, 3, 1, 2 \mod 5$ gives $3^{3(k+1)+1} + 2^{(k+1)+1} \equiv 4, 3, 1, 2 \mod 5$, which is not always 0. This suggests the inductive step is flawed.

**Alternative Approach:**
Directly check for $n=1, 2, 3, 4$ and observe a pattern. For $n=1$, $3^4 + 2^2 = 85 \equiv 0 \mod 5$. For $n=2$, $3^5 + 2^3 = 243 + 8 = 251 \equiv 1 + 3 = 4 \mod 5$. For $n=3$, $3^7 + 2^4 = 2187 + 16 = 2203 \equiv 2 +