### Part (a): The sum of the squares of two odd integers cannot be a perfect square.

**Lean4 Proof Sketch:**

```lean4
theorem sum_of_two_odd_squares_not_square (a b : ℤ) (ha : a % 2 = 1) (hb : b % 2 = 1) : ¬∃ (k : ℤ), a^2 + b^2 = k^2 := by
  rintro ⟨k, hk⟩
  have h₁ : a^2 % 4 = 1 := by
    have : a % 4 = 1 ∨ a % 4 = 3 := by omega
    rcases this with (h | h) <;> simp [h, pow_two, Int.mul_emod, Int.add_emod]
  have h₂ : b^2 % 4 = 1 := by
    have : b % 4 = 1 ∨ b % 4 = 3 := by omega
    rcases this with (h | h) <;> simp [h, pow_two, Int.mul_emod, Int.add_emod]
  have h₃ : (a^2 + b^2) % 4 = 2 := by omega
  have h₄ : k^2 % 4 = 0 ∨ k^2 % 4 = 1 := by
    have : k % 4 = 0 ∨ k % 4 = 1 ∨ k % 4 = 2 ∨ k % 4 = 3 := by omega
    rcases this with (h | h | h | h) <;> simp [h, pow_two, Int.mul_emod, Int.add_emod]
  omega
```

**Explanation:**
1. We consider the possible residues of odd integers modulo 4. An odd integer can be written as \(4k + 1\) or \(4k + 3\).
2. Squaring such integers gives:
   - \((4k + 1)^2 = 16k^2 + 8k + 1 \equiv 1 \mod 4\)
   - \((4k + 3)^2 = 16k^2 + 24k + 9 \equiv 1 \mod 4\)
3. Thus, \(a^2 \equiv 1 \mod 4\) and \(b^2 \equiv 1 \mod 4\), so \(a^2 + b^2 \equiv 2 \mod 4\).
4. The possible residues of squares modulo 4 are \(0\) and \(1\). Since \(2\) is not a possible residue, \(a^2 + b^2\) cannot be a perfect square.

### Part (b): The product of four consecutive integers is 1 less than a perfect square.

**Lean4 Proof Sketch:**

```lean4
theorem product_four_consec_int_one_less_square (n : ℤ) : ∃ (k : ℤ), n * (n + 1) * (n + 2) * (n + 3) + 1 = k^2 := by
  use (n^2 + 3*n + 1)
  ring_nf
  <;> omega
```

**Explanation:**
1. We need to show that \(n(n+1)(n+2)(n+3) + 1\) is a perfect square.
2. Let \(k = n^2 + 3n + 1\). We claim that \(k^2 = n(n+1)(n+2)(n+3) + 1\).
3. Expand \(k^2\) and verify that it equals \(n(n+1)(n+2)(n+3) + 1\):
   \[
   k^2 = (n^2 + 3n + 1)^2 = n^4 + 6n^3 + 11n^2 + 6n + 1
   \]
   \[
   n(n+1)(n+2)(n+3) + 1 = n(n^2 + 3n + 2)(n + 3) + 1 = n(n^3 + 3n^2 + 2n + 3n^2 + 9n + 6) + 1 = n^4 + 6n^3 + 11n^2 + 6n + 1
   \]
   Thus, \(k^2 = n(n+1)(n+2)(n+3) + 1\).

### Final Answer

The Lean4 proofs are provided above, and the explanations justify the claims. The first part shows that the sum of the squares of two odd integers cannot be a perfect square, while the second part demonstrates that the product of four consecutive integers is one less than a perfect square.