### Part (a): Proving that if \( d \mid n \), then \( 2^d - 1 \mid 2^n - 1 \)

**Proof:**
1. Assume \( d \mid n \). This means there exists an integer \( k \) such that \( n = d \cdot k \).
2. We can express \( 2^n - 1 \) as:
   \[
   2^n - 1 = 2^{d \cdot k} - 1 = (2^d)^k - 1.
   \]
3. The expression \( (2^d)^k - 1 \) can be factored as:
   \[
   (2^d - 1)(2^{(k-1)d} + 2^{(k-2)d} + \dots + 2^d + 1).
   \]
   This is a geometric series sum, and it is always an integer.
4. Since \( 2^d - 1 \) is a factor of \( (2^d)^k - 1 \), it follows that \( 2^d - 1 \) divides \( 2^n - 1 \).

### Part (b): Verifying that \( 2^{35} - 1 \) is divisible by 31 and 127

**Verification:**
1. **Divisibility by 31:**
   - Compute \( 2^5 \mod 31 \):
     \[
     2^5 = 32 \equiv 1 \mod 31.
     \]
   - Since \( 2^5 \equiv 1 \mod 31 \), we have:
     \[
     2^{35} = (2^5)^7 \equiv 1^7 \equiv 1 \mod 31.
     \]
     Thus, \( 2^{35} - 1 \equiv 0 \mod 31 \), so \( 31 \mid 2^{35} - 1 \).

2. **Divisibility by 127:**
   - Compute \( 2^7 \mod 127 \):
     \[
     2^7 = 128 \equiv 1 \mod 127.
     \]
   - Since \( 2^7 \equiv 1 \mod 127 \), we have:
     \[
     2^{35} = (2^7)^5 \cdot 2^0 \equiv 1^5 \cdot 1 \equiv 1 \mod 127.
     \]
     Thus, \( 2^{35} - 1 \equiv 0 \mod 127 \), so \( 127 \mid 2^{35} - 1 \).

### Lean4 Proof Sketch

```lean4
theorem part_a (d n : ℕ) (h : d ∣ n) : 2^d - 1 ∣ 2^n - 1 := by
  obtain ⟨k, rfl⟩ := h
  use (2^(d * k) - 1) / (2^d - 1)
  <;>
  simp [pow_mul, Nat.mul_sub_left_distrib, Nat.mul_sub_right_distrib, Nat.div_eq_of_eq_mul_left]
  <;>
  ring_nf
  <;>
  norm_num
  <;>
  omega
```

### Lean4 Verification for Part (b)

```lean4
theorem part_b : 31 ∣ 2^35 - 1 ∧ 127 ∣ 2^35 - 1 := by
  apply And.intro
  -- Prove 31 ∣ 2^35 - 1
  {
    apply Nat.dvd_of_mod_eq_zero
    rfl
  }
  -- Prove 127 ∣ 2^35 - 1
  {
    apply Nat.dvd_of_mod_eq_zero
    rfl
  }
```