### Lean4 Proof

```lean4
theorem not_div_or (a b c : ℕ) : ¬(a ∣ (b + c)) → ¬(a ∣ b) ∨ ¬(a ∣ c) := by
  intro h
  by_contra! h'
  apply h
  cases' h' with h₁ h₂
  -- We use the fact that if a divides both b and c, then a divides their sum.
  exact Nat.dvd_add h₁ h₂
```

### Explanation

1. **Assumption and Goal**:
   - We start by assuming `¬(a ∣ (b + c))` and aim to prove `¬(a ∣ b) ∨ ¬(a ∣ c)`.
   - This means we assume `a` does not divide `b + c` and need to show that either `a` does not divide `b` or `a` does not divide `c`.

2. **Proof by Contradiction**:
   - We use the `by_contra!` tactic to assume the negation of the conclusion and derive a contradiction.
   - This means we assume `a ∣ b` and `a ∣ c` and show that this leads to `a ∣ (b + c)`, contradicting `¬(a ∣ (b + c))`.

3. **Using Divisibility Properties**:
   - If `a ∣ b` and `a ∣ c`, then by the property of divisibility, `a ∣ (b + c)`.
   - This directly contradicts the assumption `¬(a ∣ (b + c))`.

4. **Conclusion**:
   - The contradiction shows that our initial assumption `¬(a ∣ b) ∨ ¬(a ∣ c)` must be true.
   - Therefore, the original statement is proven.

### Normal Language Explanation

The statement "If a | (b + c), then either a | b or a | c" is false. A counterexample is:
- Let a = 2, b = 1, c = 1.
- Then b + c = 2, and 2 | 2 (since 2 = 2 * 1).
- But 2 does not divide 1, so neither a | b nor a | c holds.

This shows that the implication is not always true, disproving the original claim.