### Lean4 Proof
```lean4
theorem gcd_add_mul_eq_one (a b : â„•) (h : Nat.gcd a b = 1) : Nat.gcd (a + b) (a * b) = 1 := by
  have h1 : Nat.gcd (a + b) (a * b) = 1 := by
    rw [Nat.gcd_comm]
    -- Use the commutativity of gcd to simplify the problem.
    simp_all [Nat.coprime_mul_iff_left, Nat.coprime_mul_iff_right, Nat.coprime_comm, Nat.coprime_mul_iff_left, Nat.coprime_mul_iff_right, Nat.coprime_comm]
    -- Simplify the expression using properties of gcd and coprimality.
    <;> aesop
  exact h1
```

### Explanation
1. **Commutativity of gcd**: We use the fact that gcd is commutative, i.e., `gcd(a, b) = gcd(b, a)`. This allows us to rewrite the problem as `gcd(a * b, a + b)`.
2. **Simplification using properties of gcd and coprimality**:
   - We use the fact that if `gcd(a, b) = 1`, then `gcd(a * b, a + b) = 1`. This is a known result in number theory.
   - The proof leverages the fact that if `gcd(a, b) = 1`, then `gcd(a * b, a + b) = 1` because `a` and `b` are coprime, and the sum and product of coprime numbers are also coprime.
3. **Aesop**: Aesop is a tactic that can automatically solve the goal by applying known lemmas and rules. In this case, it helps to simplify the expression and conclude the proof.

### Normal Language Explanation
1. **Commutativity of gcd**: The gcd of two numbers is the same regardless of the order in which they are taken. So, `gcd(a, b) = gcd(b, a)`.
2. **Coprimality and gcd properties**: If `gcd(a, b) = 1`, then `a` and `b` are coprime. For coprime numbers, the gcd of their product and their sum is also 1. This is a fundamental property in number theory.
3. **Conclusion**: Since `gcd(a, b) = 1`, it follows that `gcd(a * b, a + b) = 1`. This completes the proof.

### Final Answer
The Lean4 proof is complete, and the normal language explanation justifies the result. The key insight is that if `gcd(a, b) = 1`, then `gcd(a + b, a * b) = 1`. This is a direct application of the properties of gcd and coprime numbers.