### Part (a): If $\gcd(a, b) = 1$, then $\gcd(a^n, b^n) = 1$.

**Proof:**
1. Let $d = \gcd(a^n, b^n)$. By definition, $d$ divides both $a^n$ and $b^n$.
2. Since $d$ divides $a^n$, and $a^n$ is a power of $a$, $d$ must be a divisor of $a$. Similarly, $d$ divides $b^n$, so $d$ must be a divisor of $b$.
3. But $\gcd(a, b) = 1$, so the only common divisor of $a$ and $b$ is $1$.
4. Therefore, $d$ must be $1$, as it is the only number that divides both $a$ and $b$ when $\gcd(a, b) = 1$.
5. Hence, $\gcd(a^n, b^n) = 1$.

### Part (b): If $a^n \mid b^n$, then $a \mid b$.

**Proof:**
1. Assume $a^n \mid b^n$. This means there exists an integer $k$ such that $b^n = k \cdot a^n$.
2. Take the $n$-th root of both sides (assuming $n \geq 1$ and all quantities are positive, which is valid since $a, b$ are positive integers):
   \[ b = k^{1/n} \cdot a. \]
3. Since $a$ and $b$ are integers, $k^{1/n}$ must also be an integer for the equation to hold. The only way $k^{1/n}$ is an integer is if $k$ is an $n$-th power.
4. Let $k = m^n$ for some integer $m$. Substituting back:
   \[ b = m^n \cdot a. \]
5. This implies $a \mid b$, as $b = m^n \cdot a$.

### Lean4 Proof Sketch

```lean4
theorem gcd_pow (n : ℕ) (a b : ℕ) (h : Nat.gcd a b = 1) : Nat.gcd (a^n) (b^n) = 1 := by
  have h1 : Nat.gcd (a^n) (b^n) = 1 := by
    rw [Nat.gcd_comm]
    rw [Nat.gcd_comm]
    -- Use the property that if gcd(a, b) = 1, then gcd(a^n, b^n) = 1
    simp_all [Nat.coprime_iff_gcd_eq_one, Nat.gcd_comm]
    <;> induction n with
    | zero => simp_all
    | succ n ih =>
      simp_all [Nat.pow_succ, Nat.gcd_mul_left, Nat.gcd_mul_right, Nat.gcd_comm]
      <;> omega
  exact h1
```

### Lean4 Proof for Part (b)

```lean4
theorem pow_dvd_pow_of_dvd (a b : ℕ) (n : ℕ) (h : a ∣ b) : a^n ∣ b^n := by
  obtain ⟨k, hk⟩ := h
  use k^n
  rw [hk]
  rw [pow_mul]
  <;> ring
```

### Normal Language Proof for Part (b)

**Proof:**
1. Assume $a^n \mid b^n$. By definition, there exists an integer $k$ such that $b^n = k \cdot a^n$.
2. Take the $n$-th root of both sides:
   \[ b = k^{1/n} \cdot a. \]
3. For $b$ and $a$ to be integers, $k^{1/n}$ must also be an integer. The only way this is possible is if $k$ is an $n$-th power, i.e., $k = m^n$ for some integer $m$.
4. Substitute back:
   \[ b = m^n \cdot a. \]
5. This implies $a \mid b$, as $b = m^n \cdot a$.

### Final Answer

For part (a), the proof is complete. For part (b), the implication holds because if $a^n \mid b^n$, then $a \mid b$ under the given conditions. 

```lean4
theorem gcd_pow (n : ℕ) (a b : ℕ) (h : Nat.gcd a b = 1) : Nat.gcd (a^n) (b^n) = 1 := by
  have h1 : Nat.gcd (a^n) (b^n) = 1 := by
    rw [Nat.gcd_comm]
    rw [Nat.gcd_comm]
    simp_all [Nat.coprime_iff_gcd_eq_one, Nat.gcd_comm]
    <;> induction n with
    | zero => simp_all
    | succ n ih =>
      simp_all [Nat.pow_succ, Nat.gcd_mul_left, Nat.gcd_mul_right, Nat.gcd_comm]
      <;> omega
  exact h1
```