### (a) gcd(a + b, a - b) = 1 or 2

**Lean4 Proof Sketch:**
```lean4
theorem gcd_a_plus_b_a_minus_b (a b : ℕ) (h : Nat.gcd a b = 1) : Nat.gcd (a + b) (a - b) = 1 ∨ Nat.gcd (a + b) (a - b) = 2 := by
  have h₁ : Nat.gcd (a + b) (a - b) ∣ 2 * a := by
    -- Show that gcd(a + b, a - b) divides 2a
    have h₂ : Nat.gcd (a + b) (a - b) ∣ a + b := Nat.gcd_dvd_left (a + b) (a - b)
    have h₃ : Nat.gcd (a + b) (a - b) ∣ a - b := Nat.gcd_dvd_right (a + b) (a - b)
    have h₄ : Nat.gcd (a + b) (a - b) ∣ 2 * a := by
      -- Use the fact that gcd(a + b, a - b) divides both a + b and a - b
      -- to show it divides 2a
      convert dvd_add h₂ h₃ using 1 <;>
        simp [two_mul, add_assoc, add_comm, add_left_comm] <;>
        omega
    exact h₄
  have h₂ : Nat.gcd (a + b) (a - b) ∣ 2 * b := by
    -- Similarly, show that gcd(a + b, a - b) divides 2b
    have h₃ : Nat.gcd (a + b) (a - b) ∣ a + b := Nat.gcd_dvd_left (a + b) (a - b)
    have h₄ : Nat.gcd (a + b) (a - b) ∣ a - b := Nat.gcd_dvd_right (a + b) (a - b)
    have h₅ : Nat.gcd (a + b) (a - b) ∣ 2 * b := by
      -- Use the fact that gcd(a + b, a - b) divides both a + b and a - b
      -- to show it divides 2b
      convert dvd_sub h₃ h₄ using 1 <;>
        simp [two_mul, add_assoc, add_comm, add_left_comm] <;>
        omega
    exact h₅
  have h₃ : Nat.gcd (a + b) (a - b) ∣ Nat.gcd (2 * a) (2 * b) := by
    -- Since gcd(a + b, a - b) divides both 2a and 2b, it divides their gcd
    exact Nat.dvd_gcd h₁ h₂
  have h₄ : Nat.gcd (2 * a) (2 * b) = 2 * Nat.gcd a b := by
    -- The gcd of 2a and 2b is 2 times the gcd of a and b
    rw [Nat.gcd_mul_left]
    <;> simp [h]
  have h₅ : Nat.gcd (a + b) (a - b) ∣ 2 := by
    -- Since gcd(a + b, a - b) divides 2 * gcd(a, b), and gcd(a, b) = 1, it divides 2
    simp_all [h, Nat.dvd_prime Nat.prime_two]
  have h₆ : Nat.gcd (a + b) (a - b) = 1 ∨ Nat.gcd (a + b) (a - b) = 2 := by
    -- The only divisors of 2 are 1 and 2
    have h₇ : Nat.gcd (a + b) (a - b) ≤ 2 := Nat.le_of_dvd (by norm_num) h₅
    interval_cases Nat.gcd (a + b) (a - b) <;> simp_all (config := {decide := true})
  exact h₆
```

**Normal Language Proof:**
1. Let \( d = \gcd(a + b, a - b) \).
2. Since \( d \) divides both \( a + b \) and \( a - b \), it divides their linear combinations.
   - \( d \) divides \( (a + b) + (a - b) = 2a \).
   - \( d \) divides \( (a + b) - (a - b) = 2b \).
3. Thus, \( d \) divides \( \gcd(2a, 2b) = 2 \gcd(a, b) \).
4. Since \( \gcd(a, b) = 1 \), \( d \) divides 2.
5. The possible values for \( d \) are 1 and 2.

### (b) gcd(2a + b, a + 2b) = 1 or 3

**Lean4 Proof Sketch:**
```lean4
theorem gcd_2a_plus_b_a_plus_2b (a b : ℕ) (h : Nat.gcd a b = 1) : Nat.gcd (2 * a + b) (a + 2 * b) = 1 ∨ Nat.gcd (2 * a + b) (a + 2 * b) = 3 := by
  have h₁ : Nat.gcd (2 * a + b) (a + 2 * b) ∣ 3 * a := by
    -- Show that gcd(2a + b, a + 2b) divides 3a
    have h₂ : Nat.gcd (2 * a + b) (a + 2 * b) ∣ 2 * a + b := Nat.gcd_dvd_left (2 * a + b) (a + 2 * b)
    have h₃ : Nat.gcd (2 * a + b) (a + 2 * b) ∣ a + 2 * b := Nat.gcd_dvd_right (2 * a + b) (a + 2 * b)
    have h₄ : Nat.gcd (2 * a + b) (a + 2 * b) ∣ 3 * a := by
      -- Use the fact that gcd(2a + b, a + 2b) divides both 2a + b and a + 2b
      -- to show it divides 3a
      convert dvd_sub h₂ h₃ using 1 <;>
        simp [two_mul, add_assoc, add_comm, add_left_comm] <;>
        omega
    exact h₄
  have h₂ : Nat.gcd (2 * a + b) (a + 2 * b) ∣ 3 * b := by
    -- Similarly, show that gcd(2a + b, a + 2b) divides 3b
    have h₃ : Nat.gcd (2 * a + b) (a + 2 * b) ∣ 2 * a + b := Nat.gcd_dvd_left (2 * a + b) (a + 2 * b)
    have h₄ : Nat.gcd (2 * a + b) (a + 2 * b) ∣ a + 2 * b := Nat.gcd_dvd_right (2 * a + b) (a + 2 * b)
    have h₅ : Nat.gcd (2 * a + b) (a + 2 * b) ∣ 3 * b := by
      -- Use the fact that gcd(2a + b, a + 2b) divides both 2a + b and a + 2b
      -- to show it divides 3b
      convert dvd_sub h₃ h₄ using 1 <;>
        simp [two_mul, add_assoc, add_comm, add_left_comm] <;>
        omega
    exact h₅
  have h₃ : Nat.gcd (2 * a + b) (a + 2 * b) ∣ Nat.gcd (3 * a) (3 * b) := by
    -- Since gcd(2a + b, a + 2b) divides both 3a and 3b, it divides their gcd
    exact Nat.dvd_gcd h₁ h₂
  have h₄ : Nat.gcd (3 * a) (3 * b) = 3 * Nat.gcd a b := by
    -- The gcd of 3a and 3b is 3 times the gcd of a and b
    rw [Nat.gcd_mul_left]
    <;> simp [h]
  have h₅ : Nat.gcd (2 * a + b) (a + 2 * b) ∣ 3 := by
    -- Since gcd(2a