I'll prove each assertion step by step.

### (a) If $a \equiv b \pmod{n}$ and $m \mid n$, then $a \equiv b \pmod{m}$

**Proof:**
1. $a \equiv b \pmod{n}$ means $n \mid (a - b)$, so $a - b = kn$ for some integer $k$
2. $m \mid n$ means $n = lm$ for some integer $l$
3. Substituting: $a - b = k(lm) = (kl)m$
4. Therefore $m \mid (a - b)$, which means $a \equiv b \pmod{m}$

**Lean 4 statement:**
```lean
theorem part_a (a b n m : ℤ) (h1 : a ≡ b [ZMOD n]) (h2 : m ∣ n) : a ≡ b [ZMOD m] := by
  rcases h1 with ⟨k, hk⟩
  rcases h2 with ⟨l, hl⟩
  use k * l
  rw [hl] at hk
  ring_nf at hk ⊢
  exact hk
```

### (b) If $a \equiv b \pmod{n}$ and $c > 0$, then $ca \equiv cb \pmod{cn}$

**Proof:**
1. $a \equiv b \pmod{n}$ means $n \mid (a - b)$, so $a - b = kn$ for some integer $k$
2. Multiply both sides by $c$: $c(a - b) = c(kn)$
3. This gives $ca - cb = k(cn)$
4. Therefore $cn \mid (ca - cb)$, which means $ca \equiv cb \pmod{cn}$

**Lean 4 statement:**
```lean
theorem part_b (a b n : ℤ) (c : ℕ) (h : a ≡ b [ZMOD n]) : (c : ℤ) * a ≡ (c : ℤ) * b [ZMOD (c : ℤ) * n] := by
  rcases h with ⟨k, hk⟩
  use k
  ring_nf
  rw [hk]
  ring
```

### (c) If $a \equiv b \pmod{n}$ and the integers $a, b, n$ are all divisible by $d > 0$, then $a/d \equiv b/d \pmod{n/d}$

**Proof:**
1. $a \equiv b \pmod{n}$ means $n \mid (a - b)$, so $a - b = kn$ for some integer $k$
2. Since $d \mid a$, $d \mid b$, and $d \mid n$, let $a = da'$, $b = db'$, $n = dn'$
3. Substitute: $da' - db' = k(dn')$
4. Divide both sides by $d$: $a' - b' = kn'$
5. Therefore $n' \mid (a' - b')$, which means $a/d \equiv b/d \pmod{n/d}$

**Lean 4 statement:**
```lean
theorem part_c (a b n d : ℤ) (hd : d > 0) (h1 : a ≡ b [ZMOD n]) (h2 : d ∣ a) (h3 : d ∣ b) (h4 : d ∣ n) :
    a/d ≡ b/d [ZMOD n/d] := by
  rcases h1 with ⟨k, hk⟩
  rcases h2 with ⟨a', ha⟩
  rcases h3 with ⟨b', hb⟩
  rcases h4 with ⟨n', hn⟩
  use k
  rw [ha, hb, hn] at hk ⊢
  field_simp [ne_of_gt hd]
  ring_nf at hk ⊢
  exact hk
```

**Normal language output:**

All three assertions have been proven:

(a) If two numbers are congruent modulo n, and m divides n, then they are also congruent modulo m. This follows because the difference between the numbers is divisible by n, and since m divides n, m must also divide their difference.

(b) If two numbers are congruent modulo n, then multiplying both by a positive constant c gives numbers that are congruent modulo cn. This works because multiplying the congruence relationship by c scales both the numbers and the modulus appropriately.

(c) If two numbers are congruent modulo n, and all three values (a, b, and n) are divisible by d, then dividing all three by d preserves the congruence relationship with the scaled modulus n/d. This allows us to simplify congruence relationships when common factors are present.