### Step-by-Step Proof Sketch

We aim to prove by induction on \( n \) that if \( a \) is an odd integer, then for any \( n \geq 1 \),
\[
a^{2^n} \equiv 1 \pmod{2^{n+2}}.
\]

#### Base Case (\( n = 1 \)):
We need to show:
\[
a^2 \equiv 1 \pmod{2^3 = 8}.
\]
Since \( a \) is odd, write \( a = 2k + 1 \). Then:
\[
a^2 = (2k + 1)^2 = 4k(k + 1) + 1.
\]
Note that \( k(k + 1) \) is even, so \( 4k(k + 1) \) is divisible by 8. Hence:
\[
a^2 \equiv 1 \pmod{8}.
\]

#### Inductive Step:
Assume the statement holds for some \( n \geq 1 \), i.e.,
\[
a^{2^n} = 1 + 2^{n+2} \cdot m \quad \text{for some integer } m.
\]
We want to prove it for \( n + 1 \), i.e.,
\[
a^{2^{n+1}} \equiv 1 \pmod{2^{n+3}}.
\]
Note:
\[
a^{2^{n+1}} = (a^{2^n})^2 = (1 + 2^{n+2} m)^2 = 1 + 2^{n+3} m + 2^{2n+4} m^2.
\]
Since \( n \geq 1 \), \( 2n + 4 \geq n + 3 \), so \( 2^{2n+4} m^2 \) is divisible by \( 2^{n+3} \). Thus:
\[
a^{2^{n+1}} \equiv 1 + 2^{n+3} m \pmod{2^{n+3}} \equiv 1 \pmod{2^{n+3}}.
\]

#### Conclusion:
By induction, the statement holds for all \( n \geq 1 \).

---

### Lean 4 Statement and Proof

```lean
import Mathlib.Tactic

theorem odd_power_congruence (a : ℤ) (ha : Odd a) : ∀ n : ℕ, n ≥ 1 → a^(2^n) ≡ 1 [ZMOD 2^(n + 2)] := by
  intro n hn
  induction' n with k IH
  · exfalso; linarith [hn]  -- n=0 but n≥1, contradiction
  · have h : a^(2^(k + 1)) = (a^(2^k))^2 := by
      rw [pow_succ', pow_two]
    rw [h]
    have IHk : a^(2^k) ≡ 1 [ZMOD 2^(k + 2)] := IH (by omega)
    rcases IHk with ⟨t, ht⟩
    have : a^(2^k) = 1 + 2^(k + 2) * t := by linarith
    rw [this]
    ring_nf
    show (1 + 2^(k + 2) * t)^2 ≡ 1 [ZMOD 2^(k + 3)]
    rw [show (2 : ℤ)^(k + 3) = 2^(k + 2) * 2 by ring]
    refine Int.emod_eq_zero_of_dvd ⟨t + 2^(k + 1) * t^2, ?_⟩
    ring
```

### Explanation in Normal Language

We prove by induction that for any odd integer \( a \) and integer \( n \geq 1 \), \( a^{2^n} \equiv 1 \pmod{2^{n+2}} \).

- **Base Case (\( n = 1 \))**: Since \( a \) is odd, \( a^2 \equiv 1 \pmod{8} \).
- **Inductive Step**: Assume \( a^{2^k} \equiv 1 \pmod{2^{k+2}} \). Then \( a^{2^{k+1}} = (a^{2^k})^2 \equiv 1^2 = 1 \pmod{2^{k+3}} \).

The Lean code formalizes this induction, using properties of modular arithmetic and powers of 2. The key step is expanding \( (1 + 2^{k+2} \cdot t)^2 \) and showing all extra terms are divisible by \( 2^{k+3} \).

Thus, the result holds for all \( n \geq 1 \).