Let's analyze the given congruence:

For \( n \geq 1 \), show that
\[
(-13)^{n+1} \equiv (-13)^n + (-13)^{n-1} \pmod{181}.
\]

We can rewrite the congruence as:
\[
(-13)^{n+1} - (-13)^n - (-13)^{n-1} \equiv 0 \pmod{181}.
\]

Factor out \( (-13)^{n-1} \):
\[
(-13)^{n-1} \left[ (-13)^2 - (-13) - 1 \right] \equiv 0 \pmod{181}.
\]

So, it suffices to show that:
\[
(-13)^2 - (-13) - 1 \equiv 0 \pmod{181}.
\]

Compute \( (-13)^2 = 169 \), \( -(-13) = 13 \), and subtract 1:
\[
169 + 13 - 1 = 181.
\]

Thus,
\[
(-13)^2 - (-13) - 1 = 181 \equiv 0 \pmod{181}.
\]

Therefore, for any \( n \geq 1 \),
\[
(-13)^{n-1} \cdot 0 \equiv 0 \pmod{181},
\]
which confirms the original congruence.

**Conclusion:**
For all integers \( n \geq 1 \),
\[
(-13)^{n+1} \equiv (-13)^n + (-13)^{n-1} \pmod{181}.
\]

This holds because the expression \( (-13)^2 - (-13) - 1 \) is exactly 181, which is divisible by 181.