### Proofs Using Congruence Theory

We will prove each divisibility statement using congruence modulo the given divisor.

---

#### (a) Prove \( 7 \mid 5^{2n} + 3 \cdot 2^{5n-2} \) for \( n \geq 1 \)

We work modulo 7.

Note:
- \( 5 \equiv 5 \pmod{7} \), so \( 5^{2n} \equiv (5^2)^n \equiv 25^n \equiv 4^n \pmod{7} \) (since \( 25 \equiv 4 \)).
- \( 2 \equiv 2 \pmod{7} \), so \( 2^{5n-2} = 2^{5n} \cdot 2^{-2} \). We compute \( 2^{5n} \) and the multiplicative inverse of \( 2^2 = 4 \) modulo 7.

First, \( 2^3 = 8 \equiv 1 \pmod{7} \), so the order divides 3.
Thus, \( 2^{5n} = (2^3)^{(5n/3)} \) but we compute directly:
\( 2^{5n} = (2^5)^n = 32^n \equiv 4^n \pmod{7} \) (since \( 32 \equiv 4 \)).

Then \( 2^{5n-2} = 2^{5n} \cdot 2^{-2} \equiv 4^n \cdot (4)^{-1} \pmod{7} \), since \( 2^2 = 4 \).
The inverse of 4 mod 7 is 2 (since \( 4 \cdot 2 = 8 \equiv 1 \)), so:
\( 2^{5n-2} \equiv 4^n \cdot 2 \pmod{7} \).

Therefore:
\( 3 \cdot 2^{5n-2} \equiv 3 \cdot 2 \cdot 4^n = 6 \cdot 4^n \pmod{7} \).

Now the entire expression:
\( 5^{2n} + 3 \cdot 2^{5n-2} \equiv 4^n + 6 \cdot 4^n = 7 \cdot 4^n \equiv 0 \pmod{7} \).

Hence, \( 7 \mid 5^{2n} + 3 \cdot 2^{5n-2} \).

---

#### (b) Prove \( 13 \mid 3^{n+2} + 4^{2n+1} \) for \( n \geq 1 \)

Work modulo 13.

Note:
- \( 3^{n+2} = 9 \cdot 3^n \).
- \( 4^{2n+1} = 4 \cdot (4^2)^n = 4 \cdot 16^n \).

Now \( 16 \equiv 3 \pmod{13} \), so \( 16^n \equiv 3^n \).
Thus:
\( 4^{2n+1} \equiv 4 \cdot 3^n \pmod{13} \).

Also, \( 3^{n+2} \equiv 9 \cdot 3^n \pmod{13} \).

Therefore:
\( 3^{n+2} + 4^{2n+1} \equiv 9 \cdot 3^n + 4 \cdot 3^n = 13 \cdot 3^n \equiv 0 \pmod{13} \).

Hence, \( 13 \mid 3^{n+2} + 4^{2n+1} \).

---

#### (c) Prove \( 27 \mid 2^{5n+1} + 5^{n+2} \) for \( n \geq 1 \)

Work modulo 27.

We need to show \( 2^{5n+1} + 5^{n+2} \equiv 0 \pmod{27} \).

Note:
- \( 2^{5n+1} = 2 \cdot (2^5)^n = 2 \cdot 32^n \).
- \( 5^{n+2} = 25 \cdot 5^n \).

Now \( 32 \equiv 5 \pmod{27} \) (since \( 32 - 27 = 5 \)), so \( 32^n \equiv 5^n \).
Thus:
\( 2^{5n+1} \equiv 2 \cdot 5^n \pmod{27} \).

Therefore:
\( 2^{5n+1} + 5^{n+2} \equiv 2 \cdot 5^n + 25 \cdot 5^n = 27 \cdot 5^n \equiv 0 \pmod{27} \).

Hence, \( 27 \mid 2^{5n+1} + 5^{n+2} \).

---

#### (d) Prove \( 43 \mid 6^{n+2} + 7^{2n+1} \) for \( n \geq 1 \)

Work modulo 43.

Note:
- \( 6^{n+2} = 36 \cdot 6^n \).
- \( 7^{2n+1} = 7 \cdot (7^2)^n = 7 \cdot 49^n \).

Now \( 49 \equiv 6 \pmod{43} \) (since \( 49 - 43 = 6 \)), so \( 49^n \equiv 6^n \).
Thus:
\( 7^{2n+1} \equiv 7 \cdot 6^n \pmod{43} \).

Therefore:
\( 6^{n+2} + 7^{2n+1} \equiv 36 \cdot 6^n + 7 \cdot 6^n = 43 \cdot 6^n \equiv 0 \pmod{43} \).

Hence, \( 43 \mid 6^{n+2} + 7^{2n+1} \).

---

### Summary

All divisibility statements are proven by showing that the expressions are congruent to 0 modulo the given divisor, using properties of exponents and congruences.

---

### Lean 4 Statements

To verify these in Lean 4, we can state the theorems as follows:

```lean
import Mathlib.Tactic

-- (a) 7 divides 5^(2n) + 3 * 2^(5n-2)
theorem part_a (n : ℕ) (hn : n ≥ 1) : 7 ∣ 5^(2*n) + 3 * 2^(5*n - 2) := by
  -- Proof using congruence modulo 7

-- (b) 13 divides 3^(n+2) + 4^(2n+1)
theorem part_b (n : ℕ) (hn : n ≥ 1) : 13 ∣ 3^(n+2) + 4^(2*n+1) := by
  -- Proof using congruence modulo 13

-- (c) 27 divides 2^(5n+1) + 5^(n+2)
theorem part_c (n : ℕ) (hn : n ≥ 1) : 27 ∣ 2^(5*n+1) + 5^(n+2) := by
  -- Proof using congruence modulo 27

-- (d) 43 divides 6^(n+2) + 7^(2n+1)
theorem part_d (n : ℕ) (hn : n ≥ 1) : 43 ∣ 6^(n+2) + 7^(2*n+1) := by
  -- Proof using congruence modulo 43
```

The proofs in Lean would involve calculating the congruences as above, using `Nat.modEq` or similar tactics. The detailed Lean proofs are omitted here but can be constructed based on the algebraic steps provided.

---

These proofs demonstrate the power of congruence theory in establishing divisibility properties efficiently.