Let's analyze the given conditions and the statement to prove.

**Given:**
1. \( a \equiv b \pmod{n_1} \)  ⇒ \( n_1 \mid (a - b) \)
2. \( a \equiv c \pmod{n_2} \)  ⇒ \( n_2 \mid (a - c) \)

We are to prove: \( b \equiv c \pmod{n} \), where \( n = \gcd(n_1, n_2) \).

**Interpretation:**
We want to show that \( n \mid (b - c) \).

**Approach:**
From the congruences:
- \( a - b = k_1 n_1 \) for some integer \( k_1 \)
- \( a - c = k_2 n_2 \) for some integer \( k_2 \)

Subtract the second from the first:
\( (a - b) - (a - c) = k_1 n_1 - k_2 n_2 \)
⇒ \( -b + c = k_1 n_1 - k_2 n_2 \)
⇒ \( c - b = k_1 n_1 - k_2 n_2 \)

So, \( b - c = k_2 n_2 - k_1 n_1 \).

Now, let \( n = \gcd(n_1, n_2) \). Then \( n \mid n_1 \) and \( n \mid n_2 \), so \( n \mid (k_2 n_2 - k_1 n_1) \).
Therefore, \( n \mid (b - c) \), which means \( b \equiv c \pmod{n} \).

**Conclusion:**
The statement is true: under the given conditions, \( b \equiv c \pmod{\gcd(n_1, n_2)} \).

---

**Lean Statement:**
We'll state this in Lean. Note that Lean uses `\d` for divisibility and `%` for modulus, but we can use the congruence relation `≡` modulo `n`.

We assume `n1`, `n2`, `a`, `b`, `c` are integers, and define `n = gcd n1 n2`.
Then we have hypotheses `h1 : a ≡ b [MOD n1]` and `h2 : a ≡ c [MOD n2]`, and we want to prove `b ≡ c [MOD n]`.

In Lean, we can write:

```lean
import tactic
import data.int.gcd

lemma cong_mod_gcd (n1 n2 a b c : ℤ) (h1 : a ≡ b [ZMOD n1]) (h2 : a ≡ c [ZMOD n2]) :
  b ≡ c [ZMOD (int.gcd n1 n2)] :=
begin
  set n := int.gcd n1 n2 with hn_def,
  have hn : (n : ℤ) ∣ n1 ∧ (n : ℤ) ∣ n2,
  { exact ⟨int.gcd_dvd_left n1 n2, int.gcd_dvd_right n1 n2⟩ },
  rcases hn with ⟨d1, d2⟩,
  have h3 : n1 ∣ a - b := int.mod_eq_zero_of_dvd.mp h1,
  have h4 : n2 ∣ a - c := int.mod_eq_zero_of_dvd.mp h2,
  have h5 : n ∣ (a - b) := d1.trans h3,
  have h6 : n ∣ (a - c) := d2.trans h4,
  have h7 : n ∣ (b - c),
  { have : n ∣ ((a - c) - (a - b)) := int.dvd_sub h6 h5,
    simp only [sub_sub_sub_cancel_left] at this,
    exact this },
  exact int.mod_eq_zero_of_dvd.mpr h7,
end
```

**Explanation of Lean proof:**
1. We define `n` as the gcd of `n1` and `n2`.
2. We note that `n` divides both `n1` and `n2`.
3. From `h1` and `h2`, we get that `n1 ∣ (a - b)` and `n2 ∣ (a - c)`.
4. Since `n ∣ n1` and `n1 ∣ (a - b)`, we have `n ∣ (a - b)`.
5. Similarly, `n ∣ (a - c)`.
6. Then `n` divides the difference: `(a - c) - (a - b) = b - c`.
7. Therefore, `n ∣ (b - c)`, which means `b ≡ c [MOD n]`.

---

**Output in normal language:**
Given that \( a \equiv b \pmod{n_1} \) and \( a \equiv c \pmod{n_2} \), we have shown that \( b \equiv c \pmod{n} \), where \( n = \gcd(n_1, n_2) \). This is because the greatest common divisor \( n \) divides both \( n_1 \) and \( n_2 \), and hence from the congruences it follows that \( n \) divides \( b - c \). Therefore, the statement holds true.