### Step 1: Understand the Given Conditions

We are given:
1. \( ab \equiv cd \pmod{n} \)
2. \( b \equiv d \pmod{n} \)
3. \( \gcd(b, n) = 1 \)

We want to prove:
\( a \equiv c \pmod{n} \)

---

### Step 2: Rewrite the Congruences

From \( b \equiv d \pmod{n} \), we can write:
\[ d = b + kn \quad \text{for some integer } k \]

From \( ab \equiv cd \pmod{n} \), we have:
\[ ab - cd = mn \quad \text{for some integer } m \]

---

### Step 3: Substitute \(d\) into the Equation

Substitute \(d = b + kn\) into \(ab - cd\):
\[
ab - c(b + kn) = mn
\]
\[
ab - cb - ckn = mn
\]
\[
(a - c)b - ckn = mn
\]
\[
(a - c)b = mn + ckn = n(m + ck)
\]

So,
\[
(a - c)b \equiv 0 \pmod{n}
\]

---

### Step 4: Use the Coprimality Condition

We have \( (a - c)b \equiv 0 \pmod{n} \), meaning \(n\) divides \((a - c)b\).

Since \( \gcd(b, n) = 1 \), \(n\) must divide \(a - c\). Therefore:
\[
a - c \equiv 0 \pmod{n} \quad \Rightarrow \quad a \equiv c \pmod{n}
\]

---

### ✅ Final Proof

Given:
- \( ab \equiv cd \pmod{n} \)
- \( b \equiv d \pmod{n} \)
- \( \gcd(b, n) = 1 \)

From \( b \equiv d \pmod{n} \), we have \( d = b + kn \) for some integer \(k\).  
Substitute into \( ab \equiv cd \pmod{n} \):
\[
ab \equiv c(b + kn) \pmod{n}
\]
\[
ab \equiv cb + ckn \pmod{n}
\]
\[
ab - cb \equiv ckn \pmod{n}
\]
\[
(a - c)b \equiv 0 \pmod{n}
\]

Since \( \gcd(b, n) = 1 \), \(n\) divides \(a - c\), so:
\[
a \equiv c \pmod{n}
\]

---

### Lean 4 Statement & Proof

```lean
theorem congruence_proof (a b c d n : ℤ) (h1 : a * b ≡ c * d [ZMOD n]) (h2 : b ≡ d [ZMOD n]) (h3 : Nat.Coprime (Int.natAbs b) (Int.natAbs n)) :
    a ≡ c [ZMOD n] := by
  have h4 : (a - c) * b ≡ 0 [ZMOD n] := by
    calc
      (a - c) * b = a * b - c * b : by ring
      _ ≡ c * d - c * b [ZMOD n] : by rw [h1]
      _ = c * (d - b) : by ring
      _ ≡ c * 0 [ZMOD n] : by rw [show d - b ≡ 0 [ZMOD n] from ?_]
      _ = 0 : by ring

  have h5 : Nat.Coprime (Int.natAbs b) (Int.natAbs n) := h3
  -- Now use that if (a - c)*b ≡ 0 mod n and gcd(b, n)=1, then a ≡ c mod n
  -- This follows from Euclid's lemma: if n divides (a-c)*b and gcd(n,b)=1, then n divides (a-c)
  exact ...  -- Details depend on available lemmas in your context
```

**Note:** The exact Lean proof might require additional steps to handle the coprimality condition and the deduction that \(n \mid (a - c)\). You may need to use existing lemmas about coprime integers and divisibility.

---

### Output in Normal Language

**Proof:**  
Since \(b \equiv d \pmod{n}\), we can write \(d = b + kn\) for some integer \(k\). Substituting into \(ab \equiv cd \pmod{n}\) gives:
\[
ab \equiv c(b + kn) = cb + ckn \pmod{n}
\]
Subtracting \(cb\) from both sides:
\[
ab - cb \equiv ckn \pmod{n}
\]
\[
(a - c)b \equiv 0 \pmod{n}
\]
This means \(n\) divides \((a - c)b\). Since \(\gcd(b, n) = 1\), it follows that \(n\) divides \(a - c\). Therefore:
\[
a \equiv c \pmod{n}
\]

This completes the proof.