Let's construct a counterexample to show that \(a^k \equiv b^k \pmod{n}\) and \(k \equiv j \pmod{n}\) do not necessarily imply \(a^j \equiv b^j \pmod{n}\).

Choose:
- \(n = 4\)
- \(a = 2\), \(b = 4\)
- \(k = 2\), \(j = 6\)

First, check \(a^k \equiv b^k \pmod{n}\):
\(a^k = 2^2 = 4\)
\(b^k = 4^2 = 16\)
\(4 \equiv 16 \pmod{4}\) because both are divisible by 4 (remainder 0). So, \(2^2 \equiv 4^2 \pmod{4}\).

Next, check \(k \equiv j \pmod{n}\):
\(k = 2\), \(j = 6\)
\(2 \equiv 6 \pmod{4}\) because both leave remainder 2 when divided by 4.

Now, check \(a^j \equiv b^j \pmod{n}\):
\(a^j = 2^6 = 64\)
\(b^j = 4^6 = 4096\)
\(64 \equiv 0 \pmod{4}\) (since 64 is divisible by 4)
\(4096 \equiv 0 \pmod{4}\) (since 4096 is divisible by 4)
So actually \(64 \equiv 4096 \pmod{4}\). This doesn't work as a counterexample because both are 0 mod 4.

Let me try another set:

Choose:
- \(n = 4\)
- \(a = 2\), \(b = 2\) (but then it would be trivial, so need different)
Wait, need \(a \not\equiv b \pmod{n}\) for non-trivial.

Actually, we need \(a^j \not\equiv b^j \pmod{n}\).

Try:
- \(n = 8\)
- \(a = 2\), \(b = 4\)
- \(k = 2\), \(j = 10\)

First, \(a^k = 2^2 = 4\), \(b^k = 4^2 = 16\)
\(4 \equiv 16 \pmod{8}\)? \(4 \mod 8 = 4\), \(16 \mod 8 = 0\), so \(4 \not\equiv 0 \pmod{8}\). Not good.

Try:
- \(n = 3\)
- \(a = 2\), \(b = 4\)
- \(k = 2\), \(j = 5\)

\(a^k = 4\), \(b^k = 16\), \(4 \equiv 16 \pmod{3}\)? \(4 \mod 3 = 1\), \(16 \mod 3 = 1\), so yes.
\(k=2\), \(j=5\), \(2 \equiv 5 \pmod{3}\)? both remainder 2.
Now \(a^j = 2^5 = 32\), \(32 \mod 3 = 2\)
\(b^j = 4^5 = 1024\), \(1024 \mod 3\): \(1024 \div 3 = 341*3=1023\), remainder 1.
So \(32 \equiv 2 \pmod{3}\), \(1024 \equiv 1 \pmod{3}\), so \(2 \not\equiv 1 \pmod{3}\).

Perfect! So with \(n=3\), \(a=2\), \(b=4\), \(k=2\), \(j=5\):
- \(2^2 = 4 \equiv 1 \pmod{3}\), \(4^2 = 16 \equiv 1 \pmod{3}\), so \(a^k \equiv b^k \pmod{n}\).
- \(k=2\), \(j=5\), and \(2 \equiv 5 \pmod{3}\) (both remainder 2).
- But \(2^5 = 32 \equiv 2 \pmod{3}\), \(4^5 = 1024 \equiv 1 \pmod{3}\), so \(2 \not\equiv 1 \pmod{3}\), hence \(a^j \not\equiv b^j \pmod{n}\).

Therefore, this is a counterexample.

**Lean Statement:**
```lean
example : ¬ (∀ (a b : ℤ) (n k j : ℕ), a^k ≡ b^k [ZMOD n] → k ≡ j [MOD n] → a^j ≡ b^j [ZMOD n]) := by
  refine by
    intro h
    have := h 2 4 3 2 5
    have h1 : (2 : ℤ)^2 ≡ (4 : ℤ)^2 [ZMOD (3 : ℤ)]
    · norm_num [Int.modEq_iff_dvd]
      decide
    have h2 : (2 : ℕ) ≡ 5 [MOD (3 : ℕ)]
    · decide
    have h3 := this h1 h2
    norm_num [Int.modEq_iff_dvd] at h3
    -- This will show a contradiction since 2^5 = 32 ≡ 2 mod 3, 4^5=1024 ≡ 1 mod 3, and 2 ≢ 1 mod 3.
    -- Alternatively, compute:
    have : ¬ (32 : ℤ) ≡ (1024 : ℤ) [ZMOD (3 : ℤ)]
    · norm_num [Int.modEq_iff_dvd]
      decide
    exact this h3
```

**Output in Normal Language:**
We have shown that with \(a = 2\), \(b = 4\), \(n = 3\), \(k = 2\), and \(j = 5\):
- \(2^2 = 4 \equiv 1 \pmod{3}\) and \(4^2 = 16 \equiv 1 \pmod{3}\), so \(a^k \equiv b^k \pmod{n}\).
- \(k = 2\) and \(j = 5\) are both congruent to 2 modulo 3 (since \(2 \mod 3 = 2\) and \(5 \mod 3 = 2\)), so \(k \equiv j \pmod{n}\).
- However, \(2^5 = 32 \equiv 2 \pmod{3}\) and \(4^5 = 1024 \equiv 1 \pmod{3}\), and \(2 \not\equiv 1 \pmod{3}\). Therefore, \(a^j \not\equiv b^j \pmod{n}\).

This provides a specific counterexample where the implication fails.