### ‚úÖ Part (a): Divisibility by 7, 11, and 13

We aim to prove that 7, 11, and 13 all divide \( N \) if and only if they divide the integer
\[
M = (100a_2 + 10a_1 + a_0) - (100a_5 + 10a_4 + a_3) + (100a_8 + 10a_7 + a_6) - \ldots
\]

#### üîç Step 1: Key Observation
Note that \( 7 \times 11 \times 13 = 1001 \). This number plays a crucial role.

#### ‚úçÔ∏è Step 2: Express \( N \) Modulo 1001
We can write:
\[
N = a_m10^m + \ldots + a_2 10^2 + a_1 10 + a_0.
\]
Group the digits into blocks of three (from right to left), and express \( N \) modulo 1001.

Since \( 10^3 \equiv -1 \pmod{1001} \), we have:
\[
10^{3k} \equiv (-1)^k \pmod{1001}.
\]
Therefore,
\[
N \equiv \sum_{k=0}^{\lfloor m/3 \rfloor} (100a_{3k+2} + 10a_{3k+1} + a_{3k}) \cdot (-1)^k \pmod{1001}.
\]
This is exactly \( M \), i.e.,
\[
N \equiv M \pmod{1001}.
\]

#### ‚úÖ Step 3: Conclusion
Since \( 1001 = 7 \times 11 \times 13 \), we have:
\[
N \equiv M \pmod{7}, \quad N \equiv M \pmod{11}, \quad N \equiv M \pmod{13}.
\]
Thus, \( 7, 11, 13 \) all divide \( N \) if and only if they all divide \( M \).

---

### ‚úÖ Part (b): Divisibility by 6

We aim to prove that 6 divides \( N \) if and only if 6 divides
\[
M = a_0 + 4a_1 + 4a_2 + \ldots + 4a_m.
\]

#### üîç Step 1: Divisibility by 2 and 3
Since \( 6 = 2 \times 3 \), we must check divisibility by both 2 and 3.

#### ‚úçÔ∏è Step 2: Check Divisibility by 2
A number is divisible by 2 if its last digit \( a_0 \) is even. Note that \( M \equiv a_0 \pmod{2} \), because all other terms are multiples of 4 (even). So:
\[
N \text{ divisible by } 2 \iff a_0 \text{ even} \iff M \equiv 0 \pmod{2}.
\]

#### ‚úçÔ∏è Step 3: Check Divisibility by 3
We know \( N \equiv \sum_{k=0}^m a_k \pmod{3} \). Now compute \( M \mod 3 \):
\[
M = a_0 + 4a_1 + 4a_2 + \ldots + 4a_m.
\]
Since \( 4 \equiv 1 \pmod{3} \), we have:
\[
M \equiv a_0 + a_1 + a_2 + \ldots + a_m \pmod{3}.
\]
Therefore,
\[
N \equiv 0 \pmod{3} \iff \sum a_k \equiv 0 \pmod{3} \iff M \equiv 0 \pmod{3}.
\]

#### ‚úÖ Step 4: Combine Both Conditions
\( N \) is divisible by 6 if and only if it is divisible by both 2 and 3. From above:
- \( N \equiv 0 \pmod{2} \iff M \equiv 0 \pmod{2} \)
- \( N \equiv 0 \pmod{3} \iff M \equiv 0 \pmod{3} \)

Hence, \( N \equiv 0 \pmod{6} \iff M \equiv 0 \pmod{6} \).

---

### ‚úÖ Final Proofs Complete

Both statements (a) and (b) are now proven. The results are confirmed.