Let's analyze the pattern:

We have:
- 1 · 9 + 2 = 11
- 12 · 9 + 3 = 111
- 123 · 9 + 4 = 1111
- ...
- 123456789 · 9 + 10 = 1111111111

Notice that the left multiplicand is a number consisting of consecutive digits starting from 1 (1, 12, 123, ..., 123456789). The multiplier is always 9. The number added increases from 2 to 10. The result is a number consisting of all 1's, with the number of digits equal to (the number of digits in the multiplicand + 1).

Let n be the number of digits in the multiplicand (which is the number we are forming with consecutive digits). Then the multiplicand is:
   M = 1, 12, 123, ..., 123...n
We are adding (n+1) and multiplying by 9.

Claim: M * 9 + (n+1) = 111...1 (with n+1 ones).

Why does this hold?

Observe that:
   M = (10^(n-1) * 1 + 10^(n-2) * 2 + ... + 10^0 * n

But there is a known identity:
   123...n = (10^n - 1) / 9 - (n*(10^n - 1)) / (9*10^n) ? Actually, there is a simpler way.

Alternatively, note that:
   111...1 (with k ones) = (10^k - 1)/9.

So the right-hand side is R = (10^(n+1) - 1)/9.

Now, we want to show that:
   M * 9 + (n+1) = (10^(n+1) - 1)/9.

Multiply both sides by 9:
   9M * 9 + 9*(n+1) = 10^(n+1) - 1   [Wait, no: actually we have M*9 + (n+1) = R, so multiply by 9: 9M + 9(n+1) = 10^(n+1)-1? But that is not correct because R*9 = 10^(n+1)-1.

Actually, from the equation:
   M * 9 + (n+1) = (10^(n+1)-1)/9
Multiply both sides by 9:
   81 M + 9(n+1) = 10^(n+1)-1   [This seems messy]

Better: Let's express M in terms of repunits.

Actually, there is a direct formula for M:
   M = (10^(n+1) - 9n - 10) / 81   ? Not sure.

Another approach: Consider the number 123...n as part of a sequence.

Notice that:
   123...n * 9 = 111...1 - (n+1)   [from the given]

But we can prove by induction.

Base: n=1: 1*9 + 2 = 11, which is correct.

Assume for n=k: 123...k * 9 + (k+1) = 111...1 (k+1 ones).

For n=k+1: The multiplicand is 123...k(k+1) = 123...k * 10 + (k+1)

Then:
   [123...k * 10 + (k+1)] * 9 + (k+2) = 10*(123...k * 9) + 9(k+1) + (k+2)
   = 10*(111...1 (k+1 ones) - (k+1)) + 9(k+1) + (k+2)   [by induction hypothesis]
   = 10*( (10^(k+1)-1)/9 ) - 10(k+1) + 9(k+1) + (k+2)
   = (10^(k+2) - 10)/9 - (k+1) + (k+2)
   = (10^(k+2)-10)/9 + 1
   = (10^(k+2)-10 + 9)/9 = (10^(k+2)-1)/9
   which is exactly the number with (k+2) ones.

So by induction, the pattern holds for all n.

Therefore, the curious calculations hold due to this inductive property, where each step builds upon the previous one by appending the next digit and adjusting the added number accordingly.

In normal language:
The pattern works because when you take a number formed by consecutive digits (like 123...n), multiply it by 9, and then add (n+1), the result is a number consisting of (n+1) ones. This is due to the algebraic structure of these numbers and the properties of base-10 repunits (numbers like 11, 111, etc.). Each step can be derived from the previous one by scaling and adjusting, which ensures the pattern continues consistently.

Lean statement (to confirm the general result):
We can state the theorem in Lean as:

```lean
theorem curious_calc (n : ℕ) (h : n ≥ 1) : 
  (of_nat (consecutive_digits n)) * 9 + (n+1) = (10^(n+1) - 1)/9 := ...
```

But since defining `consecutive_digits n` (which forms the number 123...n) requires some work, we might instead prove by induction as above.

However, for the purpose of this explanation, we have shown why it holds.
```

The calculations hold due to a mathematical induction where for a number `M` formed by concatenating the first `n` digits (1 through n), the operation `M * 9 + (n+1)` always yields a number consisting of `n+1` ones. This is because the structure of `M` and the properties of base-10 numbers ensure that the result simplifies to `(10^(n+1) - 1)/9`, which is the repunit with `n+1` digits. Each line in the pattern corresponds to increasing `n` by 1, and the induction step shows that if it holds for `n`, it also holds for `n+1`. The base case (n=1) is true, so by induction, all are true.