Let \( t_n = \frac{n(n+1)}{2} \) be the \(n\)th triangular number. We are asked: for which values of \(n\) does \(t_n\) divide \(S_n = t_1^2 + t_2^2 + \ldots + t_n^2\)?

First, we compute \(S_n\). Note:
\[
t_k^2 = \left( \frac{k(k+1)}{2} \right)^2 = \frac{k^2 (k+1)^2}{4}.
\]
So,
\[
S_n = \sum_{k=1}^n t_k^2 = \frac{1}{4} \sum_{k=1}^n k^2 (k+1)^2.
\]
Now, \(k^2(k+1)^2 = [k(k+1)]^2\). Alternatively, we can expand:
\[
k^2(k+1)^2 = k^2(k^2 + 2k + 1) = k^4 + 2k^3 + k^2.
\]
Thus,
\[
\sum_{k=1}^n k^2(k+1)^2 = \sum_{k=1}^n (k^4 + 2k^3 + k^2) = \sum_{k=1}^n k^4 + 2\sum_{k=1}^n k^3 + \sum_{k=1}^n k^2.
\]
Using known formulas:
\[
\sum_{k=1}^n k^2 = \frac{n(n+1)(2n+1)}{6},
\]
\[
\sum_{k=1}^n k^3 = \left( \frac{n(n+1)}{2} \right)^2 = \frac{n^2(n+1)^2}{4},
\]
\[
\sum_{k=1}^n k^4 = \frac{n(n+1)(2n+1)(3n^2+3n-1)}{30}.
\]
So,
\[
\sum_{k=1}^n k^2(k+1)^2 = \frac{n(n+1)(2n+1)(3n^2+3n-1)}{30} + 2 \cdot \frac{n^2(n+1)^2}{4} + \frac{n(n+1)(2n+1)}{6}.
\]
Simplify:
\[
= \frac{n(n+1)(2n+1)(3n^2+3n-1)}{30} + \frac{n^2(n+1)^2}{2} + \frac{n(n+1)(2n+1)}{6}.
\]
Get common denominator 30:
\[
= \frac{n(n+1)(2n+1)(3n^2+3n-1)}{30} + \frac{15n^2(n+1)^2}{30} + \frac{5n(n+1)(2n+1)}{30}.
\]
So,
\[
\sum_{k=1}^n k^2(k+1)^2 = \frac{n(n+1)}{30} \left[ (2n+1)(3n^2+3n-1) + 15n(n+1) + 5(2n+1) \right].
\]
Now expand inside:
First, \((2n+1)(3n^2+3n-1) = 6n^3 + 6n^2 -2n + 3n^2 + 3n -1 = 6n^3 + 9n^2 + n -1\).
Next, \(15n(n+1) = 15n^2 + 15n\).
Next, \(5(2n+1) = 10n + 5\).
So sum:
\[
6n^3 + 9n^2 + n -1 + 15n^2 + 15n + 10n + 5 = 6n^3 + (9+15)n^2 + (1+15+10)n + (-1+5) = 6n^3 + 24n^2 + 26n + 4.
\]
Thus,
\[
\sum_{k=1}^n k^2(k+1)^2 = \frac{n(n+1)(6n^3 + 24n^2 + 26n + 4)}{30} = \frac{n(n+1) \cdot 2(3n^3 + 12n^2 + 13n + 2)}{30} = \frac{n(n+1)(3n^3 + 12n^2 + 13n + 2)}{15}.
\]
Therefore,
\[
S_n = \frac{1}{4} \cdot \frac{n(n+1)(3n^3 + 12n^2 + 13n + 2)}{15} = \frac{n(n+1)(3n^3 + 12n^2 + 13n + 2)}{60}.
\]
Now, \(t_n = \frac{n(n+1)}{2}\). So we want:
\[
t_n \mid S_n \iff \frac{n(n+1)}{2} \mid \frac{n(n+1)(3n^3 + 12n^2 + 13n + 2)}{60}.
\]
Cancel \(n(n+1)\) (assuming \(n \geq 1\), so \(n(n+1) \neq 0\)):
\[
\iff \frac{1}{2} \mid \frac{3n^3 + 12n^2 + 13n + 2}{60}.
\]
This is equivalent to:
\[
\frac{3n^3 + 12n^2 + 13n + 2}{60} \cdot 2 = \frac{3n^3 + 12n^2 + 13n + 2}{30} \text{ is an integer}.
\]
So we need \(30 \mid (3n^3 + 12n^2 + 13n + 2)\).

Thus, we need to find \(n\) such that:
\[
3n^3 + 12n^2 + 13n + 2 \equiv 0 \pmod{30}.
\]
Since \(30 = 2 \cdot 3 \cdot 5\), we check modulo 2, 3, and 5.

First, modulo 2:
\(3n^3 + 12n^2 + 13n + 2 \equiv n^3 + 0 + n + 0 = n^3 + n \pmod{2}\).
But \(n^3 + n = n(n^2+1)\). For any integer \(n\), \(n\) and \(n^2+1\) have opposite parity: if \(n\) is even, \(n^2+1\) is odd; if \(n\) is odd, \(n^2+1\) is even. So product is always even. So always divisible by 2.

Modulo 3:
\(3n^3 + 12n^2 + 13n + 2 \equiv 0 + 0 + 1n + 2 = n + 2 \pmod{3}\).
So we need \(n + 2 \equiv 0 \pmod{3} \implies n \equiv 1 \pmod{3}\).

Modulo 5:
\(3n^3 + 12n^2 + 13n + 2 \equiv 3n^3 + 2n^2 + 3n + 2 \pmod{5}\) (since \(12 \equiv 2\), \(13 \equiv 3\)).
We need this to be 0 mod 5. Check \(n \mod 5\):

- \(n=0: 0 + 0 + 0 + 2 = 2\)
- \(n=1: 3 + 2 + 3 + 2 = 10 \equiv 0\)
- \(n=2: 3*8=24≡4, +2*4=8≡3, +3*2=6≡1, +2= => 4+3+1+2=10≡0\)
- \(n=3: 3*27=81≡1, +2*9=18≡3, +3*3=9≡4, +2= =>1+3+4+2=10≡0\)
- \(n=4: 3*64=192≡2, +2*16=32≡2, +3*4=12≡2, +2= =>2+2+2+2=8≡3\)

So only \(n \equiv 1,2,3 \pmod{5}\) work (i.e., not 0 or 4).

So conditions:
1. \(n \equiv 1 \pmod{3}\)
2. \(n \not\equiv 0,4 \pmod{5}\) (i.e., \(n \equiv 1,2,3 \pmod{5}\))

Now combine modulo 15 (since lcm(3,5)=15). List \(n \mod 15\) that satisfy both:

\(n \equiv 1 \pmod{3}\): possible: 1,4,7,10,13 mod15.
But also \(n \not\equiv 0,4 \pmod{5}\): so from above, exclude 4 (since 4 mod5) and also 0 mod5 (i.e., 0,5,10,15) but we are mod15 so 0,5,10.

So from {1,4,7,10,13}:
- 1: ok (1 mod5)
- 4: not (4 mod5)
- 7: 7 mod5=2, ok
- 10: not (0 mod5)
- 13: 13 mod5=3, ok

So \(n \equiv 1,7,13 \pmod{15}\).

Therefore, \(t_n\) divides \(S_n\) if and only if \(n \equiv 1,7,13 \pmod{15}\).

We can verify with small values:
- n=1: t1=1, S1=1, divides.
- n=2: t2=3, S2=1+9=10, not divisible.
- n=3: t3=6, S3=1+9+36=46, not.
- n=4: t4=10, S4=1+9+36+100=146, not.
- n=5: t5=15, S5=1+9+36+100+225=371, not.
- n=6: t6=21, S6=1+9+36+100+225+441=812, not.
- n=7: t7=28, S7=1+9+36+100+225+441+784=1596, 1596/28=57, integer.
So pattern holds.

Thus, the values are \(n = 15k + 1, 15k + 7, 15k + 13\) for \(k \geq 0\).

In Lean, we can state:
```lean
theorem triangular_div_sum_squares (n : ℕ) :
  (nat.triangular n) ∣ (∑ k in finset.range n, (nat.triangular (k+1))^2) ↔
  n % 15 = 1 ∨ n % 15 = 7 ∨ n % 15 = 13 :=
```
But note: our \(n\) in the sum is from 1 to n, so in Lean we might adjust indexing.

Actually, careful: our \(t_n\) is triangular number for \(n\), and sum is \(t_1^2 + ... + t_n^2\). So if we define `triangular n = n*(n+1)/2` (for n≥1), then the statement is for natural numbers n≥1.

But in Lean, `nat.triangular n` is defined as `n*(n+1)/2`, and it's for `n : ℕ`, so `triangular 0 = 0`, `triangular 1=1`, etc. So we want n≥1.

We can write:
```lean
import data.nat.choose
open nat

theorem triangular_div_sum_squares (n : ℕ) (h : n ≥ 1) :
  (triangular n) ∣ (∑ k in finset.range n, (triangular (k+1))^2) ↔
  n % 15 = 1 ∨ n % 15 = 7 ∨ n % 15 = 13 :=
```
But we need to prove this. The proof would involve the algebra above and the modular conditions.

However, since the user asked to "confirm result", we have derived the condition.

**Final answer:**
\( t_n \) divides \( t_1^2 + t_2^2 + \cdots + t_n^2 \) if and only if \( n \equiv 1, 7, \) or \( 13 \pmod{15} \). That is, \( n = 15k + 1 \), \( n = 15k + 7 \), or \( n = 15k + 13 \) for some integer \( k \geq 0 \).

In Lean, the statement is:
```lean
theorem triangular_div_sum_squares (n : ℕ) (h : n ≥ 1) :
  (nat.triangular n) ∣ (∑ k in finset.range n, (nat.triangular (k+1))^2) ↔
  n % 15 = 1 ∨ n % 15 = 7 ∨ n % 15 = 13 :=
```
(Note: This Lean code is a statement; the proof would be non-trivial to code but follows the algebraic derivation.)