Let's solve the linear congruence \( 3x - 7y \equiv 11 \pmod{13} \).

First, simplify the coefficients modulo 13:
- \( 3 \equiv 3 \pmod{13} \)
- \( -7 \equiv 6 \pmod{13} \) (since \(-7 + 13 = 6\))
- \( 11 \equiv 11 \pmod{13} \)

So the congruence becomes:
\[ 3x + 6y \equiv 11 \pmod{13} \]

We can simplify further by dividing the entire congruence by the greatest common divisor (gcd) of the coefficients and the modulus. The coefficients are 3 and 6, and the modulus is 13. The gcd of (3,6,13) is 1, so we cannot simplify the modulus. However, we can simplify by dividing by common factors if possible. Notice that all coefficients and the constant are divisible by? Actually, 3, 6, and 11: gcd(3,6,11)=1, so no common factor to divide.

Alternatively, we can solve for one variable in terms of the other. Let's solve for \(x\):

\[ 3x \equiv 11 - 6y \pmod{13} \]

Multiply both sides by the modular inverse of 3 modulo 13. The inverse of 3 mod 13 is a number \(a\) such that \(3a \equiv 1 \pmod{13}\). Since \(3 \times 9 = 27 \equiv 1 \pmod{13}\) (because \(27 - 2\times13 = 27-26=1\)), so the inverse is 9.

Thus:
\[ x \equiv 9(11 - 6y) \pmod{13} \]
Compute \(9 \times 11 = 99 \equiv 99 - 7\times13 = 99 - 91 = 8 \pmod{13}\)
And \(9 \times 6y = 54y \equiv 54y - 4\times13y = 54y - 52y = 2y \pmod{13}\) (since \(54 \mod 13 = 2\))

So:
\[ x \equiv 8 - 2y \pmod{13} \]

Therefore, the general solution is:
\[ x \equiv 8 - 2y \pmod{13} \]
where \(y\) can be any integer modulo 13. That is, for each \(y \in \{0,1,2,...,12\}\), we get a corresponding \(x\).

We can also express the solution in terms of a parameter. Let \(y = t\), where \(t \in \mathbb{Z}/13\mathbb{Z}\), then:
\[ x = 8 - 2t \pmod{13} \]

So all solutions are given by:
\[ (x, y) = (8 - 2t, t) \quad \text{for } t = 0,1,2,...,12 \]

To list all solutions explicitly:
For \(t = 0\): \(x = 8\), \(y=0\)
\(t=1\): \(x=8-2=6\), \(y=1\)
\(t=2\): \(x=8-4=4\), \(y=2\)
\(t=3\): \(x=8-6=2\), \(y=3\)
\(t=4\): \(x=8-8=0\), \(y=4\)
\(t=5\): \(x=8-10=-2 \equiv 11 \pmod{13}\), \(y=5\)
\(t=6\): \(x=8-12=-4 \equiv 9 \pmod{13}\), \(y=6\)
\(t=7\): \(x=8-14=-6 \equiv 7 \pmod{13}\), \(y=7\)
\(t=8\): \(x=8-16=-8 \equiv 5 \pmod{13}\), \(y=8\)
\(t=9\): \(x=8-18=-10 \equiv 3 \pmod{13}\), \(y=9\)
\(t=10\): \(x=8-20=-12 \equiv 1 \pmod{13}\), \(y=10\)
\(t=11\): \(x=8-22=-14 \equiv -1 \equiv 12 \pmod{13}\), \(y=11\)
\(t=12\): \(x=8-24=-16 \equiv -3 \equiv 10 \pmod{13}\), \(y=12\)

So the 13 solutions are:
\[
\begin{aligned}
& (8,0), (6,1), (4,2), (2,3), (0,4), (11,5), (9,6), (7,7), (5,8), (3,9), (1,10), (12,11), (10,12)
\end{aligned}
\]

We can also write the general solution as:
\[
x \equiv 8 - 2k \pmod{13}, \quad y \equiv k \pmod{13} \quad \text{for } k \in \mathbb{Z}/13\mathbb{Z}
\]

Thus, the complete set of solutions is all pairs \((x,y)\) of the form \((8-2t, t)\) for \(t=0,1,...,12\).

**Final Answer:**
The solutions to the congruence \(3x - 7y \equiv 11 \pmod{13}\) are given by:
\[
x \equiv 8 - 2t \pmod{13}, \quad y \equiv t \pmod{13}
\]
where \(t\) is any integer modulo 13. There are 13 distinct solutions, one for each \(t \in \{0,1,2,\dots,12\}\).

Explicitly, the solutions are:
\[
(8,0), (6,1), (4,2), (2,3), (0,4), (11,5), (9,6), (7,7), (5,8), (3,9), (1,10), (12,11), (10,12)
\]

Each pair \((x,y)\) satisfies the congruence modulo 13.