I'll solve each system of congruences step by step.

### (a) System:
5x + 3y ≡ 1 (mod 7)
3x + 2y ≡ 4 (mod 7)

**Step 1:** Multiply first equation by 2: 10x + 6y ≡ 2 (mod 7) → 3x + 6y ≡ 2 (mod 7)
**Step 2:** Multiply second equation by 3: 9x + 6y ≡ 12 (mod 7) → 2x + 6y ≡ 5 (mod 7)
**Step 3:** Subtract: (3x + 6y) - (2x + 6y) ≡ 2 - 5 (mod 7) → x ≡ -3 ≡ 4 (mod 7)
**Step 4:** Substitute x ≡ 4 into second equation: 3(4) + 2y ≡ 4 → 12 + 2y ≡ 4 → 2y ≡ -8 ≡ -1 ≡ 6 (mod 7)
**Step 5:** Multiply by inverse of 2 mod 7 (which is 4): y ≡ 6×4 ≡ 24 ≡ 3 (mod 7)

**Solution:** x ≡ 4 (mod 7), y ≡ 3 (mod 7)

### (b) System:
7x + 3y ≡ 6 (mod 11)
4x + 2y ≡ 9 (mod 11)

**Step 1:** Multiply first equation by 2: 14x + 6y ≡ 12 (mod 11) → 3x + 6y ≡ 1 (mod 11)
**Step 2:** Multiply second equation by 3: 12x + 6y ≡ 27 (mod 11) → x + 6y ≡ 5 (mod 11)
**Step 3:** Subtract: (3x + 6y) - (x + 6y) ≡ 1 - 5 → 2x ≡ -4 ≡ 7 (mod 11)
**Step 4:** Multiply by inverse of 2 mod 11 (which is 6): x ≡ 7×6 ≡ 42 ≡ 9 (mod 11)
**Step 5:** Substitute x ≡ 9 into second equation: 4(9) + 2y ≡ 9 → 36 + 2y ≡ 9 → 2y ≡ -27 ≡ -5 ≡ 6 (mod 11)
**Step 6:** Multiply by inverse of 2 mod 11: y ≡ 6×6 ≡ 36 ≡ 3 (mod 11)

**Solution:** x ≡ 9 (mod 11), y ≡ 3 (mod 11)

### (c) System:
11x + 5y ≡ 7 (mod 20)
6x + 3y ≡ 8 (mod 20)

**Step 1:** Multiply first equation by 3: 33x + 15y ≡ 21 (mod 20) → 13x + 15y ≡ 1 (mod 20)
**Step 2:** Multiply second equation by 5: 30x + 15y ≡ 40 (mod 20) → 10x + 15y ≡ 0 (mod 20)
**Step 3:** Subtract: (13x + 15y) - (10x + 15y) ≡ 1 - 0 → 3x ≡ 1 (mod 20)
**Step 4:** Find inverse of 3 mod 20: 3×7 = 21 ≡ 1, so x ≡ 1×7 ≡ 7 (mod 20)
**Step 5:** Substitute x ≡ 7 into second equation: 6(7) + 3y ≡ 8 → 42 + 3y ≡ 8 → 3y ≡ -34 ≡ -34+40 ≡ 6 (mod 20)
**Step 6:** Multiply by inverse of 3 mod 20: y ≡ 6×7 ≡ 42 ≡ 2 (mod 20)

**Solution:** x ≡ 7 (mod 20), y ≡ 2 (mod 20)

### Final Answers:
(a) x ≡ 4 (mod 7), y ≡ 3 (mod 7)
(b) x ≡ 9 (mod 11), y ≡ 3 (mod 11)
(c) x ≡ 7 (mod 20), y ≡ 2 (mod 20)

Each system has a unique solution modulo the respective modulus.