I'll solve each set of simultaneous congruences step by step.

### (a) x ≡ 1 (mod 3), x ≡ 2 (mod 5), x ≡ 3 (mod 7)

Using the Chinese Remainder Theorem:
- M = 3×5×7 = 105
- M₁ = 35, M₂ = 21, M₃ = 15
- Solve: 35y₁ ≡ 1 (mod 3) → 2y₁ ≡ 1 (mod 3) → y₁ = 2
- Solve: 21y₂ ≡ 1 (mod 5) → y₂ ≡ 1 (mod 5) → y₂ = 1
- Solve: 15y₃ ≡ 1 (mod 7) → y₃ ≡ 1 (mod 7) → y₃ = 1
- x ≡ 1×35×2 + 2×21×1 + 3×15×1 = 70 + 42 + 45 = 157 ≡ 52 (mod 105)

**Result:** x ≡ 52 (mod 105)

### (b) x ≡ 5 (mod 11), x ≡ 14 (mod 29), x ≡ 15 (mod 31)

Using CRT:
- M = 11×29×31 = 9889
- M₁ = 29×31 = 899, M₂ = 11×31 = 341, M₃ = 11×29 = 319
- Solve: 899y₁ ≡ 1 (mod 11) → 8y₁ ≡ 1 (mod 11) → y₁ = 7
- Solve: 341y₂ ≡ 1 (mod 29) → 22y₂ ≡ 1 (mod 29) → y₂ = 4
- Solve: 319y₃ ≡ 1 (mod 31) → 9y₃ ≡ 1 (mod 31) → y₃ = 7
- x ≡ 5×899×7 + 14×341×4 + 15×319×7 = 31465 + 19096 + 33495 = 84056 ≡ 4941 (mod 9889)

**Result:** x ≡ 4941 (mod 9889)

### (c) x ≡ 5 (mod 6), x ≡ 4 (mod 11), x ≡ 3 (mod 17)

Using CRT:
- M = 6×11×17 = 1122
- M₁ = 11×17 = 187, M₂ = 6×17 = 102, M₃ = 6×11 = 66
- Solve: 187y₁ ≡ 1 (mod 6) → y₁ ≡ 1 (mod 6) → y₁ = 1
- Solve: 102y₂ ≡ 1 (mod 11) → 3y₂ ≡ 1 (mod 11) → y₂ = 4
- Solve: 66y₃ ≡ 1 (mod 17) → 15y₃ ≡ 1 (mod 17) → y₃ = 8
- x ≡ 5×187×1 + 4×102×4 + 3×66×8 = 935 + 1632 + 1584 = 4151 ≡ 785 (mod 1122)

**Result:** x ≡ 785 (mod 1122)

### (d) 2x ≡ 1 (mod 5), 3x ≡ 9 (mod 6), 4x ≡ 1 (mod 7), 5x ≡ 9 (mod 11)

First simplify each congruence:
1. 2x ≡ 1 (mod 5) → Multiply by inverse of 2 mod 5 (which is 3): x ≡ 3 (mod 5)
2. 3x ≡ 9 (mod 6) → Divide by gcd(3,6,9)=3: x ≡ 3 (mod 2) → x ≡ 1 (mod 2)
3. 4x ≡ 1 (mod 7) → Multiply by inverse of 4 mod 7 (which is 2): x ≡ 2 (mod 7)
4. 5x ≡ 9 (mod 11) → Multiply by inverse of 5 mod 11 (which is 9): x ≡ 81 ≡ 4 (mod 11)

Now solve: x ≡ 3 (mod 5), x ≡ 1 (mod 2), x ≡ 2 (mod 7), x ≡ 4 (mod 11)

Note that x ≡ 1 (mod 2) and x ≡ 3 (mod 5) gives x ≡ 3 (mod 10) (since numbers ≡ 3 mod 5 that are odd)

Now solve: x ≡ 3 (mod 10), x ≡ 2 (mod 7), x ≡ 4 (mod 11)
- M = 10×7×11 = 770
- M₁ = 77, M₂ = 110, M₃ = 70
- Solve: 77y₁ ≡ 1 (mod 10) → 7y₁ ≡ 1 (mod 10) → y₁ = 3
- Solve: 110y₂ ≡ 1 (mod 7) → 5y₂ ≡ 1 (mod 7) → y₂ = 3
- Solve: 70y₃ ≡ 1 (mod 11) → 4y₃ ≡ 1 (mod 11) → y₃ = 3
- x ≡ 3×77×3 + 2×110×3 + 4×70×3 = 693 + 660 + 840 = 2193 ≡ 653 (mod 770)

**Result:** x ≡ 653 (mod 770)

### Lean Statements:
```lean
-- (a)
example : ∃ x : ℤ, x ≡ 1 [ZMOD 3] ∧ x ≡ 2 [ZMOD 5] ∧ x ≡ 3 [ZMOD 7] := ⟨52, by norm_num, by norm_num, by norm_num⟩

-- (b)
example : ∃ x : ℤ, x ≡ 5 [ZMOD 11] ∧ x ≡ 14 [ZMOD 29] ∧ x ≡ 15 [ZMOD 31] := ⟨4941, by norm_num, by norm_num, by norm_num⟩

-- (c)
example : ∃ x : ℤ, x ≡ 5 [ZMOD 6] ∧ x ≡ 4 [ZMOD 11] ∧ x ≡ 3 [ZMOD 17] := ⟨785, by norm_num, by norm_num, by norm_num⟩

-- (d)
example : ∃ x : ℤ, 2*x ≡ 1 [ZMOD 5] ∧ 3*x ≡ 9 [ZMOD 6] ∧ 4*x ≡ 1 [ZMOD 7] ∧ 5*x ≡ 9 [ZMOD 11] := ⟨653, by norm_num, by norm_num, by norm_num, by norm_num⟩
```

### Final Answers:
(a) x ≡ 52 (mod 105)  
(b) x ≡ 4941 (mod 9889)  
(c) x ≡ 785 (mod 1122)  
(d) x ≡ 653 (mod 770)