### Step-by-Step Proof

#### Part (a): Verify that for all \( n \geq 1 \),
\[
2 \cdot 6 \cdot 10 \cdot 14 \cdots (4n - 2) = \frac{(2n)!}{n!}
\]

**Proof by induction:**

**Base case (\(n = 1\)):**
Left side: \(4 \cdot 1 - 2 = 2\).
Right side: \(\frac{(2 \cdot 1)!}{1!} = \frac{2!}{1!} = \frac{2}{1} = 2\).
So, the identity holds for \(n = 1\).

**Inductive step:**
Assume the identity holds for \(n = k\), i.e.,
\[
2 \cdot 6 \cdot 10 \cdots (4k - 2) = \frac{(2k)!}{k!}.
\]
We need to show it holds for \(n = k+1\), i.e.,
\[
2 \cdot 6 \cdot 10 \cdots (4k - 2) \cdot (4(k+1) - 2) = \frac{(2(k+1))!}{(k+1)!}.
\]
Note that \(4(k+1) - 2 = 4k + 2\).

Using the inductive hypothesis:
\[
\text{LHS} = \left( \frac{(2k)!}{k!} \right) \cdot (4k + 2).
\]
Now simplify:
\[
(4k + 2) = 2(2k + 1).
\]
So,
\[
\text{LHS} = \frac{(2k)!}{k!} \cdot 2(2k + 1) = \frac{2(2k + 1)(2k)!}{k!}.
\]
Now, the right side for \(n = k+1\) is:
\[
\frac{(2k + 2)!}{(k+1)!} = \frac{(2k+2)(2k+1)(2k)!}{(k+1)k!} = \frac{2(k+1)(2k+1)(2k)!}{(k+1)k!} = \frac{2(2k+1)(2k)!}{k!}.
\]
Thus, both sides are equal. Hence, by induction, the identity holds for all \(n \geq 1\).

---

#### Part (b): Use part (a) to obtain the inequality \(2^n (n!)^2 \leq (2n)!\) for all \(n \geq 1\).

From part (a), we have:
\[
2 \cdot 6 \cdot 10 \cdots (4n - 2) = \frac{(2n)!}{n!}.
\]
Notice that each term in the product on the left is at least 2. In fact, the smallest term is 2 (when \(n=1\)), and as \(n\) increases, the terms increase. Therefore, we have:
\[
2^n \leq 2 \cdot 6 \cdot 10 \cdots (4n - 2).
\]
Why? Because there are \(n\) terms in the product, and each term is \(\geq 2\), so the product is at least \(2^n\).

Thus,
\[
2^n \leq \frac{(2n)!}{n!}.
\]
Multiply both sides by \(n!\):
\[
2^n \cdot n! \leq (2n)!.
\]
But we need \(2^n (n!)^2 \leq (2n)!\). So we need to strengthen this.

Actually, observe that:
\[
2 \cdot 6 \cdot 10 \cdots (4n - 2) = \prod_{i=1}^n (4i - 2) = 2^n \prod_{i=1}^n (2i - 1).
\]
So,
\[
2^n \prod_{i=1}^n (2i - 1) = \frac{(2n)!}{n!}.
\]
Therefore,
\[
\prod_{i=1}^n (2i - 1) = \frac{(2n)!}{2^n n!}.
\]
Now, note that \(n! = 1 \cdot 2 \cdot 3 \cdots n\), and each term \(2i - 1 \geq i\) for \(i \geq 1\) (since \(2i - 1 \geq i\) for \(i \geq 1\)). So,
\[
\prod_{i=1}^n (2i - 1) \geq \prod_{i=1}^n i = n!.
\]
Hence,
\[
\frac{(2n)!}{2^n n!} \geq n!.
\]
Multiplying both sides by \(2^n n!\):
\[
(2n)! \geq 2^n (n!)^2.
\]
This is the desired inequality.

**Therefore, for all \(n \geq 1\),**
\[
2^n (n!)^2 \leq (2n)!.
\]

---

### Lean 4 Statement

```lean
import Mathlib.Data.Real.Basic
import Mathlib.Analysis.SpecialFunctions.Factorial

theorem part_a (n : ℕ) (hn : n ≥ 1) :
    (∏ i in Finset.range n, (4 * (i + 1) - 2)) = Nat.factorial (2 * n) / Nat.factorial n := by
  -- Proof by induction, base case n=1, inductive step using the identity

theorem part_b (n : ℕ) (hn : n ≥ 1) : 2^n * (Nat.factorial n)^2 ≤ Nat.factorial (2 * n) := by
  have h := part_a n hn
  -- Use the product representation and the fact that each term ≥ 2, and compare with n!
```

### Output in Normal Language

We have verified that for all integers \(n \geq 1\), the product \(2 \cdot 6 \cdot 10 \cdots (4n - 2)\) equals \(\frac{(2n)!}{n!}\). Using this identity, we derived the inequality \(2^n (n!)^2 \leq (2n)!\), which holds for all \(n \geq 1\). The key step was observing that each term in the product is at least as large as the corresponding term in \(n!\), leading to the inequality.