### Step 1: Base Cases

We verify the inequality \(a_n < 2^n\) for \(n = 1, 2, 3\):

- \(a_1 = 1 < 2^1 = 2\)
- \(a_2 = 2 < 2^2 = 4\)
- \(a_3 = 3 < 2^3 = 8\)

✅ All base cases hold.

---

### Step 2: Inductive Hypothesis

Assume that for all \(k\) such that \(1 \leq k \leq m\) (with \(m \geq 3\)), we have:
\[
a_k < 2^k
\]

---

### Step 3: Inductive Step

We want to prove that:
\[
a_{m+1} < 2^{m+1}
\]

By the recurrence:
\[
a_{m+1} = a_m + a_{m-1} + a_{m-2}
\]

Using the inductive hypothesis:
\[
a_m < 2^m, \quad a_{m-1} < 2^{m-1}, \quad a_{m-2} < 2^{m-2}
\]

So:
\[
a_{m+1} < 2^m + 2^{m-1} + 2^{m-2}
\]

Factor out \(2^{m-2}\):
\[
a_{m+1} < 2^{m-2}(2^2 + 2^1 + 1) = 2^{m-2}(4 + 2 + 1) = 2^{m-2} \cdot 7
\]

Now, compare to \(2^{m+1}\):
\[
2^{m+1} = 2^{m-2} \cdot 2^3 = 2^{m-2} \cdot 8
\]

Since \(7 < 8\), we have:
\[
2^{m-2} \cdot 7 < 2^{m-2} \cdot 8 \quad \Rightarrow \quad a_{m+1} < 2^{m+1}
\]

✅ The inductive step holds.

---

### Step 4: Conclusion

By the **Second Principle of Finite Induction** (strong induction), we conclude:
\[
a_n < 2^n \quad \text{for every positive integer } n.
\]

---

### ✅ Lean 4 Statement & Proof

```lean
theorem a_lt_2_pow (n : ℕ) (h : n ≥ 1) : a n < 2 ^ n := by
  induction' n using Nat.strong_induction_on with k IH
  rcases k with (rfl|rfl|rfl|k)
  · exact show a 1 < 2 ^ 1 by decide  -- a₁ = 1 < 2
  · exact show a 2 < 2 ^ 2 by decide  -- a₂ = 2 < 4
  · exact show a 3 < 2 ^ 3 by decide  -- a₃ = 3 < 8
  · have hk : k + 1 ≥ 4 := by omega
    have : a (k + 1) = a k + a (k - 1) + a (k - 2) := by
      rw [a_recurrence (by omega)]
    rw [this]
    have h1 : a k < 2 ^ k := IH k (by omega)
    have h2 : a (k - 1) < 2 ^ (k - 1) := IH (k - 1) (by omega)
    have h3 : a (k - 2) < 2 ^ (k - 2) := IH (k - 2) (by omega)
    have : 2 ^ k + 2 ^ (k - 1) + 2 ^ (k - 2) = 2^(k - 2) * 7 := by
      ring_nf
    rw [this]
    have : 2^(k + 1) = 2^(k - 2) * 8 := by ring
    rw [this]
    nlinarith [pow_pos (by norm_num) (k - 2)]
```

**Note:** The actual Lean proof requires defining the sequence `a` and its recurrence relation. The above sketch assumes those are already defined. The key steps are:

1. Base cases for \(n = 1, 2, 3\).
2. Inductive step using the recurrence and the strong induction hypothesis.
3. Algebraic manipulation to show \(2^{k-2} \cdot 7 < 2^{k-2} \cdot 8\).

---

### 📝 Output in Normal Language

We have shown by strong induction that for all positive integers \(n\), the sequence \(a_n\) (defined by \(a_1 = 1\), \(a_2 = 2\), \(a_3 = 3\), and \(a_n = a_{n-1} + a_{n-2} + a_{n-3}\) for \(n \geq 4\)) satisfies \(a_n < 2^n\). The base cases \(n = 1, 2, 3\) are verified directly, and the inductive step uses the recurrence and the fact that \(7 \cdot 2^{n-2} < 8 \cdot 2^{n-2} = 2^{n+1}\). Therefore, the inequality holds for all \(n \geq 1\).