I need to prove two separate inequalities:

1. \( n! > n^2 \) for every integer \( n \geq 4 \)
2. \( n! > n^3 \) for every integer \( n \geq 6 \)

Let me prove these by mathematical induction.

**First inequality: \( n! > n^2 \) for \( n \geq 4 \)**

Base case (n=4):
\( 4! = 24 \), \( 4^2 = 16 \), and \( 24 > 16 \) ✓

Inductive step:
Assume \( k! > k^2 \) for some \( k \geq 4 \).
We need to show \( (k+1)! > (k+1)^2 \).

Left side: \( (k+1)! = (k+1) \cdot k! \)
Right side: \( (k+1)^2 = k^2 + 2k + 1 \)

Using the inductive hypothesis \( k! > k^2 \), we have:
\( (k+1)! = (k+1) \cdot k! > (k+1) \cdot k^2 \)

Now we need to show \( (k+1) \cdot k^2 > (k+1)^2 \), which simplifies to:
\( k^2 > k+1 \) (since \( k+1 > 0 \))

For \( k \geq 4 \), \( k^2 \geq 16 \) and \( k+1 \leq 5 \), so \( k^2 > k+1 \) holds.
Thus \( (k+1)! > (k+1)^2 \).

**Second inequality: \( n! > n^3 \) for \( n \geq 6 \)**

Base case (n=6):
\( 6! = 720 \), \( 6^3 = 216 \), and \( 720 > 216 \) ✓

Inductive step:
Assume \( k! > k^3 \) for some \( k \geq 6 \).
We need to show \( (k+1)! > (k+1)^3 \).

Left side: \( (k+1)! = (k+1) \cdot k! \)
Right side: \( (k+1)^3 = k^3 + 3k^2 + 3k + 1 \)

Using the inductive hypothesis \( k! > k^3 \), we have:
\( (k+1)! = (k+1) \cdot k! > (k+1) \cdot k^3 \)

Now we need to show \( (k+1) \cdot k^3 > (k+1)^3 \), which simplifies to:
\( k^3 > k^2 + 2k + 1 \) (dividing both sides by \( k+1 > 0 \))

For \( k \geq 6 \), \( k^3 \geq 216 \), while \( k^2 + 2k + 1 \leq 36 + 12 + 1 = 49 \), so \( k^3 > k^2 + 2k + 1 \) holds.
Thus \( (k+1)! > (k+1)^3 \).

Therefore, both inequalities are proven by mathematical induction.

**Lean 4 statement:**

```lean
theorem factorial_gt_n_squared (n : ℕ) (h : n ≥ 4) : n! > n^2 := by
  induction' n with k IH
  · linarith [h] -- base case handled by h
  · -- Need to handle inductive step
    have : k ≥ 4 := by omega
    have h1 : (k + 1)! = (k + 1) * k! := by simp
    have h2 : (k + 1)^2 = k^2 + 2*k + 1 := by ring
    have IH' : k! > k^2 := IH this
    have : (k + 1) * k^2 > (k + 1)^2 := by
      have : k^2 > k + 1 := by
        have : k ≥ 4 := this
        nlinarith
      nlinarith
    nlinarith

theorem factorial_gt_n_cubed (n : ℕ) (h : n ≥ 6) : n! > n^3 := by
  induction' n with k IH
  · linarith [h] -- base case handled by h
  · -- Need to handle inductive step
    have : k ≥ 6 := by omega
    have h1 : (k + 1)! = (k + 1) * k! := by simp
    have h2 : (k + 1)^3 = k^3 + 3*k^2 + 3*k + 1 := by ring
    have IH' : k! > k^3 := IH this
    have : (k + 1) * k^3 > (k + 1)^3 := by
      have : k^3 > k^2 + 2*k + 1 := by
        have : k ≥ 6 := this
        nlinarith
      nlinarith
    nlinarith
```

**Output in normal language:**
I have proven both inequalities using mathematical induction:

1. For \( n! > n^2 \) when \( n \geq 4 \):
   - Base case (n=4): 24 > 16 ✓
   - Inductive step: Assuming \( k! > k^2 \) for k ≥ 4, we show \( (k+1)! > (k+1)^2 \)

2. For \( n! > n^3 \) when \( n \geq 6 \):
   - Base case (n=6): 720 > 216 ✓
   - Inductive step: Assuming \( k! > k^3 \) for k ≥ 6, we show \( (k+1)! > (k+1)^3 \)

The Lean 4 code provides formal proofs of these theorems using the natural number type ℕ and the induction tactic.