### Proof by Mathematical Induction

---

#### (a) Prove: For all \( n \geq 1 \), 
\[
\frac{1}{1^2} + \frac{1}{2^2} + \frac{1}{3^2} + \ldots + \frac{1}{n^2} \leq 2 - \frac{1}{n}.
\]

**Base Case (\(n = 1\)):**
\[
\frac{1}{1^2} = 1 \leq 2 - \frac{1}{1} = 1.
\]
✅ Inequality holds.

**Inductive Step:**  
Assume the inequality holds for \(n = k\), i.e.,
\[
\sum_{i=1}^k \frac{1}{i^2} \leq 2 - \frac{1}{k}.
\]
We need to show it holds for \(n = k+1\):
\[
\sum_{i=1}^{k+1} \frac{1}{i^2} \leq 2 - \frac{1}{k+1}.
\]

Start with the inductive hypothesis:
\[
\sum_{i=1}^{k+1} \frac{1}{i^2} = \left( \sum_{i=1}^k \frac{1}{i^2} \right) + \frac{1}{(k+1)^2} \leq \left(2 - \frac{1}{k}\right) + \frac{1}{(k+1)^2}.
\]
We want to show:
\[
2 - \frac{1}{k} + \frac{1}{(k+1)^2} \leq 2 - \frac{1}{k+1}.
\]
Subtract 2 from both sides:
\[
- \frac{1}{k} + \frac{1}{(k+1)^2} \leq - \frac{1}{k+1}.
\]
Multiply both sides by \(-1\) (reversing inequality):
\[
\frac{1}{k} - \frac{1}{(k+1)^2} \geq \frac{1}{k+1}.
\]
Multiply both sides by \(k(k+1)^2\) (positive, so inequality direction unchanged):
\[
(k+1)^2 - k \geq k(k+1).
\]
Compute left side:
\[
(k+1)^2 - k = k^2 + 2k + 1 - k = k^2 + k + 1.
\]
Right side:
\[
k(k+1) = k^2 + k.
\]
So we need:
\[
k^2 + k + 1 \geq k^2 + k,
\]
which is true since \(1 \geq 0\). ✅

Thus, the inequality holds for \(n = k+1\).  
By induction, the statement is true for all \(n \geq 1\).

---

#### (b) Prove: For all \(n \geq 1\),
\[
\frac{1}{2} + \frac{2}{2^2} + \frac{3}{2^3} + \ldots + \frac{n}{2^n} = 2 - \frac{n+2}{2^n}.
\]

**Base Case (\(n = 1\)):**
Left side: \(\frac{1}{2}\).  
Right side: \(2 - \frac{1+2}{2^1} = 2 - \frac{3}{2} = \frac{1}{2}\).  
✅ Equality holds.

**Inductive Step:**  
Assume the formula holds for \(n = k\), i.e.,
\[
\sum_{i=1}^k \frac{i}{2^i} = 2 - \frac{k+2}{2^k}.
\]
We need to show it holds for \(n = k+1\):
\[
\sum_{i=1}^{k+1} \frac{i}{2^i} = 2 - \frac{(k+1)+2}{2^{k+1}} = 2 - \frac{k+3}{2^{k+1}}.
\]

Start with the inductive hypothesis:
\[
\sum_{i=1}^{k+1} \frac{i}{2^i} = \left( \sum_{i=1}^k \frac{i}{2^i} \right) + \frac{k+1}{2^{k+1}} = \left(2 - \frac{k+2}{2^k}\right) + \frac{k+1}{2^{k+1}}.
\]
Write with common denominator \(2^{k+1}\):
\[
= 2 - \frac{2(k+2)}{2^{k+1}} + \frac{k+1}{2^{k+1}} = 2 - \frac{2k+4 - (k+1)}{2^{k+1}} = 2 - \frac{k+3}{2^{k+1}}.
\]
This matches the desired expression for \(n = k+1\). ✅

Thus, the formula holds for \(n = k+1\).  
By induction, the statement is true for all \(n \geq 1\).

---

### ✅ Both statements are proven by mathematical induction.

---

### Lean 4 Statement (for part (b) as an example):

```lean
import Mathlib.Tactic

theorem sum_n_over_2_pow_n (n : ℕ) (h : n ≥ 1) :
    (∑ i in Finset.range (n+1), (i : ℝ) / (2 : ℝ)^i) = 2 - (n + 2 : ℝ) / (2 : ℝ)^n := by
  induction' n with k IH
  · -- Base case n=0 (but n≥1, so skip? Actually, we start at n=1)
    linarith [h]
  · -- Inductive step
    -- Details would require careful calculation similar to the proof above.
    -- This is a sketch; actual Lean proof might use `ring_nf` and other tactics.
    sorry  -- Placeholder for full Lean proof.
```

*Note:* A full Lean proof would require more detailed steps, but the structure follows the inductive argument above.

---

### Output in Normal Language:

Both inequalities (a) and (b) have been proven true for all integers \(n \geq 1\) using mathematical induction. The base cases hold, and the inductive steps confirm that if the statement is true for \(n = k\), it is also true for \(n = k+1\). Therefore, by the principle of mathematical induction, the results are valid for all \(n \geq 1\).