### Step 1: Base Case (n = 1)
Left-hand side (LHS): \(1\)  
Right-hand side (RHS): \(\frac{1(1+1)}{2} = \frac{2}{2} = 1\)  
✅ LHS = RHS, so the base case holds.

### Step 2: Inductive Hypothesis
Assume the formula is true for some \(k \geq 1\):  
\[
1 + 2 + 3 + \ldots + k = \frac{k(k+1)}{2}
\]

### Step 3: Inductive Step (Prove for n = k+1)
We want to show:  
\[
1 + 2 + 3 + \ldots + k + (k+1) = \frac{(k+1)(k+2)}{2}
\]

Start with the left-hand side:  
\[
(1 + 2 + 3 + \ldots + k) + (k+1)
\]
By the inductive hypothesis, this equals:  
\[
\frac{k(k+1)}{2} + (k+1)
\]
Combine the terms:  
\[
= \frac{k(k+1) + 2(k+1)}{2} = \frac{(k+1)(k + 2)}{2}
\]
This matches the right-hand side for \(n = k+1\). ✅

### Step 4: Conclusion
By mathematical induction, the formula  
\[
1 + 2 + 3 + \ldots + n = \frac{n(n+1)}{2}
\]  
holds for all integers \(n \geq 1\).

---

### Lean 4 Proof
```lean
theorem sum_formula (n : ℕ) (h : n ≥ 1) : (Finset.range (n + 1)).sum (λ x => x) = n * (n + 1) / 2 := by
  induction' n with k IH
  · exfalso; linarith [h]  -- n ≥ 1, so base case n=0 is impossible
  · rw [Finset.sum_range_succ]
    by_cases hk : k = 0
    · subst hk; simp
    · have : k ≥ 1 := Nat.one_le_of_lt (Nat.pos_of_ne_zero hk)
      rw [IH this]
      ring
```

**Output in normal language:**  
The formula \(1 + 2 + 3 + \ldots + n = \frac{n(n+1)}{2}\) is proven true for all integers \(n \geq 1\) by mathematical induction. The base case (\(n=1\)) holds, and assuming it holds for \(n=k\), we showed it also holds for \(n=k+1\). Therefore, the formula is valid for all \(n \geq 1\).