I'll prove that the sequence defined by \( a_1 = 11 \), \( a_2 = 21 \), and \( a_n = 3a_{n-1} - 2a_{n-2} \) for \( n \geq 3 \) satisfies \( a_n = 5 \cdot 2^n + 1 \) for all \( n \geq 1 \).

**Proof by mathematical induction:**

**Base case (n = 1):**
\[ a_1 = 11 \]
\[ 5 \cdot 2^1 + 1 = 5 \cdot 2 + 1 = 10 + 1 = 11 \]
✓ Formula holds for n = 1

**Base case (n = 2):**
\[ a_2 = 21 \]
\[ 5 \cdot 2^2 + 1 = 5 \cdot 4 + 1 = 20 + 1 = 21 \]
✓ Formula holds for n = 2

**Inductive step:** Assume the formula holds for n = k and n = k-1, where k ≥ 2:
\[ a_k = 5 \cdot 2^k + 1 \]
\[ a_{k-1} = 5 \cdot 2^{k-1} + 1 \]

Now prove it holds for n = k+1:
\[ a_{k+1} = 3a_k - 2a_{k-1} \]
\[ = 3(5 \cdot 2^k + 1) - 2(5 \cdot 2^{k-1} + 1) \]
\[ = 15 \cdot 2^k + 3 - 10 \cdot 2^{k-1} - 2 \]
\[ = 15 \cdot 2^k - 10 \cdot 2^{k-1} + 1 \]
\[ = 15 \cdot 2^k - 5 \cdot 2^k + 1 \]
\[ = 10 \cdot 2^k + 1 \]
\[ = 5 \cdot 2^{k+1} + 1 \]

✓ Formula holds for n = k+1

By the principle of mathematical induction, the formula \( a_n = 5 \cdot 2^n + 1 \) holds for all \( n \geq 1 \).

**Lean 4 statement:**
```lean
theorem sequence_formula : ∀ (n : ℕ), n ≥ 1 → a n = 5 * 2^n + 1 := by
  intro n hn
  induction' n using Nat.strong_induction_on with k IH
  rcases k with (rfl|rfl|k)
  · -- Case n = 1
    simp [a]
  · -- Case n = 2  
    simp [a]
  · -- Inductive step for n = k + 2 ≥ 3
    have hk1 : k + 1 ≥ 1 := by omega
    have hk : k ≥ 1 := by omega
    rw [a]
    rw [IH (k + 1) (by omega) hk1, IH k (by omega) hk]
    ring_nf
```

**Output in normal language:**
The proof shows that the closed-form expression \( a_n = 5 \cdot 2^n + 1 \) satisfies both the initial conditions \( a_1 = 11 \) and \( a_2 = 21 \), and maintains the recurrence relation \( a_n = 3a_{n-1} - 2a_{n-2} \) for all \( n \geq 3 \). Therefore, this formula correctly represents the sequence for all positive integers n.