### Step-by-Step Proof of Bernoulli's Inequality

We aim to prove:  
If \( 1 + a > 0 \), then \( (1 + a)^n \geq 1 + n a \) for all integers \( n \geq 1 \).

We proceed by **mathematical induction**.

---

#### **Base Case (\( n = 1 \)):**
Left side: \( (1 + a)^1 = 1 + a \)  
Right side: \( 1 + 1 \cdot a = 1 + a \)  
So, \( (1 + a)^1 = 1 + a \), which satisfies the inequality (with equality).  
✅ Base case holds.

---

#### **Inductive Step:**
Assume the inequality holds for some \( n = k \geq 1 \), i.e.,
\[
(1 + a)^k \geq 1 + k a.
\]
We need to show it holds for \( n = k+1 \), i.e.,
\[
(1 + a)^{k+1} \geq 1 + (k+1)a.
\]

Start with the left-hand side:
\[
(1 + a)^{k+1} = (1 + a)^k (1 + a).
\]
By the inductive hypothesis, \( (1 + a)^k \geq 1 + k a \), and since \( 1 + a > 0 \) (given), multiplying both sides by \( (1 + a) \) (a positive number) preserves the inequality:
\[
(1 + a)^k (1 + a) \geq (1 + k a)(1 + a).
\]

Now expand the right-hand side:
\[
(1 + k a)(1 + a) = 1 + a + k a + k a^2 = 1 + (k+1)a + k a^2.
\]

Since \( k a^2 \geq 0 \) (because \( k \geq 1 \) and \( a^2 \geq 0 \)), we have:
\[
1 + (k+1)a + k a^2 \geq 1 + (k+1)a.
\]

Therefore, combining:
\[
(1 + a)^{k+1} \geq 1 + (k+1)a + k a^2 \geq 1 + (k+1)a.
\]

So,
\[
(1 + a)^{k+1} \geq 1 + (k+1)a,
\]
which completes the inductive step.

---

#### **Conclusion:**
By mathematical induction, Bernoulli's inequality holds for all integers \( n \geq 1 \), given \( 1 + a > 0 \).

---

### **Lean 4 Formalization**

```lean
theorem bernoulli_inequality (a : ℝ) (h : -1 < a) (n : ℕ) (hn : n ≥ 1) :
    (1 + a) ^ n ≥ 1 + n * a := by
  -- Base case: n = 1
  have base : (1 + a) ^ 1 ≥ 1 + 1 * a := by
    simp
  -- Inductive step
  refine Nat.le_induction base (λ k hk hind => ?_) n hn
  have hpos : 0 < 1 + a := by linarith [h]
  calc
    (1 + a) ^ (k + 1) = (1 + a) ^ k * (1 + a) := by ring
    _ ≥ (1 + k * a) * (1 + a) := by exact mul_le_mul_of_nonneg_left hind hpos.le
    _ = 1 + (k + 1) * a + k * a ^ 2 := by ring
    _ ≥ 1 + (k + 1) * a := by nlinarith [sq_nonneg a]
```

**Explanation of the Lean code:**
- We assume `a : ℝ` with `h : -1 < a` (equivalent to `1 + a > 0`).
- For `n : ℕ` with `n ≥ 1`, we prove `(1 + a)^n ≥ 1 + n * a`.
- The base case (`n=1`) is trivial (`simp` handles it).
- For the inductive step, we use `Nat.le_induction` (induction from 1 upwards).
- We use the fact that `1 + a > 0` (from `h`) to multiply inequalities.
- The calculation expands `(1 + k*a)*(1 + a)` and uses `k*a^2 ≥ 0` (since `a^2 ≥ 0`) to drop the nonnegative term.

This completes the proof.