I will prove the formula by mathematical induction.

**Statement to prove:** For all integers n ≥ 1, 1³ + 2³ + 3³ + ... + n³ = [n(n+1)/2]²

**Base case (n = 1):**
Left side: 1³ = 1
Right side: [1(1+1)/2]² = [1×2/2]² = [2/2]² = [1]² = 1
Both sides equal 1 ✓

**Inductive step:**
Assume the formula holds for some integer k ≥ 1, that is:
1³ + 2³ + ... + k³ = [k(k+1)/2]²

Now prove it holds for k+1:
Left side: 1³ + 2³ + ... + k³ + (k+1)³ = [k(k+1)/2]² + (k+1)³

Simplify the right side:
= (k+1)²[k²/4 + (k+1)]
= (k+1)²[(k² + 4(k+1))/4]
= (k+1)²[(k² + 4k + 4)/4]
= (k+1)²[(k+2)²/4]
= [(k+1)(k+2)/2]²

This equals the right side for n = k+1: [(k+1)((k+1)+1)/2]² = [(k+1)(k+2)/2]²

**Conclusion:**
By mathematical induction, the formula holds for all integers n ≥ 1.

**Lean statement:**
```lean
theorem sum_of_cubes_formula (n : ℕ) : ∑_{k=1}^n k^3 = (n*(n+1)/2)^2 := by
  induction' n with k IH
  · simp -- base case n=0 (sum is 0, both sides 0)
  · rw [Finset.sum_range_succ, IH]
    simp [Nat.succ_eq_add_one]
    ring
```

**Normal language output:**
The formula 1³ + 2³ + 3³ + ... + n³ = [n(n+1)/2]² has been proven to hold for all positive integers n using mathematical induction. The base case (n=1) was verified, and the inductive step showed that if the formula holds for some integer k, then it must also hold for k+1. Therefore, by the principle of mathematical induction, the formula is valid for all n ≥ 1.