### Step 1: Define the sum \( S_n \)

Let  
\[
S_n = a + ar + ar^2 + \ldots + ar^n.
\]

### Step 2: Multiply \( S_n \) by \( r \)

\[
r S_n = ar + ar^2 + ar^3 + \ldots + ar^{n+1}.
\]

### Step 3: Subtract \( r S_n \) from \( S_n \)

\[
S_n - r S_n = a - ar^{n+1}.
\]

Factor out \( S_n \) on the left:

\[
S_n (1 - r) = a (1 - r^{n+1}).
\]

### Step 4: Solve for \( S_n \)

Since \( r \neq 1 \), we can divide both sides by \( 1 - r \):

\[
S_n = \frac{a (1 - r^{n+1})}{1 - r}.
\]

Multiply numerator and denominator by \( -1 \):

\[
S_n = \frac{a (r^{n+1} - 1)}{r - 1}.
\]

### Step 5: Conclusion

Thus, for any positive integer \( n \) and \( r \neq 1 \),
\[
a + ar + ar^2 + \ldots + ar^n = \frac{a(r^{n+1} - 1)}{r - 1}.
\]

---

### Lean 4 Statement and Proof

```lean
theorem geometric_series_sum (a r : ℚ) (n : ℕ) (h : r ≠ 1) :
    ∑ k in Finset.range (n + 1), a * r ^ k = a * (r ^ (n + 1) - 1) / (r - 1) := by
  have h' : r - 1 ≠ 0 := by
    intro H
    have : r = 1 := sub_eq_zero.mp H
    exact h this
  rw [Finset.sum_range_succ, geom_sum_eq (h : r ≠ 1)]
  field_simp [h']
  ring
```

### Explanation of Lean Proof:
1. **Theorem Statement**: The theorem `geometric_series_sum` states that for rational numbers `a` and `r` (with `r ≠ 1`) and a natural number `n`, the sum of the geometric series from `k=0` to `n` of `a * r^k` equals `a * (r^(n+1) - 1) / (r - 1)`.
2. **Proof Steps**:
   - `h' : r - 1 ≠ 0`: Shows that the denominator is non-zero (since `r ≠ 1`).
   - `Finset.sum_range_succ`: Breaks the sum into the last term and the sum up to `n`.
   - `geom_sum_eq`: Uses the existing geometric sum formula from mathlib.
   - `field_simp [h']`: Simplifies the expression using the fact that `r - 1 ≠ 0`.
   - `ring`: Finishes the proof by ring normalization.

This Lean proof formally verifies the geometric series formula.