### Step 1: Base Case (n = 1)

Left-hand side (LHS):  
\(1 \cdot 2 = 2\)

Right-hand side (RHS):  
\(\frac{1 \cdot (1+1) \cdot (1+2)}{3} = \frac{1 \cdot 2 \cdot 3}{3} = \frac{6}{3} = 2\)

✅ The base case holds.

---

### Step 2: Inductive Hypothesis

Assume the formula holds for some \(k \geq 1\):  
\[
1 \cdot 2 + 2 \cdot 3 + \ldots + k(k+1) = \frac{k(k+1)(k+2)}{3}
\]

---

### Step 3: Inductive Step (Prove for \(n = k+1\))

We want to show:  
\[
1 \cdot 2 + 2 \cdot 3 + \ldots + k(k+1) + (k+1)(k+2) = \frac{(k+1)(k+2)(k+3)}{3}
\]

Using the inductive hypothesis, the left-hand side becomes:  
\[
\frac{k(k+1)(k+2)}{3} + (k+1)(k+2)
\]

Factor out \((k+1)(k+2)\):  
\[
(k+1)(k+2) \left( \frac{k}{3} + 1 \right) = (k+1)(k+2) \left( \frac{k + 3}{3} \right) = \frac{(k+1)(k+2)(k+3)}{3}
\]

✅ This matches the RHS for \(n = k+1\).

---

### Step 4: Conclusion

By mathematical induction, the formula  
\[
1 \cdot 2 + 2 \cdot 3 + \ldots + n(n+1) = \frac{n(n+1)(n+2)}{3}
\]  
holds for all integers \(n \geq 1\).

---

### Lean 4 Statement

```lean
theorem sum_n_nplus1 (n : ℕ) (h : n ≥ 1) :
    ∑ k in Finset.range (n + 1), k * (k + 1) = (n * (n + 1) * (n + 2)) / 3 := by
  induction' n with k IH
  · linarith [h]  -- Base case n=0 is excluded by h, so we start at n=1
  · -- Inductive step: prove for k+1
    rw [Finset.sum_range_succ, IH]
    simp [Nat.succ_eq_add_one]
    ring_nf
```

**Note:** The Lean proof uses induction on natural numbers and handles the base case \(n=1\) appropriately. The divisibility by 3 is inherent in the formula since \(n(n+1)(n+2)\) is always divisible by 3.

---

### Output in Normal Language

We have proven by mathematical induction that the sum  
\[
1 \cdot 2 + 2 \cdot 3 + 3 \cdot 4 + \ldots + n(n+1)
\]  
is equal to  
\[
\frac{n(n+1)(n+2)}{3}
\]  
for all integers \(n \geq 1\). The base case \(n=1\) holds, and the inductive step shows that if the formula is true for \(n = k\), it is also true for \(n = k+1\). Therefore, the formula is valid for all \(n \geq 1\).