I'll prove this by mathematical induction in Lean and then explain it in natural language.

**Lean Proof:**
```lean
theorem sum_of_odds (n : ℕ) : ∑ k in Finset.range n, (2 * k + 1) = n ^ 2 := by
  induction' n with k IH
  · simp -- base case n = 0
  · rw [Finset.sum_range_succ, IH]
    ring_nf
```

**Natural Language Explanation:**

**Base Case (n = 1):**
When n = 1, the left side is just the first odd number: 1
The right side is 1² = 1
So 1 = 1 ✓

**Inductive Step:**
Assume the formula holds for some positive integer k, meaning:
1 + 3 + 5 + ... + (2k - 1) = k²

Now we want to prove it holds for k + 1:
1 + 3 + 5 + ... + (2k - 1) + (2(k + 1) - 1) = (k + 1)²

The next odd number is 2(k + 1) - 1 = 2k + 1
Using our assumption:
Left side = k² + (2k + 1)
Right side = (k + 1)² = k² + 2k + 1

Since k² + (2k + 1) = k² + 2k + 1, the formula holds for k + 1.

**Conclusion:**
By the principle of mathematical induction, the formula 1 + 3 + 5 + ... + (2n - 1) = n² holds for all positive integers n ≥ 1.

**Output:** The sum of the first n odd numbers equals n squared, and this has been proven true for all positive integers using mathematical induction.