Let's address each part step by step.

### (a) Find the values of \( n \leq 7 \) for which \( n! + 1 \) is a perfect square.

We'll compute \( n! + 1 \) for \( n = 0 \) to \( n = 7 \) and check if it is a perfect square.

- \( n = 0 \): \( 0! + 1 = 1 + 1 = 2 \) (not a square).
- \( n = 1 \): \( 1! + 1 = 1 + 1 = 2 \) (not a square).
- \( n = 2 \): \( 2! + 1 = 2 + 1 = 3 \) (not a square).
- \( n = 3 \): \( 3! + 1 = 6 + 1 = 7 \) (not a square).
- \( n = 4 \): \( 4! + 1 = 24 + 1 = 25 = 5^2 \) (perfect square).
- \( n = 5 \): \( 5! + 1 = 120 + 1 = 121 = 11^2 \) (perfect square).
- \( n = 6 \): \( 6! + 1 = 720 + 1 = 721 \) (not a square, since \( 26^2 = 676 \), \( 27^2 = 729 \)).
- \( n = 7 \): \( 7! + 1 = 5040 + 1 = 5041 \). Check if it is a square: \( 71^2 = 5041 \). So, \( 5041 = 71^2 \) (perfect square).

Thus, for \( n \leq 7 \), the values where \( n! + 1 \) is a perfect square are \( n = 4, 5, 7 \).

**Lean Statement:**
```lean
-- Check for n â‰¤ 7 where n! + 1 is a perfect square.
-- n=4: 24+1=25=5^2
-- n=5: 120+1=121=11^2
-- n=7: 5040+1=5041=71^2
-- So the values are n=4, n=5, n=7.
```

**Output in normal language:**
The values of \( n \leq 7 \) for which \( n! + 1 \) is a perfect square are \( n = 4 \), \( n = 5 \), and \( n = 7 \).

---

### (b) True or false? For positive integers m and n, (mn)! = m!n! and (m + n)! = m! + n!.

We need to check both equations.

1. Is \( (mn)! = m! \cdot n! \) for all positive integers \( m, n \)?
   - Take \( m = 2, n = 2 \): \( (2 \cdot 2)! = 4! = 24 \), but \( 2! \cdot 2! = 2 \cdot 2 = 4 \). So \( 24 \neq 4 \). Hence, false.

2. Is \( (m + n)! = m! + n! \) for all positive integers \( m, n \)?
   - Take \( m = 2, n = 2 \): \( (2+2)! = 4! = 24 \), but \( 2! + 2! = 2 + 2 = 4 \). So \( 24 \neq 4 \). Hence, false.

Therefore, both statements are false.

**Lean Statement:**
```lean
-- For positive integers m and n, (mn)! = m! * n! is false.
-- Counterexample: m=2, n=2: (2*2)! = 4! = 24, but 2! * 2! = 2*2=4.
-- Similarly, (m+n)! = m! + n! is false.
-- Counterexample: m=2, n=2: (2+2)! = 24, but 2! + 2! = 4.
-- So both are false.
```

**Output in normal language:**
Both statements are false. 
- For \( (mn)! = m! \cdot n! \): a counterexample is \( m = 2, n = 2 \), where \( (2 \cdot 2)! = 24 \) but \( 2! \cdot 2! = 4 \).
- For \( (m + n)! = m! + n! \): a counterexample is \( m = 2, n = 2 \), where \( (2 + 2)! = 24 \) but \( 2! + 2! = 4 \).

---

### Final Summary:
(a) The values are \( n = 4, 5, 7 \).
(b) Both statements are false.