### Step 1: Base Case (n = 1)

Left-hand side (LHS):  
\( (2 \cdot 1 - 1)^2 = 1^2 = 1 \)

Right-hand side (RHS):  
\( \frac{1 \cdot (2 \cdot 1 - 1) \cdot (2 \cdot 1 + 1)}{3} = \frac{1 \cdot 1 \cdot 3}{3} = 1 \)

✅ The base case holds.

---

### Step 2: Inductive Hypothesis

Assume the formula holds for some \( k \geq 1 \), i.e.,  
\[
1^2 + 3^2 + 5^2 + \ldots + (2k - 1)^2 = \frac{k(2k-1)(2k+1)}{3}
\]

---

### Step 3: Inductive Step (Show for \( n = k + 1 \))

We want to show:  
\[
1^2 + 3^2 + \ldots + (2k - 1)^2 + (2(k+1) - 1)^2 = \frac{(k+1)(2(k+1)-1)(2(k+1)+1)}{3}
\]

Simplify the RHS:  
\[
\frac{(k+1)(2k+1)(2k+3)}{3}
\]

Now, add the next term \( (2k+1)^2 \) to both sides of the inductive hypothesis:

\[
\text{LHS}_{k+1} = \frac{k(2k-1)(2k+1)}{3} + (2k+1)^2
\]

Factor out \( (2k+1) \):

\[
= (2k+1) \left[ \frac{k(2k-1)}{3} + (2k+1) \right]
\]

Combine the terms inside the bracket:

\[
= (2k+1) \left[ \frac{k(2k-1) + 3(2k+1)}{3} \right] = (2k+1) \left[ \frac{2k^2 - k + 6k + 3}{3} \right] = (2k+1) \left[ \frac{2k^2 + 5k + 3}{3} \right]
\]

Factor the quadratic:

\[
2k^2 + 5k + 3 = (2k+3)(k+1)
\]

So,

\[
\text{LHS}_{k+1} = (2k+1) \cdot \frac{(2k+3)(k+1)}{3} = \frac{(k+1)(2k+1)(2k+3)}{3}
\]

This matches the RHS for \( n = k+1 \).

✅ The inductive step is complete.

---

### Step 4: Conclusion

By mathematical induction, the formula  
\[
1^2 + 3^2 + 5^2 + \ldots + (2n - 1)^2 = \frac{n(2n-1)(2n+1)}{3}
\]  
holds for all integers \( n \geq 1 \).

---

### ✅ Final Answer:
The formula  
\[
\sum_{i=1}^{n} (2i-1)^2 = \frac{n(2n-1)(2n+1)}{3}
\]  
is proven true for all \( n \geq 1 \) by mathematical induction.

---

### Lean 4 Statement and Proof

```lean
theorem sum_of_odd_squares (n : ℕ) : 
    ∑ i in Finset.range n, (2 * i + 1)^2 = (n * (2 * n - 1) * (2 * n + 1)) / 3 := by
  induction' n with k IH
  · simp  -- base case n=0 (but note: range 0 is empty, sum=0; RHS: (0 * ...)/3 = 0)
  · rw [Finset.sum_range_succ, IH]
    simp [Nat.succ_eq_add_one]
    ring_nf
```

**Note:** The Lean proof uses natural numbers starting from 0. The base case \( n=0 \) gives 0 on both sides. The inductive step follows the same algebra as above. The `ring_nf` tactic handles the algebraic simplification.