I need to use the Second Principle of Finite Induction (also called strong induction) to prove that for all n ≥ 1:

$$a^n - 1 = (a - 1)(a^{n-1} + a^{n-2} + a^{n-3} + \ldots + a + 1)$$

**Base Case (n = 1):**
Left side: a¹ - 1 = a - 1
Right side: (a - 1)(a⁰) = (a - 1)(1) = a - 1
✓ Base case holds

**Inductive Hypothesis:** Assume the statement is true for all k where 1 ≤ k ≤ m for some m ≥ 1

**Inductive Step (n = m + 1):**
We need to show:
$$a^{m+1} - 1 = (a - 1)(a^m + a^{m-1} + \ldots + a + 1)$$

Consider:
$$a^{m+1} - 1 = a(a^m - 1) + (a - 1)$$

By the inductive hypothesis (for k = m):
$$a^m - 1 = (a - 1)(a^{m-1} + a^{m-2} + \ldots + a + 1)$$

Substitute:
$$a^{m+1} - 1 = a[(a - 1)(a^{m-1} + a^{m-2} + \ldots + a + 1)] + (a - 1)$$
$$= (a - 1)[a(a^{m-1} + a^{m-2} + \ldots + a + 1) + 1]$$
$$= (a - 1)[a^m + a^{m-1} + \ldots + a^2 + a + 1]$$

This is exactly the right side for n = m + 1.

**Conclusion:** By the Second Principle of Finite Induction, the statement holds for all n ≥ 1.

---
**Lean 4 Statement:**
```lean
theorem power_minus_one_factorization (a : ℤ) (n : ℕ) (hn : n ≥ 1) :
  a^n - 1 = (a - 1) * (∑ i in Finset.range n, a^(n - 1 - i)) := by
  -- Proof using strong induction would go here
  sorry
```

---
**Normal Language Output:**
The Second Principle of Finite Induction confirms that for any integer n ≥ 1 and any real number a, the expression aⁿ - 1 can be factored as (a - 1) multiplied by the sum of all powers of a from aⁿ⁻¹ down to a⁰. This factorization holds because:

1. The base case (n = 1) works trivially
2. Assuming it works for all values up to m, we can show it must work for m + 1 by algebraically manipulating aᵐ⁺¹ - 1 using the known factorization for aᵐ - 1

This represents the standard geometric series formula where the sum of a geometric progression with ratio a is (aⁿ - 1)/(a - 1) when a ≠ 1.