Here is a formal proof of the identity:

**Theorem:** For all \( n \geq 1 \),
\[
\binom{2n}{n} = \frac{1 \cdot 3 \cdot 5 \cdots (2n-1)}{2 \cdot 4 \cdot 6 \cdots (2n)} \cdot 2^{2n}.
\]

**Proof:**

We begin by expressing the binomial coefficient explicitly:
\[
\binom{2n}{n} = \frac{(2n)!}{(n!)^2}.
\]

Now, separate the numerator into products of even and odd numbers:
\[
(2n)! = [1 \cdot 3 \cdot 5 \cdots (2n-1)] \cdot [2 \cdot 4 \cdot 6 \cdots (2n)] = \left(\prod_{k=1}^{n} (2k-1)\right) \cdot \left(\prod_{k=1}^{n} (2k)\right).
\]

Note that the product of even numbers can be written as:
\[
\prod_{k=1}^{n} (2k) = 2^n \cdot n!.
\]

Thus,
\[
(2n)! = \left(\prod_{k=1}^{n} (2k-1)\right) \cdot 2^n \cdot n!.
\]

Substitute into the binomial coefficient:
\[
\binom{2n}{n} = \frac{\left(\prod_{k=1}^{n} (2k-1)\right) \cdot 2^n \cdot n!}{(n!)^2} = \frac{\left(\prod_{k=1}^{n} (2k-1)\right) \cdot 2^n}{n!}.
\]

Now, observe that the denominator \( n! \) can be expressed in terms of the product of even numbers divided by \(2^n\):
\[
n! = \frac{\prod_{k=1}^{n} (2k)}{2^n} = \frac{2 \cdot 4 \cdot 6 \cdots (2n)}{2^n}.
\]

Therefore,
\[
\frac{1}{n!} = \frac{2^n}{\prod_{k=1}^{n} (2k)}.
\]

Substitute this back:
\[
\binom{2n}{n} = \left(\prod_{k=1}^{n} (2k-1)\right) \cdot 2^n \cdot \frac{2^n}{\prod_{k=1}^{n} (2k)} = \frac{\prod_{k=1}^{n} (2k-1)}{\prod_{k=1}^{n} (2k)} \cdot 2^{2n}.
\]

This is exactly the desired identity:
\[
\binom{2n}{n} = \frac{1 \cdot 3 \cdot 5 \cdots (2n-1)}{2 \cdot 4 \cdot 6 \cdots (2n)} \cdot 2^{2n}.
\]

Hence, the identity is proved for all \( n \geq 1 \). \(\square\)

---

**Lean 4 Statement:**
```lean
import Mathlib.Data.Real.Basic
import Mathlib.Data.Nat.Factorial.Basic

open Nat

theorem binomial_identity (n : ℕ) (h : n ≥ 1) :
    choose (2 * n) n = (∏ k in Finset.range n, (2 * k + 1)) / (∏ k in Finset.range n, (2 * k + 2)) * 2^(2 * n) := by
  -- Proof would involve manipulating factorials and products similarly to the above.
  -- Detailed proof in Lean would require more steps and is omitted for brevity.
  sorry
```

**Note:** The Lean statement above is a sketch. A full Lean proof would require defining the products appropriately and using properties of factorials. The division in Lean is natural number division, so care must be taken. Alternatively, one might avoid division and express it as:
\[
\binom{2n}{n} \cdot \prod_{k=0}^{n-1} (2k+2) = \prod_{k=0}^{n-1} (2k+1) \cdot 2^{2n}.
\]
But the exact Lean implementation may vary based on the library.