### Step 1: Express \(C_n\) and \(C_{n-1}\) using the explicit formula

Recall the explicit formula for the Catalan number:
\[
C_n = \frac{1}{n+1} \binom{2n}{n} = \frac{(2n)!}{n!(n+1)!}
\]
Similarly, for \(C_{n-1}\):
\[
C_{n-1} = \frac{1}{n} \binom{2(n-1)}{n-1} = \frac{(2n-2)!}{(n-1)! \cdot n!}
\]

### Step 2: Compute the ratio \(\frac{C_n}{C_{n-1}}\)

We want to show:
\[
C_n = \frac{2(2n-1)}{n+1} C_{n-1}
\]
This is equivalent to:
\[
\frac{C_n}{C_{n-1}} = \frac{2(2n-1)}{n+1}
\]

Now compute \(\frac{C_n}{C_{n-1}}\) using the explicit formulas:
\[
\frac{C_n}{C_{n-1}} = \frac{ \frac{(2n)!}{n!(n+1)!} }{ \frac{(2n-2)!}{(n-1)! n!} } = \frac{(2n)!}{n!(n+1)!} \cdot \frac{(n-1)! n!}{(2n-2)!}
\]

Simplify:
- Cancel \(n!\) in numerator and denominator:
\[
= \frac{(2n)!}{(n+1)!} \cdot \frac{(n-1)!}{(2n-2)!}
\]

Now write \((2n)! = (2n)(2n-1)(2n-2)!\) and \((n+1)! = (n+1)n(n-1)!\):
\[
= \frac{(2n)(2n-1)(2n-2)!}{(n+1)n(n-1)!} \cdot \frac{(n-1)!}{(2n-2)!}
\]

Cancel \((2n-2)!\) and \((n-1)!\):
\[
= \frac{(2n)(2n-1)}{(n+1)n}
\]

Simplify the fraction:
\[
= \frac{2n(2n-1)}{n(n+1)} = \frac{2(2n-1)}{n+1}
\]

Therefore:
\[
\frac{C_n}{C_{n-1}} = \frac{2(2n-1)}{n+1}
\]
which implies:
\[
C_n = \frac{2(2n-1)}{n+1} C_{n-1}
\]

### Step 3: Lean 4 Statement

To formalize this in Lean 4, we can define the Catalan numbers and prove the recurrence relation. Here is a possible Lean statement:

```lean
import Mathlib.Data.Real.Basic
import Mathlib.Combinatorics.Catalan

open Nat

theorem catalan_recurrence (n : ℕ) (h : n ≥ 1) : catalan n = 2 * (2 * n - 1) * (catalan (n - 1)) / (n + 1) := by
  rw [catalan_eq_central_binomial_div]
  rw [catalan_eq_central_binomial_div (n := n - 1)]
  -- Further steps to simplify and prove the identity
  -- (This is a sketch; the actual proof may require more details.)
```

**Note:** The exact Lean proof might require more steps and leveraging existing lemmas about binomial coefficients. The above is a template; the full proof would involve algebraic manipulation similar to the mathematical derivation.

### Step 4: Output in Normal Language

We have proven that for \(n \geq 1\), the Catalan number \(C_n\) satisfies the recurrence relation:
\[
C_n = \frac{2(2n-1)}{n+1} C_{n-1}
\]
This is derived by taking the ratio of the explicit formulas for \(C_n\) and \(C_{n-1}\), simplifying, and obtaining the desired factor. The recurrence provides an efficient way to compute Catalan numbers inductively.