I'll solve each part step by step.

### (a) Prove that for \( n \geq 2 \):
\[
\binom{2}{2} + \binom{3}{2} + \binom{4}{2} + \ldots + \binom{n}{2} = \binom{n+1}{3}
\]

**Proof by induction:**

**Base case (n=2):**
\[
\binom{2}{2} = 1 \quad \text{and} \quad \binom{2+1}{3} = \binom{3}{3} = 1
\]
So the formula holds for n=2.

**Inductive step:** Assume the formula holds for n=k:
\[
\sum_{i=2}^k \binom{i}{2} = \binom{k+1}{3}
\]
Now prove for n=k+1:
\[
\sum_{i=2}^{k+1} \binom{i}{2} = \sum_{i=2}^k \binom{i}{2} + \binom{k+1}{2} = \binom{k+1}{3} + \binom{k+1}{2}
\]
Using Pascal's identity: \(\binom{k+1}{3} + \binom{k+1}{2} = \binom{k+2}{3}\)
\[
= \binom{(k+1)+1}{3}
\]
Thus, the formula holds for n=k+1.

By induction, the formula is true for all \( n \geq 2 \).

### (b) From part (a) and \( m^2 = 2\binom{m}{2} + m \) for \( m \geq 2 \), deduce:
\[
1^2 + 2^2 + 3^2 + \ldots + n^2 = \frac{n(n+1)(2n+1)}{6}
\]

**Proof:**

From the given relation:
\[
m^2 = 2\binom{m}{2} + m \quad \text{for } m \geq 2
\]
For m=1: \( 1^2 = 1 \)

Sum from m=1 to n:
\[
\sum_{m=1}^n m^2 = 1^2 + \sum_{m=2}^n m^2 = 1 + \sum_{m=2}^n \left(2\binom{m}{2} + m\right)
\]
\[
= 1 + 2\sum_{m=2}^n \binom{m}{2} + \sum_{m=2}^n m
\]
From part (a): \(\sum_{m=2}^n \binom{m}{2} = \binom{n+1}{3}\)
\[
= 1 + 2\binom{n+1}{3} + \left(\sum_{m=1}^n m - 1\right)
\]
\[
= 2\binom{n+1}{3} + \sum_{m=1}^n m
\]
Now compute:
\[
\binom{n+1}{3} = \frac{(n+1)n(n-1)}{6}, \quad \sum_{m=1}^n m = \frac{n(n+1)}{2}
\]
So:
\[
\sum_{m=1}^n m^2 = 2\cdot\frac{(n+1)n(n-1)}{6} + \frac{n(n+1)}{2}
= \frac{(n+1)n(n-1)}{3} + \frac{n(n+1)}{2}
\]
\[
= n(n+1)\left(\frac{n-1}{3} + \frac{1}{2}\right)
= n(n+1)\left(\frac{2(n-1) + 3}{6}\right)
= n(n+1)\left(\frac{2n - 2 + 3}{6}\right)
\]
\[
= n(n+1)\left(\frac{2n + 1}{6}\right)
= \frac{n(n+1)(2n+1)}{6}
\]

### (c) Apply the formula in part (a) to prove:
\[
1·2 + 2·3 + \ldots + n(n+1) = \frac{n(n+1)(n+2)}{3}
\]

**Proof:**

Note that:
\[
k(k+1) = 2\binom{k+1}{2}
\]
So:
\[
\sum_{k=1}^n k(k+1) = \sum_{k=1}^n 2\binom{k+1}{2} = 2\sum_{k=1}^n \binom{k+1}{2}
\]
Change index: let m = k+1, then when k=1, m=2; when k=n, m=n+1
\[
= 2\sum_{m=2}^{n+1} \binom{m}{2}
\]
From part (a): \(\sum_{m=2}^{n+1} \binom{m}{2} = \binom{n+2}{3}\)
\[
= 2\binom{n+2}{3} = 2\cdot\frac{(n+2)(n+1)n}{6} = \frac{(n+2)(n+1)n}{3}
\]
\[
= \frac{n(n+1)(n+2)}{3}
\]

**Lean statement to confirm result:**
```lean
-- Part (a)
theorem sum_choose_two (n : ℕ) (h : n ≥ 2) : 
  ∑ k in range (n - 1), Nat.choose (k + 2) 2 = Nat.choose (n + 1) 3 := by
  -- Proof would use induction and Pascal's identity

-- Part (b)  
theorem sum_squares (n : ℕ) : 
  ∑ k in range n, (k + 1)^2 = (n * (n + 1) * (2 * n + 1)) / 6 := by
  -- Proof would use the relation from part (a)

-- Part (c)
theorem sum_products (n : ℕ) : 
  ∑ k in range n, (k + 1) * (k + 2) = (n * (n + 1) * (n + 2)) / 3 := by
  -- Proof would use the result from part (a)
```

**Final answers:**
- (a) The sum equals \(\binom{n+1}{3}\), proven by induction
- (b) The sum of squares equals \(\frac{n(n+1)(2n+1)}{6}\), derived using the combinatorial identity
- (c) The sum of products equals \(\frac{n(n+1)(n+2)}{3}\), obtained by applying part (a)