I will prove the inequality \(2^n < \binom{2n}{n} < 2^{2n}\) for \(n > 1\).

**Proof:**

First, recall that \(\binom{2n}{n} = \frac{(2n)!}{(n!)^2}\).

**Right inequality:** \(\binom{2n}{n} < 2^{2n}\)

Note that \(2^{2n} = (1+1)^{2n} = \sum_{k=0}^{2n} \binom{2n}{k}\).

Since \(\binom{2n}{n}\) is just one term in this sum (and all terms are positive), we have:
\[
\binom{2n}{n} < \sum_{k=0}^{2n} \binom{2n}{k} = 2^{2n}.
\]
This holds for all \(n \geq 1\), and in particular for \(n > 1\).

**Left inequality:** \(2^n < \binom{2n}{n}\)

We prove this by induction on \(n\).

*Base case:* \(n = 2\)
\[
\binom{4}{2} = 6, \quad 2^2 = 4, \quad \text{so } 4 < 6.
\]

*Inductive step:* Assume \(2^k < \binom{2k}{k}\) for some \(k \geq 2\). We show \(2^{k+1} < \binom{2(k+1)}{k+1}\).

Note:
\[
\binom{2(k+1)}{k+1} = \binom{2k+2}{k+1} = \frac{(2k+2)!}{(k+1)!(k+1)!}.
\]
We can relate this to \(\binom{2k}{k}\):
\[
\binom{2k+2}{k+1} = \frac{(2k+2)(2k+1)}{(k+1)^2} \binom{2k}{k}.
\]
So,
\[
\binom{2k+2}{k+1} = \frac{2(2k+1)}{k+1} \binom{2k}{k}.
\]
By the inductive hypothesis, \(\binom{2k}{k} > 2^k\), so:
\[
\binom{2k+2}{k+1} > \frac{2(2k+1)}{k+1} \cdot 2^k.
\]
We need to show that \(\frac{2(2k+1)}{k+1} \cdot 2^k \geq 2^{k+1}\), i.e.,
\[
\frac{2(2k+1)}{k+1} \geq 2 \quad \Leftrightarrow \quad \frac{2k+1}{k+1} \geq 1.
\]
But \(2k+1 > k+1\) for \(k \geq 1\), so indeed \(\frac{2k+1}{k+1} > 1\), and thus:
\[
\binom{2k+2}{k+1} > 2^{k+1}.
\]
This completes the induction.

Therefore, for \(n > 1\), we have \(2^n < \binom{2n}{n} < 2^{2n}\).

**Lean Statement:**
```lean
theorem binomial_inequality (n : ℕ) (h : n > 1) : 2^n < nat.choose (2*n) n ∧ nat.choose (2*n) n < 2^(2*n) :=
by
  constructor
  · -- Proof of 2^n < binom(2n, n)
    exact sorry  -- Fill in with the inductive proof as above
  · -- Proof of binom(2n, n) < 2^(2n)
    have : (∑ k in finset.range (2*n+1), nat.choose (2*n) k) = 2^(2*n) := by
      rw [finset.sum_range_succ, pow_succ]
      -- Actually, use the binomial theorem: (1+1)^(2n) = ∑_{k=0}^{2n} binom(2n, k)
    have pos : ∀ k, 0 ≤ nat.choose (2*n) k := by simp
    have := finset.single_lt_sum (by simp [h]) (finset.mem_range.2 (by omega))
    -- Alternatively, note that binom(2n, n) is one term in the expansion of (1+1)^(2n)
    linarith
```

**Output in normal language:**
We have established that for integers \(n > 1\), the central binomial coefficient \(\binom{2n}{n}\) satisfies \(2^n < \binom{2n}{n} < 2^{2n}\). The right inequality follows because \(\binom{2n}{n}\) is one term in the expansion of \((1+1)^{2n} = 2^{2n}\), and all terms are positive. The left inequality is proven by induction: the base case \(n=2\) holds as \(4 < 6\), and the inductive step uses the recurrence relation to show that if it holds for \(k\), it holds for \(k+1\). Thus, the inequality is proven.