I'll derive the binomial identity step by step.

**Given identity:**
$$\binom{2}{2} + \binom{4}{2} + \binom{6}{2} + \ldots + \binom{2n}{2} = \frac{n(n+1)(4n-1)}{6} \quad \text{for } n\geq{2}$$

**Step 1: Recognize the pattern**
The sum consists of binomial coefficients $\binom{2k}{2}$ where $k$ ranges from 1 to $n$.

**Step 2: Simplify the binomial coefficient**
Recall that $\binom{m}{2} = \frac{m(m-1)}{2}$, so:
$$\binom{2k}{2} = \frac{(2k)(2k-1)}{2} = k(2k-1)$$

**Step 3: Rewrite the sum**
$$\sum_{k=1}^{n} \binom{2k}{2} = \sum_{k=1}^{n} k(2k-1) = \sum_{k=1}^{n} (2k^2 - k)$$

**Step 4: Split into two sums**
$$= 2\sum_{k=1}^{n} k^2 - \sum_{k=1}^{n} k$$

**Step 5: Apply known summation formulas**
Using:
- $\sum_{k=1}^{n} k = \frac{n(n+1)}{2}$
- $\sum_{k=1}^{n} k^2 = \frac{n(n+1)(2n+1)}{6}$

We get:
$$= 2\left(\frac{n(n+1)(2n+1)}{6}\right) - \frac{n(n+1)}{2}$$

**Step 6: Simplify the expression**
$$= \frac{n(n+1)(2n+1)}{3} - \frac{n(n+1)}{2}$$

Find a common denominator (6):
$$= \frac{2n(n+1)(2n+1)}{6} - \frac{3n(n+1)}{6}$$

**Step 7: Combine terms**
$$= \frac{n(n+1)[2(2n+1) - 3]}{6} = \frac{n(n+1)(4n + 2 - 3)}{6} = \frac{n(n+1)(4n - 1)}{6}$$

**Final result:**
$$\binom{2}{2} + \binom{4}{2} + \binom{6}{2} + \ldots + \binom{2n}{2} = \frac{n(n+1)(4n-1)}{6}$$

**Verification for n=2:**
Left side: $\binom{2}{2} + \binom{4}{2} = 1 + 6 = 7$
Right side: $\frac{2(2+1)(8-1)}{6} = \frac{2 \cdot 3 \cdot 7}{6} = \frac{42}{6} = 7$ ✓

**Verification for n=3:**
Left side: $\binom{2}{2} + \binom{4}{2} + \binom{6}{2} = 1 + 6 + 15 = 22$
Right side: $\frac{3(3+1)(12-1)}{6} = \frac{3 \cdot 4 \cdot 11}{6} = \frac{132}{6} = 22$ ✓

The identity is proven and verified.