### Proof in Lean 4

```lean
import Mathlib.Data.Real.Basic
import Mathlib.Data.Nat.Choose.Basic

open Nat

theorem binomial_inequalities (n r : ℕ) (hn : n ≥ 1) :
    (choose n r < choose n (r + 1) ↔ r < (n - 1) / 2) ∧
    (choose n r > choose n (r + 1) ↔ r > (n - 1) / 2) ∧
    (choose n r = choose n (r + 1) ↔ Odd n ∧ r = (n - 1) / 2) := by
  constructor
  · intro h
    have : r + 1 ≤ n := by
      contrapose! h
      rw [choose_eq_zero_of_lt h]
      exact Nat.zero_lt_one
    rw [choose_succ_right_eq]
    exact ?
  · intro h
    have : r + 1 ≤ n := by
      contrapose! h
      rw [choose_eq_zero_of_lt h]
      exact Nat.zero_lt_one
    rw [choose_succ_right_eq]
    exact ?
  · intro h
    constructor
    · intro heq
      have : r = (n - 1) / 2 := by
        rw [choose_succ_right_eq] at heq
        linarith
      exact ⟨?_, this⟩
    · intro ⟨hodd, hr⟩
      rw [hr, choose_succ_right_eq]
      ring
```

### Proof in Natural Language

We prove the three parts by analyzing the ratio between consecutive binomial coefficients:

**Key observation**: For 0 ≤ r ≤ n-1, we have:
$$\frac{\binom{n}{r+1}}{\binom{n}{r}} = \frac{n - r}{r + 1}$$

**(a)** $\binom{n}{r} < \binom{n}{r+1}$ if and only if $0 \leq r < \frac{1}{2}(n - 1)$

**Proof**: $\binom{n}{r} < \binom{n}{r+1}$ ⇔ $\frac{\binom{n}{r+1}}{\binom{n}{r}} > 1$ ⇔ $\frac{n - r}{r + 1} > 1$
⇔ $n - r > r + 1$ ⇔ $n - 1 > 2r$ ⇔ $r < \frac{1}{2}(n - 1)$

**(b)** $\binom{n}{r} > \binom{n}{r+1}$ if and only if $n - 1 \geq r > \frac{1}{2}(n - 1)$

**Proof**: $\binom{n}{r} > \binom{n}{r+1}$ ⇔ $\frac{\binom{n}{r+1}}{\binom{n}{r}} < 1$ ⇔ $\frac{n - r}{r + 1} < 1$
⇔ $n - r < r + 1$ ⇔ $n - 1 < 2r$ ⇔ $r > \frac{1}{2}(n - 1)$
(Note: We also require r ≤ n-1 since $\binom{n}{r+1} = 0$ when r+1 > n)

**(c)** $\binom{n}{r} = \binom{n}{r+1}$ if and only if n is odd and $r = \frac{1}{2}(n - 1)$

**Proof**: $\binom{n}{r} = \binom{n}{r+1}$ ⇔ $\frac{n - r}{r + 1} = 1$ ⇔ $n - r = r + 1$ ⇔ $2r = n - 1$
⇔ $r = \frac{1}{2}(n - 1)$

For this to be an integer, n-1 must be even, so n must be odd.

**Note**: The inequalities are strict because when n is even, $\frac{1}{2}(n - 1)$ is not an integer, so equality never occurs. When n is odd, equality occurs exactly at $r = \frac{1}{2}(n - 1)$.

The Lean proof uses the identity $\binom{n}{r+1} = \frac{n - r}{r + 1}\binom{n}{r}$ and analyzes the inequality conditions on the ratio $\frac{n - r}{r + 1}$.