### (a) Derive Newton's identity

We aim to prove:
\[
\binom{n}{k}\binom{k}{r} = \binom{n}{r}\binom{n-r}{k-r}, \quad \text{for } n \geq k \geq r \geq 0.
\]

**Combinatorial interpretation:**

- Left side: Choose a committee of \(k\) people from \(n\), then choose a subcommittee of \(r\) from those \(k\).
- Right side: Choose a subcommittee of \(r\) people directly from \(n\), then choose the remaining \(k - r\) members from the remaining \(n - r\) people.

**Algebraic proof:**

Start with the left-hand side:
\[
\binom{n}{k}\binom{k}{r} = \frac{n!}{k!(n-k)!} \cdot \frac{k!}{r!(k-r)!} = \frac{n!}{r!(n-k)!(k-r)!}.
\]

Now, the right-hand side:
\[
\binom{n}{r}\binom{n-r}{k-r} = \frac{n!}{r!(n-r)!} \cdot \frac{(n-r)!}{(k-r)!(n-k)!} = \frac{n!}{r!(k-r)!(n-k)!}.
\]

Both sides simplify to the same expression:
\[
\frac{n!}{r!(k-r)!(n-k)!}.
\]

Hence, the identity is proved.

---

### (b) Express \(\binom{n}{k}\) in terms of its predecessor

We want to show:
\[
\binom{n}{k} = \frac{n - k + 1}{k} \binom{n}{k-1}, \quad \text{for } n \geq k \geq 1.
\]

Using Newton's identity from part (a), set \(r = k - 1\):
\[
\binom{n}{k}\binom{k}{k-1} = \binom{n}{k-1}\binom{n - (k-1)}{k - (k-1)}.
\]

Simplify:
- \(\binom{k}{k-1} = k\) (since choosing \(k-1\) from \(k\) is equivalent to choosing 1 to exclude, so \(k\) ways).
- \(\binom{n - (k-1)}{k - (k-1)} = \binom{n - k + 1}{1} = n - k + 1\).

So the equation becomes:
\[
\binom{n}{k} \cdot k = \binom{n}{k-1} \cdot (n - k + 1).
\]

Rearranging:
\[
\binom{n}{k} = \frac{n - k + 1}{k} \binom{n}{k-1}.
\]

This is the desired recurrence relation.

---

### âœ… Final Answers:

**(a)** Newton's identity is derived combinatorially and algebraically:
\[
\binom{n}{k}\binom{k}{r} = \binom{n}{r}\binom{n-r}{k-r}.
\]

**(b)** Using part (a) with \(r = k-1\), we obtain:
\[
\binom{n}{k} = \frac{n - k + 1}{k} \binom{n}{k-1}.
\]